<?xml version="1.0"?>
<rdf:RDF xmlns="https://w3id.org/arco/ontology/arco-lite/"
     xml:base="https://w3id.org/arco/ontology/arco-lite/"
     xmlns:cd="https://w3id.org/arco/ontology/context-description/"
     xmlns:dc="http://purl.org/dc/elements/1.1/"
     xmlns:dd="https://w3id.org/arco/ontology/denotative-description/"
     xmlns:l0="https://w3id.org/italia/onto/l0/"
     xmlns:ns="http://www.w3.org/2006/vcard/ns#"
     xmlns:CLV="https://w3id.org/italia/onto/CLV/"
     xmlns:owl="http://www.w3.org/2002/07/owl#"
     xmlns:rdf="http://www.w3.org/1999/02/22-rdf-syntax-ns#"
     xmlns:xml="http://www.w3.org/XML/1998/namespace"
     xmlns:xsd="http://www.w3.org/2001/XMLSchema#"
     xmlns:ADMS="https://w3id.org/italia/onto/ADMS/"
     xmlns:core="https://w3id.org/arco/ontology/core/"
     xmlns:dcat="http://www.w3.org/ns/dcat#"
     xmlns:foaf="http://xmlns.com/foaf/0.1/"
     xmlns:opla="http://ontologydesignpatterns.org/opla/"
     xmlns:prov="http://www.w3.org/ns/prov#"
     xmlns:rdfs="http://www.w3.org/2000/01/rdf-schema#"
     xmlns:a-cat="https://w3id.org/arco/ontology/catalogue/"
     xmlns:opla1="http://www.ontologydesignpatterns.org/opla/"
     xmlns:terms="http://purl.org/dc/terms/">
    <owl:Ontology rdf:about="https://w3id.org/arco/ontology/arco-lite">
        <owl:versionIRI rdf:resource="https://w3id.org/arco/ontology/arco-lite/0.1"/>
        <owl:imports rdf:resource="https://w3id.org/arco/ontology/catalogue/1.2"/>
        <owl:imports rdf:resource="https://w3id.org/arco/ontology/context-description/1.3"/>
        <owl:imports rdf:resource="https://w3id.org/arco/ontology/core/1.3"/>
        <owl:imports rdf:resource="https://w3id.org/arco/ontology/denotative-description/1.3"/>
        <owl:imports rdf:resource="https://w3id.org/arco/ontology/location/1.3"/>
        <owl:imports rdf:resource="https://w3id.org/italia/onto/CLV/1.0"/>
        <rdfs:label xml:lang="en">Arco Lite Ontology (ArCo network)</rdfs:label>
        <rdfs:label xml:lang="it">Ontologia Arco Leggera (ArCo network)</rdfs:label>
    </owl:Ontology>



    <!--
    ///////////////////////////////////////////////////////////////////////////////////////
    //
    // Annotation properties
    //
    ///////////////////////////////////////////////////////////////////////////////////////
     -->




    <!-- http://www.w3.org/2002/07/owl#inverseOf -->

    <owl:AnnotationProperty rdf:about="http://www.w3.org/2002/07/owl#inverseOf"/>



    <!-- https://w3id.org/arco/ontology/arco-lite/iccdNormTag -->

    <owl:AnnotationProperty rdf:about="https://w3id.org/arco/ontology/arco-lite/iccdNormTag"/>



    <!--
    ///////////////////////////////////////////////////////////////////////////////////////
    //
    // Object Properties
    //
    ///////////////////////////////////////////////////////////////////////////////////////
     -->




     <!-- https://w3id.org/arco/ontology/arco-lite/hasAnisotropy -->

     <owl:ObjectProperty rdf:about="https://w3id.org/arco/ontology/arco-lite/hasAnisotropy">
         <rdfs:subPropertyOf rdf:resource="https://w3id.org/arco/ontology/arco-lite/hasOpticCharacteristic"/>
         <owl:inverseOf rdf:resource="https://w3id.org/arco/ontology/arco-lite/isAnisotropyOf"/>
         <rdfs:domain rdf:resource="http://www.w3.org/2002/07/owl#Thing"/>
         <rdfs:range rdf:resource="https://w3id.org/arco/ontology/natural-specimen-description/OpticCharacteristic"/>
         <rdfs:comment xml:lang="it">Questa proprietà collega il campione all&apos;anisotropia</rdfs:comment>
         <rdfs:comment xml:lang="en">This property relates the specimen to the anisotropy</rdfs:comment>
         <rdfs:isDefinedBy rdf:resource="https://w3id.org/arco/ontology/arco-lite"/>
         <rdfs:label xml:lang="it">ha anisotropia</rdfs:label>
         <rdfs:label xml:lang="en">has anisotropy</rdfs:label>
         <owl:versionInfo xml:lang="it">instabile</owl:versionInfo>
         <owl:versionInfo xml:lang="en">unstable</owl:versionInfo>
         <a-cat:iccdNormTag>SM/SMM/SMMA</a-cat:iccdNormTag>
     </owl:ObjectProperty>



    <!-- https://w3id.org/arco/ontology/arco-lite/hasAttributedAuthor -->

    <owl:ObjectProperty rdf:about="https://w3id.org/arco/ontology/arco-lite/hasAttributedAuthor">
        <rdfs:subPropertyOf rdf:resource="https://w3id.org/arco/ontology/arco-lite/hasRelatedAgent"/>
        <owl:inverseOf rdf:resource="https://w3id.org/arco/ontology/arco-lite/isAttributedAuthorOf"/>
        <rdfs:domain rdf:resource="https://w3id.org/arco/ontology/context-description/AuthorshipAttribution"/>
        <rdfs:range rdf:resource="https://w3id.org/italia/onto/l0/Agent"/>
        <rdfs:comment xml:lang="it">Questa proprietà collega una situazione in cui viene attribuito un autore a un bene culturale all&apos;autore stesso.</rdfs:comment>
        <rdfs:comment xml:lang="en">This property relates a situation where an autorship is attributed to a cultural entity&apos;s author.</rdfs:comment>
        <rdfs:isDefinedBy rdf:resource="https://w3id.org/arco/ontology/arco-lite"/>
        <rdfs:label xml:lang="it">ha autore attribuito</rdfs:label>
        <rdfs:label xml:lang="en">has attributed author</rdfs:label>
        <owl:versionInfo xml:lang="it">instabile</owl:versionInfo>
        <owl:versionInfo xml:lang="en">instable</owl:versionInfo>
        <a-cat:iccdNormTag> AU/AUT/AUTN (+ AU/AUT/AUTS); AU/AAT; AU/AAT/AATN. ICCD Normativa F e FF 4.00: PD/PDF/PDFN - ICCD Normativa F 3.00: PD/PDF/PDFN o PD/PDF/PDFB</a-cat:iccdNormTag>
    </owl:ObjectProperty>



    <!-- https://w3id.org/arco/ontology/arco-lite/hasAuthor -->

    <owl:ObjectProperty rdf:about="https://w3id.org/arco/ontology/arco-lite/hasAuthor">
        <rdfs:subPropertyOf rdf:resource="https://w3id.org/arco/ontology/arco-lite/hasRelatedAgent"/>
        <owl:inverseOf rdf:resource="https://w3id.org/arco/ontology/arco-lite/isAuthorOf"/>
        <rdfs:domain rdf:resource="http://www.w3.org/2002/07/owl#Thing"/>
        <rdfs:range rdf:resource="https://w3id.org/italia/onto/l0/Agent"/>
        <rdfs:comment xml:lang="it">Questa proprietà collega un&apos;entità al suo autore/creatore.</rdfs:comment>
        <rdfs:comment xml:lang="en">This property relates an entity with its author.</rdfs:comment>
        <rdfs:isDefinedBy rdf:resource="https://w3id.org/arco/ontology/arco-lite"/>
        <rdfs:label xml:lang="it">ha autore</rdfs:label>
        <rdfs:label xml:lang="en">has author</rdfs:label>
        <owl:versionInfo xml:lang="it">instabile</owl:versionInfo>
        <owl:versionInfo xml:lang="en">unstable</owl:versionInfo>
    </owl:ObjectProperty>



    <!-- https://w3id.org/arco/ontology/arco-lite/hasCalculatedDensity -->

    <owl:ObjectProperty rdf:about="https://w3id.org/arco/ontology/arco-lite/hasCalculatedDensity">
        <rdfs:subPropertyOf rdf:resource="https://w3id.org/arco/ontology/arco-lite/hasPhysicalCharacteristic"/>
        <owl:inverseOf rdf:resource="https://w3id.org/arco/ontology/arco-lite/isCalculatedDensity"/>
        <rdfs:domain rdf:resource="http://www.w3.org/2002/07/owl#Thing"/>
        <rdfs:range rdf:resource="https://w3id.org/arco/ontology/natural-specimen-description/PhysicalCharacteristic"/>
        <rdfs:comment xml:lang="it">Questa proprietà collega un entità alla densità calcolata</rdfs:comment>
        <rdfs:comment xml:lang="en">This property relates an entity to the calculated density</rdfs:comment>
        <rdfs:isDefinedBy rdf:resource="https://w3id.org/arco/ontology/arco-lite"/>
        <rdfs:label xml:lang="it">ha densità calcolata</rdfs:label>
        <rdfs:label xml:lang="en">has calculateddensity</rdfs:label>
        <owl:versionInfo xml:lang="it">instabile</owl:versionInfo>
        <owl:versionInfo xml:lang="en">unstable</owl:versionInfo>
        <a-cat:iccdNormTag>Normativa ICCD BNM: SM/SMF/SMFF</a-cat:iccdNormTag>
    </owl:ObjectProperty>



    <!-- https://w3id.org/arco/ontology/arco-lite/hasCataloguingAgency -->

    <owl:ObjectProperty rdf:about="https://w3id.org/arco/ontology/arco-lite/hasCataloguingAgency">
        <rdfs:subPropertyOf rdf:resource="https://w3id.org/arco/ontology/arco-lite/hasRelatedAgent"/>
        <owl:inverseOf rdf:resource="https://w3id.org/arco/ontology/arco-lite/isCataloguingAgencyOf"/>
        <rdfs:domain rdf:resource="http://www.w3.org/2002/07/owl#Thing"/>
        <rdfs:range rdf:resource="https://w3id.org/italia/onto/l0/Agent"/>
        <rdfs:comment xml:lang="it">Questa proprietà collega un&apos;entità descritta in una scheda di Authority File all&apos;ente schedatore dell&apos;authority file stesso. Per esempio, l&apos;attribuzione di un autore a un bene culturale, uno scavo archeologico, una ricognizione archeologica, una bibliografia. Questa proprietà, esprimendo il significato della relazione nel nome, dà una rappresentazione semplificata della relazione che lega questa entità, l&apos;authority file, e l&apos;ente schedatore dell&apos;authority file.</rdfs:comment>
        <rdfs:comment xml:lang="en">This property relates an entity described in a authority file to the file&apos;s cataloguing institution.</rdfs:comment>
        <rdfs:isDefinedBy rdf:resource="https://w3id.org/arco/ontology/arco-lite"/>
        <rdfs:label xml:lang="it">ha ente schedatore</rdfs:label>
        <rdfs:label xml:lang="en">has cataloguing agency</rdfs:label>
        <owl:versionInfo xml:lang="it">instabile</owl:versionInfo>
        <owl:versionInfo xml:lang="en">instable</owl:versionInfo>
        <a-cat:iccdNormTag>ICCD Normativa Trasversale 4.00: AU/AUT/AUTJ; DO/BIB/BIBJ; RE/RCG/RCGJ; RE/DSC/DSCJ - ICCD Normativa F: PD/PDF/PDFJ</a-cat:iccdNormTag>
    </owl:ObjectProperty>



    <!-- https://w3id.org/arco/ontology/arco-lite/hasCataloguingAgent -->

    <owl:ObjectProperty rdf:about="https://w3id.org/arco/ontology/arco-lite/hasCataloguingAgent">
        <rdfs:subPropertyOf rdf:resource="https://w3id.org/arco/ontology/arco-lite/hasRelatedAgent"/>
        <owl:inverseOf rdf:resource="https://w3id.org/arco/ontology/arco-lite/isCataloguingAgent"/>
    </owl:ObjectProperty>



    <!-- https://w3id.org/arco/ontology/arco-lite/hasCity -->

    <owl:ObjectProperty rdf:about="https://w3id.org/arco/ontology/arco-lite/hasCity">
        <owl:inverseOf rdf:resource="https://w3id.org/arco/ontology/arco-lite/hasCity"/>
        <rdfs:comment xml:lang="it">Questa proprietà collega un catasto alla sua città.</rdfs:comment>
        <rdfs:comment xml:lang="en">This property relates the cadastre to its city.</rdfs:comment>
        <rdfs:isDefinedBy rdf:resource="https://w3id.org/arco/ontology/arco-lite"/>
        <rdfs:label xml:lang="it">ha città</rdfs:label>
        <rdfs:label xml:lang="en">has city</rdfs:label>
        <owl:versionInfo xml:lang="it">instabile</owl:versionInfo>
        <owl:versionInfo xml:lang="en">unstable</owl:versionInfo>
        <a-cat:iccdNormTag>Normativa Trasversale 4.00: CS/CTS/CTSC, Normativa RA 1.0 LG/LGC/LGCC</a-cat:iccdNormTag>
    </owl:ObjectProperty>



    <!-- https://w3id.org/arco/ontology/arco-lite/hasCollectionMember -->

    <owl:ObjectProperty rdf:about="https://w3id.org/arco/ontology/arco-lite/hasCollectionMember">
        <owl:inverseOf rdf:resource="https://w3id.org/arco/ontology/arco-lite/isCollectionMemberOf"/>
        <rdfs:domain rdf:resource="http://dati.beniculturali.it/cis/CollectionCulEnt"/>
        <rdfs:range rdf:resource="http://dati.beniculturali.it/cis/CulturalEntity"/>
        <rdfs:comment xml:lang="it">Questa proprietà collega una collezione di cultural beni culturali con il singolo bene.</rdfs:comment>
        <rdfs:comment xml:lang="en">This property relates a collection of cultural entities with the cultutal entities.</rdfs:comment>
        <rdfs:isDefinedBy rdf:resource="https://w3id.org/arco/ontology/arco-lite"/>
        <rdfs:label xml:lang="it">ha membro di collezione</rdfs:label>
        <rdfs:label xml:lang="en">has collection member</rdfs:label>
        <owl:versionInfo xml:lang="it">instabile</owl:versionInfo>
        <owl:versionInfo xml:lang="en">unstable</owl:versionInfo>
    </owl:ObjectProperty>



    <!-- https://w3id.org/arco/ontology/arco-lite/hasCollector -->

    <owl:ObjectProperty rdf:about="https://w3id.org/arco/ontology/arco-lite/hasCollector">
        <owl:inverseOf rdf:resource="https://w3id.org/arco/ontology/arco-lite/isCollectorOf"/>
        <rdfs:domain rdf:resource="http://dati.beniculturali.it/cis/CollectionCulEnt"/>
        <rdfs:range rdf:resource="https://w3id.org/italia/onto/l0/Agent"/>
        <rdfs:comment xml:lang="it">Questa proprietà collega una collezione all&apos;agente collezionista.</rdfs:comment>
        <rdfs:comment xml:lang="en">This property relates a collection of cultural entities with its collector.</rdfs:comment>
        <rdfs:isDefinedBy rdf:resource="https://w3id.org/arco/ontology/arco-lite"/>
        <rdfs:label xml:lang="it">ha collezionista</rdfs:label>
        <rdfs:label xml:lang="en">has collector</rdfs:label>
        <owl:versionInfo xml:lang="it">instabile</owl:versionInfo>
        <owl:versionInfo xml:lang="en">unstable</owl:versionInfo>
    </owl:ObjectProperty>



    <!-- https://w3id.org/arco/ontology/arco-lite/hasColour -->

    <owl:ObjectProperty rdf:about="https://w3id.org/arco/ontology/arco-lite/hasColour">
        <owl:inverseOf rdf:resource="https://w3id.org/arco/ontology/arco-lite/isColourOf"/>
        <rdfs:domain rdf:resource="http://www.w3.org/2002/07/owl#Thing"/>
        <rdfs:range rdf:resource="https://w3id.org/arco/ontology/denotative-description/TechnicalCharacteristic"/>
        <rdfs:comment xml:lang="it">Questa proprietà collega un oggetto al colore .</rdfs:comment>
        <rdfs:comment xml:lang="en">This property connects an object to the colour.</rdfs:comment>
        <rdfs:isDefinedBy rdf:resource="https://w3id.org/arco/ontology/arco-lite"/>
        <rdfs:label xml:lang="it">ha colore</rdfs:label>
        <rdfs:label xml:lang="en">has colour</rdfs:label>
        <owl:versionInfo xml:lang="it">instabile</owl:versionInfo>
        <owl:versionInfo xml:lang="en">unstable</owl:versionInfo>
    </owl:ObjectProperty>



    <!-- https://w3id.org/arco/ontology/arco-lite/hasCommittent -->

    <owl:ObjectProperty rdf:about="https://w3id.org/arco/ontology/arco-lite/hasCommittent">
        <rdfs:subPropertyOf rdf:resource="https://w3id.org/arco/ontology/arco-lite/hasRelatedAgent"/>
        <owl:inverseOf rdf:resource="https://w3id.org/arco/ontology/arco-lite/isCommittentOf"/>
        <rdfs:domain rdf:resource="https://w3id.org/arco/ontology/context-description/Commission"/>
        <rdfs:range rdf:resource="https://w3id.org/italia/onto/l0/Agent"/>
        <rdfs:comment xml:lang="it">Questa proprietà collega una situazione in cui viene indicata la committenza di un bene culturale alla persona o istituzione committente.</rdfs:comment>
        <rdfs:comment xml:lang="en">This property relates a situation where it is indicated a cultural entity&apos;s commission to the investor agent or institution.</rdfs:comment>
        <rdfs:isDefinedBy rdf:resource="https://w3id.org/arco/ontology/arco-lite"/>
        <rdfs:label xml:lang="it">ha committente</rdfs:label>
        <rdfs:label xml:lang="en">has committent</rdfs:label>
        <owl:versionInfo xml:lang="it">instabile</owl:versionInfo>
        <owl:versionInfo xml:lang="en">unstable</owl:versionInfo>
        <a-cat:iccdNormTag>ICCD Normativa Trasversale 4.00: AU/CMM/CMMN</a-cat:iccdNormTag>
    </owl:ObjectProperty>



    <!-- https://w3id.org/arco/ontology/arco-lite/hasConservationStatusType -->

    <owl:ObjectProperty rdf:about="https://w3id.org/arco/ontology/arco-lite/hasConservationStatusType">
        <owl:inverseOf rdf:resource="https://w3id.org/arco/ontology/arco-lite/isConservationStatusTypeOf"/>
        <rdfs:domain rdf:resource="http://www.w3.org/2002/07/owl#Thing"/>
        <rdfs:range rdf:resource="https://w3id.org/arco/ontology/denotative-description/ConservationStatusType"/>
        <rdfs:comment xml:lang="it">Questa proprietà associa lo stato di conservazione a uno dei valori del tipo di stato di conservazione.</rdfs:comment>
        <rdfs:comment xml:lang="en">This property relates a conservation status to one of its type&apos;s values.</rdfs:comment>
        <rdfs:isDefinedBy rdf:resource="https://w3id.org/arco/ontology/arco-lite"/>
        <rdfs:label xml:lang="it">ha tipo di stato di conservazione</rdfs:label>
        <rdfs:label xml:lang="en">has conservation status type</rdfs:label>
        <owl:versionInfo xml:lang="it">instabile</owl:versionInfo>
        <owl:versionInfo xml:lang="en">unstable</owl:versionInfo>
        <a-cat:iccdNormTag xml:lang="it">CO/STC/STCC</a-cat:iccdNormTag>
    </owl:ObjectProperty>



    <!-- https://w3id.org/arco/ontology/arco-lite/hasCompatibilityIndex -->

    <owl:ObjectProperty rdf:about="https://w3id.org/arco/ontology/arco-lite/hasCompatibilityIndex">
        <rdfs:subPropertyOf rdf:resource="https://w3id.org/arco/ontology/arco-lite/hasPhysicalCharacteristic"/>
        <owl:inverseOf rdf:resource="https://w3id.org/arco/ontology/arco-lite/isCompatibilityIndexOf"/>
        <rdfs:domain rdf:resource="http://www.w3.org/2002/07/owl#Thing"/>
        <rdfs:range rdf:resource="https://w3id.org/arco/ontology/natural-specimen-description/PhysicalCharacteristic"/>
        <rdfs:comment xml:lang="it">Questa proprietà collega un entità al compatibility index</rdfs:comment>
        <rdfs:comment xml:lang="en">This property relates an entity to the compatibility index</rdfs:comment>
        <rdfs:isDefinedBy rdf:resource="https://w3id.org/arco/ontology/arco-lite"/>
        <rdfs:label xml:lang="it">ha compatibility index</rdfs:label>
        <rdfs:label xml:lang="en">has compatibility index</rdfs:label>
        <owl:versionInfo xml:lang="it">instabile</owl:versionInfo>
        <owl:versionInfo xml:lang="en">unstable</owl:versionInfo>
        <a-cat:iccdNormTag>Normativa ICCD BNM: SM/SMF/SMFI</a-cat:iccdNormTag>
    </owl:ObjectProperty>



    <!-- https://w3id.org/arco/ontology/arco-lite/hasCopyrightHolder -->

    <owl:ObjectProperty rdf:about="https://w3id.org/arco/ontology/arco-lite/hasCopyrightHolder">
        <owl:inverseOf rdf:resource="https://w3id.org/arco/ontology/arco-lite/isCopyrightHolderOf"/>
        <rdfs:domain rdf:resource="http://www.w3.org/2002/07/owl#Thing"/>
        <rdfs:range rdf:resource="https://w3id.org/italia/onto/l0/Agent"/>
    </owl:ObjectProperty>



    <!-- https://w3id.org/arco/ontology/arco-lite/hasCreationLocation -->

    <owl:ObjectProperty rdf:about="https://w3id.org/arco/ontology/arco-lite/hasCreationLocation">
        <rdfs:subPropertyOf rdf:resource="https://w3id.org/arco/ontology/arco-lite/hasRelatedWork"/>
        <owl:inverseOf rdf:resource="https://w3id.org/arco/ontology/arco-lite/isCreationLocationOf"/>
        <rdfs:domain rdf:resource="http://www.w3.org/2002/07/owl#Thing"/>
        <rdfs:range rdf:resource="http://www.w3.org/2002/07/owl#Thing"/>
        <rdfs:comment xml:lang="it">Questa proprietà collega un bene culturale a un altro bene culturale collegato, che ne costituisce la sede di produzione/realizzazione.</rdfs:comment>
        <rdfs:comment xml:lang="en">This property relates a cultural entity to a connected cultural entity which constitutes its production site.</rdfs:comment>
        <rdfs:isDefinedBy rdf:resource="https://w3id.org/arco/ontology/arco-lite"/>
        <rdfs:label xml:lang="it">ha luogo di creazione</rdfs:label>
        <rdfs:label xml:lang="en">has creation location</rdfs:label>
        <rdfs:label xml:lang="it">è stato realizzato in</rdfs:label>
        <owl:versionInfo xml:lang="it">instabile</owl:versionInfo>
        <owl:versionInfo xml:lang="en">unstable</owl:versionInfo>
        <a-cat:iccdNormTag xml:lang="it">ICCD Normativa Trasversale 4.00: RV/RSE/RSER = &apos;è stato realizzato in&apos; (versioni precedenti: &apos;sede di realizzazione&apos;)</a-cat:iccdNormTag>
    </owl:ObjectProperty>



    <!-- https://w3id.org/arco/ontology/arco-lite/hasCrystallographicCharacteristic -->

    <owl:ObjectProperty rdf:about="https://w3id.org/arco/ontology/arco-lite/hasCrystallographicCharacteristic">
        <rdfs:subPropertyOf rdf:resource="https://w3id.org/arco/ontology/denotative-description/hasTechnicalCharacteristic"/>
        <owl:inverseOf rdf:resource="https://w3id.org/arco/ontology/arco-lite/isCrystallographicCharacteristicOf"/>
        <rdfs:domain rdf:resource="https://w3id.org/arco/ontology/natural-specimen-description/UnitCell"/>
        <rdfs:range rdf:resource="https://w3id.org/arco/ontology/natural-specimen-description/CrystallographicCharacteristic"/>
        <rdfs:comment xml:lang="it">Questa proprietà collega la cella alla caratteristica cristallografica</rdfs:comment>
        <rdfs:comment xml:lang="en">This property relates the unit cell to the crystallographic characteristic.</rdfs:comment>
        <rdfs:isDefinedBy rdf:resource="https://w3id.org/arco/ontology/arco-lite"/>
        <rdfs:label xml:lang="it">ha caratteristica cristallografica</rdfs:label>
        <rdfs:label xml:lang="en">has crystallographic characteristic</rdfs:label>
        <owl:versionInfo xml:lang="it">instabile</owl:versionInfo>
        <owl:versionInfo xml:lang="en">unstable</owl:versionInfo>
    </owl:ObjectProperty>



    <!-- https://w3id.org/arco/ontology/natural-specimen-description/hasCrystalClass -->

    <owl:ObjectProperty rdf:about="https://w3id.org/arco/ontology/arco-lite/hasCrystalClass">
        <rdfs:subPropertyOf rdf:resource="https://w3id.org/arco/ontology/arco-lite/hasCrystallographicCharacteristic"/>
        <owl:inverseOf rdf:resource="https://w3id.org/arco/ontology/arco-lite/isCrystalClassOf"/>
        <rdfs:domain rdf:resource="https://w3id.org/arco/ontology/natural-specimen-description/UnitCell"/>
        <rdfs:range rdf:resource="https://w3id.org/arco/ontology/natural-specimen-description/CrystallographicCharacteristic"/>
        <rdfs:comment xml:lang="it">Questa proprietà collega una cella alla caratteristica cristallografica</rdfs:comment>
        <rdfs:comment xml:lang="en">This property relates a unit cell to the crystallographic chatacteristic</rdfs:comment>
        <rdfs:isDefinedBy rdf:resource="https://w3id.org/arco/ontology/arco-lite"/>
        <rdfs:label xml:lang="it">ha classe cristallina</rdfs:label>
        <rdfs:label xml:lang="en">has crystal class</rdfs:label>
        <owl:versionInfo xml:lang="it">instabile</owl:versionInfo>
        <owl:versionInfo xml:lang="en">unstable</owl:versionInfo>
        <a-cat:iccdNormTag>Normativa ICCD BNM: SM/SMC/SMCL</a-cat:iccdNormTag>
    </owl:ObjectProperty>



    <!-- https://w3id.org/arco/ontology/arco-lite/hasCrystalSystem -->

    <owl:ObjectProperty rdf:about="https://w3id.org/arco/ontology/arco-lite/hasCrystalSystem">
        <rdfs:subPropertyOf rdf:resource="https://w3id.org/arco/ontology/arco-lite/hasCrystallographicCharacteristic"/>
        <owl:inverseOf rdf:resource="https://w3id.org/arco/ontology/natural-specimen-description/isCrystalSystemOf"/>
        <rdfs:domain rdf:resource="https://w3id.org/arco/ontology/natural-specimen-description/UnitCell"/>
        <rdfs:range rdf:resource="https://w3id.org/arco/ontology/arco-lite/CrystallographicCharacteristic"/>
        <rdfs:comment xml:lang="it">Questa proprietà collega una cella al sistema cristallino</rdfs:comment>
        <rdfs:comment xml:lang="en">This property relates a unit cell to the crystal system</rdfs:comment>
        <rdfs:isDefinedBy rdf:resource="https://w3id.org/arco/ontology/arco-lite"/>
        <rdfs:label xml:lang="it">ha sistema cristallino</rdfs:label>
        <rdfs:label xml:lang="en">has crystal system</rdfs:label>
        <owl:versionInfo xml:lang="it">instabile</owl:versionInfo>
        <owl:versionInfo xml:lang="en">unstable</owl:versionInfo>
        <a-cat:iccdNormTag>Normativa ICCD BNM: SM/SMC/SMCS</a-cat:iccdNormTag>
    </owl:ObjectProperty>



    <!-- https://w3id.org/arco/ontology/arco-lite/hasCulturalEntityUseFunction -->

    <owl:ObjectProperty rdf:about="https://w3id.org/arco/ontology/arco-lite/hasCulturalEntityUseFunction">
        <owl:inverseOf rdf:resource="https://w3id.org/arco/ontology/arco-lite/isCulturalEntityUseFunctionOf"/>
        <rdfs:domain rdf:resource="http://dati.beniculturali.it/cis/CulturalEntity"/>
        <rdfs:range rdf:resource="https://w3id.org/arco/ontology/context-description/UseFunction"/>
    </owl:ObjectProperty>



    <!-- https://w3id.org/arco/ontology/arco-lite/hasCulturalPropertyAddress -->

    <owl:ObjectProperty rdf:about="https://w3id.org/arco/ontology/arco-lite/hasCulturalPropertyAddress">
        <owl:inverseOf rdf:resource="https://w3id.org/arco/ontology/arco-lite/isCulturalPropertyAddressOf"/>
        <rdfs:domain rdf:resource="http://dati.beniculturali.it/cis/CulturalEntity"/>
        <rdfs:range rdf:resource="https://w3id.org/italia/onto/CLV/Address"/>
        <owl:propertyChainAxiom rdf:parseType="Collection">
            <rdf:Description rdf:about="https://w3id.org/arco/ontology/location/hasTimeIndexedTypedLocation"/>
            <rdf:Description rdf:about="https://w3id.org/arco/ontology/location/atLocation"/>
            <rdf:Description rdf:about="https://w3id.org/italia/onto/CLV/hasAddress"/>
        </owl:propertyChainAxiom>
        <owl:propertyChainAxiom rdf:parseType="Collection">
            <rdf:Description rdf:about="https://w3id.org/arco/ontology/location/hasTimeIndexedTypedLocation"/>
            <rdf:Description rdf:about="https://w3id.org/arco/ontology/location/atSite"/>
            <rdf:Description rdf:about="https://w3id.org/italia/onto/CLV/hasAddress"/>
        </owl:propertyChainAxiom>
        <rdfs:comment xml:lang="it">Questa proprietà rappresenta la relazione che collega un bene culturale all&apos;indirizzo della sua localizzazione fisica attuale, al momento della catalogazione. La relazione fornisce una rappresentazione semplificata, con ridotta espressività, della localizzazione attuale del bene culturale, e provoca la perdita delle altre informazioni che riguardano la collocazione del bene (continente, eventuale contenitore fisico, collocazione specifica nel contenitore fisico, ecc.).</rdfs:comment>
        <rdfs:comment xml:lang="en">This property represents the relationship that links a cultural property to the address of its current physical location at the cataloging time. The report provides a simplified representation, with a reduced expressivity, of the current location of the cultural property, and it causes the loss of other information regarding its location (i.e. the continent, the possible physical container, the specific location in the physical container, etc.).</rdfs:comment>
        <rdfs:isDefinedBy rdf:resource="https://w3id.org/arco/ontology/arco-lite"/>
        <rdfs:label xml:lang="en">has cultural property address</rdfs:label>
        <rdfs:label xml:lang="it">indirizzo del bene culturale</rdfs:label>
        <owl:versionInfo xml:lang="it">instabile</owl:versionInfo>
        <owl:versionInfo xml:lang="en">unstable</owl:versionInfo>
        <a-cat:iccdNormTag xml:lang="it">ICCD Normativa Trasversale 4.00: LC/PVC</a-cat:iccdNormTag>
    </owl:ObjectProperty>



    <!-- https://w3id.org/arco/ontology/arco-lite/hasCurator -->

    <owl:ObjectProperty rdf:about="https://w3id.org/arco/ontology/arco-lite/hasCurator">
        <rdfs:subPropertyOf rdf:resource="https://w3id.org/arco/ontology/arco-lite/hasRelatedAgent"/>
        <rdfs:domain rdf:resource="http://www.w3.org/2002/07/owl#Thing"/>
        <rdfs:range rdf:resource="https://w3id.org/italia/onto/l0/Agent"/>
        <rdfs:comment xml:lang="it">Questa proprietà collega un&apos;entità al suo curatore.</rdfs:comment>
        <rdfs:comment xml:lang="en">This property relates an entity with its curator.</rdfs:comment>
        <rdfs:isDefinedBy rdf:resource="https://w3id.org/arco/ontology/arco-lite"/>
        <rdfs:label xml:lang="it">ha curatore</rdfs:label>
        <rdfs:label xml:lang="en">has curator</rdfs:label>
        <owl:inverseOf></owl:inverseOf>
        <owl:versionInfo xml:lang="it">instabile</owl:versionInfo>
        <owl:versionInfo xml:lang="en">unstable</owl:versionInfo>
    </owl:ObjectProperty>



    <!-- https://w3id.org/arco/ontology/arco-lite/hasDiapason -->

    <owl:ObjectProperty rdf:about="https://w3id.org/arco/ontology/arco-lite/hasDiapason">
        <rdfs:subPropertyOf rdf:resource="https://w3id.org/arco/ontology/denotative-description/hasTechnicalCharacteristic"/>
        <owl:inverseOf rdf:resource="https://w3id.org/arco/ontology/arco-lite/isDiapasonOf"/>
        <rdfs:domain rdf:resource="http://www.w3.org/2002/07/owl#Thing"/>
        <rdfs:range rdf:resource="https://w3id.org/arco/ontology/denotative-description/TechnicalCharacteristic"/>
        <rdfs:comment xml:lang="it">Questa proprietà collega uno strumento musical al corista rilevato (nota, temperatura ed eventualmente umidità ambientale al momento della rilevazione).</rdfs:comment>
        <rdfs:comment xml:lang="en">This property relates a musical instrument to the identified diapason (note, temperature and eventually humidity during the detection).</rdfs:comment>
        <rdfs:isDefinedBy rdf:resource="https://w3id.org/arco/ontology/arco-lite"/>
        <rdfs:label xml:lang="it">ha corista</rdfs:label>
        <rdfs:label xml:lang="en">has diapason</rdfs:label>
        <owl:versionInfo xml:lang="it">instabile</owl:versionInfo>
        <owl:versionInfo xml:lang="en">unstable</owl:versionInfo>
    </owl:ObjectProperty>



    <!-- https://w3id.org/arco/ontology/arco-lite/hasDiaphaneity -->

    <owl:ObjectProperty rdf:about="https://w3id.org/arco/ontology/arco-lite/hasDiaphaneity">
        <rdfs:subPropertyOf rdf:resource="https://w3id.org/arco/ontology/arco-lite/hasPhysicalCharacteristic"/>
        <owl:inverseOf rdf:resource="https://w3id.org/arco/ontology/arco-lite/isDiaphaneityOf"/>
        <rdfs:domain rdf:resource="http://www.w3.org/2002/07/owl#Thing"/>
        <rdfs:range rdf:resource="https://w3id.org/arco/ontology/natural-specimen-description/PhysicalCharacteristic"/>
        <rdfs:comment xml:lang="it">Questa proprietà collega un entità alla diafanità</rdfs:comment>
        <rdfs:comment xml:lang="en">This property relates an entity to the diaphaneity</rdfs:comment>
        <rdfs:isDefinedBy rdf:resource="https://w3id.org/arco/ontology/arco-lite"/>
        <rdfs:label xml:lang="it">ha diafanità</rdfs:label>
        <rdfs:label xml:lang="en">has diaphaneity</rdfs:label>
        <owl:versionInfo xml:lang="it">instabile</owl:versionInfo>
        <owl:versionInfo xml:lang="en">unstable</owl:versionInfo>
        <a-cat:iccdNormTag>Normativa ICCD BNM: SM/SMF/SMFP</a-cat:iccdNormTag>
    </owl:ObjectProperty>




    <!-- https://w3id.org/arco/ontology/arco-lite/hasEditor -->

    <owl:ObjectProperty rdf:about="https://w3id.org/arco/ontology/arco-lite/hasEditor">
        <rdfs:subPropertyOf rdf:resource="https://w3id.org/arco/ontology/arco-lite/hasRelatedAgent"/>
        <owl:inverseOf rdf:resource="https://w3id.org/arco/ontology/arco-lite/isEditorOf"/>
        <rdfs:domain rdf:resource="http://www.w3.org/2002/07/owl#Thing"/>
        <rdfs:comment xml:lang="it">Questa proprietà collega un&apos;edizione all&apos;editore.</rdfs:comment>
        <rdfs:comment xml:lang="en">This property relates an edition to its editor.</rdfs:comment>
        <rdfs:isDefinedBy rdf:resource="https://w3id.org/arco/ontology/arco-lite"/>
        <rdfs:label xml:lang="it">ha editore</rdfs:label>
        <rdfs:label xml:lang="en">has editor</rdfs:label>
        <owl:versionInfo xml:lang="it">instabile</owl:versionInfo>
        <owl:versionInfo xml:lang="en">unstable</owl:versionInfo>
        <a-cat:iccdNormTag xml:lang="it">Normativa F: PD/EDI/EDIR, Normativa S: AU/EDT/EDTN</a-cat:iccdNormTag>
    </owl:ObjectProperty>



    <!-- https://w3id.org/arco/ontology/arco-lite/hasExportOffice -->

    <owl:ObjectProperty rdf:about="https://w3id.org/arco/ontology/arco-lite/hasExportOffice">
        <rdfs:subPropertyOf rdf:resource="https://w3id.org/arco/ontology/arco-lite/hasRelatedAgent"/>
        <owl:inverseOf rdf:resource="https://w3id.org/arco/ontology/arco-lite/isExportOfficeOf"/>
        <rdfs:domain rdf:resource="https://w3id.org/arco/ontology/context-description/ExportImportCertification"/>
        <rdfs:range rdf:resource="https://w3id.org/italia/onto/l0/Agent"/>
        <rdfs:comment xml:lang="it">Questa proprietà collega una certificazione di importazione/esportazione al&apos;Ufficio Esportazione che ha emesso la certificazione.</rdfs:comment>
        <rdfs:comment xml:lang="en">This property relates an export/import certification to the certifying Export Department.</rdfs:comment>
        <rdfs:isDefinedBy rdf:resource="https://w3id.org/arco/ontology/arco-lite"/>
        <rdfs:label xml:lang="it">ha ufficio esportazione</rdfs:label>
        <rdfs:label xml:lang="en">has export office</rdfs:label>
        <owl:versionInfo xml:lang="it">stabile</owl:versionInfo>
        <owl:versionInfo xml:lang="en">stable</owl:versionInfo>
        <a-cat:iccdNormTag>ICCD Normativa Trasversale 4.00: TU/ESP/ESPU</a-cat:iccdNormTag>
    </owl:ObjectProperty>



    <!-- https://w3id.org/arco/ontology/arco-lite/hasExtension -->

    <owl:ObjectProperty rdf:about="https://w3id.org/arco/ontology/arco-lite/hasExtension">
        <rdfs:subPropertyOf rdf:resource="https://w3id.org/arco/ontology/denotative-description/hasTechnicalCharacteristic"/>
        <owl:inverseOf rdf:resource="https://w3id.org/arco/ontology/arco-lite/isExtensionOf"/>
        <rdfs:domain rdf:resource="http://www.w3.org/2002/07/owl#Thing"/>
        <rdfs:range rdf:resource="https://w3id.org/arco/ontology/denotative-description/TechnicalCharacteristic"/>
        <rdfs:comment xml:lang="it">Questa proprietà collega uno strumento musicale alla sua estensione.</rdfs:comment>
        <rdfs:comment xml:lang="en">This property relates a musical instrument with its extension.</rdfs:comment>
        <rdfs:isDefinedBy rdf:resource="https://w3id.org/arco/ontology/arco-lite"/>
        <rdfs:label xml:lang="it">ha estensione musicale</rdfs:label>
        <rdfs:label xml:lang="en">has musical extension</rdfs:label>
        <owl:versionInfo xml:lang="it">instabile</owl:versionInfo>
        <owl:versionInfo xml:lang="en">unstable</owl:versionInfo>
        <a-cat:iccdNormTag>ICCD Normativa SM 4.00: AA/AAE</a-cat:iccdNormTag>
    </owl:ObjectProperty>



    <!-- https://w3id.org/arco/ontology/arco-lite/hasFindingLocation -->

    <owl:ObjectProperty rdf:about="https://w3id.org/arco/ontology/arco-lite/hasFindingLocation">
        <rdfs:subPropertyOf rdf:resource="https://w3id.org/arco/ontology/arco-lite/hasRelatedWork"/>
        <owl:inverseOf rdf:resource="https://w3id.org/arco/ontology/arco-lite/isFindingLocationOf"/>
        <rdfs:domain rdf:resource="http://www.w3.org/2002/07/owl#Thing"/>
        <rdfs:range rdf:resource="http://www.w3.org/2002/07/owl#Thing"/>
        <rdfs:comment xml:lang="it">Questa proprietà collega un bene culturale a un altro bene culturale collegato, che ne costituisce la sede di rinvenimento archeologico.</rdfs:comment>
        <rdfs:comment xml:lang="en">This property relates a cultural entity to a connected cultural entity which constitutes the site where it was rediscovered.</rdfs:comment>
        <rdfs:isDefinedBy rdf:resource="https://w3id.org/arco/ontology/arco-lite"/>
        <rdfs:label xml:lang="it">ha sede di rinvenimento</rdfs:label>
        <rdfs:label xml:lang="en">has finding location</rdfs:label>
        <rdfs:label xml:lang="it">è stato rinvenuto in</rdfs:label>
        <owl:versionInfo xml:lang="it">instabile</owl:versionInfo>
        <owl:versionInfo xml:lang="en">unstable</owl:versionInfo>
        <a-cat:iccdNormTag xml:lang="it">ICCD Normativa Trasversale 4.00: RV/RSE/RSER = &apos;è stato rinvenuto in&apos; (versioni precedenti: &apos;sede di rinvenimento&apos;)</a-cat:iccdNormTag>
    </owl:ObjectProperty>



    <!-- https://w3id.org/arco/ontology/arco-lite/hasFluorescence -->

    <owl:ObjectProperty rdf:about="https://w3id.org/arco/ontology/arco-lite/hasFluorescence">
        <rdfs:subPropertyOf rdf:resource="https://w3id.org/arco/ontology/arco-lite/hasPhysicalCharacteristic"/>
        <owl:inverseOf rdf:resource="https://w3id.org/arco/ontology/arco-lite/isFluorescenceOf"/>
        <rdfs:domain rdf:resource="http://www.w3.org/2002/07/owl#Thing"/>
        <rdfs:range rdf:resource="https://w3id.org/arco/ontology/natural-specimen-description/PhysicalCharacteristic"/>
        <rdfs:comment xml:lang="it">Questa proprietà collega un entità alla fluorescenza</rdfs:comment>
        <rdfs:comment xml:lang="en">This property relates an entity to the fluorescence</rdfs:comment>
        <rdfs:isDefinedBy rdf:resource="https://w3id.org/arco/ontology/arco-lite"/>
        <rdfs:label xml:lang="it">ha fluorescenza</rdfs:label>
        <rdfs:label xml:lang="en">has fluorescence</rdfs:label>
        <owl:versionInfo xml:lang="it">instabile</owl:versionInfo>
        <owl:versionInfo xml:lang="en">unstable</owl:versionInfo>
        <a-cat:iccdNormTag>Normativa ICCD BNM: SM/SMF/SMFL</a-cat:iccdNormTag>
    </owl:ObjectProperty>



    <!-- https://w3id.org/arco/ontology/arco-lite/hasFracture -->

    <owl:ObjectProperty rdf:about="https://w3id.org/arco/ontology/arco-lite/hasFracture">
        <rdfs:subPropertyOf rdf:resource="https://w3id.org/arco/ontology/arco-lite/hasPhysicalCharacteristic"/>
        <owl:inverseOf rdf:resource="https://w3id.org/arco/ontology/arco-lite/isFractureOf"/>
        <rdfs:domain rdf:resource="http://www.w3.org/2002/07/owl#Thing"/>
        <rdfs:range rdf:resource="https://w3id.org/arco/ontology/natural-specimen-description/PhysicalCharacteristic"/>
        <rdfs:comment xml:lang="it">Questa proprietà collega un entità alla frattura</rdfs:comment>
        <rdfs:comment xml:lang="en">This property relates an entity to the fracture</rdfs:comment>
        <rdfs:isDefinedBy rdf:resource="https://w3id.org/arco/ontology/arco-lite"/>
        <rdfs:label xml:lang="it">ha frattura</rdfs:label>
        <rdfs:label xml:lang="en">has fracture</rdfs:label>
        <owl:versionInfo xml:lang="it">instabile</owl:versionInfo>
        <owl:versionInfo xml:lang="en">unstable</owl:versionInfo>
        <a-cat:iccdNormTag>Normativa ICCD BNM: SM/SMF/SMFU</a-cat:iccdNormTag>
    </owl:ObjectProperty>



    <!-- https://w3id.org/arco/ontology/arco-lite/hasGarmentAnalysis -->

    <owl:ObjectProperty rdf:about="https://w3id.org/arco/ontology/arco-lite/hasGarmentAnalysis">
        <owl:inverseOf rdf:resource="https://w3id.org/arco/ontology/arco-lite/isGarmentAnalysisOf"/>
        <rdfs:domain rdf:resource="http://www.w3.org/2002/07/owl#Thing"/>
        <rdfs:range rdf:resource="https://w3id.org/arco/ontology/denotative-description/TechnicalCharacteristic"/>
        <rdfs:comment xml:lang="it">Questa proprietà collega un elemento di un capo di abbigliamento con l&apos;analisi dei tessuti.</rdfs:comment>
        <rdfs:comment xml:lang="en">This property relates a clothing element with its garment analysis (technical characteristic).</rdfs:comment>
        <rdfs:isDefinedBy rdf:resource="https://w3id.org/arco/ontology/arco-lite"/>
        <rdfs:label xml:lang="it">ha analisi del tessuto</rdfs:label>
        <rdfs:label xml:lang="en">has garment analysis</rdfs:label>
        <owl:versionInfo xml:lang="it">instabile</owl:versionInfo>
        <owl:versionInfo xml:lang="en">unstable</owl:versionInfo>
        <a-cat:iccdNormTag>ICCD Normativa VeAC 3.01: MT/MTCA</a-cat:iccdNormTag>
    </owl:ObjectProperty>



    <!-- https://w3id.org/arco/ontology/arco-lite/hasGladstone-DaleRelation -->

    <owl:ObjectProperty rdf:about="https://w3id.org/arco/ontology/arco-lite/hasGladstone-DaleRelation">
        <rdfs:subPropertyOf rdf:resource="https://w3id.org/arco/ontology/arco-lite/hasPhysicalCharacteristic"/>
        <owl:inverseOf rdf:resource="https://w3id.org/arco/ontology/arco-lite/isGladstone-DaleRelation"/>
        <rdfs:domain rdf:resource="http://www.w3.org/2002/07/owl#Thing"/>
        <rdfs:range rdf:resource="https://w3id.org/arco/ontology/natural-specimen-description/PhysicalCharacteristic"/>
        <rdfs:comment xml:lang="it">Questa proprietà collega un entità alla relazione Gladstone-Dale</rdfs:comment>
        <rdfs:comment xml:lang="en">This property relates an entity to the Gradstone-Dsle relation</rdfs:comment>
        <rdfs:isDefinedBy rdf:resource="https://w3id.org/arco/ontology/arco-lite"/>
        <rdfs:label xml:lang="it">ha relazione Gladstone-Dale</rdfs:label>
        <rdfs:label xml:lang="en">has Gladstone-Dale relation</rdfs:label>
        <owl:versionInfo xml:lang="it">instabile</owl:versionInfo>
        <owl:versionInfo xml:lang="en">unstable</owl:versionInfo>
        <a-cat:iccdNormTag>Normativa ICCD BNM: SM/SMF/SMFG</a-cat:iccdNormTag>
    </owl:ObjectProperty>



    <!-- https://w3id.org/arco/ontology/arco-lite/hasInventoryNumberResponsible -->

    <owl:ObjectProperty rdf:about="https://w3id.org/arco/ontology/arco-lite/hasInventoryNumberResponsible">
        <owl:inverseOf rdf:resource="https://w3id.org/arco/ontology/arco-lite/isInventoryNumberResponsibleOf"/>
        <rdfs:domain rdf:resource="https://w3id.org/arco/ontology/context-description/InventorySituation"/>
        <rdfs:range rdf:resource="https://w3id.org/italia/onto/l0/Agent"/>
        <rdfs:comment xml:lang="it">Questa proprietà collega una situazione inventariale all&apos;agente che ha inserito il numero d&apos;inventario.</rdfs:comment>
        <rdfs:comment xml:lang="en">This property relates an inventary situation with the responsible of the insertion of the inventory number.</rdfs:comment>
        <rdfs:isDefinedBy rdf:resource="https://w3id.org/arco/ontology/arco-lite"/>
        <rdfs:label xml:lang="it">ha responsabile di numero d&apos;inventario</rdfs:label>
        <rdfs:label xml:lang="en">has inventory number responsible</rdfs:label>
        <owl:versionInfo xml:lang="it">instabile</owl:versionInfo>
        <owl:versionInfo xml:lang="en">unstable</owl:versionInfo>
    </owl:ObjectProperty>



    <!-- https://w3id.org/arco/ontology/arco-lite/hasIssuer -->

    <owl:ObjectProperty rdf:about="https://w3id.org/arco/ontology/arco-lite/hasIssuer">
        <rdfs:subPropertyOf rdf:resource="https://w3id.org/arco/ontology/arco-lite/hasRelatedAgent"/>
        <owl:inverseOf rdf:resource="https://w3id.org/arco/ontology/arco-lite/isIssuerOf"/>
        <rdfs:domain rdf:resource="https://w3id.org/arco/ontology/context-description/CoinIssuance"/>
        <rdfs:range rdf:resource="https://w3id.org/italia/onto/l0/Agent"/>
        <rdfs:comment xml:lang="it">Questa proprietà collega l&apos;emissione della moneta al soggetto emittente. Questa proprietà, esprimendo il significato della relazione nel nome, dà una rappresentazione semplificata della relazione che lega questa entità e l&apos;agente; la stessa relazione è rappresentata attraverso una n-ary relation, arco-core:AgentRole, che permette di collegare l&apos;agente al ruolo che riveste nei confronti dell&apos;entità.</rdfs:comment>
        <rdfs:comment xml:lang="en">This property relates to coin&apos;s issuance to the issuer agent. In the ontology this relationship is modelled also by the class AgentRole which allows more expressiveness.</rdfs:comment>
        <rdfs:isDefinedBy rdf:resource="https://w3id.org/arco/ontology/arco-lite"/>
        <rdfs:label xml:lang="it">ha soggetto emittente</rdfs:label>
        <rdfs:label xml:lang="en">has issuer</rdfs:label>
        <owl:versionInfo xml:lang="it">instabile</owl:versionInfo>
        <owl:versionInfo xml:lang="en">unstable</owl:versionInfo>
        <a-cat:iccdNormTag xml:lang="it">ICCD Normativa NU: DA/AUE/AUEE - ICCD Normativa OA (dopo il rilascio della specifica scheda NU nel 2004 la scheda OA non è stata più utilizzata per la catalogazione di monete e medaglie): AU/EDT/EDTN. DA/CON/CONA</a-cat:iccdNormTag>
    </owl:ObjectProperty>



    <!-- https://w3id.org/arco/ontology/arco-lite/hasIssuingAgency -->

    <owl:ObjectProperty rdf:about="https://w3id.org/arco/ontology/arco-lite/hasIssuingAgency">
        <rdfs:subPropertyOf rdf:resource="https://w3id.org/arco/ontology/arco-lite/hasRelatedAgent"/>
        <owl:inverseOf rdf:resource="https://w3id.org/arco/ontology/arco-lite/isIssuingAgencyOf"/>
        <rdfs:domain rdf:resource="https://w3id.org/arco/ontology/context-description/UrbanPlanningInstrument"/>
        <rdfs:range rdf:resource="https://w3id.org/italia/onto/l0/Agent"/>
        <rdfs:comment xml:lang="it">Questa proprietà collega uno strumento urbanistico-territoriale con l&apos;ente o l&apos;amministrazione che ha emanato il provvedimento.</rdfs:comment>
        <rdfs:comment xml:lang="en">This property relates an urban-planning instrument to the institution which issued the provision.</rdfs:comment>
        <rdfs:isDefinedBy rdf:resource="https://w3id.org/arco/ontology/arco-lite"/>
        <rdfs:label xml:lang="it">ha ente che ha emanato il provvedimento</rdfs:label>
        <rdfs:label xml:lang="en">has issuing agency</rdfs:label>
        <owl:versionInfo xml:lang="it">instabile</owl:versionInfo>
        <owl:versionInfo xml:lang="en">unstable</owl:versionInfo>
        <a-cat:iccdNormTag>TU/STU/STUE</a-cat:iccdNormTag>
    </owl:ObjectProperty>



    <!-- https://w3id.org/arco/ontology/arco-lite/hasIssuingState -->

    <owl:ObjectProperty rdf:about="https://w3id.org/arco/ontology/arco-lite/hasIssuingState">
        <rdfs:subPropertyOf rdf:resource="https://w3id.org/arco/ontology/arco-lite/hasRelatedAgent"/>
        <owl:inverseOf rdf:resource="https://w3id.org/arco/ontology/arco-lite/isIssuingStateIn"/>
        <rdfs:domain rdf:resource="https://w3id.org/arco/ontology/arco-lite/CoinIssuance"/>
        <rdfs:range rdf:resource="https://w3id.org/italia/onto/l0/Agent"/>
        <rdfs:comment xml:lang="it">Questa proprietà collega l&apos;emissione della moneta alla realtà statuale emittente, coeva all&apos;emissione della moneta. Questa proprietà, esprimendo il significato della relazione nel nome, dà una rappresentazione semplificata della relazione che lega questa entità e l&apos;agente; la stessa relazione è rappresentata attraverso una n-ary relation, arco-core:AgentRole, che permette di collegare l&apos;agente al ruolo che riveste nei confronti dell&apos;entità.</rdfs:comment>
        <rdfs:comment xml:lang="en">This property relates the coin issuance to the issuing State of that historic period. In the ontology this relationship is modelled also by the class AgentRole which allows more expressiveness.</rdfs:comment>
        <rdfs:isDefinedBy rdf:resource="https://w3id.org/arco/ontology/arco-lite"/>
        <rdfs:label xml:lang="it">ha Stato emittente</rdfs:label>
        <rdfs:label xml:lang="en">has issuing State</rdfs:label>
        <owl:versionInfo xml:lang="it">instabile</owl:versionInfo>
        <owl:versionInfo xml:lang="en">unstable</owl:versionInfo>
        <a-cat:iccdNormTag xml:lang="it">ICCD Normativa NU: DA/AUE/AUES - ICCD Normativa OA (dopo il rilascio della specifica scheda NU nel 2004 la scheda OA non è stata più utilizzata per la catalogazione di monete e medaglie): AU/EDT/EDTA</a-cat:iccdNormTag>
    </owl:ObjectProperty>



    <!-- https://w3id.org/arco/ontology/arco-lite/hasIssuingState -->

    <owl:ObjectProperty rdf:about="https://w3id.org/arco/ontology/arco-lite/hasIssuingState">
        <owl:inverseOf rdf:resource="https://w3id.org/arco/ontology/arco-liten/isIssuingStateIn"/>
    </owl:ObjectProperty>



    <!-- https://w3id.org/arco/ontology/arco-lite/hasLustre -->

    <owl:ObjectProperty rdf:about="https://w3id.org/arco/ontology/arco-lite/hasLustre">
        <rdfs:subPropertyOf rdf:resource="https://w3id.org/arco/ontology/arco-lite/hasPhysicalCharacteristic"/>
        <owl:inverseOf rdf:resource="https://w3id.org/arco/ontology/arco-lite/isLustreOf"/>
        <rdfs:domain rdf:resource="http://www.w3.org/2002/07/owl#Thing"/>
        <rdfs:range rdf:resource="https://w3id.org/arco/ontology/natural-specimen-description/PhysicalCharacteristic"/>
        <rdfs:comment xml:lang="it">Questa proprietà collega un entità alla lucentezza</rdfs:comment>
        <rdfs:comment xml:lang="en">This property relates an entity to the lustre</rdfs:comment>
        <rdfs:isDefinedBy rdf:resource="https://w3id.org/arco/ontology/arco-lite"/>
        <rdfs:label xml:lang="it">ha lucentezza</rdfs:label>
        <rdfs:label xml:lang="en">has lustre</rdfs:label>
        <owl:versionInfo xml:lang="it">instabile</owl:versionInfo>
        <owl:versionInfo xml:lang="en">unstable</owl:versionInfo>
        <a-cat:iccdNormTag>Normativa ICCD BNM: SM/SMF/SMFB</a-cat:iccdNormTag>
    </owl:ObjectProperty>



    <!-- https://w3id.org/arco/ontology/arco-lite/hasMagnetism -->

    <owl:ObjectProperty rdf:about="https://w3id.org/arco/ontology/arco-lite/hasMagnetism">
        <rdfs:subPropertyOf rdf:resource="https://w3id.org/arco/ontology/arco-lite/hasPhysicalCharacteristic"/>
        <owl:inverseOf rdf:resource="https://w3id.org/arco/ontology/arco-lite/isMagnetismOf"/>
        <rdfs:domain rdf:resource="http://www.w3.org/2002/07/owl#Thing"/>
        <rdfs:range rdf:resource="https://w3id.org/arco/ontology/natural-specimen-description/PhysicalCharacteristic"/>
        <rdfs:comment xml:lang="it">Questa proprietà collega un entità al magnetismo</rdfs:comment>
        <rdfs:comment xml:lang="en">This property relates an entity to the magnetismo</rdfs:comment>
        <rdfs:isDefinedBy rdf:resource="https://w3id.org/arco/ontology/arco-lite"/>
        <rdfs:label xml:lang="it">ha magnetismo</rdfs:label>
        <rdfs:label xml:lang="en">has magnetism</rdfs:label>
        <owl:versionInfo xml:lang="it">instabile</owl:versionInfo>
        <owl:versionInfo xml:lang="en">unstable</owl:versionInfo>
        <a-cat:iccdNormTag>Normativa ICCD BNM: SM/SMF/SMFM</a-cat:iccdNormTag>
    </owl:ObjectProperty>



    <!-- https://w3id.org/arco/ontology/arco-lite/hasMaterial -->

    <owl:ObjectProperty rdf:about="https://w3id.org/arco/ontology/arco-lite/hasMaterial">
        <owl:inverseOf rdf:resource="https://w3id.org/arco/ontology/arco-lite/isMaterialOf"/>
        <rdfs:domain rdf:resource="http://www.w3.org/2002/07/owl#Thing"/>
        <rdfs:range rdf:resource="https://w3id.org/arco/ontology/denotative-description/TechnicalCharacteristic"/>
        <rdfs:comment xml:lang="it">Questa proprietà collega un&apos;entità al materiale di cui è fatta.</rdfs:comment>
        <rdfs:comment xml:lang="en">This property relates an entity with its material.</rdfs:comment>
        <rdfs:isDefinedBy rdf:resource="https://w3id.org/arco/ontology/arco-lite"/>
        <rdfs:label xml:lang="it">ha materiale</rdfs:label>
        <rdfs:label xml:lang="en">has material</rdfs:label>
        <owl:versionInfo xml:lang="it">instabile</owl:versionInfo>
        <owl:versionInfo xml:lang="en">unstable</owl:versionInfo>
        <a-cat:iccdNormTag xml:lang="it">ICCD Normativa A 3.00: SVCM, FNSM</a-cat:iccdNormTag>
    </owl:ObjectProperty>



    <!-- https://w3id.org/arco/ontology/arco-lite/hasMaterialOrTechnicque -->

    <owl:ObjectProperty rdf:about="https://w3id.org/arco/ontology/arco-lite/hasMaterialOrTechnicque">
        <owl:inverseOf rdf:resource="https://w3id.org/arco/ontology/arco-lite/isMaterialOrTechniqueOf"/>
        <rdfs:domain rdf:resource="http://www.w3.org/2002/07/owl#Thing"/>
        <rdfs:range rdf:resource="https://w3id.org/arco/ontology/denotative-description/TechnicalCharacteristic"/>
        <rdfs:comment xml:lang="it">Questa proprietà collega un oggetto alla materia e/o la tecnica con cui è realizzato l&apos;oggetto, per esempio un bene culturale. Nel dominio delle normative  ICCD per la catalogazione dei beni culturali, si rende necessaria nei casi in cui materia e tecnica sono registrate nello stesso campo, nella forma &quot;materia/ tecnica&quot;.</rdfs:comment>
        <rdfs:comment xml:lang="en">This property relates an object to the material or technique through which an object has been realized, e.g. a cultural entity. In ICCD standards for cataloguing cultural entities, this label is necessary when material and technique are registered in the same field.</rdfs:comment>
        <rdfs:isDefinedBy rdf:resource="https://w3id.org/arco/ontology/arco-lite"/>
        <rdfs:label xml:lang="it">ha materia e tecnica</rdfs:label>
        <rdfs:label xml:lang="en">has material or technique</rdfs:label>
        <owl:versionInfo xml:lang="it">instabile</owl:versionInfo>
        <owl:versionInfo xml:lang="en">unstable</owl:versionInfo>
    </owl:ObjectProperty>



    <!-- https://w3id.org/arco/ontology/arco-lite/hasMeasuredDensity -->

    <owl:ObjectProperty rdf:about="https://w3id.org/arco/ontology/arco-lite/hasMeasuredDensity">
        <rdfs:subPropertyOf rdf:resource="https://w3id.org/arco/ontology/arco-lite/hasPhysicalCharacteristic"/>
        <owl:inverseOf rdf:resource="https://w3id.org/arco/ontology/arco-lite/isMeasuredDensity"/>
        <rdfs:domain rdf:resource="http://www.w3.org/2002/07/owl#Thing"/>
        <rdfs:range rdf:resource="https://w3id.org/arco/ontology/natural-specimen-description/PhysicalCharacteristic"/>
        <rdfs:comment xml:lang="it">Questa proprietà collega un entità alla densità misurata</rdfs:comment>
        <rdfs:comment xml:lang="en">This property relates an entity to the measured density</rdfs:comment>
        <rdfs:isDefinedBy rdf:resource="https://w3id.org/arco/ontology/arco-lite"/>
        <rdfs:label xml:lang="it">ha densità misurata</rdfs:label>
        <rdfs:label xml:lang="en">has measured density</rdfs:label>
        <owl:versionInfo xml:lang="it">instabile</owl:versionInfo>
        <owl:versionInfo xml:lang="en">unstable</owl:versionInfo>
        <a-cat:iccdNormTag>Normativa ICCD BNM: SM/SMF/SMFD</a-cat:iccdNormTag>
    </owl:ObjectProperty>



    <!-- https://w3id.org/arco/ontology/arco-lite/hasMint -->

    <owl:ObjectProperty rdf:about="https://w3id.org/arco/ontology/arco-lite/hasMint">
        <rdfs:subPropertyOf rdf:resource="https://w3id.org/arco/ontology/arco-lite/hasRelatedAgent"/>
        <owl:inverseOf rdf:resource="https://w3id.org/arco/ontology/arco-lite/isMintIn"/>
        <rdfs:domain rdf:resource="https://w3id.org/arco/ontology/context-description/CoinIssuance"/>
        <rdfs:range rdf:resource="https://w3id.org/italia/onto/l0/Agent"/>
        <rdfs:comment xml:lang="it">Questa proprietà collega l&apos;emissione della moneta alla Zecca. Questa proprietà, esprimendo il significato della relazione nel nome, dà una rappresentazione semplificata della relazione che lega questa entità e l&apos;agente; la stessa relazione è rappresentata attraverso una n-ary relation, arco-core:AgentRole, che permette di collegare l&apos;agente al ruolo che riveste nei confronti dell&apos;entità.</rdfs:comment>
        <rdfs:comment xml:lang="en">This property relates the coin issuance to the Mint. In the ontology this relationship is modelled also by the class AgentRole which allows more expressiveness.</rdfs:comment>
        <rdfs:isDefinedBy rdf:resource="https://w3id.org/arco/ontology/arco-lite"/>
        <rdfs:label xml:lang="it">ha zecca</rdfs:label>
        <rdfs:label xml:lang="en">has mint</rdfs:label>
        <owl:versionInfo xml:lang="it">instabile</owl:versionInfo>
        <owl:versionInfo xml:lang="en">unstable</owl:versionInfo>
        <a-cat:iccdNormTag xml:lang="it">ICCD Normativa NU: DA/ZEC - ICCD Normativa OA (dopo il rilascio della specifica scheda NU nel 2004 la scheda OA non è stata più utilizzata per la catalogazione di monete e medaglie): AU/EDT/EDTZ</a-cat:iccdNormTag>
    </owl:ObjectProperty>



    <!-- https://w3id.org/arco/ontology/arco-lite/hasMinter -->

    <owl:ObjectProperty rdf:about="https://w3id.org/arco/ontology/arco-lite/hasMinter">
        <rdfs:subPropertyOf rdf:resource="https://w3id.org/arco/ontology/arco-lite/hasRelatedAgent"/>
        <owl:inverseOf rdf:resource="https://w3id.org/arco/ontology/arco-lite/isMinterIn"/>
        <rdfs:domain rdf:resource="https://w3id.org/arco/ontology/context-description/CoinIssuance"/>
        <rdfs:range rdf:resource="https://w3id.org/italia/onto/l0/Agent"/>
        <rdfs:comment xml:lang="it">Questa proprietà collega l&apos;emissione della moneta allo zecchiere, monetiere, maestro di zecca. Questa proprietà, esprimendo il significato della relazione nel nome, dà una rappresentazione semplificata della relazione che lega questa entità e l&apos;agente; la stessa relazione è rappresentata attraverso una n-ary relation, arco-core:AgentRole, che permette di collegare l&apos;agente al ruolo che riveste nei confronti dell&apos;entità.</rdfs:comment>
        <rdfs:comment xml:lang="en">This property relates the coin issuance to the minter. In the ontology this relationship is modelled also by the class AgentRole which allows more expressiveness.</rdfs:comment>
        <rdfs:isDefinedBy rdf:resource="https://w3id.org/arco/ontology/arco-lite"/>
        <rdfs:label xml:lang="it">ha zecchiere</rdfs:label>
        <rdfs:label xml:lang="en">has minter</rdfs:label>
        <owl:versionInfo xml:lang="it">instabile</owl:versionInfo>
        <owl:versionInfo xml:lang="en">unstable</owl:versionInfo>
        <a-cat:iccdNormTag>ICCD Normativa NU: DA/AUE/AUEZ</a-cat:iccdNormTag>
    </owl:ObjectProperty>



    <!-- https://w3id.org/arco/ontology/arco-lite/hasMohsHardness -->

    <owl:ObjectProperty rdf:about="https://w3id.org/arco/ontology/arco-lite/hasMohsHardness">
        <rdfs:subPropertyOf rdf:resource="https://w3id.org/arco/ontology/arco-lite/hasPhysicalCharacteristic"/>
        <owl:inverseOf rdf:resource="https://w3id.org/arco/ontology/arco-lite/isMohsHardnessOf"/>
        <rdfs:domain rdf:resource="http://www.w3.org/2002/07/owl#Thing"/>
        <rdfs:range rdf:resource="https://w3id.org/arco/ontology/natural-specimen-description/PhysicalCharacteristic"/>
        <rdfs:comment xml:lang="it">Questa proprietà collega un entità alla durezza secondo la scala di Mohs</rdfs:comment>
        <rdfs:comment xml:lang="en">This property relates an entity to the hardness, according to the Mohs scale </rdfs:comment>
        <rdfs:isDefinedBy rdf:resource="https://w3id.org/arco/ontology/arco-lite"/>
        <rdfs:label xml:lang="it">ha durezza secondo la scala di Mohs</rdfs:label>
        <rdfs:label xml:lang="en">has Mohs scale hardness</rdfs:label>
        <owl:versionInfo xml:lang="it">instabile</owl:versionInfo>
        <owl:versionInfo xml:lang="en">unstable</owl:versionInfo>
        <a-cat:iccdNormTag>Normativa ICCD BNM: SM/SMF/SMFH</a-cat:iccdNormTag>
    </owl:ObjectProperty>



    <!-- https://w3id.org/arco/ontology/arco-lite/hasMusicalEnsemble -->

    <owl:ObjectProperty rdf:about="https://w3id.org/arco/ontology/arco-lite/hasMusicalEnsemble">
        <rdfs:subPropertyOf rdf:resource="https://w3id.org/arco/ontology/arco-lite/hasRelatedAgent"/>
        <owl:inverseOf rdf:resource="https://w3id.org/arco/ontology/arco-lite/isMusicalEnsembleOf"/>
        <rdfs:domain rdf:resource="http://dati.beniculturali.it/cis/CulturalEntity"/>
        <rdfs:range rdf:resource="https://w3id.org/italia/onto/l0/Agent"/>
        <rdfs:comment xml:lang="it">Questa proprietà collega uno strumento musicale al gruppo di musicisti (bande, complessi musicali, associazioni corali, ecc.) in cui lo strumento assume, o ha assunto, abitualmente un ruolo esecutivo. Questa relazione è modellata anche, con maggiore potere espressivo, tramite il pattern AgentRole, che collega lo strumento musicale a una situazione in cui un agente ha rivestito un ruolo (in questo caso, organico musicale).</rdfs:comment>
        <rdfs:comment xml:lang="en">This property relates a musical instrument to the musical ensemble that played it. In the ontology this relationship is modelled also by the class AgentRole which allows more expressiveness.</rdfs:comment>
        <rdfs:isDefinedBy rdf:resource="https://w3id.org/arco/ontology/arco-lite"/>
        <rdfs:label xml:lang="it">ha organico musicale</rdfs:label>
        <rdfs:label xml:lang="en">has musical ensemble</rdfs:label>
        <owl:versionInfo xml:lang="it">instabile</owl:versionInfo>
        <owl:versionInfo xml:lang="en">unstable</owl:versionInfo>
        <a-cat:iccdNormTag>ICCD Normativa SM 4.00: OS/OSD</a-cat:iccdNormTag>
    </owl:ObjectProperty>



    <!-- https://w3id.org/arco/ontology/arco-lite/hasMusicalTemperament -->

    <owl:ObjectProperty rdf:about="https://w3id.org/arco/ontology/arco-lite/hasMusicalTemperament">
        <rdfs:subPropertyOf rdf:resource="https://w3id.org/arco/ontology/denotative-description/hasTechnicalCharacteristic"/>
        <owl:inverseOf rdf:resource="https://w3id.org/arco/ontology/arco-lite/isMusicalTemperamentOf"/>
        <rdfs:domain rdf:resource="http://www.w3.org/2002/07/owl#Thing"/>
        <rdfs:range rdf:resource="https://w3id.org/arco/ontology/denotative-description/TechnicalCharacteristic"/>
        <rdfs:comment xml:lang="it">Questa proprietà collega uno strumento al temperamento adottato, soprattutto in caso di oggetto in condizioni originali, o dopo un restauro, dello strumento musicale. Per gli idiofoni a tasti fissi (come xilofoni, litofoni, metallofoni) rappresenta la successione degli intervalli.</rdfs:comment>
        <rdfs:comment xml:lang="en">This property relates a musical instrument to the adopted temperament, especially in relation to an object in its original conditions, or after its restoration. For idiophones with fixed keys (e.g. xylophone, litophone, metallophone) the temperament represents the succession of intervals.</rdfs:comment>
        <rdfs:isDefinedBy rdf:resource="https://w3id.org/arco/ontology/arco-lite"/>
        <rdfs:label xml:lang="it">ha temperamento</rdfs:label>
        <rdfs:label xml:lang="en">has musical temperament</rdfs:label>
        <owl:versionInfo xml:lang="it">instabile</owl:versionInfo>
        <owl:versionInfo xml:lang="en">unstable</owl:versionInfo>
        <a-cat:iccdNormTag>ICCD Normativa SM 4.00: AA/AAP</a-cat:iccdNormTag>
    </owl:ObjectProperty>



    <!-- https://w3id.org/arco/ontology/arco-lite/hasMusician -->

    <owl:ObjectProperty rdf:about="https://w3id.org/arco/ontology/arco-lite/hasMusician">
        <rdfs:subPropertyOf rdf:resource="https://w3id.org/arco/ontology/arco-lite/hasRelatedAgent"/>
        <owl:inverseOf rdf:resource="https://w3id.org/arco/ontology/arco-lite/isMusicianOf"/>
        <rdfs:domain rdf:resource="http://dati.beniculturali.it/cis/CulturalEntity"/>
        <rdfs:range rdf:resource="https://w3id.org/italia/onto/l0/Agent"/>
        <rdfs:comment xml:lang="it">Questa proprietà collega uno strumento musicale a una persona che assume - o ha assunto - un ruolo certo come esecutore dello strumento. Questa relazione è modellata anche, con maggiore potere espressivo, tramite il pattern AgentRole, che collega lo strumento musicale a una situazione in cui un agente ha rivestito un ruolo (in questo caso, chitarrista, flautista, pianista, ecc., o genericamente musicista).</rdfs:comment>
        <rdfs:comment xml:lang="en">This property relates a musical instrument to the person who plays (in the present or past) a certain role as the instrument&apos;s exectutor. In the ontology this relationship is modelled also by the class AgentRole which allows more expressiveness.</rdfs:comment>
        <rdfs:isDefinedBy rdf:resource="https://w3id.org/arco/ontology/arco-lite"/>
        <rdfs:label xml:lang="it">ha musicista</rdfs:label>
        <rdfs:label xml:lang="en">has musician</rdfs:label>
        <owl:versionInfo xml:lang="it">instabile</owl:versionInfo>
        <owl:versionInfo xml:lang="en">unstable</owl:versionInfo>
        <a-cat:iccdNormTag>ICCD Normativa SM 4.00: MU/MUTN</a-cat:iccdNormTag>
    </owl:ObjectProperty>



    <!-- https://w3id.org/arco/ontology/arco-lite/hasOfficialInCharge -->

    <owl:ObjectProperty rdf:about="https://w3id.org/arco/ontology/arco-lite/hasOfficialInCharge">
        <rdfs:subPropertyOf rdf:resource="https://w3id.org/arco/ontology/arco-lite/hasRelatedAgent"/>
        <owl:inverseOf rdf:resource="https://w3id.org/arco/ontology/arco-lite/isOfficialInChargeOf"/>
        <rdfs:domain>
            <owl:Class>
                <owl:unionOf rdf:parseType="Collection">
                    <rdf:Description rdf:about="https://w3id.org/arco/ontology/catalogue/CatalogueRecord"/>
                    <rdf:Description rdf:about="https://w3id.org/arco/ontology/catalogue/CatalogueRecordVersion"/>
                </owl:unionOf>
            </owl:Class>
        </rdfs:domain>
        <rdfs:range rdf:resource="https://w3id.org/italia/onto/l0/Agent"/>
        <rdfs:comment xml:lang="it">Questa proprietà rappresenta la relazione che collega la prima versione di una scheda di catalogo al relativo funzionario responsabile. La relazione tra il ruolo e l&apos;ente che lo riveste è espressa nel nome della proprietà, che quindi ne fornisce una rappresentazione semplificata, con ridotta espressività. Nell&apos;ontologia questa relazione è modellata anche, in maniera più espressiva, dalla classe TimeIndexedRole, che permette di collegare l&apos;ente, il suo ruolo e la sua corrispondente estensione temporale.</rdfs:comment>
        <rdfs:isDefinedBy rdf:resource="https://w3id.org/arco/ontology/arco-lite"/>
        <rdfs:label xml:lang="it">ha funzionario responsabile</rdfs:label>
        <rdfs:label xml:lang="en">has official in charge</rdfs:label>
        <owl:versionInfo xml:lang="it">instabile</owl:versionInfo>
        <owl:versionInfo xml:lang="en">unstable</owl:versionInfo>
        <iccdNormTag>ICCD Normativa Trasvesale 4.00: CM/FUR, CM/AGG/AGGF</iccdNormTag>
    </owl:ObjectProperty>



    <!-- https://w3id.org/arco/ontology/arco-lite/hasOperator -->

    <owl:ObjectProperty rdf:about="https://w3id.org/arco/ontology/arco-lite/hasOperator">
        <rdfs:subPropertyOf rdf:resource="https://w3id.org/arco/ontology/arco-lite/hasRelatedAgent"/>
        <owl:inverseOf rdf:resource="https://w3id.org/arco/ontology/arco-lite/isOperatorOf"/>
        <rdfs:domain>
            <owl:Class>
                <owl:unionOf rdf:parseType="Collection">
                    <rdf:Description rdf:about="https://w3id.org/italia/onto/l0/Activity"/>
                    <rdf:Description rdf:about="https://w3id.org/italia/onto/l0/Object"/>
                </owl:unionOf>
            </owl:Class>
        </rdfs:domain>
        <rdfs:range rdf:resource="https://w3id.org/italia/onto/l0/Agent"/>
        <rdfs:comment xml:lang="it">Questa proprietà collega un&apos;attività (per esempio, un&apos;indagine o un intervento su un bene culturale) all&apos;operatore dell&apos;attività. La relazione tra il ruolo e l&apos;agente che lo riveste è espressa nel nome della proprietà, che quindi ne fornisce una rappresentazione semplificata, con ridotta espressività. Nell&apos;ontologia questa relazione è modellata anche, in maniera più espressiva, dalla classe AgentRole, che permette di collegare l&apos;agente e il suo ruolo.</rdfs:comment>
        <rdfs:comment xml:lang="en">This property relates an activity to the agent who performed the activity. In the ontology this relationship is modelled also by the class AgentRole which allows more expressiveness.</rdfs:comment>
        <rdfs:isDefinedBy rdf:resource="https://w3id.org/arco/ontology/arco-lite"/>
        <rdfs:label xml:lang="it">ha operatore</rdfs:label>
        <rdfs:label xml:lang="en">has operator</rdfs:label>
        <owl:versionInfo xml:lang="it">instabile</owl:versionInfo>
        <owl:versionInfo xml:lang="en">unstable</owl:versionInfo>
        <a-cat:iccdNormTag xml:lang="it">ICCD Normativa Trasversale: RE/IND/INDN; CO/RST/RSTN - ICCD Normativa SM e BDM 4.00: DR/DRL - ICCD normative di versioni precedenti: RE/AIN/AINR. RS/ALB/ALBO; CO/ALB/ALBO. Normativa BNB: RB/RBR/RBRA</a-cat:iccdNormTag>
    </owl:ObjectProperty>



    <!-- https://w3id.org/arco/ontology/arco-lite/hasOpticalPhenomena -->

    <owl:ObjectProperty rdf:about="https://w3id.org/arco/ontology/arco-lite/hasOpticalPhenomena">
        <rdfs:subPropertyOf rdf:resource="https://w3id.org/arco/ontology/arco-lite/hasPhysicalCharacteristic"/>
        <owl:inverseOf rdf:resource="https://w3id.org/arco/ontology/arco-lite/isOpticalPhenomenaOf"/>
        <rdfs:domain rdf:resource="http://www.w3.org/2002/07/owl#Thing"/>
        <rdfs:range rdf:resource="https://w3id.org/arco/ontology/natural-specimen-description/PhysicalCharacteristic"/>
        <rdfs:comment xml:lang="it">Questa proprietà collega un entità al fenomeno ottico</rdfs:comment>
        <rdfs:comment xml:lang="en">This property relates an entity to the optical phenomena</rdfs:comment>
        <rdfs:isDefinedBy rdf:resource="https://w3id.org/arco/ontology/arco-lite"/>
        <rdfs:label xml:lang="it">ha fenomeno ottico</rdfs:label>
        <rdfs:label xml:lang="en">has optical phenomena</rdfs:label>
        <owl:versionInfo xml:lang="it">instabile</owl:versionInfo>
        <owl:versionInfo xml:lang="en">unstable</owl:versionInfo>
        <a-cat:iccdNormTag>Normativa ICCD BNM: SM/SMF/SMFO</a-cat:iccdNormTag>
    </owl:ObjectProperty>



    <!-- https://w3id.org/arco/ontology/arco-lite/hasOpticCharacteristic -->

    <owl:ObjectProperty rdf:about="https://w3id.org/arco/ontology/arco-lite/hasOpticCharacteristic">
      <rdfs:subPropertyOf rdf:resource="https://w3id.org/arco/ontology/arco-lite/hasPhysicalCharacteristic"/>
        <owl:inverseOf rdf:resource="https://w3id.org/arco/ontology/arco-lite/isOpticCharacteristicOf"/>
        <rdfs:domain rdf:resource="http://www.w3.org/2002/07/owl#Thing"/>
        <rdfs:range rdf:resource="https://w3id.org/arco/ontology/natural-specimen-description/OpticCharacteristic"/>
        <rdfs:comment xml:lang="it">Questa proprietà collega un entità a una caratteristica ottica</rdfs:comment>
        <rdfs:comment xml:lang="en">This property relates an entity to the optic characteristic</rdfs:comment>
        <rdfs:isDefinedBy rdf:resource="https://w3id.org/arco/ontology/arco-lite"/>
        <rdfs:label xml:lang="it">ha caratteristica ottica</rdfs:label>
        <rdfs:label xml:lang="en">has optic characteristic</rdfs:label>
        <owl:versionInfo xml:lang="it">instabile</owl:versionInfo>
        <owl:versionInfo xml:lang="en">unstable</owl:versionInfo>
    </owl:ObjectProperty>



    <!-- https://w3id.org/arco/ontology/arco-lite/hasOwner -->

    <owl:ObjectProperty rdf:about="https://w3id.org/arco/ontology/arco-lite/hasOwner">
        <rdfs:subPropertyOf rdf:resource="https://w3id.org/arco/ontology/arco-lite/hasRelatedAgent"/>
        <owl:inverseOf rdf:resource="https://w3id.org/arco/ontology/arco-lite/isOwnerOf"/>
        <rdfs:domain rdf:resource="http://www.w3.org/2002/07/owl#Thing"/>
        <rdfs:range rdf:resource="https://w3id.org/italia/onto/l0/Agent"/>
        <rdfs:comment xml:lang="it">Questa proprietà collega un&apos;oggetto al suo proprietario .</rdfs:comment>
        <rdfs:comment xml:lang="en">This property relates an object to its owner.</rdfs:comment>
        <rdfs:isDefinedBy rdf:resource="https://w3id.org/arco/ontology/arco-lite"/>
        <rdfs:label xml:lang="it">ha proprietario</rdfs:label>
        <rdfs:label xml:lang="en">has owner</rdfs:label>
        <owl:versionInfo xml:lang="it">instabile</owl:versionInfo>
        <owl:versionInfo xml:lang="en">unstable</owl:versionInfo>
        <a-cat:iccdNormTag>ICCD Normativa Trasversale 4.00: TU/CDG/CDGS</a-cat:iccdNormTag>
    </owl:ObjectProperty>



    <!-- https://w3id.org/arco/ontology/arco-lite/hasPhosphorescence -->

    <owl:ObjectProperty rdf:about="https://w3id.org/arco/ontology/arco-lite/hasPhosphorescence">
        <rdfs:subPropertyOf rdf:resource="https://w3id.org/arco/ontology/arco-lite/hasPhysicalCharacteristic"/>
        <owl:inverseOf rdf:resource="https://w3id.org/arco/ontology/arco-lite/isPhosphorescenceOf"/>
        <rdfs:domain rdf:resource="http://www.w3.org/2002/07/owl#Thing"/>
        <rdfs:range rdf:resource="https://w3id.org/arco/ontology/natural-specimen-description/PhysicalCharacteristic"/>
        <rdfs:comment xml:lang="it">Questa proprietà collega un entità alla fosforescenza</rdfs:comment>
        <rdfs:comment xml:lang="en">This property relates an entity to the phosphorescence</rdfs:comment>
        <rdfs:isDefinedBy rdf:resource="https://w3id.org/arco/ontology/arco-lite"/>
        <rdfs:label xml:lang="it">ha fosforescenza</rdfs:label>
        <rdfs:label xml:lang="en">has phosphorescence</rdfs:label>
        <owl:versionInfo xml:lang="it">instabile</owl:versionInfo>
        <owl:versionInfo xml:lang="en">unstable</owl:versionInfo>
        <a-cat:iccdNormTag>Normativa ICCD BNM: SM/SMF/SMFS</a-cat:iccdNormTag>
    </owl:ObjectProperty>



    <!-- https://w3id.org/arco/ontology/arco-lite/hasPhotoColour -->

    <owl:ObjectProperty rdf:about="https://w3id.org/arco/ontology/arco-lite/hasPhotoColour">
        <rdfs:subPropertyOf rdf:resource="https://w3id.org/arco/ontology/denotative-description/hasTechnicalCharacteristic"/>
        <owl:inverseOf rdf:resource="https://w3id.org/arco/ontology/arco-lite/isPhotoColourOf"/>
        <rdfs:domain rdf:resource="http://www.w3.org/2002/07/owl#Thing"/>
        <rdfs:range rdf:resource="https://w3id.org/arco/ontology/denotative-description/TechnicalCharacteristic"/>
        <rdfs:comment xml:lang="it">Questo individuo collega una fotografia digitale al colore della fotografia digitale, ovvero se trattasi di fotografia in bianco/nero o a colori.</rdfs:comment>
        <rdfs:comment xml:lang="en">This property relates a digital photograph to its colour, i.e. black and white or colours.</rdfs:comment>
        <rdfs:isDefinedBy rdf:resource="https://w3id.org/arco/ontology/arco-lite"/>
        <rdfs:label xml:lang="it">ha colore della foto</rdfs:label>
        <rdfs:label xml:lang="en">has photo colour</rdfs:label>
        <owl:versionInfo xml:lang="it">instabile</owl:versionInfo>
        <owl:versionInfo xml:lang="en">unstable</owl:versionInfo>
    </owl:ObjectProperty>



    <!-- https://w3id.org/arco/ontology/arco-lite/hasPhotoSize -->

    <owl:ObjectProperty rdf:about="https://w3id.org/arco/ontology/arco-lite/hasPhotoSize">
        <rdfs:subPropertyOf rdf:resource="https://w3id.org/arco/ontology/denotative-description/hasTechnicalCharacteristic"/>
        <owl:inverseOf rdf:resource="https://w3id.org/arco/ontology/arco-lite/isPhotoSizeOf"/>
        <rdfs:domain rdf:resource="http://www.w3.org/2002/07/owl#Thing"/>
        <rdfs:range rdf:resource="https://w3id.org/arco/ontology/denotative-description/TechnicalCharacteristic"/>
        <rdfs:comment xml:lang="it">Questa proprietà collega una risorsa digitale al formato della risorsa, inteso come la dimensione standardizzata (es.: per i materiali fotografici negativi, positivi, ecc.).</rdfs:comment>
        <rdfs:comment xml:lang="en">This property relates a digital photograph to its format, intended as the photographic material&apos;s standardised size (e.g. negative, positives).</rdfs:comment>
        <rdfs:isDefinedBy rdf:resource="https://w3id.org/arco/ontology/arco-lite"/>
        <rdfs:label xml:lang="it">ha dimensioni della foto</rdfs:label>
        <rdfs:label xml:lang="en">has photo size</rdfs:label>
        <owl:versionInfo xml:lang="it">instabile</owl:versionInfo>
        <owl:versionInfo xml:lang="en">unstable</owl:versionInfo>
    </owl:ObjectProperty>



    <!-- https://w3id.org/arco/ontology/arco-lite/hasPhotographer -->

    <owl:ObjectProperty rdf:about="https://w3id.org/arco/ontology/arco-lite/hasPhotographer">
        <rdfs:subPropertyOf rdf:resource="https://w3id.org/arco/ontology/arco-lite/hasRelatedAgent"/>
        <owl:inverseOf rdf:resource="https://w3id.org/arco/ontology/arco-lite/isPhotographerOf"/>
        <rdfs:domain rdf:resource="https://w3id.org/arco/ontology/context-description/ObservationSurvey"/>
        <rdfs:range rdf:resource="https://w3id.org/italia/onto/l0/Agent"/>
        <rdfs:comment xml:lang="it">Questa proprietà collega un&apos;indagine di rilevamento di un bene demo-etno-antropologico al fotografo professionista (diverso dal rilevatore) che ha effettuato la ripresa. La relazione tra il ruolo e l&apos;agente che lo riveste è espressa nel nome della proprietà, che quindi ne fornisce una rappresentazione semplificata, con ridotta espressività. Nell&apos;ontologia questa relazione è modellata anche, in maniera più espressiva, dalla classe AgentRole, che permette di collegare l&apos;agente e il suo ruolo.</rdfs:comment>
        <rdfs:comment xml:lang="en">This property relates an observation survey of a demo-etno-antropologic entity to the professional photographer who took the shot. In the ontology this relationship is modelled also by the class AgentRole which allows more expressiveness.</rdfs:comment>
        <rdfs:isDefinedBy rdf:resource="https://w3id.org/arco/ontology/arco-lite"/>
        <rdfs:label xml:lang="it">ha fotografo</rdfs:label>
        <rdfs:label xml:lang="en">has photographer</rdfs:label>
        <owl:versionInfo xml:lang="it">instabile</owl:versionInfo>
        <owl:versionInfo xml:lang="en">unstable</owl:versionInfo>
        <a-cat:iccdNormTag>ICCD Normativa BDI 3.00: DR/DRG</a-cat:iccdNormTag>
    </owl:ObjectProperty>



    <!-- https://w3id.org/arco/ontology/arco-lite/hasPhysicalCharacteristic -->

    <owl:ObjectProperty rdf:about="https://w3id.org/arco/ontology/arco-lite/hasPhysicalCharacteristic">
        <rdfs:subPropertyOf rdf:resource="https://w3id.org/arco/ontology/denotative-description/hasTechnicalCharacteristic"/>
        <owl:inverseOf rdf:resource="https://w3id.org/arco/ontology/arco-lite/isPhysicalCharacteristicOf"/>
        <rdfs:domain rdf:resource="http://www.w3.org/2002/07/owl#Thing"/>
        <rdfs:range rdf:resource="https://w3id.org/arco/ontology/natural-specimen-description/PhysicalCharacteristic"/>
        <rdfs:comment xml:lang="it">Questa proprietà collega un entità alla caratteristica fisica</rdfs:comment>
        <rdfs:comment xml:lang="en">This property relates an entity to the physical characteristic</rdfs:comment>
        <rdfs:isDefinedBy rdf:resource="https://w3id.org/arco/ontology/arco-lite"/>
        <rdfs:label xml:lang="it">ha caratteristica fisica</rdfs:label>
        <rdfs:label xml:lang="en">has physical characteristic</rdfs:label>
        <owl:versionInfo xml:lang="it">instabile</owl:versionInfo>
        <owl:versionInfo xml:lang="en">unstable</owl:versionInfo>
        <a-cat:iccdNormTag>Normativa ICCD BNM: SM/SMF</a-cat:iccdNormTag>
    </owl:ObjectProperty>



    <!-- https://w3id.org/arco/ontology/arco-lite/hasPixelDimension -->

    <owl:ObjectProperty rdf:about="https://w3id.org/arco/ontology/arco-lite/hasPixelDimension">
        <rdfs:subPropertyOf rdf:resource="https://w3id.org/arco/ontology/denotative-description/hasTechnicalCharacteristic"/>
        <owl:inverseOf rdf:resource="https://w3id.org/arco/ontology/arco-lite/isPixelDimensionOf"/>
        <rdfs:domain rdf:resource="http://www.w3.org/2002/07/owl#Thing"/>
        <rdfs:range rdf:resource="https://w3id.org/arco/ontology/denotative-description/TechnicalCharacteristic"/>
        <rdfs:comment xml:lang="it">Questa proprietà collega un&apos;immagine digitale (es.: fotografia) alle dimensioni, in pixel, dell&apos;immagine.</rdfs:comment>
        <rdfs:comment xml:lang="en">This property relates a digital resource to its size in pixels.</rdfs:comment>
        <rdfs:isDefinedBy rdf:resource="https://w3id.org/arco/ontology/arco-lite"/>
        <rdfs:label xml:lang="it">ha dimensioni in pixel</rdfs:label>
        <rdfs:label xml:lang="en">has pixel dimension</rdfs:label>
        <owl:versionInfo xml:lang="it">instabile</owl:versionInfo>
        <owl:versionInfo xml:lang="en">unstable</owl:versionInfo>
    </owl:ObjectProperty>



    <!-- https://w3id.org/arco/ontology/arco-lite/hasPleochroism -->

    <owl:ObjectProperty rdf:about="https://w3id.org/arco/ontology/arco-lite/hasPleochroism">
        <rdfs:subPropertyOf rdf:resource="https://w3id.org/arco/ontology/arco-lite/hasOpticCharacteristic"/>
        <owl:inverseOf rdf:resource="https://w3id.org/arco/ontology/arco-lite/isPleochroismOf"/>
        <rdfs:domain rdf:resource="http://www.w3.org/2002/07/owl#Thing"/>
        <rdfs:range rdf:resource="https://w3id.org/arco/ontology/natural-specimen-description/OpticCharacteristic"/>
        <rdfs:comment xml:lang="it">Questa proprietà collega il campione al pleocroismo</rdfs:comment>
        <rdfs:comment xml:lang="en">This property relates the specimen to the pleochroism</rdfs:comment>
        <rdfs:isDefinedBy rdf:resource="https://w3id.org/arco/ontology/arco-lite"/>
        <rdfs:label xml:lang="it">ha pleocroismo</rdfs:label>
        <rdfs:label xml:lang="en">has pleochroism</rdfs:label>
        <owl:versionInfo xml:lang="it">instabile</owl:versionInfo>
        <owl:versionInfo xml:lang="en">unstable</owl:versionInfo>
        <a-cat:iccdNormTag>SM/SMM/SMMP. SM/SMO/SMOP</a-cat:iccdNormTag>
    </owl:ObjectProperty>



    <!-- https://w3id.org/arco/ontology/arco-lite/hasPointGroup -->

    <owl:ObjectProperty rdf:about="https://w3id.org/arco/ontology/arco-lite/hasPointGroup">
        <rdfs:subPropertyOf rdf:resource="https://w3id.org/arco/ontology/arco-lite/hasCrystallographicCharacteristic"/>
        <owl:inverseOf rdf:resource="https://w3id.org/arco/ontology/natural-specimen-description/isPointGroupOf"/>
        <rdfs:domain rdf:resource="https://w3id.org/arco/ontology/natural-specimen-description/UnitCell"/>
        <rdfs:range rdf:resource="https://w3id.org/arco/ontology/natural-specimen-description/CrystallographicCharacteristic"/>
        <rdfs:comment xml:lang="it">Questa proprietà collega una cella al gruppo puntuale</rdfs:comment>
        <rdfs:comment xml:lang="en">This property relates a unit cell to the point group</rdfs:comment>
        <rdfs:isDefinedBy rdf:resource="https://w3id.org/arco/ontology/arco-lite"/>
        <rdfs:label xml:lang="it">ha gruppo puntuale</rdfs:label>
        <rdfs:label xml:lang="en">has point group</rdfs:label>
        <owl:versionInfo xml:lang="it">instabile</owl:versionInfo>
        <owl:versionInfo xml:lang="en">unstable</owl:versionInfo>
        <a-cat:iccdNormTag>Normativa ICCD BNM: SM/SMC/SMCP</a-cat:iccdNormTag>
    </owl:ObjectProperty>



    <!-- https://w3id.org/arco/ontology/arco-lite/hasPreferredAuthor -->

    <owl:ObjectProperty rdf:about="https://w3id.org/arco/ontology/arco-lite/hasPreferredAuthor">
        <owl:inverseOf rdf:resource="https://w3id.org/arco/ontology/arco-lite/isPreferredAuthorOf"/>
        <rdfs:domain rdf:resource="http://www.w3.org/2002/07/owl#Thing"/>
        <rdfs:range rdf:resource="https://w3id.org/italia/onto/l0/Agent"/>
    </owl:ObjectProperty>



    <!-- https://w3id.org/arco/ontology/arco-lite/hasPreviousLocation -->

    <owl:ObjectProperty rdf:about="https://w3id.org/arco/ontology/arco-lite/hasPreviousLocation">
        <rdfs:subPropertyOf rdf:resource="https://w3id.org/arco/ontology/arco-lite/hasRelatedWork"/>
        <owl:inverseOf rdf:resource="https://w3id.org/arco/ontology/arco-lite/isPreviousLocationOf"/>
        <rdfs:domain rdf:resource="http://www.w3.org/2002/07/owl#Thing"/>
        <rdfs:range rdf:resource="http://www.w3.org/2002/07/owl#Thing"/>
        <rdfs:comment xml:lang="it">Questa proprietà collega un bene culturale a un altro bene culturale collegato, che ne costituisce la sede di provenienza, prima della sua attuale collocazione.</rdfs:comment>
        <rdfs:comment xml:lang="en">This property relates a cultural entity to a connected cultural entity which constitutes its provenance location before its current position.</rdfs:comment>
        <rdfs:label xml:lang="it">era contenuto in</rdfs:label>
        <rdfs:label xml:lang="it">ha sede di provenienza</rdfs:label>
        <rdfs:label xml:lang="en">has previous location</rdfs:label>
        <owl:versionInfo xml:lang="it">instabili</owl:versionInfo>
        <owl:versionInfo xml:lang="en">unstable</owl:versionInfo>
        <a-cat:iccdNormTag xml:lang="it">ICCD Normativa Trasversale 4.00: RV/RSE/RSER = &apos;era contenuto in&apos; (versioni precedenti: &apos;sede di provenienza&apos;)</a-cat:iccdNormTag>
    </owl:ObjectProperty>



    <!-- https://w3id.org/arco/ontology/arco-lite/hasPreviousOwner -->

    <owl:ObjectProperty rdf:about="https://w3id.org/arco/ontology/arco-lite/hasPreviousOwner">
        <owl:inverseOf rdf:resource="https://w3id.org/arco/ontology/arco-lite/isPreviousOwnerOf"/>
        <rdfs:domain rdf:resource="http://www.w3.org/2002/07/owl#Thing"/>
        <rdfs:range rdf:resource="https://w3id.org/italia/onto/l0/Agent"/>
    </owl:ObjectProperty>



    <!-- https://w3id.org/arco/ontology/arco-lite/hasProponentAgency -->

    <owl:ObjectProperty rdf:about="https://w3id.org/arco/ontology/arco-lite/hasProponentAgency">
        <rdfs:subPropertyOf rdf:resource="https://w3id.org/arco/ontology/arco-lite/hasRelatedAgent"/>
        <owl:inverseOf rdf:resource="https://w3id.org/arco/ontology/arco-lite/isProponentAgencyOf"/>
        <rdfs:domain>
            <owl:Class>
                <owl:unionOf rdf:parseType="Collection">
                    <rdf:Description rdf:about="http://dati.beniculturali.it/cis/CulturalEntity"/>
                    <rdf:Description rdf:about="https://w3id.org/arco/ontology/context-description/ProtectiveMeasure"/>
                </owl:unionOf>
            </owl:Class>
        </rdfs:domain>
        <rdfs:range rdf:resource="https://w3id.org/italia/onto/l0/Agent"/>
        <rdfs:comment xml:lang="it">Questa proprietà collega un&apos;entità, che può essere direttamente il bene culturale o specificamente il provvedimento di tutela relativo al bene culturale, all&apos;ente proponente, ovvero al soggetto che ha proposto il provvedimento, identificato per mezzo della denominazione per esteso oppure, nel caso di Enti accreditati dall&apos;ICCD, del relativo codice assegnato dall&apos;Istituto. La relazione tra il ruolo e l&apos;agente che lo riveste è espressa, in maniera generica, nel nome della proprietà, che quindi ne fornisce una rappresentazione semplificata, con ridotta espressività. Nell&apos;ontologia questa relazione è modellata anche, in maniera più espressiva, dalla classe AgentRole, che permette di collegare l&apos;agente e il suo ruolo.</rdfs:comment>
        <rdfs:comment xml:lang="en">This property relates an entity (e.g a cultural entity or a cultual entity&apos;s protective measure) to the proposing institution. In the ontology this relationship is modelled also by the class AgentRole which allows more expressiveness.</rdfs:comment>
        <rdfs:isDefinedBy rdf:resource="https://w3id.org/arco/ontology/arco-lite"/>
        <rdfs:label xml:lang="it">ha ente proponente</rdfs:label>
        <rdfs:label xml:lang="en">has proponet agency</rdfs:label>
        <owl:versionInfo xml:lang="it">instabile</owl:versionInfo>
        <owl:versionInfo xml:lang="en">unstable</owl:versionInfo>
        <a-cat:iccdNormTag>ICCD Normativa Trasversale 4.00: TU/NVC/NVCA; Versioni precedenti: CD/EPR</a-cat:iccdNormTag>
    </owl:ObjectProperty>



    <!-- https://w3id.org/arco/ontology/arco-lite/hasRadioactivity -->

    <owl:ObjectProperty rdf:about="https://w3id.org/arco/ontology/arco-lite/hasRadioactivity">
        <rdfs:subPropertyOf rdf:resource="https://w3id.org/arco/ontology/arco-lite/hasPhysicalCharacteristic"/>
        <owl:inverseOf rdf:resource="https://w3id.org/arco/ontology/arco-lite/isRadioactivityOf"/>
        <rdfs:domain rdf:resource="http://www.w3.org/2002/07/owl#Thing"/>
        <rdfs:range rdf:resource="https://w3id.org/arco/ontology/natural-specimen-description/PhysicalCharacteristic"/>
        <rdfs:comment xml:lang="it">Questa proprietà collega un entità alla radioattività</rdfs:comment>
        <rdfs:comment xml:lang="en">This property relates an entity to the radioactivity</rdfs:comment>
        <rdfs:isDefinedBy rdf:resource="https://w3id.org/arco/ontology/arco-lite"/>
        <rdfs:label xml:lang="it">ha radioattività</rdfs:label>
        <rdfs:label xml:lang="en">has radioactivity</rdfs:label>
        <owl:versionInfo xml:lang="it">instabile</owl:versionInfo>
        <owl:versionInfo xml:lang="en">unstable</owl:versionInfo>
        <a-cat:iccdNormTag>Normativa ICCD BNM: SM/SMF/SMFV</a-cat:iccdNormTag>
    </owl:ObjectProperty>



    <!-- https://w3id.org/arco/ontology/arco-lite/hasRealizationDate -->

    <owl:ObjectProperty rdf:about="https://w3id.org/arco/ontology/arco-lite/hasRealizationDate">
        <owl:inverseOf rdf:resource="https://w3id.org/arco/ontology/arco-lite/isRealizationDateOf"/>
        <rdfs:domain rdf:resource="http://www.w3.org/2002/07/owl#Thing"/>
        <rdfs:range rdf:resource="https://w3id.org/italia/onto/TI/TimeInterval"/>
        <rdfs:comment xml:lang="it">Questa proprietà collega un&apos;entità alla sua data di realizazione.</rdfs:comment>
        <rdfs:comment xml:lang="en">This property relates an entity with its realization date.</rdfs:comment>
        <rdfs:isDefinedBy rdf:resource="https://w3id.org/arco/ontology/arco-lite"/>
        <rdfs:label xml:lang="it">ha data di realizzazione</rdfs:label>
        <rdfs:label xml:lang="en">has realization date</rdfs:label>
        <owl:versionInfo xml:lang="it">instabile</owl:versionInfo>
        <owl:versionInfo xml:lang="en">unstable</owl:versionInfo>
    </owl:ObjectProperty>



    <!-- https://w3id.org/arco/ontology/arco-lite/hasRecipient -->

    <owl:ObjectProperty rdf:about="https://w3id.org/arco/ontology/arco-lite/hasRecipient">
        <owl:inverseOf rdf:resource="https://w3id.org/arco/ontology/arco-lite/hasTransferor"/>
        <rdfs:domain rdf:resource="https://w3id.org/italia/onto/l0/Object"/>
        <rdfs:range rdf:resource="https://w3id.org/italia/onto/l0/Agent"/>
        <rdfs:comment xml:lang="it">Questa proprietà collega un&apos;entità al suo destinatario.</rdfs:comment>
        <rdfs:comment xml:lang="en">This property relates an entity with its recipient.</rdfs:comment>
        <rdfs:isDefinedBy rdf:resource="https://w3id.org/arco/ontology/arco-lite"/>
        <rdfs:label xml:lang="it">ha destinatario</rdfs:label>
        <rdfs:label xml:lang="en">has recipient</rdfs:label>
        <owl:versionInfo xml:lang="it">instabile</owl:versionInfo>
        <owl:versionInfo xml:lang="en">unstable</owl:versionInfo>
    </owl:ObjectProperty>



    <!-- https://w3id.org/arco/ontology/arco-lite/hasRelatedAgent -->

    <owl:ObjectProperty rdf:about="https://w3id.org/arco/ontology/arco-lite/hasRelatedAgent">
        <owl:inverseOf rdf:resource="https://w3id.org/arco/ontology/arco-lite/isRelatedAgentTo"/>
        <rdfs:domain rdf:resource="http://www.w3.org/2002/07/owl#Thing"/>
        <rdfs:range rdf:resource="https://w3id.org/italia/onto/l0/Agent"/>
        <rdfs:comment xml:lang="it">Questa proprietà collega un&apos;entità di qualsiasi tipo a un agente che è collegato in qualche modo a quell&apos;entità. È una relazione generica che viene usata per quei casi in cui non sia possibile definire in maniera più precisa la natura della relazione.</rdfs:comment>
        <rdfs:comment xml:lang="en">This property is used to associate an entity of any kind to an agent related to that entity in some way. It is used when it is not possible to express the relation in a more specific way.</rdfs:comment>
        <rdfs:isDefinedBy rdf:resource="https://w3id.org/arco/ontology/arco-lite"/>
        <rdfs:label xml:lang="it">ha agente correlato</rdfs:label>
        <rdfs:label xml:lang="en">has related agent</rdfs:label>
        <owl:versionInfo xml:lang="it">instabile</owl:versionInfo>
        <owl:versionInfo xml:lang="en">unstable</owl:versionInfo>
        <a-cat:iccdNormTag xml:lang="it">ICCD Normativa Trasversale: AU/NMC</a-cat:iccdNormTag>
    </owl:ObjectProperty>



    <!-- https://w3id.org/arco/ontology/arco-lite/hasRelatedWork -->

    <owl:ObjectProperty rdf:about="https://w3id.org/arco/ontology/arco-lite/hasRelatedWork">
        <owl:inverseOf rdf:resource="https://w3id.org/arco/ontology/arco-lite/isWorkRelatedTo"/>
        <rdfs:domain rdf:resource="http://www.w3.org/2002/07/owl#Thing"/>
        <rdfs:range rdf:resource="http://www.w3.org/2002/07/owl#Thing"/>
        <rdfs:comment xml:lang="it">Questa proprietà collega un bene culturale a un&apos;altra opera collegata (es.: copia, fase preparatoria, etc.), che può essere essa stessa un bene culturale.</rdfs:comment>
        <rdfs:comment xml:lang="en">This property relates a cultural property to a related work (e.g. copy, preparatory work).</rdfs:comment>
        <rdfs:isDefinedBy rdf:resource="https://w3id.org/arco/ontology/arco-lite"/>
        <rdfs:label xml:lang="it">ha opera collegata</rdfs:label>
        <rdfs:label xml:lang="en">has related work</rdfs:label>
        <owl:versionInfo xml:lang="it">instabile</owl:versionInfo>
        <owl:versionInfo xml:lang="en">unstable</owl:versionInfo>
    </owl:ObjectProperty>



    <!-- https://w3id.org/arco/ontology/arco-lite/hasResolution -->

    <owl:ObjectProperty rdf:about="https://w3id.org/arco/ontology/arco-lite/hasResolution">
        <rdfs:subPropertyOf rdf:resource="https://w3id.org/arco/ontology/denotative-description/hasTechnicalCharacteristic"/>
        <owl:inverseOf rdf:resource="https://w3id.org/arco/ontology/denotative-description/isResolutionOf"/>
        <rdfs:domain rdf:resource="http://www.w3.org/2002/07/owl#Thing"/>
        <rdfs:range rdf:resource="https://w3id.org/arco/ontology/denotative-description/TechnicalCharacteristic"/>
        <rdfs:comment xml:lang="it">Questa proprietà collega una fotografia alla risoluzione e al valore specifico utilizzati per la memorizzazione di una fotografia digitale.</rdfs:comment>
        <rdfs:comment xml:lang="en">This property relates a digital resource to theresolution used for storing it.</rdfs:comment>
        <rdfs:isDefinedBy rdf:resource="https://w3id.org/arco/ontology/arco-lite"/>
        <rdfs:label xml:lang="it">ha risoluzione</rdfs:label>
        <rdfs:label xml:lang="en">has resolution</rdfs:label>
        <owl:versionInfo xml:lang="it">instabile</owl:versionInfo>
        <owl:versionInfo xml:lang="en">unstable</owl:versionInfo>
    </owl:ObjectProperty>



    <!-- https://w3id.org/arco/ontology/arco-lite/hasResponsibleAgent -->

    <owl:ObjectProperty rdf:about="https://w3id.org/arco/ontology/arco-lite/hasResponsibleAgent">
        <rdfs:subPropertyOf rdf:resource="https://w3id.org/arco/ontology/arco-lite/hasRelatedAgent"/>
        <owl:inverseOf rdf:resource="https://w3id.org/arco/ontology/arco-lite/isResponsibleAgentOf"/>
        <rdfs:range rdf:resource="https://w3id.org/italia/onto/l0/Agent"/>
        <rdfs:comment xml:lang="it">Questa properietà collega una scheda su cui si analizza un bene culturale per finalità diverse da quella della catalogazione del patrimonio all&apos;Ente o al soggetto che ha prodotto la scheda o che gestisce la banca dati di cui la scheda fa parte.</rdfs:comment>
        <rdfs:comment xml:lang="en">This property relates a cultural property record to the agency or the person that created that record or manages the database where the record is. (RecordResponsibleAgent).</rdfs:comment>
        <rdfs:isDefinedBy rdf:resource="https://w3id.org/arco/ontology/arco-lite"/>
        <rdfs:label xml:lang="it">ha agente responsabile</rdfs:label>
        <rdfs:label xml:lang="en">has responsible agent</rdfs:label>
        <owl:versionInfo xml:lang="it">instabile</owl:versionInfo>
        <owl:versionInfo xml:lang="en">unstable</owl:versionInfo>
        <a-cat:iccdNormTag>ICCD Notmativa Trasversale 4.00: AC/ACS/ACSE, DA/APP/APPE, RE/IND/INDE-RCG/RCGR-DSC/DSCFFOI/FOIE, CM/ISP/ISPN, CO/RST/RSTE</a-cat:iccdNormTag>
    </owl:ObjectProperty>



    <!-- https://w3id.org/arco/ontology/arco-lite/hasResponsibleResearchAndCompilation -->

    <owl:ObjectProperty rdf:about="https://w3id.org/arco/ontology/arco-lite/hasResponsibleResearchAndCompilation">
        <rdfs:subPropertyOf rdf:resource="https://w3id.org/arco/ontology/arco-lite/hasCataloguingAgent"/>
        <owl:inverseOf rdf:resource="https://w3id.org/arco/ontology/arco-lite/isResponsibleResearchAndCompilationOf"/>
        <rdfs:domain>
            <owl:Class>
                <owl:unionOf rdf:parseType="Collection">
                    <rdf:Description rdf:about="https://w3id.org/arco/ontology/catalogue/CatalogueRecord"/>
                    <rdf:Description rdf:about="https://w3id.org/arco/ontology/catalogue/CatalogueRecordVersion"/>
                </owl:unionOf>
            </owl:Class>
        </rdfs:domain>
        <rdfs:range rdf:resource="https://w3id.org/italia/onto/l0/Agent"/>
        <rdfs:comment xml:lang="it">Questa proprietà rappresenta la relazione che collega la prima versione di una scheda di catalogo al relativo responsabile ricerca e redazione. La relazione tra il ruolo e l&apos;ente che lo riveste è espressa nel nome della proprietà, che quindi ne fornisce una rappresentazione semplificata, con ridotta espressività. Nell&apos;ontologia questa relazione è modellata anche, in maniera più espressiva, dalla classe TimeIndexedRole, che permette di collegare l&apos;ente, il suo ruolo e la sua corrispondente estensione temporale.</rdfs:comment>
        <rdfs:isDefinedBy rdf:resource="https://w3id.org/arco/ontology/arco-lite"/>
        <rdfs:label xml:lang="it">ha responsabile ricerca e redazione</rdfs:label>
        <rdfs:label xml:lang="en">has responsible research and compilation</rdfs:label>
        <owl:versionInfo xml:lang="it">instabile</owl:versionInfo>
        <owl:versionInfo xml:lang="en">instable</owl:versionInfo>
        <iccdNormTag>CM/CMP/CMPN</iccdNormTag>
    </owl:ObjectProperty>



    <!-- https://w3id.org/arco/ontology/arco-lite/hasRightHolder -->

    <owl:ObjectProperty rdf:about="https://w3id.org/arco/ontology/arco-lite/hasRightHolder">
        <rdfs:subPropertyOf rdf:resource="https://w3id.org/arco/ontology/arco-lite/hasRelatedAgent"/>
        <owl:inverseOf rdf:resource="https://w3id.org/arco/ontology/arco-lite/isRightHolderOf"/>
        <rdfs:domain rdf:resource="http://www.w3.org/2002/07/owl#Thing"/>
        <rdfs:range rdf:resource="https://w3id.org/italia/onto/l0/Agent"/>
        <rdfs:comment xml:lang="it">Questa proprietà collega un&apos;entità con l&apos;agente detentore dei diritti.</rdfs:comment>
        <rdfs:comment xml:lang="en">This property relates an entity with its right holder.</rdfs:comment>
        <rdfs:isDefinedBy rdf:resource="https://w3id.org/arco/ontology/arco-lite"/>
        <rdfs:label xml:lang="it">ha detentore dei diritti</rdfs:label>
        <rdfs:label xml:lang="en">has copyright holder</rdfs:label>
        <owl:versionInfo xml:lang="it">instabile</owl:versionInfo>
        <owl:versionInfo xml:lang="en">unstable</owl:versionInfo>
        <a-cat:iccdNormTag>ICCD Normativa  F, OAC: TU/CPR/CPRN</a-cat:iccdNormTag>
    </owl:ObjectProperty>



    <!-- https://w3id.org/arco/ontology/arco-lite/hasScientificDirector -->

    <owl:ObjectProperty rdf:about="https://w3id.org/arco/ontology/arco-lite/hasScientificDirector">
        <rdfs:subPropertyOf rdf:resource="https://w3id.org/arco/ontology/arco-lite/hasRelatedAgent"/>
        <owl:inverseOf rdf:resource="https://w3id.org/arco/ontology/arco-lite/isScientificDirectorOf"/>
        <rdfs:domain rdf:resource="http://www.w3.org/2002/07/owl#Thing"/>
        <rdfs:range rdf:resource="https://w3id.org/italia/onto/l0/Agent"/>
        <rdfs:comment xml:lang="it">Questa proprietà collega un&apos;entità (es. una ricerca) al suo responsabile scientifico. La relazione tra il ruolo e l&apos;agente che lo riveste è espressa nel nome della proprietà, che quindi ne fornisce una rappresentazione semplificata, con ridotta espressività. Nell&apos;ontologia questa relazione è modellata anche, in maniera più espressiva, dalla classe AgentRole, che permette di collegare l&apos;agente e il suo ruolo.</rdfs:comment>
        <rdfs:comment xml:lang="en">This property relates an entity (e.g. a research) to its scientific responsible. In the ontology this relationship is modelled also by the class AgentRole which allows more expressiveness.</rdfs:comment>
        <rdfs:isDefinedBy rdf:resource="https://w3id.org/arco/ontology/arco-lite"/>
        <rdfs:label xml:lang="it">ha responsabile scientifico</rdfs:label>
        <rdfs:label xml:lang="en">has scientific director</rdfs:label>
        <owl:versionInfo xml:lang="it">instabile</owl:versionInfo>
        <owl:versionInfo xml:lang="en">unstable</owl:versionInfo>
        <a-cat:iccdNormTag>ICCD Normativa Trasversale 4.00: RE/RCG/RCGA-FOI/FOIS,
          ICCD Normativa SM e BDM 4.00: DR/DRR</a-cat:iccdNormTag>
    </owl:ObjectProperty>



    <!-- https://w3id.org/arco/ontology/arco-lite/hasSecondaryAuthor -->

    <owl:ObjectProperty rdf:about="https://w3id.org/arco/ontology/arco-lite/hasSecondaryAuthor">
        <rdfs:subPropertyOf rdf:resource="https://w3id.org/arco/ontology/arco-lite/hasRelatedAgent"/>
        <owl:inverseOf rdf:resource="https://w3id.org/arco/ontology/arco-lite/isSecondaryAuthorOf"/>
        <rdfs:domain rdf:resource="http://www.w3.org/2002/07/owl#Thing"/>
        <rdfs:range rdf:resource="https://w3id.org/italia/onto/l0/Agent"/>
        <rdfs:comment xml:lang="it">Questa proprietà collega un&apos;entità al suo autore secondario, come ad esempio l&apos;autore di un contributo o una parte di una pubblicazione.</rdfs:comment>
        <rdfs:comment xml:lang="en">This property relates an entity to its secondary authors. For example an author of a publication&apos;s contribution or section.</rdfs:comment>
        <rdfs:isDefinedBy rdf:resource="https://w3id.org/arco/ontology/arco-lite"/>
        <rdfs:label xml:lang="it">ha autore secondario</rdfs:label>
        <rdfs:label xml:lang="en">has secondary author</rdfs:label>
        <owl:versionInfo xml:lang="it">instabile</owl:versionInfo>
        <owl:versionInfo xml:lang="en">unstable</owl:versionInfo>
        <a-cat:iccdNormTag>ICCD Normative VeAC e AT 3.01: DO/BSE/BSER</a-cat:iccdNormTag>
    </owl:ObjectProperty>



    <!-- https://w3id.org/arco/ontology/arco-lite/hasShape -->

    <owl:ObjectProperty rdf:about="https://w3id.org/arco/ontology/arco-lite/hasShape">
        <rdfs:subPropertyOf rdf:resource="https://w3id.org/arco/ontology/denotative-description/hasTechnicalCharacteristic"/>
        <owl:inverseOf rdf:resource="https://w3id.org/arco/ontology/arco-lite/isShapeOf"/>
        <rdfs:domain rdf:resource="http://www.w3.org/2002/07/owl#Thing"/>
        <rdfs:range rdf:resource="https://w3id.org/arco/ontology/denotative-description/TechnicalCharacteristic"/>
        <rdfs:comment xml:lang="it">Questa proprietà collega un oggetto al formato dell&apos;oggetto, per oggetti bidimensionali (es.: ottagonale, tondo)</rdfs:comment>
        <rdfs:comment xml:lang="en">This property relates an object to its shape. It is used for bidimensional objects, e.g. octagonal or round shape.</rdfs:comment>
        <rdfs:isDefinedBy rdf:resource="https://w3id.org/arco/ontology/arco-lite"/>
        <rdfs:label xml:lang="it">ha forma</rdfs:label>
        <rdfs:label xml:lang="en">has shape</rdfs:label>
        <owl:versionInfo xml:lang="it">instabile</owl:versionInfo>
        <owl:versionInfo xml:lang="en">unstable</owl:versionInfo>
        <a-cat:iccdNormTag xml:lang="it">Normativa A 3.00: SCLF, CPFF+CPFQ, SVCC+SVCQ, SOFF+SOFQ,
          ICCD Normativa BNB: DB/DBX/DBXX</a-cat:iccdNormTag>
    </owl:ObjectProperty>



    <!-- https://w3id.org/arco/ontology/arco-lite/hasSoundEngineer -->

    <owl:ObjectProperty rdf:about="https://w3id.org/arco/ontology/arco-lite/hasSoundEngineer">
        <rdfs:subPropertyOf rdf:resource="https://w3id.org/arco/ontology/arco-lite/hasRelatedAgent"/>
        <owl:inverseOf rdf:resource="https://w3id.org/arco/ontology/arco-lite/isSoundEngineerOf"/>
        <rdfs:comment xml:lang="it">Questa proprietà collega un&apos;indagine di rilevamento di un bene demo-etno-antropologico al fonico professionista (diverso dal rilevatore) che ha effettuato la registrazione sonora. La relazione tra il ruolo e l&apos;agente che lo riveste è espressa nel nome della proprietà, che quindi ne fornisce una rappresentazione semplificata, con ridotta espressività. Nell&apos;ontologia questa relazione è modellata anche, in maniera più espressiva, dalla classe AgentRole, che permette di collegare l&apos;agente e il suo ruolo.</rdfs:comment>
        <rdfs:comment xml:lang="en">This property relates an observation survey of a demo-etno-antropologic entity to the sound engineer who recorded it. In the ontology this relationship is modelled also by the class AgentRole which allows more expressiveness.</rdfs:comment>
        <rdfs:isDefinedBy rdf:resource="https://w3id.org/arco/ontology/arco-lite"/>
        <rdfs:label xml:lang="it">ha fonico</rdfs:label>
        <rdfs:label xml:lang="en">has sound engineer</rdfs:label>
        <owl:versionInfo xml:lang="it">instabile</owl:versionInfo>
        <owl:versionInfo xml:lang="en">unstable</owl:versionInfo>
    </owl:ObjectProperty>



    <!-- https://w3id.org/arco/ontology/arco-lite/hasSpaceGroup -->

    <owl:ObjectProperty rdf:about="https://w3id.org/arco/ontology/arco-lite/hasSpaceGroup">
        <rdfs:subPropertyOf rdf:resource="https://w3id.org/arco/ontology/arco-lite/hasCrystallographicCharacteristic"/>
        <owl:inverseOf rdf:resource="https://w3id.org/arco/ontology/arco-lite/isSpaceGroupOf"/>
        <rdfs:domain rdf:resource="https://w3id.org/arco/ontology/natural-specimen-description/UnitCell"/>
        <rdfs:range rdf:resource="https://w3id.org/arco/ontology/natural-specimen-description/CrystallographicCharacteristic"/>
        <rdfs:comment xml:lang="it">Questa proprietà collega una cella al gruppo spaziale</rdfs:comment>
        <rdfs:comment xml:lang="en">This property relates a unit cell to the space group</rdfs:comment>
        <rdfs:isDefinedBy rdf:resource="https://w3id.org/arco/ontology/arco-lite"/>
        <rdfs:label xml:lang="it">ha gruppo spaziale</rdfs:label>
        <rdfs:label xml:lang="en">has space group</rdfs:label>
        <owl:versionInfo xml:lang="it">instabile</owl:versionInfo>
        <owl:versionInfo xml:lang="en">unstable</owl:versionInfo>
        <a-cat:iccdNormTag>Normativa ICCD BNM: SM/SMC/SMCG</a-cat:iccdNormTag>
    </owl:ObjectProperty>



    <!-- https://w3id.org/arco/ontology/arco-lite/hasSponsor -->

    <owl:ObjectProperty rdf:about="https://w3id.org/arco/ontology/arco-lite/hasSponsor">
        <rdfs:subPropertyOf rdf:resource="https://w3id.org/arco/ontology/arco-lite/hasRelatedAgent"/>
        <owl:inverseOf rdf:resource="https://w3id.org/arco/ontology/arco-lite/isSponsorOf"/>
        <rdfs:domain rdf:resource="https://w3id.org/italia/onto/l0/Activity"/>
        <rdfs:range rdf:resource="https://w3id.org/italia/onto/l0/Agent"/>
        <rdfs:comment xml:lang="it">Questa proprietà collega un&apos;attività (per esempio, un&apos;indagine o un intervento su un bene culturale) all&apos;ente o al soggetto che ha finanziato l&apos;attività.</rdfs:comment>
        <rdfs:comment xml:lang="en">This property relates an activity to its investor. The investor may be an institution or an agent.</rdfs:comment>
        <rdfs:isDefinedBy rdf:resource="https://w3id.org/arco/ontology/arco-lite"/>
        <rdfs:label xml:lang="it">ha finanziatore</rdfs:label>
        <rdfs:label xml:lang="en">has sponsor</rdfs:label>
        <owl:versionInfo xml:lang="it">instabile</owl:versionInfo>
        <owl:versionInfo xml:lang="en">unstable</owl:versionInfo>
        <a-cat:iccdNormTag>ICCD Normativa Trasversale 4.00: RS/RST/RSTR; RE/IND/INDR</a-cat:iccdNormTag>
    </owl:ObjectProperty>



    <!-- https://w3id.org/arco/ontology/arco-lite/hasStorageMethodOrColourDepth -->

    <owl:ObjectProperty rdf:about="https://w3id.org/arco/ontology/arco-lite/hasStorageMethodOrColourDepth">
        <rdfs:subPropertyOf rdf:resource="https://w3id.org/arco/ontology/denotative-description/hasTechnicalCharacteristic"/>
        <owl:inverseOf rdf:resource="https://w3id.org/arco/ontology/arco-lite/isStorageMethodOrColourDepthOf"/>
        <rdfs:domain rdf:resource="http://www.w3.org/2002/07/owl#Thing"/>
        <rdfs:range rdf:resource="https://w3id.org/arco/ontology/denotative-description/TechnicalCharacteristic"/>
        <rdfs:comment xml:lang="it">Questa proprietà collega una fotografia al metodo e alla profondità di colore con cui è stata memorizzata la fotografia digitale.</rdfs:comment>
        <rdfs:comment xml:lang="en">This property relates a digital photograph to the method and color depth through which a digital photograph has been stored.</rdfs:comment>
        <rdfs:isDefinedBy rdf:resource="https://w3id.org/arco/ontology/arco-lite"/>
        <rdfs:label xml:lang="it">ha metodo di memorizzazione e profondità del colore</rdfs:label>
        <rdfs:label xml:lang="en">has storage method or colour depth</rdfs:label>
        <owl:versionInfo xml:lang="it">instabile</owl:versionInfo>
        <owl:versionInfo xml:lang="en">unstable</owl:versionInfo>
    </owl:ObjectProperty>



    <!-- https://w3id.org/arco/ontology/arco-lite/hasStreak -->

    <owl:ObjectProperty rdf:about="https://w3id.org/arco/ontology/arco-lite/hasStreak">
        <rdfs:subPropertyOf rdf:resource="https://w3id.org/arco/ontology/arco-lite/hasPhysicalCharacteristic"/>
        <owl:inverseOf rdf:resource="https://w3id.org/arco/ontology/arco-lite/isStreakOf"/>
        <rdfs:domain rdf:resource="http://www.w3.org/2002/07/owl#Thing"/>
        <rdfs:range rdf:resource="https://w3id.org/arco/ontology/natural-specimen-description/PhysicalCharacteristic"/>
        <rdfs:comment xml:lang="it">Questa proprietà collega un entità al colore della polvere</rdfs:comment>
        <rdfs:comment xml:lang="en">This property relates an entity to the streak</rdfs:comment>
        <rdfs:isDefinedBy rdf:resource="https://w3id.org/arco/ontology/arco-lite"/>
        <rdfs:label xml:lang="it">ha colore della polvere</rdfs:label>
        <rdfs:label xml:lang="en">has streak</rdfs:label>
        <owl:versionInfo xml:lang="it">instabile</owl:versionInfo>
        <owl:versionInfo xml:lang="en">unstable</owl:versionInfo>
        <a-cat:iccdNormTag>Normativa ICCD BNM: SM/SMF/SMFT</a-cat:iccdNormTag>
    </owl:ObjectProperty>



    <!-- https://w3id.org/arco/ontology/arco-lite/hasTechnique -->

    <owl:ObjectProperty rdf:about="https://w3id.org/arco/ontology/arco-lite/hasTechnique">
        <owl:inverseOf rdf:resource="https://w3id.org/arco/ontology/arco-lite/isTechniqueOf"/>
        <rdfs:domain rdf:resource="http://www.w3.org/2002/07/owl#Thing"/>
        <rdfs:range rdf:resource="https://w3id.org/arco/ontology/denotative-description/TechnicalCharacteristic"/>
        <rdfs:comment xml:lang="it">Questa proprietà collega un&apos;entità alla tecnica usata per realizzarla.</rdfs:comment>
        <rdfs:comment xml:lang="en">This property relates an entity with the technique used to create it.</rdfs:comment>
        <rdfs:isDefinedBy rdf:resource="https://w3id.org/arco/ontology/arco-lite"/>
        <rdfs:label xml:lang="it">ha tecnica</rdfs:label>
        <rdfs:label xml:lang="en">has technique</rdfs:label>
        <owl:versionInfo xml:lang="it">instabile</owl:versionInfo>
        <owl:versionInfo xml:lang="en">unstable</owl:versionInfo>
        <a-cat:iccdNormTag xml:lang="it">Normativa A 3.00: SCSC, FNSC, SOEC+SOEF</a-cat:iccdNormTag>
    </owl:ObjectProperty>



    <!-- https://w3id.org/arco/ontology/denotative-description/hasTemperament -->

    <owl:ObjectProperty rdf:about="https://w3id.org/arco/ontology/arco-lite/hasTemperament">
        <rdfs:subPropertyOf rdf:resource="https://w3id.org/arco/ontology/denotative-description/hasTechnicalCharacteristic"/>
        <owl:inverseOf rdf:resource="https://w3id.org/arco/ontology/arco-lite/isTemperamentOf"/>
        <rdfs:domain rdf:resource="http://www.w3.org/2002/07/owl#Thing"/>
        <rdfs:range rdf:resource="https://w3id.org/arco/ontology/denotative-description/TechnicalCharacteristic"/>
        <rdfs:comment xml:lang="it">Questa proprietà collega uno strumento al temperamento adottato, soprattutto in caso di oggetto in condizioni originali, o dopo un restauro, dello strumento musicale. Per gli idiofoni a tasti fissi (come xilofoni, litofoni, metallofoni) rappresenta la successione degli intervalli.</rdfs:comment>
        <rdfs:comment xml:lang="en">This property relates a musical instrument to the adopted temperament, especially in relation to an object in its original conditions, or after its restoration. For idiophones with fixed keys (e.g. xylophone, litophone, metallophone) the temperament represents the succession of intervals.</rdfs:comment>
        <rdfs:isDefinedBy rdf:resource="https://w3id.org/arco/ontology/arco-lite"/>
        <rdfs:label xml:lang="it">ha temperamento</rdfs:label>
        <rdfs:label xml:lang="en">has temperament</rdfs:label>
        <owl:versionInfo xml:lang="it">instabile</owl:versionInfo>
        <owl:versionInfo xml:lang="en">unstable</owl:versionInfo>
    </owl:ObjectProperty>



    <!-- https://w3id.org/arco/ontology/arco-lite/hasTenacity -->

    <owl:ObjectProperty rdf:about="https://w3id.org/arco/ontology/arco-lite/hasTenacity">
        <rdfs:subPropertyOf rdf:resource="https://w3id.org/arco/ontology/arco-lite/hasPhysicalCharacteristic"/>
        <owl:inverseOf rdf:resource="https://w3id.org/arco/ontology/arco-lite/isTenacityOf"/>
        <rdfs:domain rdf:resource="http://www.w3.org/2002/07/owl#Thing"/>
        <rdfs:range rdf:resource="https://w3id.org/arco/ontology/natural-specimen-description/PhysicalCharacteristic"/>
        <rdfs:comment xml:lang="it">Questa proprietà collega un entità alla tenacità</rdfs:comment>
        <rdfs:comment xml:lang="en">This property relates an entity to the tenacity</rdfs:comment>
        <rdfs:isDefinedBy rdf:resource="https://w3id.org/arco/ontology/arco-lite"/>
        <rdfs:label xml:lang="it">ha tenacità</rdfs:label>
        <rdfs:label xml:lang="en">has tenacity</rdfs:label>
        <owl:versionInfo xml:lang="it">instabile</owl:versionInfo>
        <owl:versionInfo xml:lang="en">unstable</owl:versionInfo>
        <a-cat:iccdNormTag>Normativa ICCD BNM: SM/SMF/SMFE</a-cat:iccdNormTag>
    </owl:ObjectProperty>



    <!-- https://w3id.org/arco/ontology/arco-lite/hasTransferor -->

    <owl:ObjectProperty rdf:about="https://w3id.org/arco/ontology/arco-lite/hasTransferor">
        <rdfs:domain rdf:resource="https://w3id.org/italia/onto/l0/Object"/>
        <rdfs:range rdf:resource="https://w3id.org/italia/onto/l0/Agent"/>
        <rdfs:comment xml:lang="it">Questa proprietà collega un&apos;entità con il suo cedente.</rdfs:comment>
        <rdfs:comment xml:lang="en">This property relates an entity with its transferor.</rdfs:comment>
        <rdfs:isDefinedBy rdf:resource="https://w3id.org/arco/ontology/arco-lite"/>
        <rdfs:label xml:lang="it">ha cedente</rdfs:label>
        <rdfs:label xml:lang="en">has transferor</rdfs:label>
        <owl:versionInfo xml:lang="it">instabile</owl:versionInfo>
        <owl:versionInfo xml:lang="en">unstable</owl:versionInfo>
    </owl:ObjectProperty>



    <!-- https://w3id.org/arco/ontology/arco-lite/hasTuning -->

    <owl:ObjectProperty rdf:about="https://w3id.org/arco/ontology/arco-lite/hasTuning">
        <rdfs:subPropertyOf rdf:resource="https://w3id.org/arco/ontology/denotative-description/hasTechnicalCharacteristic"/>
        <owl:inverseOf rdf:resource="https://w3id.org/arco/ontology/arco-lite/isTuningOf"/>
        <rdfs:domain rdf:resource="http://www.w3.org/2002/07/owl#Thing"/>
        <rdfs:range rdf:resource="https://w3id.org/arco/ontology/denotative-description/TechnicalCharacteristic"/>
        <rdfs:comment xml:lang="it">Questa proprietà collega uno strumento musicale alla sua accordatura.</rdfs:comment>
        <rdfs:comment xml:lang="en">This property relates a musical instrument with its tuning.</rdfs:comment>
        <rdfs:isDefinedBy rdf:resource="https://w3id.org/arco/ontology/arco-lite"/>
        <rdfs:label xml:lang="it">ha accordatura</rdfs:label>
        <rdfs:label xml:lang="en">has tuning</rdfs:label>
        <owl:versionInfo xml:lang="it">instabile</owl:versionInfo>
        <owl:versionInfo xml:lang="en">unstable</owl:versionInfo>
        <a-cat:iccdNormTag>ICCD Normativa SM 4.00: AA/AAA</a-cat:iccdNormTag>
    </owl:ObjectProperty>



    <!-- https://w3id.org/arco/ontology/arco-lite/hasUrbanPlanningEnvironmentalRelationWith -->

    <owl:ObjectProperty rdf:about="https://w3id.org/arco/ontology/arco-lite/hasUrbanPlanningEnvironmentalRelationWith">
        <rdfs:subPropertyOf rdf:resource="https://w3id.org/arco/ontology/arco-lite/hasRelatedWork"/>
        <rdfs:subPropertyOf rdf:resource="https://w3id.org/arco/ontology/arco-lite/isWorkRelatedTo"/>
        <rdfs:domain rdf:resource="http://www.w3.org/2002/07/owl#Thing"/>
        <rdfs:range rdf:resource="http://www.w3.org/2002/07/owl#Thing"/>
        <rdfs:comment xml:lang="en">This property relates a cultural entity to another cultural entity, in an planning environmental relation.</rdfs:comment>
        <rdfs:comment xml:lang="it">rdfs:comment
Questa proprietà collega un bene culturale a un altro bene culturale collegato, con cui è in relazione urbanistico-ambientale.</rdfs:comment>
        <rdfs:isDefinedBy rdf:resource="https://w3id.org/arco/ontology/arco-lite"/>
        <rdfs:label xml:lang="it">ha relazione urbanistico-ambientale con</rdfs:label>
        <rdfs:label xml:lang="en">has planning environmental relation with</rdfs:label>
        <owl:versionInfo xml:lang="it">instabile</owl:versionInfo>
        <owl:versionInfo xml:lang="en">unstable</owl:versionInfo>
        <a-cat:iccdNormTag xml:lang="it">ICCD Normativa Trasversale 4.00: RV/RSE/RSER = &apos;è in relazione urbanistico - ambientale con&apos; (versioni precedenti: &apos;relazione urbanistico ambientale&apos;)</a-cat:iccdNormTag>
    </owl:ObjectProperty>



    <!-- https://w3id.org/arco/ontology/arco-lite/hasUser -->

    <owl:ObjectProperty rdf:about="https://w3id.org/arco/ontology/arco-lite/hasUser">
        <rdfs:subPropertyOf rdf:resource="https://w3id.org/arco/ontology/arco-lite/involvesAgent"/>
        <rdfs:domain rdf:resource="http://www.w3.org/2002/07/owl#Thing"/>
        <rdfs:range rdf:resource="https://w3id.org/italia/onto/l0/Agent"/>
        <rdfs:comment xml:lang="it">Questa proprietà collega un&apos;entità a un utente, inteso come agente che ha fatto uso di quell&apos;entità. Per esempio, può collegare un vestimento antico o contemporaneo al fruitore stesso, oppure un particolare uso di un bene culturale al tipo di utente coinvolto in quell&apos;uso.</rdfs:comment>
        <rdfs:comment xml:lang="en">This property relates an entity to the user, intended as the agent who employed the entity.</rdfs:comment>
        <rdfs:isDefinedBy rdf:resource="https://w3id.org/arco/ontology/arco-lite"/>
        <rdfs:label xml:lang="it">ha utente</rdfs:label>
        <rdfs:label xml:lang="en">has user</rdfs:label>
        <owl:versionInfo xml:lang="it">instabile</owl:versionInfo>
        <owl:versionInfo xml:lang="en">unstable</owl:versionInfo>
        <a-cat:iccdNormTag>ICCD Normativa Trasversale: UT/UTU/UTUN; Normativa VeAC: AU/FRU/FRUF</a-cat:iccdNormTag>
    </owl:ObjectProperty>



    <!-- https://w3id.org/arco/ontology/arco-lite/hasVhnHardness -->

    <owl:ObjectProperty rdf:about="https://w3id.org/arco/ontology/arco-lite/hasVhnHardness">
        <rdfs:subPropertyOf rdf:resource="https://w3id.org/arco/ontology/arco-lite/hasPhysicalCharacteristic"/>
        <owl:inverseOf rdf:resource="https://w3id.org/arco/ontology/arco-lite/isVhnHardnessOf"/>
        <rdfs:domain rdf:resource="http://www.w3.org/2002/07/owl#Thing"/>
        <rdfs:range rdf:resource="https://w3id.org/arco/ontology/natural-specimen-description/PhysicalCharacteristic"/>
        <rdfs:comment xml:lang="it">Questa proprietà collega un entità alla durezza secondo la scala VHN</rdfs:comment>
        <rdfs:comment xml:lang="en">This property relates an entity to the hardness, according to the VHN scale </rdfs:comment>
        <rdfs:isDefinedBy rdf:resource="https://w3id.org/arco/ontology/arco-lite"/>
        <rdfs:label xml:lang="it">ha durezza secondo la scala VHN</rdfs:label>
        <rdfs:label xml:lang="en">has VHN scale hardness</rdfs:label>
        <owl:versionInfo xml:lang="it">instabile</owl:versionInfo>
        <owl:versionInfo xml:lang="en">unstable</owl:versionInfo>
        <a-cat:iccdNormTag>Normativa ICCD BNM: SM/SMF/SMFN</a-cat:iccdNormTag>
    </owl:ObjectProperty>



    <!-- https://w3id.org/arco/ontology/arco-lite/hasVideoOperator -->

    <owl:ObjectProperty rdf:about="https://w3id.org/arco/ontology/arco-lite/hasVideoOperator">
        <rdfs:subPropertyOf rdf:resource="https://w3id.org/arco/ontology/arco-lite/hasRelatedAgent"/>
        <owl:inverseOf rdf:resource="https://w3id.org/arco/ontology/arco-lite/isVideoOperatorOf"/>
        <rdfs:range rdf:resource="https://w3id.org/italia/onto/l0/Agent"/>
        <rdfs:comment xml:lang="it">Questa proprietà collega un&apos;entità (per esempio, una registrazione) all&apos;operatore dell&apos;entità. La relazione tra il ruolo e l&apos;agente che lo riveste è espressa nel nome della proprietà, che quindi ne fornisce una rappresentazione semplificata, con ridotta espressività. Nell&apos;ontologia questa relazione è modellata anche, in maniera più espressiva, dalla classe AgentRole, che permette di collegare l&apos;agente e il suo ruolo.</rdfs:comment>
        <rdfs:comment xml:lang="en">This property relates an entity to the agent who recorded it. In the ontology this relationship is modelled also by the class AgentRole which allows more expressiveness.</rdfs:comment>
        <rdfs:isDefinedBy rdf:resource="https://w3id.org/arco/ontology/context-description"/>
        <rdfs:label xml:lang="it">ha videooperatore</rdfs:label>
        <rdfs:label xml:lang="en">has video operator</rdfs:label>
        <owl:versionInfo xml:lang="it">instabile</owl:versionInfo>
        <owl:versionInfo xml:lang="en">unstable</owl:versionInfo>
    </owl:ObjectProperty>



    <!-- https://w3id.org/arco/ontology/arco-lite/involves -->

    <owl:ObjectProperty rdf:about="https://w3id.org/arco/ontology/arco-lite/involves">
        <rdfs:subPropertyOf rdf:resource="https://w3id.org/arco/ontology/arco-lite/isWorkRelatedTo"/>
        <owl:inverseOf rdf:resource="https://w3id.org/arco/ontology/arco-lite/isInvolvedIn"/>
        <rdfs:domain rdf:resource="http://www.w3.org/2002/07/owl#Thing"/>
        <rdfs:range rdf:resource="http://www.w3.org/2002/07/owl#Thing"/>
        <rdfs:comment xml:lang="it">Questa è la proprietà inversa di &apos;is involved in&apos;, che collega un bene culturale a un altro bene culturale collegato, di tipo immateriale, in cui è coinvolto.</rdfs:comment>
        <rdfs:comment xml:lang="en">This is the inverse property of &apos;is involved in&apos;, which relates a cultural entity to another involved cultural entity (e.g. immaterial).</rdfs:comment>
        <rdfs:isDefinedBy rdf:resource="https://w3id.org/arco/ontology/arco-lite"/>
        <rdfs:label xml:lang="it">coinvolge</rdfs:label>
        <rdfs:label xml:lang="en">involves</rdfs:label>
        <owl:versionInfo xml:lang="it">instabile</owl:versionInfo>
        <owl:versionInfo xml:lang="en">unstable</owl:versionInfo>
    </owl:ObjectProperty>



    <!-- https://w3id.org/arco/ontology/arco-lite/involvesAgent -->

    <owl:ObjectProperty rdf:about="https://w3id.org/arco/ontology/arco-lite/involvesAgent"/>



    <!-- https://w3id.org/arco/ontology/arco-lite/involvesMainAgent -->

    <owl:ObjectProperty rdf:about="https://w3id.org/arco/ontology/arco-lite/involvesMainAgent">
        <owl:inverseOf rdf:resource="https://w3id.org/arco/ontology/arco-lite/isMainAgentInvolvedIn"/>
        <rdfs:domain rdf:resource="http://www.w3.org/2002/07/owl#Thing"/>
        <rdfs:range rdf:resource="https://w3id.org/italia/onto/l0/Agent"/>
        <rdfs:comment xml:lang="it">Questa proprietà collega un&apos;entità all&apos;agente principale coinvolto.</rdfs:comment>
        <rdfs:comment xml:lang="en">This property relates an entity to the main involved agent.</rdfs:comment>
        <rdfs:isDefinedBy rdf:resource="https://w3id.org/arco/ontology/arco-lite"/>
        <rdfs:label xml:lang="it">coinvolge agente principale</rdfs:label>
        <rdfs:label xml:lang="en">involves main agent</rdfs:label>
        <owl:versionInfo xml:lang="it">instabile</owl:versionInfo>
        <owl:versionInfo xml:lang="en">unstable</owl:versionInfo>
    </owl:ObjectProperty>



    <!-- https://w3id.org/arco/ontology/arco-lite/isAgentRelatedTo -->

    <owl:ObjectProperty rdf:about="https://w3id.org/arco/ontology/arco-lite/isAgentRelatedTo"/>



    <!-- https://w3id.org/arco/ontology/arco-lite/isAnisotropyOf -->

    <owl:ObjectProperty rdf:about="https://w3id.org/arco/ontology/arco-lite/isAnisotropyOf">
        <rdfs:subPropertyOf rdf:resource="https://w3id.org/arco/ontology/arco-lite/isOpticCharacteristicOf"/>
        <rdfs:domain rdf:resource="https://w3id.org/arco/ontology/natural-specimen-description/OpticCharacteristic"/>
        <rdfs:range rdf:resource="http://www.w3.org/2002/07/owl#Thing"/>
        <rdfs:comment xml:lang="it">Questa proprietà collega l&apos;anisotropia al campione</rdfs:comment>
        <rdfs:comment xml:lang="en">This property relates the anisotropy to the specimen</rdfs:comment>
        <rdfs:isDefinedBy rdf:resource="https://w3id.org/arco/ontology/arco-lite"/>
        <rdfs:label xml:lang="en">is anisotropy of</rdfs:label>
        <rdfs:label xml:lang="it">è anisotropia di</rdfs:label>
        <owl:versionInfo xml:lang="it">instabile</owl:versionInfo>
        <owl:versionInfo xml:lang="en">unstable</owl:versionInfo>
        <a-cat:iccdNormTag>SM/SMM/SMMA</a-cat:iccdNormTag>
    </owl:ObjectProperty>



    <!-- https://w3id.org/arco/ontology/arco-lite/isAttributedAuthorOf -->

    <owl:ObjectProperty rdf:about="https://w3id.org/arco/ontology/arco-lite/isAttributedAuthorOf">
        <rdfs:subPropertyOf rdf:resource="https://w3id.org/arco/ontology/arco-lite/isAgentRelatedTo"/>
        <rdfs:domain rdf:resource="https://w3id.org/italia/onto/l0/Agent"/>
        <rdfs:range rdf:resource="https://w3id.org/arco/ontology/context-description/AuthorshipAttribution"/>
        <rdfs:comment xml:lang="it">Questa è la proprietà inversa a &quot;ha autore attribuito&quot;.</rdfs:comment>
        <rdfs:comment xml:lang="en">This is the inverse property of &quot;has attributed author&quot;.</rdfs:comment>
        <rdfs:isDefinedBy rdf:resource="https://w3id.org/arco/ontology/arco-lite"/>
        <rdfs:label xml:lang="en">is attributed author in</rdfs:label>
        <rdfs:label xml:lang="it">è autore attribuito in</rdfs:label>
        <owl:versionInfo xml:lang="it">instabile</owl:versionInfo>
        <owl:versionInfo xml:lang="en">unstable</owl:versionInfo>
    </owl:ObjectProperty>



    <!-- https://w3id.org/arco/ontology/arco-lite/isAuthorOf -->

    <owl:ObjectProperty rdf:about="https://w3id.org/arco/ontology/arco-lite/isAuthorOf">
        <rdfs:subPropertyOf rdf:resource="https://w3id.org/arco/ontology/arco-lite/isRelatedAgentTo"/>
        <rdfs:domain rdf:resource="https://w3id.org/italia/onto/l0/Agent"/>
        <rdfs:range rdf:resource="http://www.w3.org/2002/07/owl#Thing"/>
        <owl:propertyChainAxiom rdf:parseType="Collection">
            <rdf:Description rdf:about="https://w3id.org/arco/ontology/arco-lite/isAttributedAuthorOf"/>
            <rdf:Description rdf:about="https://w3id.org/arco/ontology/context-description/isAuthorshipAttributionOf"/>
        </owl:propertyChainAxiom>
        <rdfs:comment xml:lang="it">Questa proprietà collega un agente (autore) all&apos;entità realizzata.</rdfs:comment>
        <rdfs:comment xml:lang="en">This property relates an agent (author) with its realized entity.</rdfs:comment>
        <rdfs:isDefinedBy rdf:resource="https://w3id.org/arco/ontology/arco-lite"/>
        <rdfs:label xml:lang="en">is author of</rdfs:label>
        <rdfs:label xml:lang="it">è autore di</rdfs:label>
        <owl:versionInfo xml:lang="it">instabile</owl:versionInfo>
        <owl:versionInfo xml:lang="en">unstable</owl:versionInfo>
    </owl:ObjectProperty>



    <!-- https://w3id.org/arco/ontology/arco-lite/isCalculatedDensityOf -->

    <owl:ObjectProperty rdf:about="https://w3id.org/arco/ontology/arco-lite/isCalculatedDensityOf">
        <rdfs:subPropertyOf rdf:resource="https://w3id.org/arco/ontology/arco-lite/isPhysicalCharacteristicOf"/>
        <rdfs:domain rdf:resource="https://w3id.org/arco/ontology/natural-specimen-description/PhysicalCharacteristic"/>
        <rdfs:range rdf:resource="http://www.w3.org/2002/07/owl#Thing"/>
        <rdfs:comment xml:lang="it">Questa proprietà collega la densità calcolata a un entità.</rdfs:comment>
        <rdfs:comment xml:lang="en">This property relates the calculated density to an entity.</rdfs:comment>
        <rdfs:isDefinedBy rdf:resource="https://w3id.org/arco/ontology/arco-lite"/>
        <rdfs:label xml:lang="en">is calculated density of</rdfs:label>
        <rdfs:label xml:lang="it">è densità calcolata di</rdfs:label>
        <owl:versionInfo xml:lang="it">instabile</owl:versionInfo>
        <owl:versionInfo xml:lang="en">unstable</owl:versionInfo>
    </owl:ObjectProperty>



    <!-- https://w3id.org/arco/ontology/arco-lite/isCataloguingAgencyOf -->

    <owl:ObjectProperty rdf:about="https://w3id.org/arco/ontology/arco-lite/isCataloguingAgencyOf">
        <rdfs:subPropertyOf rdf:resource="https://w3id.org/arco/ontology/arco-lite/isAgentRelatedTo"/>
        <rdfs:domain rdf:resource="https://w3id.org/italia/onto/l0/Agent"/>
        <rdfs:range rdf:resource="http://www.w3.org/2002/07/owl#Thing"/>
        <rdfs:comment xml:lang="it">Questa proprietà collega l&apos;ente schedatore dell&apos;authority file a un&apos;entità descritta in una scheda di Authority File.</rdfs:comment>
        <rdfs:comment xml:lang="en">This property relates the file&apos;s cataloguing institution to an entity described in a authority file.</rdfs:comment>
        <rdfs:isDefinedBy rdf:resource="https://w3id.org/arco/ontology/arco-lite"/>
        <rdfs:label xml:lang="en">is cataloguing agency of</rdfs:label>
        <rdfs:label xml:lang="it">è ente schedatore di</rdfs:label>
        <owl:versionInfo xml:lang="it">instabile</owl:versionInfo>
        <owl:versionInfo xml:lang="en">instable</owl:versionInfo>
    </owl:ObjectProperty>



    <!-- https://w3id.org/arco/ontology/arco-lite/isCataloguingAgent -->

    <owl:ObjectProperty rdf:about="https://w3id.org/arco/ontology/arco-lite/isCataloguingAgent">
        <rdfs:subPropertyOf rdf:resource="https://w3id.org/arco/ontology/arco-lite/isRelatedAgentTo"/>
    </owl:ObjectProperty>



    <!-- https://w3id.org/arco/ontology/arco-lite/isCataloguingAgentOf -->

    <owl:ObjectProperty rdf:about="https://w3id.org/arco/ontology/arco-lite/isCataloguingAgentOf"/>



    <!-- https://w3id.org/arco/ontology/arco-lite/isCityOf -->

    <owl:ObjectProperty rdf:about="https://w3id.org/arco/ontology/arco-lite/isCityOf">
        <rdfs:comment xml:lang="it">Questa proprietà collega una città al suo catasto.</rdfs:comment>
        <rdfs:comment xml:lang="en">This property relates a city with its cadastre.</rdfs:comment>
        <rdfs:isDefinedBy rdf:resource="https://w3id.org/arco/ontology/arco-lite"/>
        <rdfs:label xml:lang="en">is city of</rdfs:label>
        <rdfs:label xml:lang="it">è città di</rdfs:label>
        <owl:versionInfo xml:lang="it">instabile</owl:versionInfo>
        <owl:versionInfo xml:lang="en">unstable</owl:versionInfo>
    </owl:ObjectProperty>



    <!-- https://w3id.org/arco/ontology/arco-lite/isClassifiedByCurrentTaxon -->

    <owl:ObjectProperty rdf:about="https://w3id.org/arco/ontology/arco-lite/isClassifiedByCurrentTaxon">
        <rdfs:subPropertyOf rdf:resource="https://w3id.org/arco/ontology/core/isClassifiedBy"/>
        <owl:inverseOf rdf:resource="https://w3id.org/arco/ontology/arco-lite/isCurrentTaxonOf"/>
        <rdfs:comment xml:lang="it">Questa proprietà collega un campione alla sua classificazione tassonomica corrente.</rdfs:comment>
        <rdfs:comment xml:lang="en">This property relates a sepcimen to its current classified taxon.</rdfs:comment>
        <rdfs:isDefinedBy rdf:resource="https://w3id.org/arco/ontology/arco-lite"/>
        <rdfs:label xml:lang="en">is classified by current taxon</rdfs:label>
        <rdfs:label xml:lang="it">è classificato dal taxon corrente</rdfs:label>
        <owl:versionInfo xml:lang="it">instabile</owl:versionInfo>
        <owl:versionInfo xml:lang="en">unstable</owl:versionInfo>
    </owl:ObjectProperty>



    <!-- https://w3id.org/arco/ontology/arco-lite/isClassifiedByOriginalTaxon -->

    <owl:ObjectProperty rdf:about="https://w3id.org/arco/ontology/arco-lite/isClassifiedByOriginalTaxon">
        <rdfs:subPropertyOf rdf:resource="https://w3id.org/arco/ontology/core/isClassifiedBy"/>
        <owl:inverseOf rdf:resource="https://w3id.org/arco/ontology/arco-lite/isOriginalTaxonOf"/>
        <rdfs:comment xml:lang="it">Questa proprietà collega un campione alla sua classificazione tassonomica originale.</rdfs:comment>
        <rdfs:comment xml:lang="en">This property relates a sepcimen to its originale classified taxon.</rdfs:comment>
        <rdfs:isDefinedBy rdf:resource="https://w3id.org/arco/ontology/arco-lite"/>
        <rdfs:label xml:lang="en">is classified by original taxon</rdfs:label>
        <rdfs:label xml:lang="it">è classificato dal taxon originale</rdfs:label>
        <owl:versionInfo xml:lang="it">instabile</owl:versionInfo>
        <owl:versionInfo xml:lang="en">unstable</owl:versionInfo>
    </owl:ObjectProperty>



    <!-- https://w3id.org/arco/ontology/arco-lite/isCollectionMemberOf -->

    <owl:ObjectProperty rdf:about="https://w3id.org/arco/ontology/arco-lite/isCollectionMemberOf">
        <rdfs:domain rdf:resource="http://dati.beniculturali.it/cis/CulturalEntity"/>
        <rdfs:range rdf:resource="http://dati.beniculturali.it/cis/CollectionCulEnt"/>
        <rdfs:comment xml:lang="it">Questa proprietà collega un bene culturale con la sua collezione.</rdfs:comment>
        <rdfs:comment xml:lang="en">This property relates a cultural entity with its collection.</rdfs:comment>
        <rdfs:isDefinedBy rdf:resource="https://w3id.org/arco/ontology/arco-lite"/>
        <rdfs:label xml:lang="en">is collection member of</rdfs:label>
        <rdfs:label xml:lang="it">è membro della collezione</rdfs:label>
        <owl:versionInfo xml:lang="it">instabile</owl:versionInfo>
        <owl:versionInfo xml:lang="en">unstable</owl:versionInfo>
    </owl:ObjectProperty>



    <!-- https://w3id.org/arco/ontology/arco-lite/isCollectorOf -->

    <owl:ObjectProperty rdf:about="https://w3id.org/arco/ontology/arco-lite/isCollectorOf">
        <rdfs:domain rdf:resource="https://w3id.org/italia/onto/l0/Agent"/>
        <rdfs:range rdf:resource="http://dati.beniculturali.it/cis/CollectionCulEnt"/>
        <rdfs:comment xml:lang="it">Questa proprietà collega l&apos;agente collezionista con la collezione.</rdfs:comment>
        <rdfs:comment xml:lang="en">This property relates the collector with their collection.</rdfs:comment>
        <rdfs:isDefinedBy rdf:resource="https://w3id.org/arco/ontology/arco-lite"/>
        <rdfs:label xml:lang="en">is collector of</rdfs:label>
        <rdfs:label xml:lang="en">è collezionista di</rdfs:label>
        <owl:versionInfo xml:lang="it">instabile</owl:versionInfo>
        <owl:versionInfo xml:lang="en">unstable</owl:versionInfo>
    </owl:ObjectProperty>



    <!-- https://w3id.org/arco/ontology/arco-lite/isColourOf -->

    <owl:ObjectProperty rdf:about="https://w3id.org/arco/ontology/arco-lite/isColourOf">
        <rdfs:domain rdf:resource="https://w3id.org/arco/ontology/denotative-description/TechnicalCharacteristic"/>
        <rdfs:range rdf:resource="http://www.w3.org/2002/07/owl#Thing"/>
        <rdfs:comment xml:lang="it">Questa proprietà collega il colore all&apos;oggetto.</rdfs:comment>
        <rdfs:comment xml:lang="en">This property connects the colour to the object.</rdfs:comment>
        <rdfs:isDefinedBy rdf:resource="https://w3id.org/arco/ontology/arco-lite"/>
        <rdfs:label xml:lang="en">is colour of</rdfs:label>
        <rdfs:label xml:lang="it">è colore di</rdfs:label>
        <owl:versionInfo xml:lang="it">instabile</owl:versionInfo>
        <owl:versionInfo xml:lang="en">unstable</owl:versionInfo>
    </owl:ObjectProperty>



    <!-- https://w3id.org/arco/ontology/arco-lite/isCommittentOf -->

    <owl:ObjectProperty rdf:about="https://w3id.org/arco/ontology/arco-lite/isCommittentOf">
        <rdfs:subPropertyOf rdf:resource="https://w3id.org/arco/ontology/arco-lite/isAgentRelatedTo"/>
        <rdfs:domain rdf:resource="https://w3id.org/italia/onto/l0/Agent"/>
        <rdfs:range rdf:resource="https://w3id.org/arco/ontology/context-description/Commission"/>
        <rdfs:comment xml:lang="it">Questa proprietà collega una persona o istituzione committente a una situazione in cui viene indicata la committenza di un bene culturale.</rdfs:comment>
        <rdfs:comment xml:lang="en">This property relates an agent that is committent of a cultural property to the identification of the commission of that cultural property.</rdfs:comment>
        <rdfs:isDefinedBy rdf:resource="https://w3id.org/arco/ontology/arco-lite"/>
        <rdfs:label xml:lang="en">is committent of</rdfs:label>
        <rdfs:label xml:lang="it">è committente di</rdfs:label>
        <owl:versionInfo xml:lang="it">instabile</owl:versionInfo>
        <owl:versionInfo xml:lang="en">unstable</owl:versionInfo>
        <a-cat:iccdNormTag>ICCD Normativa Trasversale 4.00: AU/CMM/CMMN</a-cat:iccdNormTag>
    </owl:ObjectProperty>



    <!-- https://w3id.org/arco/ontology/arco-lite/isCompatibilityIndexOf -->

    <owl:ObjectProperty rdf:about="https://w3id.org/arco/ontology/arco-lite/isCompatibilityIndexOf">
        <rdfs:subPropertyOf rdf:resource="https://w3id.org/arco/ontology/arco-lite/isPhysicalCharacteristicOf"/>
        <rdfs:domain rdf:resource="https://w3id.org/arco/ontology/natural-specimen-description/PhysicalCharacteristic"/>
        <rdfs:range rdf:resource="http://www.w3.org/2002/07/owl#Thing"/>
        <rdfs:comment xml:lang="it">Questa proprietà collega il Compatibility Index a un entità.</rdfs:comment>
        <rdfs:comment xml:lang="en">This property relates the Compatibility Index to an entity.</rdfs:comment>
        <rdfs:isDefinedBy rdf:resource="https://w3id.org/arco/ontology/arco-lite"/>
        <rdfs:label xml:lang="en">is Compatibility Index of</rdfs:label>
        <rdfs:label xml:lang="it">è Compatibility Index di</rdfs:label>
        <owl:versionInfo xml:lang="it">instabile</owl:versionInfo>
        <owl:versionInfo xml:lang="en">unstable</owl:versionInfo>
    </owl:ObjectProperty>



    <!-- https://w3id.org/arco/ontology/arco-lite/isConservationStatusTypeOf -->

    <owl:ObjectProperty rdf:about="https://w3id.org/arco/ontology/arco-lite/isConservationStatusTypeOf">
        <rdfs:domain rdf:resource="https://w3id.org/arco/ontology/denotative-description/ConservationStatusType"/>
        <rdfs:range rdf:resource="http://www.w3.org/2002/07/owl#Thing"/>
        <rdfs:comment xml:lang="it">Questa è la proprietà inversa di &quot;ha tipo di stato di conservazione&quot;.</rdfs:comment>
        <rdfs:comment xml:lang="en">This is the inverse property of &quot;has conservation status type&quot;.</rdfs:comment>
        <rdfs:isDefinedBy rdf:resource="https://w3id.org/arco/ontology/arco-lite"/>
        <rdfs:label xml:lang="en">is conservation status type of</rdfs:label>
        <rdfs:label xml:lang="it">è tipo di stato di conservazione</rdfs:label>
        <owl:versionInfo xml:lang="it">instabile</owl:versionInfo>
        <owl:versionInfo xml:lang="en">unstable</owl:versionInfo>
    </owl:ObjectProperty>



    <!-- https://w3id.org/arco/ontology/arco-lite/isCopyrightHolderOf -->

    <owl:ObjectProperty rdf:about="https://w3id.org/arco/ontology/arco-lite/isCopyrightHolderOf">
        <rdfs:domain rdf:resource="https://w3id.org/italia/onto/l0/Agent"/>
        <rdfs:range rdf:resource="http://www.w3.org/2002/07/owl#Thing"/>
    </owl:ObjectProperty>



    <!-- https://w3id.org/arco/ontology/arco-lite/isCreationLocationOf -->

    <owl:ObjectProperty rdf:about="https://w3id.org/arco/ontology/arco-lite/isCreationLocationOf">
        <rdfs:subPropertyOf rdf:resource="https://w3id.org/arco/ontology/arco-lite/isWorkRelatedTo"/>
        <rdfs:domain rdf:resource="http://www.w3.org/2002/07/owl#Thing"/>
        <rdfs:range rdf:resource="http://www.w3.org/2002/07/owl#Thing"/>
        <rdfs:comment xml:lang="it">Questa è la proprietà inversa di &quot;ha luogo di creazione&quot;.</rdfs:comment>
        <rdfs:comment xml:lang="en">This is the inverse property of &quot;has creation location&quot;.</rdfs:comment>
        <rdfs:isDefinedBy rdf:resource="https://w3id.org/arco/ontology/arco-lite"/>
        <rdfs:label xml:lang="en">is creation location of</rdfs:label>
        <rdfs:label xml:lang="it">è luogo di realizzazione di</rdfs:label>
        <owl:versionInfo xml:lang="it">instabile</owl:versionInfo>
        <owl:versionInfo xml:lang="en">unstable</owl:versionInfo>
    </owl:ObjectProperty>



    <!-- https://w3id.org/arco/ontology/arco-lite/isCrystalClassOf -->

    <owl:ObjectProperty rdf:about="https://w3id.org/arco/ontology/arco-lite/isCrystalClassOf">
        <rdfs:subPropertyOf rdf:resource="https://w3id.org/arco/ontology/arco-lite/isCrystallographicCharacteristicOf"/>
        <rdfs:domain rdf:resource="https://w3id.org/arco/ontology/natural-specimen-description/CrystallographicCharacteristic"/>
        <rdfs:range rdf:resource="https://w3id.org/arco/ontology/natural-specimen-description/UnitCell"/>
        <rdfs:comment xml:lang="it">Questa proprietà collega la classe cristallina a una cella</rdfs:comment>
        <rdfs:comment xml:lang="en">This property relates the crystal class to a unit cell</rdfs:comment>
        <rdfs:isDefinedBy rdf:resource="https://w3id.org/arco/ontology/arco-lite"/>
        <rdfs:label xml:lang="en">is crystal class of</rdfs:label>
        <rdfs:label xml:lang="it">è classe cristallina di</rdfs:label>
        <owl:versionInfo xml:lang="it">instabile</owl:versionInfo>
        <owl:versionInfo xml:lang="en">unstable</owl:versionInfo>
    </owl:ObjectProperty>



    <!-- https://w3id.org/arco/ontology/arco-lite/isCrystalSystemOf -->

    <owl:ObjectProperty rdf:about="https://w3id.org/arco/ontology/arco-lite/isCrystalSystemOf">
        <rdfs:subPropertyOf rdf:resource="https://w3id.org/arco/ontology/arco-lite/isCrystallographicCharacteristicOf"/>
        <rdfs:domain rdf:resource="https://w3id.org/arco/ontology/natural-specimen-description/CrystallographicCharacteristic"/>
        <rdfs:range rdf:resource="https://w3id.org/arco/ontology/natural-specimen-description/UnitCell"/>
        <rdfs:comment xml:lang="it">Questa proprietà collega il sistema cristallino a una cella</rdfs:comment>
        <rdfs:comment xml:lang="en">This property relates the crystal system to a unit cell</rdfs:comment>
        <rdfs:isDefinedBy rdf:resource="https://w3id.org/arco/ontology/arco-lite"/>
        <rdfs:label xml:lang="en">is crystal system of</rdfs:label>
        <rdfs:label xml:lang="it">è sistema cristallino di</rdfs:label>
        <owl:versionInfo xml:lang="it">instabile</owl:versionInfo>
        <owl:versionInfo xml:lang="en">unstable</owl:versionInfo>
    </owl:ObjectProperty>



    <!-- https://w3id.org/arco/ontology/arco-lite/isCrystallographicCharacteristicOf -->

    <owl:ObjectProperty rdf:about="https://w3id.org/arco/ontology/arco-lite/isCrystallographicCharacteristicOf">
        <rdfs:subPropertyOf rdf:resource="https://w3id.org/arco/ontology/denotative-description/isTechnicalCharacteristicOf"/>
        <rdfs:domain rdf:resource="https://w3id.org/arco/ontology/natural-specimen-description/CrystallographicCharacteristic"/>
        <rdfs:range rdf:resource="https://w3id.org/arco/ontology/natural-specimen-description/UnitCell"/>
        <rdfs:comment xml:lang="it">Questa proprietà collega la caratteristica cristallografica alla cella</rdfs:comment>
        <rdfs:comment xml:lang="en">This property relates crystallographc characteristic to the unit cell.</rdfs:comment>
        <rdfs:isDefinedBy rdf:resource="https://w3id.org/arco/ontology/arco-lite"/>
        <rdfs:label xml:lang="en">is crystallographic characteristic of</rdfs:label>
        <rdfs:label xml:lang="it">è caratteristica cristallografica di</rdfs:label>
        <owl:versionInfo xml:lang="it">instabile</owl:versionInfo>
        <owl:versionInfo xml:lang="en">unstable</owl:versionInfo>
    </owl:ObjectProperty>



    <!-- https://w3id.org/arco/ontology/arco-lite/isCulturalEntityUseFunctionOf -->

    <owl:ObjectProperty rdf:about="https://w3id.org/arco/ontology/arco-lite/isCulturalEntityUseFunctionOf">
        <rdfs:domain rdf:resource="https://w3id.org/arco/ontology/context-description/UseFunction"/>
        <rdfs:range rdf:resource="http://dati.beniculturali.it/cis/CulturalEntity"/>
    </owl:ObjectProperty>



    <!-- https://w3id.org/arco/ontology/arco-lite/isCulturalPropertyAddressOf -->

    <owl:ObjectProperty rdf:about="https://w3id.org/arco/ontology/arco-lite/isCulturalPropertyAddressOf">
        <rdfs:domain rdf:resource="https://w3id.org/italia/onto/CLV/Address"/>
        <rdfs:range rdf:resource="http://dati.beniculturali.it/cis/CulturalEntity"/>
        <owl:propertyChainAxiom rdf:parseType="Collection">
            <rdf:Description rdf:about="https://w3id.org/italia/onto/CLV/isAddressFor"/>
            <rdf:Description rdf:about="https://w3id.org/arco/ontology/location/isLocationIn"/>
            <rdf:Description rdf:about="https://w3id.org/arco/ontology/location/isTimeIndexedTypedLocationOf"/>
        </owl:propertyChainAxiom>
        <owl:propertyChainAxiom rdf:parseType="Collection">
            <rdf:Description rdf:about="https://w3id.org/italia/onto/CLV/isAddressFor"/>
            <rdf:Description rdf:about="https://w3id.org/arco/ontology/location/isSiteIn"/>
            <rdf:Description rdf:about="https://w3id.org/arco/ontology/location/isTimeIndexedTypedLocationOf"/>
        </owl:propertyChainAxiom>
    </owl:ObjectProperty>



    <!-- https://w3id.org/arco/ontology/arco-lite/isCuratorOf -->

    <owl:ObjectProperty rdf:about="https://w3id.org/arco/ontology/arco-lite/isCuratorOf">
        <rdfs:subPropertyOf rdf:resource="https://w3id.org/arco/ontology/arco-lite/isRelatedAgentTo"/>
        <rdfs:domain rdf:resource="https://w3id.org/italia/onto/l0/Agent"/>
        <rdfs:range rdf:resource="http://www.w3.org/2002/07/owl#Thing"/>
        <rdfs:comment xml:lang="it">Questa proprietà collega il curatore a un&apos;entità.</rdfs:comment>
        <rdfs:comment xml:lang="en">This property relates the curator to an entity.</rdfs:comment>
        <rdfs:isDefinedBy rdf:resource="https://w3id.org/arco/ontology/arco-lite"/>
        <rdfs:label xml:lang="en">is curator of</rdfs:label>
        <rdfs:label xml:lang="it">è curatore di</rdfs:label>
        <owl:inverseOf></owl:inverseOf>
        <owl:versionInfo xml:lang="it">instabile</owl:versionInfo>
        <owl:versionInfo xml:lang="en">unstable</owl:versionInfo>
    </owl:ObjectProperty>



    <!-- https://w3id.org/arco/ontology/arco-lite/isCurrentTaxonOf -->

    <owl:ObjectProperty rdf:about="https://w3id.org/arco/ontology/arco-lite/isCurrentTaxonOf">
        <rdfs:subPropertyOf rdf:resource="https://w3id.org/arco/ontology/core/classifies"/>
        <rdfs:comment xml:lang="it">Questa proprietà collega una classificazione tassonomica corrente al suo campione.</rdfs:comment>
        <rdfs:comment xml:lang="en">This property relates s current classified taxon to its specimen.</rdfs:comment>
        <rdfs:isDefinedBy rdf:resource="https://w3id.org/arco/ontology/arco-lite"/>
        <rdfs:label xml:lang="en">is current taxon of</rdfs:label>
        <rdfs:label xml:lang="it">è taxon corrente di</rdfs:label>
        <owl:versionInfo xml:lang="it">instabile</owl:versionInfo>
        <owl:versionInfo xml:lang="en">unstable</owl:versionInfo>
    </owl:ObjectProperty>



    <!-- https://w3id.org/arco/ontology/arco-lite/isDiapasonOf -->

    <owl:ObjectProperty rdf:about="https://w3id.org/arco/ontology/arco-lite/isDiapasonOf">
        <rdfs:subPropertyOf rdf:resource="https://w3id.org/arco/ontology/denotative-description/isTechnicalCharacteristicOf"/>
        <rdfs:domain rdf:resource="https://w3id.org/arco/ontology/denotative-description/TechnicalCharacteristic"/>
        <rdfs:range rdf:resource="http://www.w3.org/2002/07/owl#Thing"/>
        <rdfs:comment xml:lang="it">Questa proprietà è l&apos;inversa di &quot;ha corista&quot;.</rdfs:comment>
        <rdfs:comment xml:lang="en">This is the inverse property of &quot;has diapason&quot;.</rdfs:comment>
        <rdfs:isDefinedBy rdf:resource="https://w3id.org/arco/ontology/arco-lite"/>
        <rdfs:label xml:lang="en">is diapason of</rdfs:label>
        <rdfs:label xml:lang="it">è corista di</rdfs:label>
        <owl:versionInfo xml:lang="it">instabile</owl:versionInfo>
        <owl:versionInfo xml:lang="en">unstable</owl:versionInfo>
    </owl:ObjectProperty>



    <!-- https://w3id.org/arco/ontology/arco-lite/isDiaphaneityOf -->

    <owl:ObjectProperty rdf:about="https://w3id.org/arco/ontology/arco-lite/isDiaphaneityOf">
        <rdfs:subPropertyOf rdf:resource="https://w3id.org/arco/ontology/arco-lite/isPhysicalCharacteristicOf"/>
        <rdfs:domain rdf:resource="https://w3id.org/arco/ontology/natural-specimen-description/PhysicalCharacteristic"/>
        <rdfs:range rdf:resource="http://www.w3.org/2002/07/owl#Thing"/>
        <rdfs:comment xml:lang="it">Questa proprietà collega la diafanità a un entità.</rdfs:comment>
        <rdfs:comment xml:lang="en">This property relates the diaphaneity to an entity.</rdfs:comment>
        <rdfs:isDefinedBy rdf:resource="https://w3id.org/arco/ontology/arco-lite"/>
        <rdfs:label xml:lang="en">is diaphaneity of</rdfs:label>
        <rdfs:label xml:lang="it">è diafanità di</rdfs:label>
        <owl:versionInfo xml:lang="it">instabile</owl:versionInfo>
        <owl:versionInfo xml:lang="en">unstable</owl:versionInfo>
    </owl:ObjectProperty>



    <!-- https://w3id.org/arco/ontology/arco-lite/isEditorOf -->

    <owl:ObjectProperty rdf:about="https://w3id.org/arco/ontology/arco-lite/isEditorOf">
        <rdfs:subPropertyOf rdf:resource="https://w3id.org/arco/ontology/arco-lite/isRelatedAgentTo"/>
        <rdfs:domain rdf:resource="https://w3id.org/italia/onto/l0/Agent"/>
        <rdfs:range rdf:resource="http://www.w3.org/2002/07/owl#Thing"/>
        <rdfs:comment xml:lang="it">Questa proprietà collega un&apos;editore alla sua edizione.</rdfs:comment>
        <rdfs:comment xml:lang="en">This property relates an editor with the edition.</rdfs:comment>
        <rdfs:isDefinedBy rdf:resource="https://w3id.org/arco/ontology/arco-lite"/>
        <rdfs:label xml:lang="en">is editor of</rdfs:label>
        <rdfs:label xml:lang="it">è editore di</rdfs:label>
        <owl:versionInfo xml:lang="it">instabile</owl:versionInfo>
        <owl:versionInfo xml:lang="en">unstable</owl:versionInfo>
        <a-cat:iccdNormTag xml:lang="it">Normativa F: PD/EDI/EDIR, Normativa S: AU/EDT/EDTN</a-cat:iccdNormTag>
    </owl:ObjectProperty>



    <!-- https://w3id.org/arco/ontology/arco-lite/isExportOfficeOf -->

    <owl:ObjectProperty rdf:about="https://w3id.org/arco/ontology/arco-lite/isExportOfficeOf">
        <rdfs:subPropertyOf rdf:resource="https://w3id.org/arco/ontology/arco-lite/isAgentRelatedTo"/>
        <rdfs:domain rdf:resource="https://w3id.org/italia/onto/l0/Agent"/>
        <rdfs:range rdf:resource="https://w3id.org/arco/ontology/context-description/ExportImportCertification"/>
        <rdfs:comment xml:lang="it">Questa proprietà collega un ufficio di esportazione a un certificazione di esportazione/importazione.</rdfs:comment>
        <rdfs:comment xml:lang="en">This property relates an export office to an export/import certification.</rdfs:comment>
        <rdfs:isDefinedBy rdf:resource="https://w3id.org/arco/ontology/arco-lite"/>
        <rdfs:label xml:lang="en">is export office of</rdfs:label>
        <rdfs:label xml:lang="it">è ufficio esportazione di</rdfs:label>
        <owl:versionInfo xml:lang="it">instabile</owl:versionInfo>
        <owl:versionInfo xml:lang="en">unstable</owl:versionInfo>
        <a-cat:iccdNormTag>ICCD Normativa Trasversale 4.00: TU/ESP/ESPU</a-cat:iccdNormTag>
    </owl:ObjectProperty>



    <!-- https://w3id.org/arco/ontology/arco-lite/isExtensionOf -->

    <owl:ObjectProperty rdf:about="https://w3id.org/arco/ontology/arco-lite/isExtensionOf">
        <rdfs:subPropertyOf rdf:resource="https://w3id.org/arco/ontology/denotative-description/isTechnicalCharacteristicOf"/>
        <rdfs:domain rdf:resource="https://w3id.org/arco/ontology/denotative-description/TechnicalCharacteristic"/>
        <rdfs:range rdf:resource="http://www.w3.org/2002/07/owl#Thing"/>
        <rdfs:comment xml:lang="it">Questa proprietà è l&apos;inversa di &quot;è estensione di&quot;.</rdfs:comment>
        <rdfs:comment xml:lang="en">This is the inverse property of &quot;has extension&quot;.</rdfs:comment>
        <rdfs:isDefinedBy rdf:resource="https://w3id.org/arco/ontology/arco-lite"/>
        <rdfs:label xml:lang="en">is extension of</rdfs:label>
        <rdfs:label xml:lang="it">è estensione musicale di</rdfs:label>
        <owl:versionInfo xml:lang="it">instabile</owl:versionInfo>
        <owl:versionInfo xml:lang="en">unstable</owl:versionInfo>
        <a-cat:iccdNormTag>ICCD Normativa SM 4.00: AA/AAE</a-cat:iccdNormTag>
    </owl:ObjectProperty>



    <!-- https://w3id.org/arco/ontology/arco-lite/isFindingLocationOf -->

    <owl:ObjectProperty rdf:about="https://w3id.org/arco/ontology/arco-lite/isFindingLocationOf">
        <rdfs:subPropertyOf rdf:resource="https://w3id.org/arco/ontology/arco-lite/isWorkRelatedTo"/>
        <rdfs:domain rdf:resource="http://www.w3.org/2002/07/owl#Thing"/>
        <rdfs:range rdf:resource="http://www.w3.org/2002/07/owl#Thing"/>
        <rdfs:comment xml:lang="it">Questa è la proprietà inversa di &quot;ha luogo di ritrovamento&quot;.</rdfs:comment>
        <rdfs:comment xml:lang="en">This is the inverse property of &quot;has finding location&quot;.</rdfs:comment>
        <rdfs:isDefinedBy rdf:resource="https://w3id.org/arco/ontology/aco-lite"/>
        <rdfs:label xml:lang="en">is findifng location of</rdfs:label>
        <rdfs:label xml:lang="it">è luogo di ritrovamento di</rdfs:label>
        <owl:versionInfo xml:lang="it">instabile</owl:versionInfo>
        <owl:versionInfo xml:lang="en">unstable</owl:versionInfo>
    </owl:ObjectProperty>



    <!-- https://w3id.org/arco/ontology/arco-lite/isFluorescenceOf -->

    <owl:ObjectProperty rdf:about="https://w3id.org/arco/ontology/arco-lite/isFluorescenceOf">
        <rdfs:subPropertyOf rdf:resource="https://w3id.org/arco/ontology/arco-lite/isPhysicalCharacteristicOf"/>
        <rdfs:domain rdf:resource="https://w3id.org/arco/ontology/natural-specimen-description/PhysicalCharacteristic"/>
        <rdfs:range rdf:resource="http://www.w3.org/2002/07/owl#Thing"/>
        <rdfs:comment xml:lang="it">Questa proprietà collega la fluorescenza a un entità.</rdfs:comment>
        <rdfs:comment xml:lang="en">This property relates the fluorescence to an entity.</rdfs:comment>
        <rdfs:isDefinedBy rdf:resource="https://w3id.org/arco/ontology/arco-lite"/>
        <rdfs:label xml:lang="en">is fluorescence of</rdfs:label>
        <rdfs:label xml:lang="it">è fluorescenza di</rdfs:label>
        <owl:versionInfo xml:lang="it">instabile</owl:versionInfo>
        <owl:versionInfo xml:lang="en">unstable</owl:versionInfo>
    </owl:ObjectProperty>



    <!-- https://w3id.org/arco/ontology/arco-lite/isFractureOf -->

    <owl:ObjectProperty rdf:about="https://w3id.org/arco/ontology/arco-lite/isFractureOf">
        <rdfs:subPropertyOf rdf:resource="https://w3id.org/arco/ontology/arco-lite/isPhysicalCharacteristicOf"/>
        <rdfs:domain rdf:resource="https://w3id.org/arco/ontology/natural-specimen-description/PhysicalCharacteristic"/>
        <rdfs:range rdf:resource="http://www.w3.org/2002/07/owl#Thing"/>
        <rdfs:comment xml:lang="it">Questa proprietà collega la frattura a un entità.</rdfs:comment>
        <rdfs:comment xml:lang="en">This property relates the fracture to an entity.</rdfs:comment>
        <rdfs:isDefinedBy rdf:resource="https://w3id.org/arco/ontology/arco-lite"/>
        <rdfs:label xml:lang="en">is fracture of</rdfs:label>
        <rdfs:label xml:lang="it">è frattura di</rdfs:label>
        <owl:versionInfo xml:lang="it">instabile</owl:versionInfo>
        <owl:versionInfo xml:lang="en">unstable</owl:versionInfo>
    </owl:ObjectProperty>



    <!-- https://w3id.org/arco/ontology/arco-lite/isGarmentAnalysisOf -->

    <owl:ObjectProperty rdf:about="https://w3id.org/arco/ontology/arco-lite/isGarmentAnalysisOf">
        <owl:inverseOf rdf:resource="https://w3id.org/arco/ontology/arco-lite/hasGarmentAnalysis"/>
        <rdfs:domain rdf:resource="https://w3id.org/arco/ontology/denotative-description/TechnicalCharacteristic"/>
        <rdfs:range rdf:resource="http://www.w3.org/2002/07/owl#Thing"/>
        <rdfs:comment xml:lang="it">Questa proprietà collega l&apos;analisi del tessuto (caratteristica tecnica) con un elemento di un vestimento.</rdfs:comment>
        <rdfs:comment xml:lang="en">This property relates the garment analysis with its element of clothing.</rdfs:comment>
        <rdfs:isDefinedBy rdf:resource="https://w3id.org/arco/ontology/clothing-description"/>
        <rdfs:label xml:lang="en">is garment analysis of</rdfs:label>
        <rdfs:label xml:lang="it">è analisi del tessuto di</rdfs:label>
        <owl:versionInfo xml:lang="it">instabile</owl:versionInfo>
        <owl:versionInfo xml:lang="en">unstable</owl:versionInfo>
        <a-cat:iccdNormTag>ICCD Normativa VeAC 3.01: MT/MTCA</a-cat:iccdNormTag>
    </owl:ObjectProperty>



    <!-- https://w3id.org/arco/ontology/arco-lite/isGladstone-DaleRelation -->

    <owl:ObjectProperty rdf:about="https://w3id.org/arco/ontology/arco-lite/isGladstone-DaleRelation">
        <rdfs:subPropertyOf rdf:resource="https://w3id.org/arco/ontology/arco-lite/isPhysicalCharacteristicOf"/>
        <rdfs:domain rdf:resource="https://w3id.org/arco/ontology/natural-specimen-description/PhysicalCharacteristic"/>
        <rdfs:range rdf:resource="http://www.w3.org/2002/07/owl#Thing"/>
        <rdfs:comment xml:lang="it">Questa proprietà collega la relazione Gladstone-Dale a un entità.</rdfs:comment>
        <rdfs:comment xml:lang="en">This property relates the Gladstone-Dale to an entity.</rdfs:comment>
        <rdfs:isDefinedBy rdf:resource="https://w3id.org/arco/ontology/arco-lite"/>
        <rdfs:label xml:lang="en">is Gladstone-Dale relation of</rdfs:label>
        <rdfs:label xml:lang="it">è relazione Gladstone-Dale di</rdfs:label>
        <owl:versionInfo xml:lang="it">instabile</owl:versionInfo>
        <owl:versionInfo xml:lang="en">unstable</owl:versionInfo>
    </owl:ObjectProperty>



    <!-- https://w3id.org/arco/ontology/arco-lite/isInventoryNumberResponsibleOf -->

    <owl:ObjectProperty rdf:about="https://w3id.org/arco/ontology/arco-lite/isInventoryNumberResponsibleOf">
        <rdfs:domain rdf:resource="https://w3id.org/italia/onto/l0/Agent"/>
        <rdfs:range rdf:resource="https://w3id.org/arco/ontology/context-description/InventorySituation"/>
        <rdfs:comment xml:lang="it">Questa proprietà collega l&apos;agente responsabile dell&apos;inserimento del numero inventariale di un&apos;entità alla situazione inventariale.</rdfs:comment>
        <rdfs:comment xml:lang="en">This property relates the responsible of the inventory number to the inventory situation.</rdfs:comment>
        <rdfs:isDefinedBy rdf:resource="https://w3id.org/arco/ontology/arco-lite"/>
        <rdfs:label xml:lang="en">is inventory number responsible of</rdfs:label>
        <rdfs:label xml:lang="it">è responsabile di numero inventariale di</rdfs:label>
        <owl:versionInfo xml:lang="it">instabile</owl:versionInfo>
        <owl:versionInfo xml:lang="en">unstable</owl:versionInfo>
    </owl:ObjectProperty>



    <!-- https://w3id.org/arco/ontology/arco-lite/isInvolvedIn -->

    <owl:ObjectProperty rdf:about="https://w3id.org/arco/ontology/arco-lite/isInvolvedIn">
        <rdfs:subPropertyOf rdf:resource="https://w3id.org/arco/ontology/arco-lite/hasRelatedWork"/>
        <rdfs:domain rdf:resource="http://www.w3.org/2002/07/owl#Thing"/>
        <rdfs:range rdf:resource="http://www.w3.org/2002/07/owl#Thing"/>
        <rdfs:comment xml:lang="it">Questa proprietà collega un bene culturale a un altro bene culturale collegato, di tipo immateriale, in cui è coinvolto.</rdfs:comment>
        <rdfs:comment xml:lang="en">This property relates a cultural entity to another involved  cultural entity (e.g. immaterial).</rdfs:comment>
        <rdfs:isDefinedBy rdf:resource="https://w3id.org/arco/ontology/arco-lite"/>
        <rdfs:label xml:lang="en">is involved in</rdfs:label>
        <rdfs:label xml:lang="it">è coinvolto in</rdfs:label>
        <owl:versionInfo xml:lang="it">instabile</owl:versionInfo>
        <owl:versionInfo xml:lang="en">unstable</owl:versionInfo>
        <a-cat:iccdNormTag xml:lang="it">ICCD Normativa Trasversale 4.00: RV/RSE/RSER = &apos;è coinvolto in&apos; (versioni precedenti: &apos;esecuzione/evento di riferimento&apos;)</a-cat:iccdNormTag>
    </owl:ObjectProperty>



    <!-- https://w3id.org/arco/ontology/arco-lite/isIssuerOf -->

    <owl:ObjectProperty rdf:about="https://w3id.org/arco/ontology/arco-lite/isIssuerOf">
        <rdfs:subPropertyOf rdf:resource="https://w3id.org/arco/ontology/arco-lite/isAgentRelatedTo"/>
        <rdfs:domain rdf:resource="https://w3id.org/italia/onto/l0/Agent"/>
        <rdfs:range rdf:resource="https://w3id.org/arco/ontology/context-description/CoinIssuance"/>
        <rdfs:comment xml:lang="it">Questa è la proprietà inversa di &quot;ha emittente&quot;.</rdfs:comment>
        <rdfs:comment xml:lang="en">This is the inverse property of &quot;has issuer&quot;.</rdfs:comment>
        <rdfs:isDefinedBy rdf:resource="https://w3id.org/arco/ontology/arco-lite"/>
        <rdfs:label xml:lang="en">is issuer in</rdfs:label>
        <rdfs:label xml:lang="it">è soggetto emittente di</rdfs:label>
        <owl:versionInfo xml:lang="it">instabile</owl:versionInfo>
        <owl:versionInfo xml:lang="it">unstable</owl:versionInfo>
    </owl:ObjectProperty>



    <!-- https://w3id.org/arco/ontology/arco-lite/isIssuingAgencyOf -->

    <owl:ObjectProperty rdf:about="https://w3id.org/arco/ontology/arco-lite/isIssuingAgencyOf">
        <rdfs:subPropertyOf rdf:resource="https://w3id.org/arco/ontology/arco-lite/isAgentRelatedTo"/>
        <rdfs:domain rdf:resource="https://w3id.org/italia/onto/l0/Agent"/>
        <rdfs:range rdf:resource="https://w3id.org/arco/ontology/context-description/UrbanPlanningInstrument"/>
        <rdfs:comment xml:lang="it">Questa è la proprietà inversa di &quot;ha ente che ha emanato il provvedimento&quot;.</rdfs:comment>
        <rdfs:comment xml:lang="en">This is the inverse property of &quot;has issuing agency&quot;.</rdfs:comment>
        <rdfs:isDefinedBy rdf:resource="https://w3id.org/arco/ontology/arco-lite"/>
        <rdfs:label xml:lang="en">is issuing agency of</rdfs:label>
        <rdfs:label xml:lang="it">è ente che ha emanato il provvedimento</rdfs:label>
        <owl:versionInfo xml:lang="it">instabile</owl:versionInfo>
        <owl:versionInfo xml:lang="en">unstable</owl:versionInfo>
    </owl:ObjectProperty>



    <!-- https://w3id.org/arco/ontology/arco-lite/isIssuingStateIn -->

    <owl:ObjectProperty rdf:about="https://w3id.org/arco/ontology/arco-lite/isIssuingStateIn"/>



    <!-- https://w3id.org/arco/ontology/arco-lite/isLocatedIn -->

    <owl:ObjectProperty rdf:about="https://w3id.org/arco/ontology/arco-lite/isLocatedIn">
        <rdfs:subPropertyOf rdf:resource="https://w3id.org/arco/ontology/arco-lite/hasRelatedWork"/>
        <owl:inverseOf rdf:resource="https://w3id.org/arco/ontology/arco-lite/isLocationOf"/>
        <rdfs:domain rdf:resource="http://www.w3.org/2002/07/owl#Thing"/>
        <rdfs:range rdf:resource="http://www.w3.org/2002/07/owl#Thing"/>
        <rdfs:comment xml:lang="it">Questa proprietà collega un bene culturale a un altro bene culturale collegato, che ne costituisce il luogo di collocazione.</rdfs:comment>
        <rdfs:comment xml:lang="en">This property relates a cultural entity to a connected cultural entity which constitutes its location area.</rdfs:comment>
        <rdfs:isDefinedBy rdf:resource="https://w3id.org/arco/ontology/arco-lite"/>
        <rdfs:label xml:lang="it">ha luogo di collocazione</rdfs:label>
        <rdfs:label xml:lang="en">is located in</rdfs:label>
        <rdfs:label xml:lang="it">è contenuto in</rdfs:label>
        <owl:versionInfo xml:lang="it">stabile</owl:versionInfo>
        <owl:versionInfo xml:lang="en">unstable</owl:versionInfo>
        <a-cat:iccdNormTag xml:lang="it">ICCD Normativa Trasversale 4.00: RV/RSE/RSER = &apos;è contenuto in&apos; (versioni precedenti: &apos;luogo di collocazione/localizzazione&apos;; &apos;scheda contenitore&apos;)</a-cat:iccdNormTag>
    </owl:ObjectProperty>



    <!-- https://w3id.org/arco/ontology/arco-lite/isLocationOf -->

    <owl:ObjectProperty rdf:about="https://w3id.org/arco/ontology/arco-lite/isLocationOf">
        <rdfs:subPropertyOf rdf:resource="https://w3id.org/arco/ontology/arco-lite/isWorkRelatedTo"/>
        <rdfs:domain rdf:resource="http://www.w3.org/2002/07/owl#Thing"/>
        <rdfs:range rdf:resource="http://www.w3.org/2002/07/owl#Thing"/>
        <rdfs:comment rdf:resource="https://w3id.org/arco/ontology/arco-lite"/>
        <rdfs:comment xml:lang="it">Questa proprietà, inversa di &apos;is located in&apos;, collega un bene culturale a un altro bene culturale collegato, che costituisce il luogo di collocazione del primo.</rdfs:comment>
        <rdfs:comment xml:lang="en">This property, inverse of &apos;is located in&apos;, relates a cultural entity to a connected cultural entity, which constitutes its location area.</rdfs:comment>
        <rdfs:label xml:lang="en">is location of</rdfs:label>
        <rdfs:label xml:lang="it">è luogo di collocazione di</rdfs:label>
        <owl:versionInfo xml:lang="it">instabile</owl:versionInfo>
        <owl:versionInfo xml:lang="en">unstable</owl:versionInfo>
    </owl:ObjectProperty>



    <!-- https://w3id.org/arco/ontology/arco-lite/isLustreOf -->

    <owl:ObjectProperty rdf:about="https://w3id.org/arco/ontology/arco-lite/isLustreOf">
        <rdfs:subPropertyOf rdf:resource="https://w3id.org/arco/ontology/arco-lite/isPhysicalCharacteristicOf"/>
        <rdfs:domain rdf:resource="https://w3id.org/arco/ontology/natural-specimen-description/PhysicalCharacteristic"/>
        <rdfs:range rdf:resource="http://www.w3.org/2002/07/owl#Thing"/>
        <rdfs:comment xml:lang="it">Questa proprietà collega la lucentezza a un entità.</rdfs:comment>
        <rdfs:comment xml:lang="en">This property relates the lustre to an entity.</rdfs:comment>
        <rdfs:isDefinedBy rdf:resource="https://w3id.org/arco/ontology/arco-lite"/>
        <rdfs:label xml:lang="en">is lustre of</rdfs:label>
        <rdfs:label xml:lang="it">è lucentezza di</rdfs:label>
        <owl:versionInfo xml:lang="it">instabile</owl:versionInfo>
        <owl:versionInfo xml:lang="en">unstable</owl:versionInfo>
    </owl:ObjectProperty>



    <!-- https://w3id.org/arco/ontology/arco-lite/isMagnetismOf -->

    <owl:ObjectProperty rdf:about="https://w3id.org/arco/ontology/arco-lite/isMagnetismOf">
        <rdfs:subPropertyOf rdf:resource="https://w3id.org/arco/ontology/arco-lite/isPhysicalCharacteristicOf"/>
        <rdfs:domain rdf:resource="https://w3id.org/arco/ontology/natural-specimen-description/PhysicalCharacteristic"/>
        <rdfs:range rdf:resource="http://www.w3.org/2002/07/owl#Thing"/>
        <rdfs:comment xml:lang="it">Questa proprietà collega il magnetismo a un entità.</rdfs:comment>
        <rdfs:comment xml:lang="en">This property relates the magnetism to an entity.</rdfs:comment>
        <rdfs:isDefinedBy rdf:resource="https://w3id.org/arco/ontology/arco-lite"/>
        <rdfs:label xml:lang="en">is magnetism of</rdfs:label>
        <rdfs:label xml:lang="it">è magnetismo di</rdfs:label>
        <owl:versionInfo xml:lang="it">instabile</owl:versionInfo>
        <owl:versionInfo xml:lang="en">unstable</owl:versionInfo>
    </owl:ObjectProperty>



    <!-- https://w3id.org/arco/ontology/arco-lite/isMainAgentInvolvedIn -->

    <owl:ObjectProperty rdf:about="https://w3id.org/arco/ontology/arco-lite/isMainAgentInvolvedIn">
        <rdfs:domain rdf:resource="https://w3id.org/italia/onto/l0/Agent"/>
        <rdfs:range rdf:resource="http://www.w3.org/2002/07/owl#Thing"/>
        <rdfs:comment xml:lang="it">Questa proprietà collega il principale agente coinvolto a un&apos;entità.</rdfs:comment>
        <rdfs:comment xml:lang="en">This property relates a main involved agent with its entity.</rdfs:comment>
        <rdfs:isDefinedBy rdf:resource="https://w3id.org/arco/ontology/arco-lite"/>
        <rdfs:label xml:lang="en">is main agent involved in</rdfs:label>
        <rdfs:label xml:lang="it">è agente principale coinvolto in</rdfs:label>
        <owl:versionInfo xml:lang="it">instabile</owl:versionInfo>
        <owl:versionInfo xml:lang="en">unstable</owl:versionInfo>
    </owl:ObjectProperty>



    <!-- https://w3id.org/arco/ontology/arco-lite/isMaterialOf -->

    <owl:ObjectProperty rdf:about="https://w3id.org/arco/ontology/arco-lite/isMaterialOf">
        <rdfs:domain rdf:resource="https://w3id.org/arco/ontology/denotative-description/TechnicalCharacteristic"/>
        <rdfs:range rdf:resource="http://www.w3.org/2002/07/owl#Thing"/>
        <rdfs:comment xml:lang="it">Questa proprietà collega un materiale all&apos;entità composta da quel materiale.</rdfs:comment>
        <rdfs:comment xml:lang="en">This property relates a material with its entity.</rdfs:comment>
        <rdfs:isDefinedBy rdf:resource="https://w3id.org/arco/ontology/arco-lite"/>
        <rdfs:label xml:lang="en">is material of</rdfs:label>
        <rdfs:label xml:lang="it">è materia di</rdfs:label>
        <owl:versionInfo xml:lang="it">instabile</owl:versionInfo>
        <owl:versionInfo xml:lang="en">unstable</owl:versionInfo>
    </owl:ObjectProperty>



    <!-- https://w3id.org/arco/ontology/arco-lite/isMaterialOrTechniqueOf -->

    <owl:ObjectProperty rdf:about="https://w3id.org/arco/ontology/arco-lite/isMaterialOrTechniqueOf">
        <rdfs:domain rdf:resource="https://w3id.org/arco/ontology/denotative-description/TechnicalCharacteristic"/>
        <rdfs:range rdf:resource="http://www.w3.org/2002/07/owl#Thing"/>
        <rdfs:comment xml:lang="it">Questa è la proprietà inversa di &quot;ha materia e tecnica&quot;</rdfs:comment>
        <rdfs:comment xml:lang="en">This is the inverse property of &quot;has material or technique&quot;</rdfs:comment>
        <rdfs:isDefinedBy rdf:resource="https://w3id.org/arco/ontology/arco-lite"/>
        <rdfs:label xml:lang="en">is material or technique of</rdfs:label>
        <rdfs:label xml:lang="it">è materia e tecnica di</rdfs:label>
        <owl:versionInfo xml:lang="it">stabile</owl:versionInfo>
        <owl:versionInfo xml:lang="en">stable</owl:versionInfo>
    </owl:ObjectProperty>



    <!-- https://w3id.org/arco/ontology/arco-lite/isMeasuredDensity -->

    <owl:ObjectProperty rdf:about="https://w3id.org/arco/ontology/arco-lite/isMeasuredDensity">
        <rdfs:subPropertyOf rdf:resource="https://w3id.org/arco/ontology/arco-lite/isPhysicalCharacteristicOf"/>
        <rdfs:domain rdf:resource="https://w3id.org/arco/ontology/natural-specimen-description/PhysicalCharacteristic"/>
        <rdfs:range rdf:resource="http://www.w3.org/2002/07/owl#Thing"/>
        <rdfs:comment xml:lang="it">Questa proprietà collega la densità misurata a un entità.</rdfs:comment>
        <rdfs:comment xml:lang="en">This property relates the measured density to an entity.</rdfs:comment>
        <rdfs:isDefinedBy rdf:resource="https://w3id.org/arco/ontology/arco-lite"/>
        <rdfs:label xml:lang="en">is measured density of</rdfs:label>
        <rdfs:label xml:lang="it">è densità misurata di</rdfs:label>
        <owl:versionInfo xml:lang="it">instabile</owl:versionInfo>
        <owl:versionInfo xml:lang="en">unstable</owl:versionInfo>
    </owl:ObjectProperty>



    <!-- https://w3id.org/arco/ontology/arco-lite/isMintIn -->

    <owl:ObjectProperty rdf:about="https://w3id.org/arco/ontology/arco-lite/isMintIn">
        <rdfs:subPropertyOf rdf:resource="https://w3id.org/arco/ontology/arco-lite/isAgentRelatedTo"/>
        <rdfs:domain rdf:resource="https://w3id.org/italia/onto/l0/Agent"/>
        <rdfs:range rdf:resource="https://w3id.org/arco/ontology/context-description/CoinIssuance"/>
        <rdfs:comment xml:lang="it">Questa è la proprietà inversa di &quot;ha zecca&quot;.</rdfs:comment>
        <rdfs:comment xml:lang="en">This is the inverse property of &quot;has mint&quot;.</rdfs:comment>
        <rdfs:isDefinedBy rdf:resource="https://w3id.org/arco/ontology/arco-lite"/>
        <rdfs:label xml:lang="en">is mint in</rdfs:label>
        <rdfs:label xml:lang="it">è zecca in</rdfs:label>
        <owl:versionInfo xml:lang="it">instabile</owl:versionInfo>
        <owl:versionInfo xml:lang="en">unstable</owl:versionInfo>
    </owl:ObjectProperty>



    <!-- https://w3id.org/arco/ontology/arco-lite/isMinterIn -->

    <owl:ObjectProperty rdf:about="https://w3id.org/arco/ontology/arco-lite/isMinterIn">
        <rdfs:subPropertyOf rdf:resource="https://w3id.org/arco/ontology/arco-lite/isAgentRelatedTo"/>
        <rdfs:domain rdf:resource="https://w3id.org/italia/onto/l0/Agent"/>
        <rdfs:range rdf:resource="https://w3id.org/arco/ontology/context-description/CoinIssuance"/>
        <rdfs:comment xml:lang="it">Questa è la proprietà inversa di &quot;ha zecchiere&quot;.</rdfs:comment>
        <rdfs:comment xml:lang="en">This is the inverse property of &quot;has minter&quot;.</rdfs:comment>
        <rdfs:isDefinedBy rdf:resource="https://w3id.org/arco/ontology/arco-lite"/>
        <rdfs:label xml:lang="en">in minter in</rdfs:label>
        <rdfs:label xml:lang="it">è zecchiere in</rdfs:label>
        <owl:versionInfo xml:lang="it">instabile</owl:versionInfo>
        <owl:versionInfo xml:lang="en">unstable</owl:versionInfo>
    </owl:ObjectProperty>



    <!-- https://w3id.org/arco/ontology/arco-lite/isMohsHardnessOf -->

    <owl:ObjectProperty rdf:about="https://w3id.org/arco/ontology/arco-lite/isMohsHardnessOf">
        <rdfs:subPropertyOf rdf:resource="https://w3id.org/arco/ontology/arco-lite/isPhysicalCharacteristicOf"/>
        <rdfs:domain rdf:resource="https://w3id.org/arco/ontology/natural-specimen-description/PhysicalCharacteristic"/>
        <rdfs:range rdf:resource="http://www.w3.org/2002/07/owl#Thing"/>
        <rdfs:comment xml:lang="it">Questa proprietà collega la durezza secondo la scala di Mohs a un entità.</rdfs:comment>
        <rdfs:comment xml:lang="en">This property relates the hardness according to the Mohs scale to an entity.</rdfs:comment>
        <rdfs:isDefinedBy rdf:resource="https://w3id.org/arco/ontology/arco-lite"/>
        <rdfs:label xml:lang="en">is Mohs scale hardness of</rdfs:label>
        <rdfs:label xml:lang="it">è durezza secondo la scala di Mohs di</rdfs:label>
        <owl:versionInfo xml:lang="it">instabile</owl:versionInfo>
        <owl:versionInfo xml:lang="en">unstable</owl:versionInfo>
    </owl:ObjectProperty>



    <!-- https://w3id.org/arco/ontology/arco-lite/isMusicalEnsembleOf -->

    <owl:ObjectProperty rdf:about="https://w3id.org/arco/ontology/arco-lite/isMusicalEnsembleOf">
        <rdfs:subPropertyOf rdf:resource="https://w3id.org/arco/ontology/arco-lite/isAgentRelatedTo"/>
        <rdfs:domain rdf:resource="https://w3id.org/italia/onto/l0/Agent"/>
        <rdfs:range rdf:resource="http://dati.beniculturali.it/cis/CulturalEntity"/>
        <rdfs:comment xml:lang="it">Questa proprietà collega il gruppo di musicisti (bande, complessi musicali, associazioni corali, ecc.) in cui uno strumento assume, o ha assunto, abitualmente un ruolo esecutivo al relativo strumento musicale.</rdfs:comment>
        <rdfs:comment xml:lang="en">This property relates the musical ensamble where an instument is (or were) played to the related musical instrument.</rdfs:comment>
        <rdfs:isDefinedBy rdf:resource="https://w3id.org/arco/ontology/arco-lite"/>
        <rdfs:label xml:lang="en">is musical ensemble of</rdfs:label>
        <rdfs:label xml:lang="it">è organico musicale di</rdfs:label>
        <owl:versionInfo xml:lang="it">instabile</owl:versionInfo>
        <owl:versionInfo xml:lang="en">unstable</owl:versionInfo>
    </owl:ObjectProperty>



    <!-- https://w3id.org/arco/ontology/arco-lite/isMusicalTemperamentOf -->

    <owl:ObjectProperty rdf:about="https://w3id.org/arco/ontology/arco-lite/isMusicalTemperamentOf">
        <rdfs:subPropertyOf rdf:resource="https://w3id.org/arco/ontology/denotative-description/isTechnicalCharacteristicOf"/>
        <rdfs:domain rdf:resource="https://w3id.org/arco/ontology/denotative-description/TechnicalCharacteristic"/>
        <rdfs:range rdf:resource="http://www.w3.org/2002/07/owl#Thing"/>
        <rdfs:comment xml:lang="it">Questa proprietà è l&apos;inversa di &quot;ha temperamento musicale&quot;.</rdfs:comment>
        <rdfs:comment xml:lang="en">This is the inverse property of &quot;has musical temperament&quot;.</rdfs:comment>
        <rdfs:isDefinedBy rdf:resource="https://w3id.org/arco/ontology/arco-lite"/>
        <rdfs:label xml:lang="en">is musical temperament of</rdfs:label>
        <rdfs:label xml:lang="it">è temperamento musicale di</rdfs:label>
        <owl:versionInfo xml:lang="it">instabile</owl:versionInfo>
        <owl:versionInfo xml:lang="en">unstable</owl:versionInfo>
        <a-cat:iccdNormTag>ICCD Normativa SM 4.00: AA/AAP</a-cat:iccdNormTag>
    </owl:ObjectProperty>



    <!-- https://w3id.org/arco/ontology/arco-lite/isMusicianOf -->

    <owl:ObjectProperty rdf:about="https://w3id.org/arco/ontology/arco-lite/isMusicianOf">
        <rdfs:subPropertyOf rdf:resource="https://w3id.org/arco/ontology/arco-lite/isAgentRelatedTo"/>
        <rdfs:domain rdf:resource="https://w3id.org/italia/onto/l0/Agent"/>
        <rdfs:range rdf:resource="http://dati.beniculturali.it/cis/CulturalEntity"/>
        <rdfs:comment xml:lang="it">Questa proprietà collega una persona che assume - o ha assunto - un ruolo certo come esecutore di uno strumento musicale al relativo strumento.</rdfs:comment>
        <rdfs:comment xml:lang="en">This property relates the person who plays (in the present or past) a certain role as a musical instrument&apos;s exectutor to the related instrument.</rdfs:comment>
        <rdfs:isDefinedBy rdf:resource="https://w3id.org/arco/ontology/arco-lite"/>
        <rdfs:label xml:lang="en">is musician of</rdfs:label>
        <rdfs:label xml:lang="it">è musicista di</rdfs:label>
        <owl:versionInfo xml:lang="it">instabile</owl:versionInfo>
        <owl:versionInfo xml:lang="en">unstable</owl:versionInfo>
    </owl:ObjectProperty>



    <!-- https://w3id.org/arco/ontology/arco-lite/isOfficialInChargeOf -->

    <owl:ObjectProperty rdf:about="https://w3id.org/arco/ontology/arco-lite/isOfficialInChargeOf">
      <rdfs:subPropertyOf rdf:resource="https://w3id.org/arco/ontology/catalogue/isCataloguingAgentOf"/>
      <rdfs:domain rdf:resource="https://w3id.org/italia/onto/l0/Agent"/>
      <rdfs:range>
        <owl:Class>
            <owl:unionOf rdf:parseType="Collection">
                <rdf:Description rdf:about="https://w3id.org/arco/ontology/catalogue/CatalogueRecord"/>
                <rdf:Description rdf:about="https://w3id.org/arco/ontology/catalogue/CatalogueRecordVersion"/>
            </owl:unionOf>
        </owl:Class>
      </rdfs:range>
      <rdfs:comment xml:lang="it">Questa è la proprietà inversa a &quot;ha funzionario responsabile&quot;.</rdfs:comment>
      <rdfs:comment xml:lang="en">This is the inverse property of &quot;has official in charge&quot;.</rdfs:comment>
      <rdfs:isDefinedBy rdf:resource="https://w3id.org/arco/ontology/arco-lite"/>
      <rdfs:label xml:lang="en">is official in charge of</rdfs:label>
      <rdfs:label xml:lang="it">è funzionario responsabile di</rdfs:label>
      <owl:versionInfo xml:lang="it">instabile</owl:versionInfo>
      <owl:versionInfo xml:lang="en">unstable</owl:versionInfo>
    </owl:ObjectProperty>


    <!-- https://w3id.org/arco/ontology/arco-lite/isOperatorOf -->

    <owl:ObjectProperty rdf:about="https://w3id.org/arco/ontology/arco-lite/isOperatorOf">
        <rdfs:subPropertyOf rdf:resource="https://w3id.org/arco/ontology/arco-lite/isAgentRelatedTo"/>
        <rdfs:subPropertyOf rdf:resource="https://w3id.org/arco/ontology/arco-lite/isRelatedAgentTo"/>
        <rdfs:domain rdf:resource="https://w3id.org/italia/onto/l0/Agent"/>
        <rdfs:range>
          <owl:Class>
              <owl:unionOf rdf:parseType="Collection">
                  <rdf:Description rdf:about="https://w3id.org/italia/onto/l0/Activity"/>
                  <rdf:Description rdf:about="https://w3id.org/italia/onto/l0/Object"/>
              </owl:unionOf>
          </owl:Class>
        </rdfs:range>
        <rdfs:comment xml:lang="it">Questa è la proprietà inversa di &quot;ha operatore dell&apos;attività&quot;.</rdfs:comment>
        <rdfs:comment xml:lang="en">This is the inverse property of &quot;has activity operator&quot;.</rdfs:comment>
        <rdfs:isDefinedBy rdf:resource="https://w3id.org/arco/ontology/arco-lite"/>
        <rdfs:label xml:lang="en">is activity operator of</rdfs:label>
        <rdfs:label xml:lang="it">è operatore dell&apos;attività</rdfs:label>
        <owl:versionInfo xml:lang="it">instabile</owl:versionInfo>
        <owl:versionInfo xml:lang="en">unstable</owl:versionInfo>
    </owl:ObjectProperty>



    <!-- https://w3id.org/arco/ontology/arco-lite/isOpticCharacteristicOf -->

    <owl:ObjectProperty rdf:about="https://w3id.org/arco/ontology/arco-lite/isOpticCharacteristicOf">
      <rdfs:subPropertyOf rdf:resource="https://w3id.org/arco/ontology/arco-lite/isPhysicalCharacteristicOf"/>
        <rdfs:domain rdf:resource="https://w3id.org/arco/ontology/natural-specimen-description/OpticCharacteristic"/>
        <rdfs:range rdf:resource="http://www.w3.org/2002/07/owl#Thing"/>
        <rdfs:comment xml:lang="it">Questa proprietà collega una caratteristica ottica a una entità</rdfs:comment>
        <rdfs:comment xml:lang="en">This property relatesthe optic characteristic to an entity</rdfs:comment>
        <rdfs:isDefinedBy rdf:resource="https://w3id.org/arco/ontology/arco-lite"/>
        <rdfs:label xml:lang="it">ha caratteristica ottica</rdfs:label>
        <rdfs:label xml:lang="en">has optic characteristic</rdfs:label>
        <owl:versionInfo xml:lang="it">instabile</owl:versionInfo>
        <owl:versionInfo xml:lang="en">unstable</owl:versionInfo>
    </owl:ObjectProperty>



    <!-- https://w3id.org/arco/ontology/arco-lite/isOpticalPhenomenaOf -->

    <owl:ObjectProperty rdf:about="https://w3id.org/arco/ontology/arco-lite/isOpticalPhenomenaOf">
        <rdfs:subPropertyOf rdf:resource="https://w3id.org/arco/ontology/arco-lite/isPhysicalCharacteristicOf"/>
        <rdfs:domain rdf:resource="https://w3id.org/arco/ontology/natural-specimen-description/PhysicalCharacteristic"/>
        <rdfs:range rdf:resource="http://www.w3.org/2002/07/owl#Thing"/>
        <rdfs:comment xml:lang="it">Questa proprietà collega il fenomeno ottico a un entità.</rdfs:comment>
        <rdfs:comment xml:lang="en">This property relates the oprtical phenomena to an entity.</rdfs:comment>
        <rdfs:isDefinedBy rdf:resource="https://w3id.org/arco/ontology/arco-lite"/>
        <rdfs:label xml:lang="en">is optical phenomena of</rdfs:label>
        <rdfs:label xml:lang="it">è fenomeno ottico di</rdfs:label>
        <owl:versionInfo xml:lang="it">instabile</owl:versionInfo>
        <owl:versionInfo xml:lang="en">unstable</owl:versionInfo>
    </owl:ObjectProperty>



    <!-- https://w3id.org/arco/ontology/arco-lite/isOriginalTaxonOf -->

    <owl:ObjectProperty rdf:about="https://w3id.org/arco/ontology/arco-lite/isOriginalTaxonOf">
        <rdfs:subPropertyOf rdf:resource="https://w3id.org/arco/ontology/core/classifies"/>
        <rdfs:comment xml:lang="it">Questa proprietà collega una classificazione tassonomica originale al suo campione.</rdfs:comment>
        <rdfs:comment xml:lang="en">This property relates an original classified taxon to its specimen.</rdfs:comment>
        <rdfs:isDefinedBy rdf:resource="https://w3id.org/arco/ontology/arco-lite"/>
        <rdfs:label xml:lang="en">is original taxon of</rdfs:label>
        <rdfs:label xml:lang="it">è taxon originale di</rdfs:label>
        <owl:versionInfo xml:lang="it">instabile</owl:versionInfo>
        <owl:versionInfo xml:lang="en">unstable</owl:versionInfo>
    </owl:ObjectProperty>



    <!-- https://w3id.org/arco/ontology/arco-lite/isOwnerOf -->

    <owl:ObjectProperty rdf:about="https://w3id.org/arco/ontology/arco-lite/isOwnerOf">
        <rdfs:subPropertyOf rdf:resource="https://w3id.org/arco/ontology/arco-lite/isAgentRelatedTo"/>
        <rdfs:domain rdf:resource="https://w3id.org/italia/onto/l0/Agent"/>
        <rdfs:range rdf:resource="http://www.w3.org/2002/07/owl#Thing"/>
        <rdfs:comment xml:lang="it">Questa proprietà, inversa a &quot;ha proprietario&quot;, collega un agente al bene culturale, di cui l&apos;agente ha la proprietà.</rdfs:comment>
        <rdfs:comment xml:lang="en">This class relates an agent, that is the owner of a cultural property, to that cultural property.</rdfs:comment>
        <rdfs:isDefinedBy rdf:resource="https://w3id.org/arco/ontology/arco-lite"/>
        <rdfs:label xml:lang="en">is owner in</rdfs:label>
        <rdfs:label xml:lang="it">è proprietario in</rdfs:label>
        <owl:versionInfo xml:lang="it">instabile</owl:versionInfo>
        <owl:versionInfo xml:lang="en">unstable</owl:versionInfo>
        <a-cat:iccdNormTag>ICCD Normativa Trasversale 4.00: TU/CDG/CDGS</a-cat:iccdNormTag>
    </owl:ObjectProperty>



    <!-- https://w3id.org/arco/ontology/arco-lite/isPhosphorescenceOf -->

    <owl:ObjectProperty rdf:about="https://w3id.org/arco/ontology/arco-lite/isPhosphorescenceOf">
        <rdfs:subPropertyOf rdf:resource="https://w3id.org/arco/ontology/arco-lite/isPhysicalCharacteristicOf"/>
        <rdfs:domain rdf:resource="https://w3id.org/arco/ontology/natural-specimen-description/PhysicalCharacteristic"/>
        <rdfs:range rdf:resource="http://www.w3.org/2002/07/owl#Thing"/>
        <rdfs:comment xml:lang="it">Questa proprietà collega la fosforescenza a un entità.</rdfs:comment>
        <rdfs:comment xml:lang="en">This property relates the phosphorescence to an entity.</rdfs:comment>
        <rdfs:isDefinedBy rdf:resource="https://w3id.org/arco/ontology/arco-lite"/>
        <rdfs:label xml:lang="en">is phosphorescence of</rdfs:label>
        <rdfs:label xml:lang="it">è fosforescenza di</rdfs:label>
        <owl:versionInfo xml:lang="it">instabile</owl:versionInfo>
        <owl:versionInfo xml:lang="en">unstable</owl:versionInfo>
    </owl:ObjectProperty>



    <!-- https://w3id.org/arco/ontology/arco-lite/isPhotoColourOf -->

    <owl:ObjectProperty rdf:about="https://w3id.org/arco/ontology/arco-lite/isPhotoColourOf">
        <rdfs:subPropertyOf rdf:resource="https://w3id.org/arco/ontology/denotative-description/isTechnicalCharacteristicOf"/>
        <rdfs:domain rdf:resource="https://w3id.org/arco/ontology/denotative-description/TechnicalCharacteristic"/>
        <rdfs:range rdf:resource="http://www.w3.org/2002/07/owl#Thing"/>
        <rdfs:comment xml:lang="it">Questa è la proprietà inversa a &quot;ha colore della foto&quot;</rdfs:comment>
        <rdfs:comment xml:lang="en">This is the inverse property of &quot;has photo colour&quot;</rdfs:comment>
        <rdfs:isDefinedBy rdf:resource="https://w3id.org/arco/ontology/arco-lite"/>
        <rdfs:label xml:lang="en">is photo colour of</rdfs:label>
        <rdfs:label xml:lang="it">è colore della foto</rdfs:label>
        <owl:versionInfo xml:lang="it">instabile</owl:versionInfo>
        <owl:versionInfo xml:lang="en">unstable</owl:versionInfo>
    </owl:ObjectProperty>



    <!-- https://w3id.org/arco/ontology/arco-lite/isPhotoSizeOf -->

    <owl:ObjectProperty rdf:about="https://w3id.org/arco/ontology/arco-lite/isPhotoSizeOf">
        <rdfs:subPropertyOf rdf:resource="https://w3id.org/arco/ontology/denotative-description/isTechnicalCharacteristicOf"/>
        <rdfs:domain rdf:resource="https://w3id.org/arco/ontology/denotative-description/TechnicalCharacteristic"/>
        <rdfs:range rdf:resource="http://www.w3.org/2002/07/owl#Thing"/>
        <rdfs:comment xml:lang="it">Questa è la proprietà inversa a &quot;ha dimensioni della foto&quot;</rdfs:comment>
        <rdfs:comment xml:lang="en">This is the inverse property of &quot;has photo size&quot;</rdfs:comment>
        <rdfs:isDefinedBy rdf:resource="https://w3id.org/arco/ontology/arco-lite"/>
        <rdfs:label xml:lang="en">is photo size of</rdfs:label>
        <rdfs:label xml:lang="it">è dimensione della foto</rdfs:label>
        <owl:versionInfo xml:lang="it">instabile</owl:versionInfo>
        <owl:versionInfo xml:lang="en">unstable</owl:versionInfo>
    </owl:ObjectProperty>



    <!-- https://w3id.org/arco/ontology/arco-lite/isPhotographerOf -->

    <owl:ObjectProperty rdf:about="https://w3id.org/arco/ontology/arco-lite/isPhotographerOf">
        <rdfs:subPropertyOf rdf:resource="https://w3id.org/arco/ontology/arco-lite/isRelatedAgentTo"/>
        <rdfs:domain rdf:resource="https://w3id.org/italia/onto/l0/Agent"/>
        <rdfs:range rdf:resource="https://w3id.org/arco/ontology/context-description/ObservationSurvey"/>
        <rdfs:comment xml:lang="it">Questa proprietà collega il fotografo professionista (diverso dal rilevatore) che ha effettuato l&apos;indagine all&apos;indagine di rilevamento di un bene demo-etno-antropologico.</rdfs:comment>
        <rdfs:comment xml:lang="en">This property relates the professional photographer who took the shot to the observation survey of a demo-etno-antropologic entity.</rdfs:comment>
        <rdfs:isDefinedBy rdf:resource="https://w3id.org/arco/ontology/arco-lite"/>
        <rdfs:label xml:lang="en">is photographer of</rdfs:label>
        <rdfs:label xml:lang="it">è fotografo di</rdfs:label>
        <owl:versionInfo xml:lang="it">instabile</owl:versionInfo>
        <owl:versionInfo xml:lang="en">unstable</owl:versionInfo>
    </owl:ObjectProperty>



    <!-- https://w3id.org/arco/ontology/arco-lite/isPhysicalCharacteristicOf -->

    <owl:ObjectProperty rdf:about="https://w3id.org/arco/ontology/arco-lite/isPhysicalCharacteristicOf">
        <rdfs:subPropertyOf rdf:resource="https://w3id.org/arco/ontology/denotative-description/isTechnicalCharacteristicOf"/>
        <rdfs:domain rdf:resource="https://w3id.org/arco/ontology/natural-specimen-description/PhysicalCharacteristic"/>
        <rdfs:range rdf:resource="http://www.w3.org/2002/07/owl#Thing"/>
        <rdfs:comment xml:lang="it">Questa proprietà collega la carattteristica fisica a un entità.</rdfs:comment>
        <rdfs:comment xml:lang="en">This property relates the physical characteristic to an entity.</rdfs:comment>
        <rdfs:isDefinedBy rdf:resource="https://w3id.org/arco/ontology/arco-lite"/>
        <rdfs:label xml:lang="en">is physical characteristic of</rdfs:label>
        <rdfs:label xml:lang="it">è caratteristica fisica di</rdfs:label>
        <owl:versionInfo xml:lang="it">instabile</owl:versionInfo>
        <owl:versionInfo xml:lang="en">unstable</owl:versionInfo>
    </owl:ObjectProperty>



    <!-- https://w3id.org/arco/ontology/arco-lite/isPixelDimensionOf -->

    <owl:ObjectProperty rdf:about="https://w3id.org/arco/ontology/arco-lite/isPixelDimensionOf">
        <rdfs:subPropertyOf rdf:resource="https://w3id.org/arco/ontology/denotative-description/isTechnicalCharacteristicOf"/>
        <rdfs:domain rdf:resource="https://w3id.org/arco/ontology/denotative-description/TechnicalCharacteristic"/>
        <rdfs:range rdf:resource="http://www.w3.org/2002/07/owl#Thing"/>
        <rdfs:comment xml:lang="it">Questa è la proprietà inversa di &quot;ha dimensioni in pixel&quot;</rdfs:comment>
        <rdfs:comment xml:lang="en">This is the inverse property of &quot;has pixel dimension&quot;</rdfs:comment>
        <rdfs:isDefinedBy rdf:resource="https://w3id.org/arco/ontology/arco-lite"/>
        <rdfs:label xml:lang="en">is pixel dimension of</rdfs:label>
        <rdfs:label xml:lang="it">è dimensione in pixel di</rdfs:label>
        <owl:versionInfo xml:lang="it">instabile</owl:versionInfo>
        <owl:versionInfo xml:lang="en">unstable</owl:versionInfo>
    </owl:ObjectProperty>



    <!-- https://w3id.org/arco/ontology/arco-lite/isPleochroismOf -->

    <owl:ObjectProperty rdf:about="https://w3id.org/arco/ontology/arco-lite/isPleochroismOf">
        <rdfs:subPropertyOf rdf:resource="https://w3id.org/arco/ontology/arco-lite/isOpticCharacteristicOf"/>
        <rdfs:domain rdf:resource="https://w3id.org/arco/ontology/natural-specimen-description/OpticCharacteristic"/>
        <rdfs:range rdf:resource="http://www.w3.org/2002/07/owl#Thing"/>
        <rdfs:comment xml:lang="it">Questa proprietà collega il pleocroismo al campione</rdfs:comment>
        <rdfs:comment xml:lang="en">This property relates the pleochroism to the specimen</rdfs:comment>
        <rdfs:isDefinedBy rdf:resource="https://w3id.org/arco/ontology/arco-lite"/>
        <rdfs:label xml:lang="en">is pleochroism of</rdfs:label>
        <rdfs:label xml:lang="it">è pleocroismo di</rdfs:label>
        <owl:versionInfo xml:lang="it">instabile</owl:versionInfo>
        <owl:versionInfo xml:lang="en">unstable</owl:versionInfo>
    </owl:ObjectProperty>



    <!-- https://w3id.org/arco/ontology/arco-lite/isPointGroupOf -->

    <owl:ObjectProperty rdf:about="https://w3id.org/arco/ontology/arco-lite/isPointGroupOf">
        <rdfs:subPropertyOf rdf:resource="https://w3id.org/arco/ontology/arco-lite/isCrystallographicCharacteristicOf"/>
        <rdfs:domain rdf:resource="https://w3id.org/arco/ontology/natural-specimen-description/CrystallographicCharacteristic"/>
        <rdfs:range rdf:resource="https://w3id.org/arco/ontology/natural-specimen-description/UnitCell"/>
        <rdfs:comment xml:lang="it">Questa proprietà collega il gruppo puntuale a una cella</rdfs:comment>
        <rdfs:comment xml:lang="en">This property relates the point group to a unit cell</rdfs:comment>
        <rdfs:isDefinedBy rdf:resource="https://w3id.org/arco/ontology/arco-lite"/>
        <rdfs:label xml:lang="en">is point group of</rdfs:label>
        <rdfs:label xml:lang="it">è gruppo puntuale di</rdfs:label>
        <owl:versionInfo xml:lang="it">instabile</owl:versionInfo>
        <owl:versionInfo xml:lang="en">unstable</owl:versionInfo>
    </owl:ObjectProperty>



    <!-- https://w3id.org/arco/ontology/arco-lite/isPreferredAuthorOf -->

    <owl:ObjectProperty rdf:about="https://w3id.org/arco/ontology/arco-lite/isPreferredAuthorOf">
        <rdfs:domain rdf:resource="https://w3id.org/italia/onto/l0/Agent"/>
        <rdfs:range rdf:resource="http://www.w3.org/2002/07/owl#Thing"/>
        <rdfs:label xml:lang="it">è autore preferito di</rdfs:label>
    </owl:ObjectProperty>



    <!-- https://w3id.org/arco/ontology/arco-lite/isPreviousLocationOf -->

    <owl:ObjectProperty rdf:about="https://w3id.org/arco/ontology/arco-lite/isPreviousLocationOf">
        <rdfs:subPropertyOf rdf:resource="https://w3id.org/arco/ontology/arco-lite/isWorkRelatedTo"/>
        <rdfs:domain rdf:resource="http://www.w3.org/2002/07/owl#Thing"/>
        <rdfs:range rdf:resource="http://www.w3.org/2002/07/owl#Thing"/>
        <rdfs:comment xml:lang="it">Questa è la proprietà inversa di &quot;ha sede di provenienza&quot;.</rdfs:comment>
        <rdfs:comment xml:lang="en">This is the inverse property of &quot;has previous location&quot;.</rdfs:comment>
        <rdfs:isDefinedBy rdf:resource="https:/w3id.org/arco/ontology/arco-lite"/>
        <rdfs:label xml:lang="en">is previous location of</rdfs:label>
        <rdfs:label xml:lang="it">è sede di provenienza di</rdfs:label>
        <owl:versionInfo xml:lang="it">instabile</owl:versionInfo>
        <owl:versionInfo xml:lang="en">unstable</owl:versionInfo>
    </owl:ObjectProperty>



    <!-- https://w3id.org/arco/ontology/arco-lite/isPreviousOwnerOf -->

    <owl:ObjectProperty rdf:about="https://w3id.org/arco/ontology/arco-lite/isPreviousOwnerOf">
        <rdfs:domain rdf:resource="https://w3id.org/italia/onto/l0/Agent"/>
        <rdfs:range rdf:resource="http://www.w3.org/2002/07/owl#Thing"/>
    </owl:ObjectProperty>



    <!-- https://w3id.org/arco/ontology/arco-lite/isProponentAgencyOf -->

    <owl:ObjectProperty rdf:about="https://w3id.org/arco/ontology/arco-lite/isProponentAgencyOf">
        <rdfs:subPropertyOf rdf:resource="https://w3id.org/arco/ontology/arco-lite/isAgentRelatedTo"/>
        <rdfs:domain rdf:resource="https://w3id.org/italia/onto/l0/Agent"/>
        <rdfs:range>
            <owl:Class>
                <owl:unionOf rdf:parseType="Collection">
                    <rdf:Description rdf:about="http://dati.beniculturali.it/cis/CulturalEntity"/>
                    <rdf:Description rdf:about="https://w3id.org/arco/ontology/context-description/ProtectiveMeasure"/>
                </owl:unionOf>
            </owl:Class>
        </rdfs:range>
        <rdfs:comment xml:lang="it">Questa proprietà collega all&apos;ente proponente, ovvero il soggetto che ha proposto il provvedimento (identificato per mezzo della denominazione per esteso oppure, nel caso di Enti accreditati dall&apos;ICCD, del relativo codice assegnato dall&apos;Istituto) al provvedimento di tutela relativo al bene culturale, oppure direttamente al bene culturale. La relazione tra il ruolo e l&apos;agente che lo riveste è espressa, in maniera generica, nel nome della proprietà, che quindi ne fornisce una rappresentazione semplificata, con ridotta espressività. Nell&apos;ontologia questa relazione è modellata anche, in maniera più espressiva, dalla classe AgentRole, che permette di collegare l&apos;agente e il suo ruolo.</rdfs:comment>
        <rdfs:comment xml:lang="en">This property relates an agent that is a proponent agency of a protective measure of a cultural property to the protective measure or to the cultural entity itself. The relation is declared in the name of the property, but within the ontology this relation is also modeled, in a more expressive way, through the class AgentRole.</rdfs:comment>
        <rdfs:isDefinedBy rdf:resource="https://w3id.org/arco/ontology/arco-lite"/>
        <rdfs:label xml:lang="en">is proponent agency of</rdfs:label>
        <rdfs:label xml:lang="it">è ente proponente di</rdfs:label>
        <owl:versionInfo xml:lang="it">instabile</owl:versionInfo>
        <owl:versionInfo xml:lang="en">unstable</owl:versionInfo>
        <a-cat:iccdNormTag>ICCD Normativa Trasversale 4.00: TU/NVC/NVCA</a-cat:iccdNormTag>
    </owl:ObjectProperty>



    <!-- https://w3id.org/arco/ontology/arco-lite/isRadioactivityOf -->

    <owl:ObjectProperty rdf:about="https://w3id.org/arco/ontology/arco-lite/isRadioactivityOf">
        <rdfs:subPropertyOf rdf:resource="https://w3id.org/arco/ontology/arco-lite/isPhysicalCharacteristicOf"/>
        <rdfs:domain rdf:resource="https://w3id.org/arco/ontology/natural-specimen-description/PhysicalCharacteristic"/>
        <rdfs:range rdf:resource="http://www.w3.org/2002/07/owl#Thing"/>
        <rdfs:comment xml:lang="it">Questa proprietà collega la radioattività a un entità.</rdfs:comment>
        <rdfs:comment xml:lang="en">This property relates the radioactivity to an entity.</rdfs:comment>
        <rdfs:isDefinedBy rdf:resource="https://w3id.org/arco/ontology/arco-lite"/>
        <rdfs:label xml:lang="en">is radioactivity of</rdfs:label>
        <rdfs:label xml:lang="it">è radioattività di</rdfs:label>
        <owl:versionInfo xml:lang="it">instabile</owl:versionInfo>
        <owl:versionInfo xml:lang="en">unstable</owl:versionInfo>
    </owl:ObjectProperty>



    <!-- https://w3id.org/arco/ontology/arco-lite/isRealizationDateOf -->

    <owl:ObjectProperty rdf:about="https://w3id.org/arco/ontology/arco-lite/isRealizationDateOf">
        <rdfs:domain rdf:resource="https://w3id.org/italia/onto/TI/TimeInterval"/>
        <rdfs:range rdf:resource="http://www.w3.org/2002/07/owl#Thing"/>
        <rdfs:comment xml:lang="it">Questa proprietà collega la data di realizzazione co la sua entità.</rdfs:comment>
        <rdfs:comment xml:lang="en">This property relates a realization date with its entity.</rdfs:comment>
        <rdfs:isDefinedBy rdf:resource="https://w3id.org/arco/ontology/arco-lite"/>
        <rdfs:label xml:lang="en">is realization date of</rdfs:label>
        <rdfs:label xml:lang="it">è data di realizzazione di</rdfs:label>
        <owl:versionInfo xml:lang="it">instabile</owl:versionInfo>
        <owl:versionInfo xml:lang="en">unstable</owl:versionInfo>
    </owl:ObjectProperty>



    <!-- https://w3id.org/arco/ontology/arco-lite/isRelatedAgentTo -->

    <owl:ObjectProperty rdf:about="https://w3id.org/arco/ontology/arco-lite/isRelatedAgentTo">
        <rdfs:domain rdf:resource="http://www.w3.org/2002/07/owl#Thing"/>
        <rdfs:range rdf:resource="https://w3id.org/italia/onto/l0/Agent"/>
        <rdfs:comment xml:lang="it">Questa proprietà collega un agente che è collegato in qualche modo a un&apos;entità di qualsiasi tipo a quell&apos;entità. È una relazione generica che viene usata per quei casi in cui non sia possibile definire in maniera più precisa la natura della relazione.</rdfs:comment>
        <rdfs:comment xml:lang="en">This property is used to associate an agent related in some way to an entity of any kind to that entity. It is used when it is not possible to express the relation in a more specific way.</rdfs:comment>
        <rdfs:isDefinedBy rdf:resource="https://w3id.org/arco/ontology/arco-lite"/>
        <rdfs:label xml:lang="en">is related agent to</rdfs:label>
        <rdfs:label xml:lang="it">è agente correlato a</rdfs:label>
        <owl:versionInfo xml:lang="it">instabile</owl:versionInfo>
        <owl:versionInfo xml:lang="en">unstable</owl:versionInfo>
    </owl:ObjectProperty>



    <!-- https://w3id.org/arco/ontology/arco-lite/isResolutionOf -->

    <owl:ObjectProperty rdf:about="https://w3id.org/arco/ontology/arco-lite/isResolutionOf">
        <rdfs:subPropertyOf rdf:resource="https://w3id.org/arco/ontology/denotative-description/isTechnicalCharacteristicOf"/>
        <rdfs:domain rdf:resource="https://w3id.org/arco/ontology/denotative-description/TechnicalCharacteristic"/>
        <rdfs:range rdf:resource="http://www.w3.org/2002/07/owl#Thing"/>
        <rdfs:comment xml:lang="it">Questa è la proprietà inversa a &quot;ha risoluzione&quot;</rdfs:comment>
        <rdfs:comment xml:lang="en">This is the inverse property of &quot;has resolution&quot;</rdfs:comment>
        <rdfs:isDefinedBy rdf:resource="https://w3id.org/arco/ontology/arco-lite"/>
        <rdfs:label xml:lang="en">is resolution of</rdfs:label>
        <rdfs:label xml:lang="it">è risoluzione di</rdfs:label>
        <owl:versionInfo xml:lang="it">instabile</owl:versionInfo>
        <owl:versionInfo xml:lang="en">unstable</owl:versionInfo>
    </owl:ObjectProperty>



    <!-- https://w3id.org/arco/ontology/arco-lite/isResponsibleAgentOf -->

    <owl:ObjectProperty rdf:about="https://w3id.org/arco/ontology/arco-lite/isResponsibleAgentOf">
        <rdfs:subPropertyOf rdf:resource="https://w3id.org/arco/ontology/arco-lite/isRelatedAgentTo"/>
        <rdfs:domain rdf:resource="https://w3id.org/italia/onto/l0/Agent"/>
        <rdfs:comment xml:lang="it">Questa proprietà collega l&apos;Ente o il soggetto che ha prodotto la scheda o che gestisce la banca dati di cui la scheda fa parte alla scheda stessa.</rdfs:comment>
        <rdfs:comment xml:lang="en">This property relates the agency or the person that created the record or manages the database where the record is to the record itself.</rdfs:comment>
        <rdfs:isDefinedBy rdf:resource="https://w3id.org/arco/ontology/arco-lite"/>
        <rdfs:label xml:lang="en">is responsible agent</rdfs:label>
        <rdfs:label xml:lang="it">è ente responsabile</rdfs:label>
        <owl:versionInfo xml:lang="it">instabile</owl:versionInfo>
        <owl:versionInfo xml:lang="en">unstable</owl:versionInfo>
        <a-cat:iccdNormTag>ICCD Normativa Trasversale 4.00: AC/ACS/ACSE</a-cat:iccdNormTag>
    </owl:ObjectProperty>



    <!-- https://w3id.org/arco/ontology/arco-lite/isResponsibleResearchAndCompilationOf -->

    <owl:ObjectProperty rdf:about="https://w3id.org/arco/ontology/arco-lite/isResponsibleResearchAndCompilationOf">
        <rdfs:subPropertyOf rdf:resource="https://w3id.org/arco/ontology/arco-lite/isCataloguingAgentOf"/>
        <rdfs:domain rdf:resource="https://w3id.org/italia/onto/l0/Agent"/>
        <rdfs:range>
            <owl:Class>
                <owl:unionOf rdf:parseType="Collection">
                    <rdf:Description rdf:about="https://w3id.org/arco/ontology/catalogue/CatalogueRecord"/>
                    <rdf:Description rdf:about="https://w3id.org/arco/ontology/catalogue/CatalogueRecordVersion"/>
                </owl:unionOf>
            </owl:Class>
        </rdfs:range>
        <rdfs:comment xml:lang="it">Questa è la proprietà inversa a &quot;ha responsabile ricerca e redazione&quot;.</rdfs:comment>
        <rdfs:comment xml:lang="en">This is the inverse property of &quot;has responsible research and compilation&quot;.</rdfs:comment>
        <rdfs:isDefinedBy rdf:resource="https://w3id.org/arco/ontology/arco-lite"/>
        <rdfs:label xml:lang="en">is responsible research and compilation of</rdfs:label>
        <rdfs:label xml:lang="it">è responsabile ricerca e redazione di</rdfs:label>
        <owl:versionInfo xml:lang="it">instabile</owl:versionInfo>
        <owl:versionInfo xml:lang="en">instable</owl:versionInfo>
    </owl:ObjectProperty>



    <!-- https://w3id.org/arco/ontology/arco-lite/isReusedBy -->

    <owl:ObjectProperty rdf:about="https://w3id.org/arco/ontology/arco-lite/isReusedBy">
        <rdfs:subPropertyOf rdf:resource="https://w3id.org/arco/ontology/arco-lite/hasRelatedWork"/>
        <owl:inverseOf rdf:resource="https://w3id.org/arco/ontology/arco-lite/reuses"/>
        <rdfs:domain rdf:resource="http://www.w3.org/2002/07/owl#Thing"/>
        <rdfs:range rdf:resource="http://www.w3.org/2002/07/owl#Thing"/>
        <rdfs:comment xml:lang="it">Questa proprietà collega un bene culturale a un altro bene culturale collegato che lo riutilizza in tutto o in parte.</rdfs:comment>
        <rdfs:comment xml:lang="en">This property relates a cultural entity to a connected cultural entity that reuse it or a part of it.</rdfs:comment>
        <rdfs:isDefinedBy rdf:resource="https://w3id.org/arco/ontology/arco-lite"/>
        <rdfs:label xml:lang="en">is reused by</rdfs:label>
        <rdfs:label xml:lang="it">è riutilizzato in</rdfs:label>
        <owl:versionInfo xml:lang="it">instabile</owl:versionInfo>
        <owl:versionInfo xml:lang="en">unstable</owl:versionInfo>
        <a-cat:iccdNormTag xml:lang="it">ICCD Normativa Trasversale 4.00: RV/RSE/RSER = &apos;è riutilizzato in&apos; (versioni precedenti: &apos;bene composto&apos;)</a-cat:iccdNormTag>
    </owl:ObjectProperty>



    <!-- https://w3id.org/arco/ontology/arco-lite/isRightHolderOf -->

    <owl:ObjectProperty rdf:about="https://w3id.org/arco/ontology/arco-lite/isRightHolderOf">
        <rdfs:subPropertyOf rdf:resource="https://w3id.org/arco/ontology/arco-lite/isRelatedAgentTo"/>
        <rdfs:domain rdf:resource="https://w3id.org/italia/onto/l0/Agent"/>
        <rdfs:range rdf:resource="http://www.w3.org/2002/07/owl#Thing"/>
        <rdfs:comment xml:lang="en">Questa proprietà collega un agente detentore di diritti con l&apos;entità.</rdfs:comment>
        <rdfs:comment xml:lang="en">This property relates a right holder with its entity.</rdfs:comment>
        <rdfs:isDefinedBy rdf:resource="https://w3id.org/arco/ontology/arco-lite"/>
        <rdfs:label xml:lang="en">is right holder of</rdfs:label>
        <rdfs:label xml:lang="it">è detentore dei diritti di</rdfs:label>
        <owl:versionInfo xml:lang="it">instabile</owl:versionInfo>
        <owl:versionInfo xml:lang="en">unstable</owl:versionInfo>
    </owl:ObjectProperty>



    <!-- https://w3id.org/arco/ontology/arco-lite/isScientificDirectorOf -->

    <owl:ObjectProperty rdf:about="https://w3id.org/arco/ontology/arco-lite/isScientificDirectorOf">
        <rdfs:subPropertyOf rdf:resource="https://w3id.org/arco/ontology/arco-lite/isRelatedAgentTo"/>
        <rdfs:domain rdf:resource="https://w3id.org/italia/onto/l0/Agent"/>
        <rdfs:range rdf:resource="http://www.w3.org/2002/07/owl#Thing"/>
        <rdfs:comment xml:lang="it">Questa è la proprietà inversa a &quot;ha referente verifica scientifica&quot;.</rdfs:comment>
        <rdfs:comment xml:lang="en">This is the inverse property of &quot;has scientific director&quot;.</rdfs:comment>
        <rdfs:isDefinedBy rdf:resource="https://w3id.org/arco/ontology/arco-lite"/>
        <rdfs:label xml:lang="en">is scientific director of</rdfs:label>
        <rdfs:label xml:lang="it">è referente verifica scientifica di</rdfs:label>
        <owl:versionInfo xml:lang="it">instabile</owl:versionInfo>
        <owl:versionInfo xml:lang="en">unstable</owl:versionInfo>
    </owl:ObjectProperty>



    <!-- https://w3id.org/arco/ontology/arco-lite/isSecondaryAuthorOf -->

    <owl:ObjectProperty rdf:about="https://w3id.org/arco/ontology/arco-lite/isSecondaryAuthorOf"/>



    <!-- https://w3id.org/arco/ontology/arco-lite/isShapeOf -->

    <owl:ObjectProperty rdf:about="https://w3id.org/arco/ontology/arco-lite/isShapeOf">
        <rdfs:subPropertyOf rdf:resource="https://w3id.org/arco/ontology/denotative-description/isTechnicalCharacteristicOf"/>
        <rdfs:domain rdf:resource="https://w3id.org/arco/ontology/denotative-description/TechnicalCharacteristic"/>
        <rdfs:range rdf:resource="http://www.w3.org/2002/07/owl#Thing"/>
        <rdfs:comment xml:lang="it">Questa è la proprietà inversa di &quot;ha forma&quot;</rdfs:comment>
        <rdfs:comment xml:lang="en">This is the inverse property of &quot;has shape&quot;</rdfs:comment>
        <rdfs:isDefinedBy rdf:resource="https://w3id.org/arco/ontology/arco-lite"/>
        <rdfs:label xml:lang="it">ha forma di</rdfs:label>
        <rdfs:label xml:lang="en">is shape of</rdfs:label>
        <owl:versionInfo xml:lang="it">instabile</owl:versionInfo>
        <owl:versionInfo xml:lang="en">unstable</owl:versionInfo>
    </owl:ObjectProperty>



    <!-- https://w3id.org/arco/ontology/arco-lite/isSoundEngineerOf -->

    <owl:ObjectProperty rdf:about="https://w3id.org/arco/ontology/arco-lite/isSoundEngineerOf">
        <rdfs:subPropertyOf rdf:resource="https://w3id.org/arco/ontology/arco-lite/isRelatedAgentTo"/>
        <rdfs:domain rdf:resource="https://w3id.org/italia/onto/l0/Agent"/>
        <rdfs:range rdf:resource="https://w3id.org/arco/ontology/context-description/ObservationSurvey"/>
        <rdfs:comment xml:lang="it">Questa proprietà collega il fonico professionista (diverso dal rilevatore) che ha effettuato la registrazione sonora all&apos;indagine di rilevamento di un bene demo-etno-antropologico.</rdfs:comment>
        <rdfs:comment xml:lang="en">This property relates the sound engineer who recorded an observation survey to the related observation survey of a demo-etno-antropologic entity.</rdfs:comment>
        <rdfs:isDefinedBy rdf:resource="https://w3id.org/arco/ontology/arco-lite"/>
        <rdfs:label xml:lang="en">is sound engineer of</rdfs:label>
        <rdfs:label xml:lang="it">è fonico di</rdfs:label>
        <owl:versionInfo xml:lang="it">instabile</owl:versionInfo>
        <owl:versionInfo xml:lang="en">unstable</owl:versionInfo>
    </owl:ObjectProperty>



    <!-- https://w3id.org/arco/ontology/arco-lite/isSpaceGroupOf -->

    <owl:ObjectProperty rdf:about="https://w3id.org/arco/ontology/arco-lite/isSpaceGroupOf">
        <rdfs:subPropertyOf rdf:resource="https://w3id.org/arco/ontology/arco-lite/isCrystallographicCharacteristicOf"/>
        <rdfs:domain rdf:resource="https://w3id.org/arco/ontology/natural-specimen-description/CrystallographicCharacteristic"/>
        <rdfs:range rdf:resource="https://w3id.org/arco/ontology/natural-specimen-description/UnitCell"/>
        <rdfs:comment xml:lang="it">Questa proprietà collega il gruppo spaziale a una cella</rdfs:comment>
        <rdfs:comment xml:lang="en">This property relates the space group to a unit cell</rdfs:comment>
        <rdfs:isDefinedBy rdf:resource="https://w3id.org/arco/ontology/arco-lite"/>
        <rdfs:label xml:lang="en">is space group of</rdfs:label>
        <rdfs:label xml:lang="it">è gruppo spaziale di</rdfs:label>
        <owl:versionInfo xml:lang="it">instabile</owl:versionInfo>
        <owl:versionInfo xml:lang="en">unstable</owl:versionInfo>
    </owl:ObjectProperty>



    <!-- https://w3id.org/arco/ontology/arco-lite/isSponsorOf -->

    <owl:ObjectProperty rdf:about="https://w3id.org/arco/ontology/arco-lite/isSponsorOf">
        <rdfs:subPropertyOf rdf:resource="https://w3id.org/arco/ontology/arco-lite/isRelatedAgentTo"/>
        <rdfs:domain rdf:resource="https://w3id.org/italia/onto/l0/Agent"/>
        <rdfs:range rdf:resource="https://w3id.org/italia/onto/l0/Activity"/>
        <rdfs:comment xml:lang="it">Questa è la proprietà inversa a &quot;ha sponsor dell&apos;attività&quot;.</rdfs:comment>
        <rdfs:comment xml:lang="en">This is the inverse property of &quot;has activity sponsor&quot;.</rdfs:comment>
        <rdfs:isDefinedBy rdf:resource="https://w3id.org/arco/ontology/arco-lite"/>
        <rdfs:label xml:lang="en">is sponsor of</rdfs:label>
        <rdfs:label xml:lang="it">è finanziatore di</rdfs:label>
        <owl:versionInfo xml:lang="it">instabile</owl:versionInfo>
        <owl:versionInfo xml:lang="en">unstable</owl:versionInfo>
    </owl:ObjectProperty>



    <!-- https://w3id.org/arco/ontology/arco-lite/isStorageMethodOrColourDepthOf -->

    <owl:ObjectProperty rdf:about="https://w3id.org/arco/ontology/arco-lite/isStorageMethodOrColourDepthOf">
        <rdfs:subPropertyOf rdf:resource="https://w3id.org/arco/ontology/denotative-description/isTechnicalCharacteristicOf"/>
        <rdfs:domain rdf:resource="https://w3id.org/arco/ontology/denotative-description/TechnicalCharacteristic"/>
        <rdfs:range rdf:resource="http://www.w3.org/2002/07/owl#Thing"/>
        <rdfs:comment xml:lang="it">Questa è la proprietà inversa di &quot;ha metodo di memorizzazione e profondità del colore&quot;.</rdfs:comment>
        <rdfs:comment xml:lang="en">This is the inverse property of &quot;has storage method or colour depth&quot;.</rdfs:comment>
        <rdfs:isDefinedBy rdf:resource="https://w3id.org/arco/ontology/arco-lite"/>
        <rdfs:label xml:lang="en">is storage method or colour depth of</rdfs:label>
        <rdfs:label xml:lang="it">è metodo di memorizzazione e profondità del colore di</rdfs:label>
        <owl:versionInfo xml:lang="it">instabile</owl:versionInfo>
        <owl:versionInfo xml:lang="en">unstable</owl:versionInfo>
    </owl:ObjectProperty>



    <!-- https://w3id.org/arco/ontology/arco-lite/isStreakOf -->

    <owl:ObjectProperty rdf:about="https://w3id.org/arco/ontology/arco-lite/isStreakOf">
        <rdfs:subPropertyOf rdf:resource="https://w3id.org/arco/ontology/arco-lite/isPhysicalCharacteristicOf"/>
        <rdfs:domain rdf:resource="https://w3id.org/arco/ontology/natural-specimen-description/PhysicalCharacteristic"/>
        <rdfs:range rdf:resource="http://www.w3.org/2002/07/owl#Thing"/>
        <rdfs:comment xml:lang="it">Questa proprietà collega il colore della polvere a un entità.</rdfs:comment>
        <rdfs:comment xml:lang="en">This property relates the streak to an entity.</rdfs:comment>
        <rdfs:isDefinedBy rdf:resource="https://w3id.org/arco/ontology/arco-lite"/>
        <rdfs:label xml:lang="en">is streak of</rdfs:label>
        <rdfs:label xml:lang="it">è colore della polvere di</rdfs:label>
        <owl:versionInfo xml:lang="it">instabile</owl:versionInfo>
        <owl:versionInfo xml:lang="en">unstable</owl:versionInfo>
    </owl:ObjectProperty>


    <!-- https://w3id.org/arco/ontology/arco-lite/isTechniqueOf -->

    <owl:ObjectProperty rdf:about="https://w3id.org/arco/ontology/arco-lite/isTechniqueOf">
        <rdfs:domain rdf:resource="https://w3id.org/arco/ontology/denotative-description/TechnicalCharacteristic"/>
        <rdfs:range rdf:resource="http://www.w3.org/2002/07/owl#Thing"/>
        <rdfs:comment xml:lang="it">Questa proprietà collega una tecnica con un&apos;entità realizzata con quella tecnica.</rdfs:comment>
        <rdfs:comment xml:lang="en">This property relates a technique with its entity.</rdfs:comment>
        <rdfs:isDefinedBy rdf:resource="https://w3id.org/arco/ontology/arco-lite"/>
        <rdfs:label xml:lang="en">is technique of</rdfs:label>
        <rdfs:label xml:lang="it">è tecnica di</rdfs:label>
        <owl:versionInfo xml:lang="it">instabile</owl:versionInfo>
        <owl:versionInfo xml:lang="en">unstable</owl:versionInfo>
    </owl:ObjectProperty>



    <!-- https://w3id.org/arco/ontology/arco-lite/isTemperamentOf -->

    <owl:ObjectProperty rdf:about="https://w3id.org/arco/ontology/arco-lite/isTemperamentOf">
        <rdfs:subPropertyOf rdf:resource="https://w3id.org/arco/ontology/denotative-description/isTechnicalCharacteristicOf"/>
        <rdfs:domain rdf:resource="https://w3id.org/arco/ontology/denotative-description/TechnicalCharacteristic"/>
        <rdfs:range rdf:resource="http://www.w3.org/2002/07/owl#Thing"/>
        <rdfs:comment xml:lang="it">Questa è la proprietà inversa di &quot;ha temperamento&quot;.</rdfs:comment>
        <rdfs:comment xml:lang="en">This is the inverse property of &quot;has temperament&quot;.</rdfs:comment>
        <rdfs:isDefinedBy rdf:resource="https://w3id.org/arco/ontology/arco-lite"/>
        <rdfs:label xml:lang="en">is temperament of</rdfs:label>
        <rdfs:label xml:lang="it">è temperamento di</rdfs:label>
        <owl:versionInfo xml:lang="it">instabile</owl:versionInfo>
        <owl:versionInfo xml:lang="en">unstable</owl:versionInfo>
    </owl:ObjectProperty>



    <!-- https://w3id.org/arco/ontology/arco-lite/isTenacityOf -->

    <owl:ObjectProperty rdf:about="https://w3id.org/arco/ontology/arco-lite/isTenacityOf">
        <rdfs:subPropertyOf rdf:resource="https://w3id.org/arco/ontology/arco-lite/isPhysicalCharacteristicOf"/>
        <rdfs:domain rdf:resource="https://w3id.org/arco/ontology/natural-specimen-description/PhysicalCharacteristic"/>
        <rdfs:range rdf:resource="http://www.w3.org/2002/07/owl#Thing"/>
        <rdfs:comment xml:lang="it">Questa proprietà collega la tenacità a un entità.</rdfs:comment>
        <rdfs:comment xml:lang="en">This property relates the tenacity to an entity.</rdfs:comment>
        <rdfs:isDefinedBy rdf:resource="https://w3id.org/arco/ontology/arco-lite"/>
        <rdfs:label xml:lang="en">is tenacity of</rdfs:label>
        <rdfs:label xml:lang="it">è tenacità di</rdfs:label>
        <owl:versionInfo xml:lang="it">instabile</owl:versionInfo>
        <owl:versionInfo xml:lang="en">unstable</owl:versionInfo>
    </owl:ObjectProperty>



    <!-- https://w3id.org/arco/ontology/arco-lite/isTuningOf -->

    <owl:ObjectProperty rdf:about="https://w3id.org/arco/ontology/arco-lite/isTuningOf">
        <rdfs:subPropertyOf rdf:resource="https://w3id.org/arco/ontology/denotative-description/isTechnicalCharacteristicOf"/>
        <rdfs:domain rdf:resource="https://w3id.org/arco/ontology/denotative-description/TechnicalCharacteristic"/>
        <rdfs:range rdf:resource="http://www.w3.org/2002/07/owl#Thing"/>
        <rdfs:comment xml:lang="it">Questa è la proprietà inversa di &quot;ha accordatura&quot;.</rdfs:comment>
        <rdfs:comment xml:lang="en">This is the inverse property of &quot;has tuning&quot;.</rdfs:comment>
        <rdfs:isDefinedBy rdf:resource="https://w3id.org/arco/ontology/arco-lite"/>
        <rdfs:label xml:lang="en">is tuning of</rdfs:label>
        <rdfs:label xml:lang="it">è accordatura di</rdfs:label>
        <owl:versionInfo xml:lang="it">instabile</owl:versionInfo>
        <owl:versionInfo xml:lang="en">unstable</owl:versionInfo>
        <a-cat:iccdNormTag>ICCD Normativa SM 4.00: AA/AAA</a-cat:iccdNormTag>
    </owl:ObjectProperty>



    <!-- https://w3id.org/arco/ontology/arco-lite/isUserOf -->

    <owl:ObjectProperty rdf:about="https://w3id.org/arco/ontology/arco-lite/isUserOf">
        <rdfs:subPropertyOf rdf:resource="https://w3id.org/arco/ontology/core/isAgentInvolvedIn"/>
        <rdfs:domain rdf:resource="https://w3id.org/italia/onto/l0/Agent"/>
        <rdfs:range rdf:resource="http://www.w3.org/2002/07/owl#Thing"/>
        <rdfs:comment xml:lang="it">Questa proprietà collega un utente, inteso come agente che ha fatto uso di un&apos;entità, all&apos;entità stessa.</rdfs:comment>
        <rdfs:comment xml:lang="en">This property relates the user, intended as the agent who employed an entity, to the related entity.</rdfs:comment>
        <rdfs:isDefinedBy rdf:resource="https://w3id.org/arco/ontology/arco-lite"/>
        <rdfs:label xml:lang="en">is user of</rdfs:label>
        <rdfs:label xml:lang="it">è utente di</rdfs:label>
        <owl:versionInfo xml:lang="it">stabile</owl:versionInfo>
        <owl:versionInfo xml:lang="en">stable</owl:versionInfo>
    </owl:ObjectProperty>



    <!-- https://w3id.org/arco/ontology/arco-lite/isVhnHardnessOf -->

    <owl:ObjectProperty rdf:about="https://w3id.org/arco/ontology/arco-lite/isVhnHardnessOf">
        <rdfs:subPropertyOf rdf:resource="https://w3id.org/arco/ontology/arco-lite/isPhysicalCharacteristicOf"/>
        <rdfs:domain rdf:resource="https://w3id.org/arco/ontology/natural-specimen-description/PhysicalCharacteristic"/>
        <rdfs:range rdf:resource="http://www.w3.org/2002/07/owl#Thing"/>
        <rdfs:comment xml:lang="it">Questa proprietà collega la durezza secondo la scala VHN a un entità.</rdfs:comment>
        <rdfs:comment xml:lang="en">This property relates the hardness according to the VHN scale to an entity.</rdfs:comment>
        <rdfs:isDefinedBy rdf:resource="https://w3id.org/arco/ontology/arco-lite"/>
        <rdfs:label xml:lang="en">is VHN scale hardness of</rdfs:label>
        <rdfs:label xml:lang="it">è durezza secondo la scala VHN di</rdfs:label>
        <owl:versionInfo xml:lang="it">instabile</owl:versionInfo>
        <owl:versionInfo xml:lang="en">unstable</owl:versionInfo>
    </owl:ObjectProperty>



    <!-- https://w3id.org/arco/ontology/arco-lite/isVideoOperatorOf -->

    <owl:ObjectProperty rdf:about="https://w3id.org/arco/ontology/arco-lite/isVideoOperatorOf">
        <rdfs:subPropertyOf rdf:resource="https://w3id.org/arco/ontology/arco-lite/isRelatedAgentTo"/>
        <rdfs:domain rdf:resource="https://w3id.org/italia/onto/l0/Agent"/>
        <rdfs:comment xml:lang="it">Questa è la proprietà inversa di &quot;ha video operatore&quot;.</rdfs:comment>
        <rdfs:comment xml:lang="en">This is the inverse property of &quot;has video operator&quot;.</rdfs:comment>
        <rdfs:isDefinedBy rdf:resource="https://w3id.org/arco/ontology/arco-lite"/>
        <rdfs:label xml:lang="en">is video operator of</rdfs:label>
        <rdfs:label xml:lang="it">è video operatore di</rdfs:label>
        <owl:versionInfo xml:lang="it">instabile</owl:versionInfo>
        <owl:versionInfo xml:lang="en">unstable</owl:versionInfo>
    </owl:ObjectProperty>



    <!-- https://w3id.org/arco/ontology/arco-lite/isWorkRelatedTo -->

    <owl:ObjectProperty rdf:about="https://w3id.org/arco/ontology/arco-lite/isWorkRelatedTo">
        <rdfs:domain rdf:resource="http://www.w3.org/2002/07/owl#Thing"/>
        <rdfs:range rdf:resource="http://www.w3.org/2002/07/owl#Thing"/>
        <rdfs:comment xml:lang="it">Questa è la proprietà inversa a &quot;ha opera collegata&quot;.</rdfs:comment>
        <rdfs:comment xml:lang="en">This is the inverse property of &quot;has related work&quot;.</rdfs:comment>
        <rdfs:isDefinedBy rdf:resource="https://w3id.org/arco/ontology/arco-lite"/>
        <rdfs:label xml:lang="en">is work related to</rdfs:label>
        <rdfs:label xml:lang="it">è opera collegata a</rdfs:label>
        <owl:versionInfo xml:lang="it">instabile</owl:versionInfo>
        <owl:versionInfo xml:lang="en">unstable</owl:versionInfo>
    </owl:ObjectProperty>



    <!-- https://w3id.org/arco/ontology/arco-lite/reuses -->

    <owl:ObjectProperty rdf:about="https://w3id.org/arco/ontology/arco-lite/reuses">
        <rdfs:subPropertyOf rdf:resource="https://w3id.org/arco/ontology/arco-lite/isWorkRelatedTo"/>
        <rdfs:domain rdf:resource="http://www.w3.org/2002/07/owl#Thing"/>
        <rdfs:range rdf:resource="http://www.w3.org/2002/07/owl#Thing"/>
        <rdfs:comment xml:lang="it">Questa è la proprietà inversa di &apos;è riutilizzato da&apos;, che collega un bene culturale a un altro bene culturale collegato che lo riutilizza in tutto o in parte.</rdfs:comment>
        <rdfs:comment xml:lang="en">This is the invers property of &apos;is reused by&apos;, which relates a cultural entity to a connected cultural entity that reuse it or a part of it.</rdfs:comment>
        <rdfs:isDefinedBy rdf:resource="https://w3id.org/arco/ontology/arco-lite"/>
        <rdfs:label xml:lang="en">reuses</rdfs:label>
        <rdfs:label xml:lang="it">riutilizza</rdfs:label>
        <owl:versionInfo xml:lang="it">instabile</owl:versionInfo>
        <owl:versionInfo xml:lang="en">unstable</owl:versionInfo>
    </owl:ObjectProperty>



    <!-- https://w3id.org/arco/ontology/arco-liten/isIssuingStateIn -->

    <owl:ObjectProperty rdf:about="https://w3id.org/arco/ontology/arco-liten/isIssuingStateIn">
        <rdfs:subPropertyOf rdf:resource="https://w3id.org/arco/ontology/arco-lite/isAgentRelatedTo"/>
        <rdfs:domain rdf:resource="https://w3id.org/italia/onto/l0/Agent"/>
        <rdfs:range rdf:resource="https://w3id.org/arco/ontology/context-description/CoinIssuance"/>
        <rdfs:comment xml:lang="it">Questa è la proprietà inversa di &quot;ha stato emittente&quot;.</rdfs:comment>
        <rdfs:comment xml:lang="en">This is the inverse property of &quot;has issuing state&quot;.</rdfs:comment>
        <rdfs:isDefinedBy rdf:resource="https://w3id.org/arco/ontology/arco-lite"/>
        <rdfs:label xml:lang="en">is issuing state in</rdfs:label>
        <rdfs:label xml:lang="it">è stato emittente in</rdfs:label>
        <owl:versionInfo xml:lang="it">instabile</owl:versionInfo>
        <owl:versionInfo xml:lang="en">unstable</owl:versionInfo>
    </owl:ObjectProperty>



    <!-- https://w3id.org/arco/ontology/context-description/isAttributedAuthorIn -->

    <owl:ObjectProperty rdf:about="https://w3id.org/arco/ontology/context-description/isAttributedAuthorIn"/>



    <!-- https://w3id.org/arco/ontology/context-description/isAuthorshipAttributionOf -->

    <owl:ObjectProperty rdf:about="https://w3id.org/arco/ontology/context-description/isAuthorshipAttributionOf"/>



    <!-- https://w3id.org/arco/ontology/location/atLocation -->

    <owl:ObjectProperty rdf:about="https://w3id.org/arco/ontology/location/atLocation"/>



    <!-- https://w3id.org/arco/ontology/location/atSite -->

    <owl:ObjectProperty rdf:about="https://w3id.org/arco/ontology/location/atSite"/>



    <!-- https://w3id.org/arco/ontology/location/hasTimeIndexedTypedLocation -->

    <owl:ObjectProperty rdf:about="https://w3id.org/arco/ontology/location/hasTimeIndexedTypedLocation"/>



    <!-- https://w3id.org/arco/ontology/location/isLocationIn -->

    <owl:ObjectProperty rdf:about="https://w3id.org/arco/ontology/location/isLocationIn"/>



    <!-- https://w3id.org/arco/ontology/location/isSiteIn -->

    <owl:ObjectProperty rdf:about="https://w3id.org/arco/ontology/location/isSiteIn"/>



    <!-- https://w3id.org/arco/ontology/location/isTimeIndexedTypedLocationOf -->

    <owl:ObjectProperty rdf:about="https://w3id.org/arco/ontology/location/isTimeIndexedTypedLocationOf"/>



    <!-- https://w3id.org/italia/onto/CLV/hasAddress -->

    <owl:ObjectProperty rdf:about="https://w3id.org/italia/onto/CLV/hasAddress"/>



    <!-- https://w3id.org/italia/onto/CLV/isAddressFor -->

    <owl:ObjectProperty rdf:about="https://w3id.org/italia/onto/CLV/isAddressFor"/>



    <!--
    ///////////////////////////////////////////////////////////////////////////////////////
    //
    // Data properties
    //
    ///////////////////////////////////////////////////////////////////////////////////////
     -->




    <!-- https://w3id.org/arco/ontology/arco-lite/age -->

    <owl:DatatypeProperty rdf:about="https://w3id.org/arco/ontology/arco-lite/age">
        <rdfs:domain rdf:resource="http://www.w3.org/2002/07/owl#Thing"/>
        <rdfs:range rdf:resource="http://www.w3.org/2000/01/rdf-schema#Literal"/>
        <rdfs:comment xml:lang="it">Questa proprietà collega un&apos;entità alla sua età.</rdfs:comment>
        <rdfs:comment xml:lang="en">This property relates an entity with its age.</rdfs:comment>
        <rdfs:isDefinedBy rdf:resource="https://w3id.org/arco/ontology/arco-lite"/>
        <rdfs:label xml:lang="en">Age</rdfs:label>
        <rdfs:label xml:lang="it">Età</rdfs:label>
        <owl:versionInfo xml:lang="it">instabile</owl:versionInfo>
        <owl:versionInfo xml:lang="en">unstable</owl:versionInfo>
        <a-cat:iccdNormTag>Normativa BDI 4.00: ATTE, AIFH, VIFH, FIFH</a-cat:iccdNormTag>
    </owl:DatatypeProperty>



    <!-- https://w3id.org/arco/ontology/arco-lite/alternativeDesignation -->

    <owl:DatatypeProperty rdf:about="https://w3id.org/arco/ontology/arco-lite/alternativeDesignation">
        <rdfs:domain rdf:resource="http://www.w3.org/2002/07/owl#Thing"/>
        <rdfs:range rdf:resource="http://www.w3.org/2000/01/rdf-schema#Literal"/>
        <rdfs:comment xml:lang="it">Questa proprietà collega un&apos;entità alla sua denominazione alternativa.</rdfs:comment>
        <rdfs:comment xml:lang="en">This property relates an entity with its alternative designation.</rdfs:comment>
        <rdfs:isDefinedBy rdf:resource="https://w3id.org/arco/ontology/arco-lite"/>
        <rdfs:label xml:lang="en">alternative designation</rdfs:label>
        <rdfs:label xml:lang="it">denominazione alternativa</rdfs:label>
        <owl:versionInfo xml:lang="it">instabile</owl:versionInfo>
        <owl:versionInfo xml:lang="en">unstable</owl:versionInfo>
    </owl:DatatypeProperty>



    <!-- https://w3id.org/arco/ontology/arco-lite/alternativeInventoryNumber -->

    <owl:DatatypeProperty rdf:about="https://w3id.org/arco/ontology/arco-lite/alternativeInventoryNumber">
        <rdfs:domain rdf:resource="http://www.w3.org/2002/07/owl#Thing"/>
        <rdfs:range rdf:resource="http://www.w3.org/2000/01/rdf-schema#Literal"/>
        <rdfs:comment xml:lang="it">Questa proprietà collega un&apos;entità al suo numero di inventario alternativo.</rdfs:comment>
        <rdfs:comment xml:lang="en">This property relates an entity with its alternative inventory number.</rdfs:comment>
        <rdfs:isDefinedBy rdf:resource="https://w3id.org/arco/ontology/arco-lite"/>
        <rdfs:label xml:lang="en">alternative inventory number</rdfs:label>
        <rdfs:label xml:lang="it">numero d&apos;inventario alternativo</rdfs:label>
        <owl:versionInfo xml:lang="it">instabile</owl:versionInfo>
        <owl:versionInfo xml:lang="en">unstable</owl:versionInfo>
    </owl:DatatypeProperty>



    <!-- https://w3id.org/arco/ontology/arco-lite/assignedDesignation -->

    <owl:DatatypeProperty rdf:about="https://w3id.org/arco/ontology/arco-lite/assignedDesignation">
        <rdfs:domain rdf:resource="http://www.w3.org/2002/07/owl#Thing"/>
        <rdfs:range rdf:resource="http://www.w3.org/2000/01/rdf-schema#Literal"/>
        <rdfs:comment xml:lang="it">Questa proprietà rappresenta la denominazione attribuita di un oggetto.</rdfs:comment>
        <rdfs:comment xml:lang="en">This property represents the assigned designation of an object.</rdfs:comment>
        <rdfs:isDefinedBy rdf:resource="https://w3id.org/arco/ontology/arco-lite"/>
        <rdfs:label xml:lang="en">assigned designation</rdfs:label>
        <rdfs:label xml:lang="it">denominazione attribuita</rdfs:label>
        <owl:versionInfo xml:lang="it">instabile</owl:versionInfo>
        <owl:versionInfo xml:lang="en">unstable</owl:versionInfo>
    </owl:DatatypeProperty>



    <!-- https://w3id.org/arco/ontology/arco-lite/culturalPropertyValue -->

    <owl:DatatypeProperty rdf:about="https://w3id.org/arco/ontology/arco-lite/culturalPropertyValue">
        <rdfs:domain rdf:resource="http://dati.beniculturali.it/cis/CulturalEntity"/>
        <rdfs:range rdf:resource="http://www.w3.org/2000/01/rdf-schema#Literal"/>
        <rdfs:comment xml:lang="it">Questa proprietà rappresenta il valore economico di un bene culturale. Nel caso di una collezione, questa proprietà rappresenta il valore del bene desunto, quando presente, dall&apos;inventario della collezione o dal suo prezzo di acquisto o vendita. Nel caso di un inventario patrimoniale, questa proprietà rappresenta la stima patrimoniale del bene. Il valore viene preceduto dalla specifica della valuta.</rdfs:comment>
        <rdfs:comment xml:lang="en">This property represents cultural entity&apos;s economic value.. The value is preceded by the currency specification.</rdfs:comment>
        <rdfs:isDefinedBy rdf:resource="https://w3id.org/arco/ontology/arco-lite"/>
        <rdfs:label xml:lang="en">cultural property value</rdfs:label>
        <rdfs:label xml:lang="it">valore del bene culturale</rdfs:label>
        <owl:versionInfo xml:lang="it">instabile</owl:versionInfo>
        <owl:versionInfo xml:lang="en">unstable</owl:versionInfo>
        <a-cat:iccdNormTag xml:lang="it">ICCD Normativa Trasversale 4.00: UB/COL/COLV; UB/INP/INP/INPA; UB/STI</a-cat:iccdNormTag>
    </owl:DatatypeProperty>



    <!-- https://w3id.org/arco/ontology/arco-lite/currentDesignation -->

    <owl:DatatypeProperty rdf:about="https://w3id.org/arco/ontology/arco-lite/currentDesignation">
        <rdfs:domain rdf:resource="http://www.w3.org/2002/07/owl#Thing"/>
        <rdfs:range rdf:resource="http://www.w3.org/2000/01/rdf-schema#Literal"/>
        <rdfs:comment xml:lang="it">Questa proprietà rappresenta la denominazione attuale di un oggetto.</rdfs:comment>
        <rdfs:comment xml:lang="en">This property represents the current designation of an object.</rdfs:comment>
        <rdfs:isDefinedBy rdf:resource="https://w3id.org/arco/ontology/arco-lite"/>
        <rdfs:label xml:lang="en">current designation</rdfs:label>
        <rdfs:label xml:lang="it">denominazione attuale</rdfs:label>
        <owl:deprecated rdf:datatype="http://www.w3.org/2001/XMLSchema#boolean">true</owl:deprecated>
        <owl:versionInfo xml:lang="it">instabile</owl:versionInfo>
        <owl:versionInfo xml:lang="en">unstable</owl:versionInfo>
    </owl:DatatypeProperty>



    <!-- https://w3id.org/arco/ontology/arco-lite/currentInventoryNumber -->

    <owl:DatatypeProperty rdf:about="https://w3id.org/arco/ontology/arco-lite/currentInventoryNumber">
        <rdfs:domain rdf:resource="http://www.w3.org/2002/07/owl#Thing"/>
        <rdfs:range rdf:resource="http://www.w3.org/2000/01/rdf-schema#Literal"/>
        <rdfs:comment xml:lang="it">Questa proprietà collega un&apos;entità al suo numero d&apos;inventario corrente.</rdfs:comment>
        <rdfs:comment xml:lang="en">This property relates an entity with its current inventory number.</rdfs:comment>
        <rdfs:isDefinedBy rdf:resource="https://w3id.org/arco/ontology/arco-lite"/>
        <rdfs:label xml:lang="en">current inventory number</rdfs:label>
        <rdfs:label xml:lang="it">numero di inventario corrente</rdfs:label>
        <owl:versionInfo xml:lang="it">instabile</owl:versionInfo>
        <owl:versionInfo xml:lang="en">unstable</owl:versionInfo>
    </owl:DatatypeProperty>



    <!-- https://w3id.org/arco/ontology/arco-lite/customaryDesignation -->

    <owl:DatatypeProperty rdf:about="https://w3id.org/arco/ontology/arco-lite/customaryDesignation">
        <rdfs:domain rdf:resource="http://www.w3.org/2002/07/owl#Thing"/>
        <rdfs:range rdf:resource="http://www.w3.org/2000/01/rdf-schema#Literal"/>
        <rdfs:comment xml:lang="it">Questa proprietà rappresenta la denominazione consuetudinaria di un oggetto.</rdfs:comment>
        <rdfs:comment xml:lang="en">This property represents the usual designation of an object.</rdfs:comment>
        <rdfs:isDefinedBy rdf:resource="https://w3id.org/arco/ontology/arco-lite"/>
        <rdfs:label xml:lang="en">customary designation</rdfs:label>
        <rdfs:label xml:lang="it">denominazione consuetudinaria</rdfs:label>
        <owl:versionInfo xml:lang="it">instabile</owl:versionInfo>
        <owl:versionInfo xml:lang="en">unstable</owl:versionInfo>
    </owl:DatatypeProperty>



    <!-- https://w3id.org/arco/ontology/arco-lite/depiction -->

    <owl:DatatypeProperty rdf:about="https://w3id.org/arco/ontology/arco-lite/depiction">
        <rdfs:domain rdf:resource="http://www.w3.org/2002/07/owl#Thing"/>
        <rdfs:range rdf:resource="http://www.w3.org/2001/XMLSchema#anyURI"/>
        <rdfs:comment xml:lang="it">Questa proprietà collega un&apos;entità all&apos;uri della sua rappresentazione.</rdfs:comment>
        <rdfs:comment xml:lang="en">This property relates an enitity to the uri of its graphic representation.</rdfs:comment>
        <rdfs:isDefinedBy rdf:resource="https://w3id.org/arco/ontology/arco-lite"/>
        <rdfs:label xml:lang="en">depiction</rdfs:label>
        <rdfs:label xml:lang="it">rappresentazione</rdfs:label>
        <owl:versionInfo xml:lang="it">instabile</owl:versionInfo>
        <owl:versionInfo xml:lang="en">unstable</owl:versionInfo>
    </owl:DatatypeProperty>



    <!-- https://w3id.org/arco/ontology/arco-lite/dialectalDesignation -->

    <owl:DatatypeProperty rdf:about="https://w3id.org/arco/ontology/arco-lite/dialectalDesignation">
        <rdfs:domain rdf:resource="http://www.w3.org/2002/07/owl#Thing"/>
        <rdfs:range rdf:resource="http://www.w3.org/2000/01/rdf-schema#Literal"/>
        <rdfs:comment xml:lang="it">Questa proprietà rappresenta la denominazione dialettale di un oggetto.</rdfs:comment>
        <rdfs:comment xml:lang="en">This property represents the dialectal designation of an object.</rdfs:comment>
        <rdfs:isDefinedBy rdf:resource="https://w3id.org/arco/ontology/arco-lite"/>
        <rdfs:label xml:lang="it">denominazione dialettale</rdfs:label>
        <rdfs:label xml:lang="en">dialectal designation</rdfs:label>
        <owl:versionInfo xml:lang="it">instabile</owl:versionInfo>
        <owl:versionInfo xml:lang="en">unstable</owl:versionInfo>
    </owl:DatatypeProperty>



    <!-- https://w3id.org/arco/ontology/arco-lite/historicalDesignation -->

    <owl:DatatypeProperty rdf:about="https://w3id.org/arco/ontology/arco-lite/historicalDesignation">
        <rdfs:domain rdf:resource="http://www.w3.org/2002/07/owl#Thing"/>
        <rdfs:range rdf:resource="http://www.w3.org/2000/01/rdf-schema#Literal"/>
        <rdfs:comment xml:lang="it">Questa proprietà rappresenta la denominazione storica di un oggetto.</rdfs:comment>
        <rdfs:comment xml:lang="en">This property represents the historical designation of an object.</rdfs:comment>
        <rdfs:isDefinedBy rdf:resource="https://w3id.org/arco/ontology/arco-lite"/>
        <rdfs:label xml:lang="it">denominazione storica</rdfs:label>
        <rdfs:label xml:lang="en">historical designation</rdfs:label>
        <owl:versionInfo xml:lang="it">instabile</owl:versionInfo>
        <owl:versionInfo xml:lang="en">unstable</owl:versionInfo>
    </owl:DatatypeProperty>



    <!-- https://w3id.org/arco/ontology/arco-lite/idiomaticDesignation -->

    <owl:DatatypeProperty rdf:about="https://w3id.org/arco/ontology/arco-lite/idiomaticDesignation">
        <rdfs:domain rdf:resource="http://www.w3.org/2002/07/owl#Thing"/>
        <rdfs:range rdf:resource="http://www.w3.org/2000/01/rdf-schema#Literal"/>
        <rdfs:comment xml:lang="it">Questa proprietà rappresenta la denominazione idiomatica di un oggetto.</rdfs:comment>
        <rdfs:comment xml:lang="en">This property represents the idiomatic designation of an object.</rdfs:comment>
        <rdfs:isDefinedBy rdf:resource="https://w3id.org/arco/ontology/arco-lite"/>
        <rdfs:label xml:lang="it">denominazione idiomatica</rdfs:label>
        <rdfs:label xml:lang="en">idiomatic designation</rdfs:label>
        <owl:versionInfo xml:lang="it">instabile</owl:versionInfo>
        <owl:versionInfo xml:lang="en">unstable</owl:versionInfo>
    </owl:DatatypeProperty>



    <!-- https://w3id.org/arco/ontology/arco-lite/internationalIdentifier -->

    <owl:DatatypeProperty rdf:about="https://w3id.org/arco/ontology/arco-lite/internationalIdentifier">
        <rdfs:subPropertyOf rdf:resource="https://w3id.org/italia/onto/l0/identifier"/>
        <rdfs:domain rdf:resource="http://www.w3.org/2002/07/owl#Thing"/>
        <rdfs:range rdf:resource="http://www.w3.org/2000/01/rdf-schema#Literal"/>
        <rdfs:comment xml:lang="it">Questa proprietà collega un&apos;entità al suo identificativo internazionale.</rdfs:comment>
        <rdfs:comment xml:lang="en">This property relates an entity with its international identifier.</rdfs:comment>
        <rdfs:isDefinedBy rdf:resource="https://w3id.org/arco/ontology/arco-lite"/>
        <rdfs:label xml:lang="it">identificativo internazionale</rdfs:label>
        <rdfs:label xml:lang="en">international identifier</rdfs:label>
        <owl:versionInfo xml:lang="it">instabile</owl:versionInfo>
        <owl:versionInfo xml:lang="en">unstable</owl:versionInfo>
    </owl:DatatypeProperty>



    <!-- https://w3id.org/arco/ontology/arco-lite/localDesignation -->

    <owl:DatatypeProperty rdf:about="https://w3id.org/arco/ontology/arco-lite/localDesignation">
        <rdfs:domain rdf:resource="http://www.w3.org/2002/07/owl#Thing"/>
        <rdfs:range rdf:resource="http://www.w3.org/2000/01/rdf-schema#Literal"/>
        <rdfs:comment xml:lang="it">Questa proprietà rappresenta la denominazione locale di un oggetto.</rdfs:comment>
        <rdfs:comment xml:lang="en">This property represents the local designation of an object.</rdfs:comment>
        <rdfs:isDefinedBy rdf:resource="https://w3id.org/arco/ontology/arco-lite"/>
        <rdfs:label xml:lang="it">denominazione locale</rdfs:label>
        <rdfs:label xml:lang="en">local designation</rdfs:label>
        <owl:versionInfo xml:lang="it">instabile</owl:versionInfo>
        <owl:versionInfo xml:lang="en">unstable</owl:versionInfo>
    </owl:DatatypeProperty>



    <!-- https://w3id.org/arco/ontology/arco-lite/localIdentifier -->

    <owl:DatatypeProperty rdf:about="https://w3id.org/arco/ontology/arco-lite/localIdentifier">
        <rdfs:subPropertyOf rdf:resource="https://w3id.org/italia/onto/l0/identifier"/>
        <rdfs:domain rdf:resource="http://www.w3.org/2002/07/owl#Thing"/>
        <rdfs:range rdf:resource="http://www.w3.org/2000/01/rdf-schema#Literal"/>
        <rdfs:comment xml:lang="it">Questa proprietà collega un&apos;entità al suo identificativo locale.</rdfs:comment>
        <rdfs:comment xml:lang="en">This property relates an entity with its local identifier.</rdfs:comment>
        <rdfs:isDefinedBy rdf:resource="https://w3id.org/arco/ontology/arco-lite"/>
        <rdfs:label xml:lang="it">identificativo locale</rdfs:label>
        <rdfs:label xml:lang="en">local identifier</rdfs:label>
        <owl:versionInfo xml:lang="it">instabile</owl:versionInfo>
        <owl:versionInfo xml:lang="en">unstable</owl:versionInfo>
        <a-cat:iccdNormTag>ICCD Normativa Trasversale 4.00: DO/FTA/FTAN, DO/DRA7DRAN, DO/VDC/VDCN, DO/REG/REGN, DO/FNT/FNTI</a-cat:iccdNormTag>
    </owl:DatatypeProperty>



    <!-- https://w3id.org/arco/ontology/arco-lite/nationalIdentifier -->

    <owl:DatatypeProperty rdf:about="https://w3id.org/arco/ontology/arco-lite/nationalIdentifier">
        <rdfs:subPropertyOf rdf:resource="https://w3id.org/italia/onto/l0/identifier"/>
        <rdfs:domain rdf:resource="http://www.w3.org/2002/07/owl#Thing"/>
        <rdfs:isDefinedBy rdf:resource="https://w3id.org/arco/ontology/arco-lite"/>
        <rdfs:label xml:lang="it">identificativo nazionale</rdfs:label>
        <rdfs:label xml:lang="en">national ientifier</rdfs:label>
        <rdfs:seeAlso xml:lang="it">Questa proprietà collega un&apos;entità al suo identificativo nazionale</rdfs:seeAlso>
        <rdfs:seeAlso xml:lang="en">This property relates an entity with its national identifier</rdfs:seeAlso>
        <owl:versionInfo xml:lang="it">instabile</owl:versionInfo>
        <owl:versionInfo xml:lang="en">unstable</owl:versionInfo>
    </owl:DatatypeProperty>



    <!-- https://w3id.org/arco/ontology/arco-lite/originalDesignation -->

    <owl:DatatypeProperty rdf:about="https://w3id.org/arco/ontology/arco-lite/originalDesignation">
        <rdfs:domain rdf:resource="http://www.w3.org/2002/07/owl#Thing"/>
        <rdfs:range rdf:resource="http://www.w3.org/2000/01/rdf-schema#Literal"/>
        <rdfs:comment xml:lang="it">Questa proprietà rappresenta la denominazione originale di un oggetto.</rdfs:comment>
        <rdfs:comment xml:lang="en">This property represents the original designation of an object.</rdfs:comment>
        <rdfs:isDefinedBy rdf:resource="https://w3id.org/arco/ontology/arco-lite"/>
        <rdfs:label xml:lang="it">denominazione originale</rdfs:label>
        <rdfs:label xml:lang="en">original designation</rdfs:label>
        <owl:versionInfo xml:lang="it">instabile</owl:versionInfo>
        <owl:versionInfo xml:lang="en">unstable</owl:versionInfo>
    </owl:DatatypeProperty>



    <!-- https://w3id.org/arco/ontology/arco-lite/slangDesignation -->

    <owl:DatatypeProperty rdf:about="https://w3id.org/arco/ontology/arco-lite/slangDesignation">
        <rdfs:domain rdf:resource="http://www.w3.org/2002/07/owl#Thing"/>
        <rdfs:range rdf:resource="http://www.w3.org/2000/01/rdf-schema#Literal"/>
        <rdfs:comment xml:lang="it">Questa proprietà rappresenta la denominazione gergale di un oggetto.</rdfs:comment>
        <rdfs:comment xml:lang="en">This property represents the slang designation of an object.</rdfs:comment>
        <rdfs:isDefinedBy rdf:resource="https://w3id.org/arco/ontology/arco-lite"/>
        <rdfs:label xml:lang="it">denominazione gergale</rdfs:label>
        <rdfs:label xml:lang="en">slang designation</rdfs:label>
        <owl:versionInfo xml:lang="it">instabile</owl:versionInfo>
        <owl:versionInfo xml:lang="en">unstable</owl:versionInfo>
    </owl:DatatypeProperty>



    <!-- https://w3id.org/arco/ontology/arco-lite/toponym -->

    <owl:DatatypeProperty rdf:about="https://w3id.org/arco/ontology/arco-lite/toponym">
        <rdfs:domain rdf:resource="https://w3id.org/italia/onto/CLV/Feature"/>
        <rdfs:range rdf:resource="http://www.w3.org/2000/01/rdf-schema#Literal"/>
        <rdfs:comment rdf:resource="https:w3id.org/arco/ontology/arco-lite"/>
        <rdfs:comment xml:lang="it">Questa proprietà collega un luogo al suo toponimo.</rdfs:comment>
        <rdfs:comment xml:lang="en">This property relates a feature with its toponym.</rdfs:comment>
        <rdfs:label xml:lang="it">toponimo</rdfs:label>
        <rdfs:label xml:lang="it">toponym</rdfs:label>
        <owl:versionInfo xml:lang="it">instabile</owl:versionInfo>
        <owl:versionInfo xml:lang="en">unstable</owl:versionInfo>
    </owl:DatatypeProperty>



    <!-- https://w3id.org/arco/ontology/arco-lite/uniqueIdentifier -->

    <owl:DatatypeProperty rdf:about="https://w3id.org/arco/ontology/arco-lite/uniqueIdentifier">
        <rdfs:subPropertyOf rdf:resource="https://w3id.org/italia/onto/l0/identifier"/>
        <rdfs:domain rdf:resource="http://www.w3.org/2002/07/owl#Thing"/>
        <rdfs:range rdf:resource="http://www.w3.org/2000/01/rdf-schema#Literal"/>
        <rdfs:comment xml:lang="it">Questa proprietà collega un&apos;entità al suo identificativo univoco.</rdfs:comment>
        <rdfs:comment xml:lang="en">This property relates an entity with its unique identifier.</rdfs:comment>
        <rdfs:isDefinedBy rdf:resource="https://w3id.org/arco/ontology/arco-lite"/>
        <rdfs:label xml:lang="it">identificativo univoco</rdfs:label>
        <rdfs:label xml:lang="en">unique identifier</rdfs:label>
        <owl:versionInfo xml:lang="it">instabile</owl:versionInfo>
        <owl:versionInfo xml:lang="en">unstable</owl:versionInfo>
    </owl:DatatypeProperty>



    <!--
    ///////////////////////////////////////////////////////////////////////////////////////
    //
    // Classes
    //
    ///////////////////////////////////////////////////////////////////////////////////////
     -->




    <!-- http://dati.beniculturali.it/cis/CollectionCulEnt -->

    <owl:Class rdf:about="http://dati.beniculturali.it/cis/CollectionCulEnt"/>



    <!-- https://w3id.org/arco/ontology/arco-lite/CoinIssuance -->

    <owl:Class rdf:about="https://w3id.org/arco/ontology/arco-lite/CoinIssuance"/>



    <!-- https://w3id.org/arco/ontology/context-description/InventorySituation -->

    <owl:Class rdf:about="https://w3id.org/arco/ontology/context-description/InventorySituation"/>



    <!-- https://w3id.org/arco/ontology/context-description/UseFunction -->

    <owl:Class rdf:about="https://w3id.org/arco/ontology/context-description/UseFunction"/>



    <!-- https://w3id.org/arco/ontology/denotative-description/TechnicalCharacteristic -->

    <owl:Class rdf:about="https://w3id.org/arco/ontology/denotative-description/TechnicalCharacteristic"/>



    <!-- https://w3id.org/italia/onto/CLV/Address -->

    <owl:Class rdf:about="https://w3id.org/italia/onto/CLV/Address"/>



    <!-- https://w3id.org/italia/onto/CLV/Feature -->

    <owl:Class rdf:about="https://w3id.org/italia/onto/CLV/Feature"/>



    <!-- https://w3id.org/italia/onto/l0/Activity -->

    <owl:Class rdf:about="https://w3id.org/italia/onto/l0/Activity"/>



    <!--
    ///////////////////////////////////////////////////////////////////////////////////////
    //
    // Individuals
    //
    ///////////////////////////////////////////////////////////////////////////////////////
     -->




    <!-- https://w3id.org/arco/ontology/arco-lite/GarmentAnalysis -->

    <owl:NamedIndividual rdf:about="https://w3id.org/arco/ontology/arco-lite/GarmentAnalysis">
        <rdf:type rdf:resource="https://w3id.org/arco/ontology/denotative-description/TechnicalCharacteristic"/>
        <rdfs:comment xml:lang="it">Questo individuo rappresenta la definizione tecnica completa dei tessuti, secondo le norme fornite dal C.I.E.T.A., o dei merletti, oppure rappresenta la distinzione fra tessuto unito e tessuto operato.</rdfs:comment>
        <rdfs:comment xml:lang="en">This individual represents the techincal definition of textured fabrics of an ancient or contemporary garment, according to the standard provided by C.I.E.T.A., or laces. It can also represent the dinstrinction between plain fabric and textured fabric.</rdfs:comment>
        <rdfs:isDefinedBy rdf:resource="https://w3id.org/arco/ontology/clothing-description"/>
        <rdfs:label xml:lang="it">Analisi del vestimento</rdfs:label>
        <rdfs:label xml:lang="en">Garment analysis</rdfs:label>
        <owl:versionInfo xml:lang="it">instabile</owl:versionInfo>
        <owl:versionInfo xml:lang="en">unstable</owl:versionInfo>
        <a-cat:iccdNormTag>ICCD Normativa VeAC: MT/MTC/MTCA</a-cat:iccdNormTag>
    </owl:NamedIndividual>
</rdf:RDF>



<!-- Generated by the OWL API (version 4.5.9.2019-02-01T07:24:44Z) https://github.com/owlcs/owlapi -->
