<?xml version="1.0"?>
<rdf:RDF xmlns="https://w3id.org/arco/ontology/arco/"
     xml:base="https://w3id.org/arco/ontology/arco/"
     xmlns:dc="http://purl.org/dc/elements/1.1/"
     xmlns:l0="https://w3id.org/italia/onto/l0/"
     xmlns:ns="http://www.w3.org/2006/vcard/ns#"
     xmlns:CLV="https://w3id.org/italia/onto/CLV/"
     xmlns:cis="http://dati.beniculturali.it/cis/"
     xmlns:owl="http://www.w3.org/2002/07/owl#"
     xmlns:rdf="http://www.w3.org/1999/02/22-rdf-syntax-ns#"
     xmlns:xml="http://www.w3.org/XML/1998/namespace"
     xmlns:xsd="http://www.w3.org/2001/XMLSchema#"
     xmlns:a-cd="https://w3id.org/arco/ontology/context-description/"
     xmlns:a-ce="https://w3id.org/arco/ontology/cultural-event/"
     xmlns:a-dd="https://w3id.org/arco/ontology/denotative-description/"
     xmlns:adms="https://w3id.org/italia/onto/ADMS/"
     xmlns:arco="https://w3id.org/arco/ontology/arco/"
     xmlns:core="https://w3id.org/arco/ontology/core/"
     xmlns:dcat="http://www.w3.org/ns/dcat#"
     xmlns:foaf="http://xmlns.com/foaf/0.1/"
     xmlns:opla="http://ontologydesignpatterns.org/opla/"
     xmlns:prov="http://www.w3.org/ns/prov#"
     xmlns:rdfs="http://www.w3.org/2000/01/rdf-schema#"
     xmlns:a-cat="https://w3id.org/arco/ontology/catalogue/"
     xmlns:a-loc="https://w3id.org/arco/ontology/location/"
     xmlns:opla1="http://www.ontologydesignpatterns.org/opla/"
     xmlns:terms="http://purl.org/dc/terms/"
     xmlns:roapit="https://w3id.org/italia/onto/RO/"
     xmlns:tiapit="https://w3id.org/italia/onto/TI/">
    <owl:Ontology rdf:about="https://w3id.org/arco/ontology/movable-property">
        <owl:versionIRI rdf:resource="https://w3id.org/arco/ontology/movable-property"/>
        <owl:imports rdf:resource="https://w3id.org/arco/ontology/catalogue"/>
        <owl:imports rdf:resource="https://w3id.org/arco/ontology/context-description"/>
        <owl:imports rdf:resource="https://w3id.org/arco/ontology/core"/>
        <owl:imports rdf:resource="https://w3id.org/arco/ontology/cultural-event"/>
        <owl:imports rdf:resource="https://w3id.org/arco/ontology/denotative-description"/>
        <owl:imports rdf:resource="https://w3id.org/arco/ontology/location"/>
        <opla:reusesPatternAsTemplate rdf:resource="http://www.ontologydesignpatterns.org/cp/owl/classification.owl"/>
        <opla:reusesPatternAsTemplate rdf:resource="http://www.ontologydesignpatterns.org/cp/owl/collectionentity.owl"/>
        <opla:reusesPatternAsTemplate rdf:resource="http://www.ontologydesignpatterns.org/cp/owl/componency.owl"/>
        <opla:reusesPatternAsTemplate rdf:resource="http://www.ontologydesignpatterns.org/cp/owl/partof.owl"/>
        <opla:reusesPatternAsTemplate rdf:resource="http://www.ontologydesignpatterns.org/cp/owl/situation.owl"/>
        <opla:reusesPatternAsTemplate rdf:resource="http://www.ontologydesignpatterns.org/cp/owl/timeindexedclassification.owl"/>
        <dc:creator>Aldo Gangemi (ISTC-CNR, STLab)</dc:creator>
        <dc:creator>Andrea Nuzzolese (ISTC-CNR, STLab)</dc:creator>
        <dc:creator>Chiara Veninata (MiBAC, ICCD)</dc:creator>
        <dc:creator>Ludovica Marinucci (ISTC-CNR, STLab)</dc:creator>
        <dc:creator>Margherita Porena (ISTC-CNR, STLab)</dc:creator>
        <dc:creator>Maria Letizia Mancinelli (MiBAC, ICCD)</dc:creator>
        <dc:creator>Valentina Carriero (ISTC-CNR, STLab)</dc:creator>
        <dc:creator>Valentina Presutti (ISTC-CNR, STLab)</dc:creator>
        <dc:description xml:lang="it">Questo è il modulo dei Beni Mobili. Qui si modellano informazioni specifiche relative ai beni mobili.</dc:description>
        <dc:description xml:lang="en">The Movable Property module is the ontology describing information about movable cultural property.</dc:description>
        <dc:language rdf:resource="http://publications.europa.eu/resource/authority/language/ENG"/>
        <dc:language rdf:resource="http://publications.europa.eu/resource/authority/language/ITA"/>
        <dc:title xml:lang="en">Movable property Ontology (ArCo network)</dc:title>
        <dc:title xml:lang="it">Ontologia dei Beni Mobili (ArCo network)</dc:title>
        <terms:issued>2020-06-23</terms:issued>
        <terms:license rdf:resource="https://creativecommons.org/licenses/by-sa/4.0/"/>
        <terms:license rdf:resource="https://w3id.org/italia/controlled-vocabulary/licences/A31_CCBYSA40"/>
        <terms:modified>2020-06-23</terms:modified>
        <rdfs:comment xml:lang="it">Questo è il modulo dei Beni Mobili. Qui si modellano informazioni specifiche relative ai beni mobili.
In questo modulo sono riusati come template i seguenti Ontology Design Patterns:
- http://www.ontologydesignpatterns.org/cp/owl/partof.owl
- http://www.ontologydesignpatterns.org/cp/owl/situation.owl
- http://www.ontologydesignpatterns.org/cp/owl/timeindexedclassification.owl</rdfs:comment>
        <rdfs:comment xml:lang="en">The Movable Property module is the ontology describing information about movable cultural property.
In this module the following Ontology Design Patterns have been used:
- http://www.ontologydesignpatterns.org/cp/owl/partof.owl
- http://www.ontologydesignpatterns.org/cp/owl/situation.owl
- http://www.ontologydesignpatterns.org/cp/owl/timeindexedclassification.owl</rdfs:comment>
        <rdfs:label xml:lang="en">Movable Property Ontology (ArCo network)</rdfs:label>
        <rdfs:label xml:lang="it">Ontologia dei Beni Mobili (ArCo network)</rdfs:label>
        <owl:versionInfo xml:lang="en">Version 0.1</owl:versionInfo>
        <owl:versionInfo xml:lang="it">Versione 0.1</owl:versionInfo>
    </owl:Ontology>
    


    <!-- 
    ///////////////////////////////////////////////////////////////////////////////////////
    //
    // Annotation properties
    //
    ///////////////////////////////////////////////////////////////////////////////////////
     -->

    


    <!-- http://ontologydesignpatterns.org/opla/isNativeTo -->

    <owl:AnnotationProperty rdf:about="http://ontologydesignpatterns.org/opla/isNativeTo"/>
    


    <!-- http://ontologydesignpatterns.org/opla/reusesPatternAsTemplate -->

    <owl:AnnotationProperty rdf:about="http://ontologydesignpatterns.org/opla/reusesPatternAsTemplate"/>
    


    <!-- http://purl.org/dc/elements/1.1/creator -->

    <owl:AnnotationProperty rdf:about="http://purl.org/dc/elements/1.1/creator"/>
    


    <!-- http://purl.org/dc/elements/1.1/description -->

    <owl:AnnotationProperty rdf:about="http://purl.org/dc/elements/1.1/description"/>
    


    <!-- http://purl.org/dc/elements/1.1/language -->

    <owl:AnnotationProperty rdf:about="http://purl.org/dc/elements/1.1/language"/>
    


    <!-- http://purl.org/dc/elements/1.1/title -->

    <owl:AnnotationProperty rdf:about="http://purl.org/dc/elements/1.1/title"/>
    


    <!-- http://purl.org/dc/terms/issued -->

    <owl:AnnotationProperty rdf:about="http://purl.org/dc/terms/issued"/>
    


    <!-- http://purl.org/dc/terms/license -->

    <owl:AnnotationProperty rdf:about="http://purl.org/dc/terms/license"/>
    


    <!-- http://purl.org/dc/terms/modified -->

    <owl:AnnotationProperty rdf:about="http://purl.org/dc/terms/modified"/>
    


    <!-- https://w3id.org/arco/ontology/catalogue/iccdNormTag -->

    <owl:AnnotationProperty rdf:about="https://w3id.org/arco/ontology/catalogue/iccdNormTag"/>
    


    <!-- https://w3id.org/arco/ontology/core/iccdNormTag -->

    <owl:AnnotationProperty rdf:about="https://w3id.org/arco/ontology/core/iccdNormTag"/>
    


    <!-- 
    ///////////////////////////////////////////////////////////////////////////////////////
    //
    // Object Properties
    //
    ///////////////////////////////////////////////////////////////////////////////////////
     -->

    


    <!-- https://w3id.org/arco/ontology/context-description/hasCollection -->

    <owl:ObjectProperty rdf:about="https://w3id.org/arco/ontology/context-description/hasCollection"/>
    


    <!-- https://w3id.org/arco/ontology/context-description/isCollectionIn -->

    <owl:ObjectProperty rdf:about="https://w3id.org/arco/ontology/context-description/isCollectionIn"/>
    


    <!-- https://w3id.org/arco/ontology/core/hasLocation -->

    <owl:ObjectProperty rdf:about="https://w3id.org/arco/ontology/core/hasLocation"/>
    


    <!-- https://w3id.org/arco/ontology/core/hasSituation -->

    <owl:ObjectProperty rdf:about="https://w3id.org/arco/ontology/core/hasSituation"/>
    


    <!-- https://w3id.org/arco/ontology/core/hasType -->

    <owl:ObjectProperty rdf:about="https://w3id.org/arco/ontology/core/hasType"/>
    


    <!-- https://w3id.org/arco/ontology/core/isClassifiedBy -->

    <rdf:Description rdf:about="https://w3id.org/arco/ontology/core/isClassifiedBy">
        <owl:propertyChainAxiom rdf:parseType="Collection">
            <rdf:Description rdf:about="https://w3id.org/arco/ontology/core/hasClassificationInTime"/>
            <rdf:Description rdf:about="https://w3id.org/arco/ontology/movable-property/hasTaxon"/>
        </owl:propertyChainAxiom>
    </rdf:Description>
    


    <!-- https://w3id.org/arco/ontology/core/isLocationOf -->

    <owl:ObjectProperty rdf:about="https://w3id.org/arco/ontology/core/isLocationOf"/>
    


    <!-- https://w3id.org/arco/ontology/core/isSituationOf -->

    <owl:ObjectProperty rdf:about="https://w3id.org/arco/ontology/core/isSituationOf"/>
    


    <!-- https://w3id.org/arco/ontology/core/isTypeOf -->

    <owl:ObjectProperty rdf:about="https://w3id.org/arco/ontology/core/isTypeOf"/>
    


    <!-- https://w3id.org/arco/ontology/denotative-description/hasFontStyle -->

    <owl:ObjectProperty rdf:about="https://w3id.org/arco/ontology/denotative-description/hasFontStyle"/>
    


    <!-- https://w3id.org/arco/ontology/denotative-description/hasMeasurementCollection -->

    <owl:ObjectProperty rdf:about="https://w3id.org/arco/ontology/denotative-description/hasMeasurementCollection"/>
    


    <!-- https://w3id.org/arco/ontology/denotative-description/hasOrientation -->

    <owl:ObjectProperty rdf:about="https://w3id.org/arco/ontology/denotative-description/hasOrientation"/>
    


    <!-- https://w3id.org/arco/ontology/movable-property/hasAccession -->

    <owl:ObjectProperty rdf:about="https://w3id.org/arco/ontology/movable-property/hasAccession">
        <owl:inverseOf rdf:resource="https://w3id.org/arco/ontology/movable-property/isAccessionOf"/>
        <rdf:type rdf:resource="http://www.w3.org/2002/07/owl#FunctionalProperty"/>
        <rdfs:domain rdf:resource="http://dati.beniculturali.it/cis/CulturalEntity"/>
        <rdfs:range rdf:resource="https://w3id.org/arco/ontology/movable-property/Accession"/>
        <rdfs:comment xml:lang="it">Questa proprietà collega il campione all&apos;accessione presso l&apos;ente di riferimento</rdfs:comment>
        <rdfs:comment xml:lang="en">This property relates the specimen to the accession to an agency</rdfs:comment>
        <rdfs:isDefinedBy rdf:resource="https://w3id.org/arco/ontology/movable-property"/>
        <rdfs:label xml:lang="it">ha accessione</rdfs:label>
        <rdfs:label xml:lang="en">has accession</rdfs:label>
        <owl:versionInfo xml:lang="it">instabile</owl:versionInfo>
        <owl:versionInfo xml:lang="en">unstable</owl:versionInfo>
        <a-cat:iccdNormTag>Normativa ICCD BNB: SB/ABC</a-cat:iccdNormTag>
    </owl:ObjectProperty>
    


    <!-- https://w3id.org/arco/ontology/movable-property/hasAssociatedPreparation -->

    <owl:ObjectProperty rdf:about="https://w3id.org/arco/ontology/movable-property/hasAssociatedPreparation">
        <owl:inverseOf rdf:resource="https://w3id.org/arco/ontology/movable-property/isAssociatedPreparationOf"/>
        <rdfs:domain rdf:resource="http://dati.beniculturali.it/cis/CulturalEntity"/>
        <rdfs:range rdf:resource="https://w3id.org/arco/ontology/movable-property/Preparation"/>
        <rdfs:comment xml:lang="it">Questa proprietà collega il campione al preparato associato ad esso</rdfs:comment>
        <rdfs:comment xml:lang="en">This property relates a specimen to its preparation</rdfs:comment>
        <rdfs:isDefinedBy rdf:resource="https://w3id.org/arco/ontology/movable-property"/>
        <rdfs:label xml:lang="it">ha preparato associato</rdfs:label>
        <rdfs:label xml:lang="en">has associated preparation</rdfs:label>
        <owl:versionInfo xml:lang="it">instabile</owl:versionInfo>
        <owl:versionInfo xml:lang="en">unstable</owl:versionInfo>
        <a-cat:iccdNormTag>Normativa ICCD BNB: DB/DBR</a-cat:iccdNormTag>
    </owl:ObjectProperty>
    


    <!-- https://w3id.org/arco/ontology/movable-property/hasBotanicalRevision -->

    <owl:ObjectProperty rdf:about="https://w3id.org/arco/ontology/movable-property/hasBotanicalRevision">
        <owl:inverseOf rdf:resource="https://w3id.org/arco/ontology/movable-property/isBotanicalRevisionOf"/>
        <rdfs:domain rdf:resource="http://dati.beniculturali.it/cis/CulturalEntity"/>
        <rdfs:range rdf:resource="https://w3id.org/arco/ontology/movable-property/BotanicalRevision"/>
        <rdfs:comment xml:lang="it">Questa proprietà collega un campione con la revisione a cui è stato sottoposto</rdfs:comment>
        <rdfs:comment xml:lang="en">This property relates aspecimen to a botanical revision</rdfs:comment>
        <rdfs:isDefinedBy rdf:resource="https://w3id.org/arco/ontology/movable-property"/>
        <rdfs:label xml:lang="it">ha revisione botanica</rdfs:label>
        <rdfs:label xml:lang="en">has botanical revision</rdfs:label>
        <owl:versionInfo xml:lang="it">instabile</owl:versionInfo>
        <owl:versionInfo xml:lang="en">unstable</owl:versionInfo>
        <a-cat:iccdNormTag>Normativa ICCD BNB: RB/RBR</a-cat:iccdNormTag>
    </owl:ObjectProperty>
    


    <!-- https://w3id.org/arco/ontology/movable-property/hasCloseIndividual -->

    <owl:ObjectProperty rdf:about="https://w3id.org/arco/ontology/movable-property/hasCloseIndividual">
        <owl:inverseOf rdf:resource="https://w3id.org/arco/ontology/movable-property/isCloseIndivisualOf"/>
        <rdfs:domain rdf:resource="http://dati.beniculturali.it/cis/CulturalEntity"/>
        <rdfs:range rdf:resource="https://w3id.org/arco/ontology/movable-property/CloseIndividual"/>
        <rdfs:comment xml:lang="it">Questa proprietà collega il campione all&apos;individuo vicino</rdfs:comment>
        <rdfs:comment xml:lang="en">This property relates  the specimen to the close individual</rdfs:comment>
        <rdfs:label xml:lang="it">ha individuo vicino</rdfs:label>
        <rdfs:label xml:lang="en">has close individual</rdfs:label>
        <owl:versionInfo xml:lang="it">instabile</owl:versionInfo>
        <owl:versionInfo xml:lang="en">unstable</owl:versionInfo>
        <a-cat:iccdNormTag>ICCD Normativa BNB: LR/LRI/LRIV</a-cat:iccdNormTag>
    </owl:ObjectProperty>
    


    <!-- https://w3id.org/arco/ontology/movable-property/hasCollectingSite -->

    <owl:ObjectProperty rdf:about="https://w3id.org/arco/ontology/movable-property/hasCollectingSite">
        <rdfs:subPropertyOf rdf:resource="https://w3id.org/arco/ontology/core/hasLocation"/>
        <owl:inverseOf rdf:resource="https://w3id.org/arco/ontology/movable-property/isCollectingSiteOf"/>
        <rdf:type rdf:resource="http://www.w3.org/2002/07/owl#FunctionalProperty"/>
        <rdfs:domain rdf:resource="http://www.w3.org/2002/07/owl#Thing"/>
        <rdfs:range rdf:resource="https://w3id.org/arco/ontology/movable-property/CollectingSite"/>
        <rdfs:comment xml:lang="it">Questa proprietà collega il campione al luogo di raccolta</rdfs:comment>
        <rdfs:comment xml:lang="en">This property relates the specimen to the collecting site</rdfs:comment>
        <rdfs:label xml:lang="it">ha luogo di raccolta</rdfs:label>
        <rdfs:label xml:lang="en">has collecting site</rdfs:label>
        <owl:versionInfo xml:lang="it">instabile</owl:versionInfo>
        <owl:versionInfo xml:lang="en">unstable</owl:versionInfo>
        <a-cat:iccdNormTag>ICCD Normativa BNB: LR/LRI</a-cat:iccdNormTag>
    </owl:ObjectProperty>
    


    <!-- https://w3id.org/arco/ontology/movable-property/hasDirectHigherRank -->

    <owl:ObjectProperty rdf:about="https://w3id.org/arco/ontology/movable-property/hasDirectHigherRank">
        <rdfs:subPropertyOf rdf:resource="https://w3id.org/arco/ontology/movable-property/hasHigherRank"/>
        <owl:inverseOf rdf:resource="https://w3id.org/arco/ontology/movable-property/hasDirectLowerRank"/>
        <rdfs:domain rdf:resource="https://w3id.org/arco/ontology/movable-property/BiologicalTaxon"/>
        <rdfs:range rdf:resource="https://w3id.org/arco/ontology/movable-property/BiologicalTaxon"/>
        <rdfs:comment xml:lang="it">Questa proprietà collega due taxa, dove la prima è più specifica della seconda e non ci sono altri taxa che siano più generali del primo e più specifici del secondo.</rdfs:comment>
        <rdfs:comment xml:lang="en">This property relates two taxa, where the first is more specific then the second and there is no other taxon that is both more general than the first and more specific than the second.</rdfs:comment>
        <rdfs:isDefinedBy rdf:resource="https://w3id.org/arco/ontology/movable-property"/>
        <rdfs:label xml:lang="it">ha rango superiore diretto</rdfs:label>
        <rdfs:label xml:lang="en">has direct higher rank</rdfs:label>
        <owl:versionInfo xml:lang="it">instabile</owl:versionInfo>
        <owl:versionInfo xml:lang="en">unstable</owl:versionInfo>
    </owl:ObjectProperty>
    


    <!-- https://w3id.org/arco/ontology/movable-property/hasDirectLowerRank -->

    <owl:ObjectProperty rdf:about="https://w3id.org/arco/ontology/movable-property/hasDirectLowerRank">
        <rdfs:subPropertyOf rdf:resource="https://w3id.org/arco/ontology/movable-property/hasLowerRank"/>
        <rdfs:domain rdf:resource="https://w3id.org/arco/ontology/movable-property/BiologicalTaxon"/>
        <rdfs:range rdf:resource="https://w3id.org/arco/ontology/movable-property/BiologicalTaxon"/>
        <rdfs:comment xml:lang="it">Questa proprietà collega due taxa, dove la prima è meno specifica della seconda e non ci sono altri taxa che siano più specifici del primo e più denerali del secondo.</rdfs:comment>
        <rdfs:comment xml:lang="en">This property relates two taxa, where the first is less specific then the second and there is no other taxon that is both more specific than the first and more general than the second.</rdfs:comment>
        <rdfs:isDefinedBy rdf:resource="https://w3id.org/arco/ontology/movable-property"/>
        <rdfs:label xml:lang="it">ha rango inferiore diretto</rdfs:label>
        <rdfs:label xml:lang="en">has direct lower rank</rdfs:label>
        <owl:versionInfo xml:lang="it">instabile</owl:versionInfo>
        <owl:versionInfo xml:lang="en">unstable</owl:versionInfo>
    </owl:ObjectProperty>
    


    <!-- https://w3id.org/arco/ontology/movable-property/hasFluidDynamism -->

    <owl:ObjectProperty rdf:about="https://w3id.org/arco/ontology/movable-property/hasFluidDynamism">
        <owl:inverseOf rdf:resource="https://w3id.org/arco/ontology/movable-property/isFluidDynamismOf"/>
        <rdf:type rdf:resource="http://www.w3.org/2002/07/owl#FunctionalProperty"/>
        <rdfs:domain rdf:resource="https://w3id.org/arco/ontology/movable-property/CollectingSite"/>
        <rdfs:range rdf:resource="https://w3id.org/arco/ontology/movable-property/FluidDynamism"/>
        <rdfs:comment xml:lang="it">Questa proprietà collega il luogo di raccolta all&apos;idrodinamismo</rdfs:comment>
        <rdfs:comment xml:lang="en">This property relates the collecting site to the fluid dynamism</rdfs:comment>
        <rdfs:isDefinedBy rdf:resource="https://w3id.org/arco/ontology/movable-property"/>
        <rdfs:label xml:lang="it">ha idrodinamismo</rdfs:label>
        <rdfs:label xml:lang="en">has fluid dynamism</rdfs:label>
        <owl:versionInfo xml:lang="it">instabile</owl:versionInfo>
        <owl:versionInfo xml:lang="en">unstable</owl:versionInfo>
        <a-cat:iccdNormTag>ICCD Normativa BNB: LR/LRI/LRID</a-cat:iccdNormTag>
    </owl:ObjectProperty>
    


    <!-- https://w3id.org/arco/ontology/movable-property/hasHigherRank -->

    <owl:ObjectProperty rdf:about="https://w3id.org/arco/ontology/movable-property/hasHigherRank">
        <owl:inverseOf rdf:resource="https://w3id.org/arco/ontology/movable-property/hasLowerRank"/>
        <rdfs:domain rdf:resource="https://w3id.org/arco/ontology/movable-property/BiologicalTaxon"/>
        <rdfs:range rdf:resource="https://w3id.org/arco/ontology/movable-property/BiologicalTaxon"/>
        <rdfs:comment xml:lang="it">Questa proprietà collega due taxa, dove la prima è più specifica della seconda.</rdfs:comment>
        <rdfs:comment xml:lang="en">This property relates two taxa, where the first is more specific than the second.</rdfs:comment>
        <rdfs:isDefinedBy rdf:resource="https://w3id.org/arco/ontology/movable-property"/>
        <rdfs:label xml:lang="it">ha rango superiore</rdfs:label>
        <rdfs:label xml:lang="en">has higher rank</rdfs:label>
        <owl:versionInfo xml:lang="it">instabile</owl:versionInfo>
        <owl:versionInfo xml:lang="en">unstable</owl:versionInfo>
    </owl:ObjectProperty>
    


    <!-- https://w3id.org/arco/ontology/movable-property/hasHostIndividual -->

    <owl:ObjectProperty rdf:about="https://w3id.org/arco/ontology/movable-property/hasHostIndividual">
        <owl:inverseOf rdf:resource="https://w3id.org/arco/ontology/movable-property/isHostIndividualOf"/>
        <rdfs:domain rdf:resource="http://dati.beniculturali.it/cis/CulturalEntity"/>
        <rdfs:range rdf:resource="https://w3id.org/arco/ontology/movable-property/HostIndividual"/>
        <rdfs:comment xml:lang="it">Questa proprietà collega il campione all&apos;indivduo ospite</rdfs:comment>
        <rdfs:comment xml:lang="en">This property relates the specimen to the host individual</rdfs:comment>
        <rdfs:label xml:lang="it">ha individuo ospite</rdfs:label>
        <rdfs:label xml:lang="en">has host individual</rdfs:label>
        <owl:versionInfo xml:lang="it">instabile</owl:versionInfo>
        <owl:versionInfo xml:lang="en">unstable</owl:versionInfo>
        <a-cat:iccdNormTag>ICCD Normativa BNB: LR/LRI/LRIM</a-cat:iccdNormTag>
    </owl:ObjectProperty>
    


    <!-- https://w3id.org/arco/ontology/movable-property/hasIncline -->

    <owl:ObjectProperty rdf:about="https://w3id.org/arco/ontology/movable-property/hasIncline">
        <owl:inverseOf rdf:resource="https://w3id.org/arco/ontology/movable-property/isInclineOf"/>
        <rdf:type rdf:resource="http://www.w3.org/2002/07/owl#FunctionalProperty"/>
        <rdfs:domain rdf:resource="https://w3id.org/arco/ontology/movable-property/Substrate"/>
        <rdfs:range rdf:resource="https://w3id.org/arco/ontology/movable-property/Incline"/>
        <rdfs:comment xml:lang="it">Questa proprietà  collega il luogo di raccolta all&apos;inclinazione</rdfs:comment>
        <rdfs:comment xml:lang="en">This property relates the collecting site to the incline</rdfs:comment>
        <rdfs:label xml:lang="it">ha inclinazione</rdfs:label>
        <rdfs:label xml:lang="en">has incline</rdfs:label>
        <owl:versionInfo xml:lang="it">instabile</owl:versionInfo>
        <owl:versionInfo xml:lang="en">unstable</owl:versionInfo>
        <a-cat:iccdNormTag>ICCD Normativa BNB: LR/LRI/LRII</a-cat:iccdNormTag>
    </owl:ObjectProperty>
    


    <!-- https://w3id.org/arco/ontology/movable-property/hasLabel -->

    <owl:ObjectProperty rdf:about="https://w3id.org/arco/ontology/movable-property/hasLabel">
        <owl:inverseOf rdf:resource="https://w3id.org/arco/ontology/movable-property/isLabelOf"/>
        <rdfs:domain rdf:resource="http://dati.beniculturali.it/cis/CulturalEntity"/>
        <rdfs:range rdf:resource="https://w3id.org/arco/ontology/movable-property/Label"/>
        <rdfs:comment xml:lang="it">Questa proprietà collega un bene culturale ad un&apos;etichetta</rdfs:comment>
        <rdfs:comment xml:lang="en">This property relates a cultural property to a label.</rdfs:comment>
        <rdfs:isDefinedBy rdf:resource="https://w3id.org/arco/ontology/movable-property"/>
        <rdfs:label xml:lang="it">ha etichetta</rdfs:label>
        <rdfs:label xml:lang="en">has label</rdfs:label>
        <owl:versionInfo xml:lang="it">instabile</owl:versionInfo>
        <owl:versionInfo xml:lang="en">unstable</owl:versionInfo>
        <a-cat:iccdNormTag>ICCD Normativa BNB: SB/SBE</a-cat:iccdNormTag>
    </owl:ObjectProperty>
    


    <!-- https://w3id.org/arco/ontology/movable-property/hasLanguage -->

    <owl:ObjectProperty rdf:about="https://w3id.org/arco/ontology/movable-property/hasLanguage">
        <owl:inverseOf rdf:resource="https://w3id.org/arco/ontology/movable-property/isLanguageOf"/>
        <rdfs:domain rdf:resource="http://www.w3.org/2002/07/owl#Thing"/>
        <rdfs:range rdf:resource="https://w3id.org/arco/ontology/movable-property/Language"/>
        <rdfs:comment xml:lang="it">Questa proprietà collega una cosa alla lingua</rdfs:comment>
        <rdfs:comment xml:lang="en">This property realtes a thing to the language</rdfs:comment>
        <rdfs:isDefinedBy rdf:resource="https://w3id.org/arco/ontology/movable-property"/>
        <rdfs:label xml:lang="it">ha lingua</rdfs:label>
        <rdfs:label xml:lang="en">has language</rdfs:label>
        <owl:versionInfo xml:lang="it">instabile</owl:versionInfo>
        <owl:versionInfo xml:lang="en">unstable</owl:versionInfo>
        <a-cat:iccdNormTag>ICCD Normativa BNB: SB/SBE/SBEL</a-cat:iccdNormTag>
    </owl:ObjectProperty>
    


    <!-- https://w3id.org/arco/ontology/movable-property/hasLowerRank -->

    <owl:ObjectProperty rdf:about="https://w3id.org/arco/ontology/movable-property/hasLowerRank">
        <rdfs:domain rdf:resource="https://w3id.org/arco/ontology/movable-property/BiologicalTaxon"/>
        <rdfs:range rdf:resource="https://w3id.org/arco/ontology/movable-property/BiologicalTaxon"/>
        <rdfs:comment xml:lang="it">Questa proprietà collega due taxa, dove la prima è meno specifica della seconda.</rdfs:comment>
        <rdfs:comment xml:lang="en">This property relates two taxa, where the first is less specific than the second.</rdfs:comment>
        <rdfs:isDefinedBy rdf:resource="https://w3id.org/arco/ontology/movable-property"/>
        <rdfs:label xml:lang="it">ha rango inferiore</rdfs:label>
        <rdfs:label xml:lang="en">has lower rank</rdfs:label>
        <owl:versionInfo xml:lang="it">instabile</owl:versionInfo>
        <owl:versionInfo xml:lang="en">unstable</owl:versionInfo>
    </owl:ObjectProperty>
    


    <!-- https://w3id.org/arco/ontology/movable-property/hasNaturalEnvironment -->

    <owl:ObjectProperty rdf:about="https://w3id.org/arco/ontology/movable-property/hasNaturalEnvironment">
        <owl:inverseOf rdf:resource="https://w3id.org/arco/ontology/movable-property/isNaturalEnvironmentOf"/>
        <rdf:type rdf:resource="http://www.w3.org/2002/07/owl#FunctionalProperty"/>
        <rdfs:domain rdf:resource="https://w3id.org/arco/ontology/movable-property/Substrate"/>
        <rdfs:range rdf:resource="https://w3id.org/arco/ontology/movable-property/NaturalEnvironment"/>
        <rdfs:comment xml:lang="it">Questa proprietà collega il substrato all&apos;ambiente</rdfs:comment>
        <rdfs:comment xml:lang="en">This property relates the substrate to the natural environment</rdfs:comment>
        <rdfs:isDefinedBy rdf:resource="https://w3id.org/arco/ontology/movable-property"/>
        <rdfs:label xml:lang="it">ha ambiente naturale</rdfs:label>
        <rdfs:label xml:lang="en">has natural environment</rdfs:label>
        <owl:versionInfo xml:lang="it">instabile</owl:versionInfo>
        <owl:versionInfo xml:lang="en">unstable</owl:versionInfo>
        <a-cat:iccdNormTag>ICCD Normativa BNB: LR/LRI/LRIB</a-cat:iccdNormTag>
    </owl:ObjectProperty>
    


    <!-- https://w3id.org/arco/ontology/movable-property/hasPreservationType -->

    <owl:ObjectProperty rdf:about="https://w3id.org/arco/ontology/movable-property/hasPreservationType">
        <rdfs:subPropertyOf rdf:resource="https://w3id.org/arco/ontology/core/hasType"/>
        <owl:inverseOf rdf:resource="https://w3id.org/arco/ontology/movable-property/isPreservationTypeOf"/>
        <rdfs:domain rdf:resource="https://w3id.org/arco/ontology/movable-property/FruitSample"/>
        <rdfs:range rdf:resource="https://w3id.org/arco/ontology/movable-property/PreservationType"/>
        <rdfs:comment xml:lang="it">Questa proprietà collega un campione al tipo di conservazione</rdfs:comment>
        <rdfs:comment xml:lang="en">This property relates a specimen to the type of preservation</rdfs:comment>
        <rdfs:isDefinedBy rdf:resource="https://w3id.org/arco/ontology/movable-property"/>
        <rdfs:label xml:lang="it">ha tipo di conservazione</rdfs:label>
        <rdfs:label xml:lang="en">has preservation type</rdfs:label>
        <owl:versionInfo xml:lang="it">instabile</owl:versionInfo>
        <owl:versionInfo xml:lang="en">unstable</owl:versionInfo>
        <a-cat:iccdNormTag>Normativa ICCD BNB: DB/DBC/DBCX</a-cat:iccdNormTag>
    </owl:ObjectProperty>
    


    <!-- https://w3id.org/arco/ontology/movable-property/hasRelatedSample -->

    <owl:ObjectProperty rdf:about="https://w3id.org/arco/ontology/movable-property/hasRelatedSample">
        <owl:inverseOf rdf:resource="https://w3id.org/arco/ontology/movable-property/isRelatedSampleOf"/>
        <rdfs:domain rdf:resource="http://dati.beniculturali.it/cis/CulturalEntity"/>
        <rdfs:range rdf:resource="https://w3id.org/arco/ontology/movable-property/Sample"/>
        <rdfs:comment xml:lang="it">Questa proprietà collega un campione ai reperti delle collezioni ancillari</rdfs:comment>
        <rdfs:comment xml:lang="en">This property relates a specimen to sample belonging to ancillary collection</rdfs:comment>
        <rdfs:isDefinedBy rdf:resource="https://w3id.org/arco/ontology/movable-property"/>
        <rdfs:label xml:lang="it">ha reperto associato</rdfs:label>
        <rdfs:label xml:lang="en">has related sample</rdfs:label>
        <owl:versionInfo xml:lang="it">instabile</owl:versionInfo>
        <owl:versionInfo xml:lang="en">unstable</owl:versionInfo>
        <a-cat:iccdNormTag>Normativa ICCD BNB: DB/DBC, DB/DBX, DB/DBS, DB/DBP</a-cat:iccdNormTag>
    </owl:ObjectProperty>
    


    <!-- https://w3id.org/arco/ontology/movable-property/hasSampleForm -->

    <owl:ObjectProperty rdf:about="https://w3id.org/arco/ontology/movable-property/hasSampleForm">
        <owl:inverseOf rdf:resource="https://w3id.org/arco/ontology/movable-property/isSampleFormOf"/>
        <rdfs:domain rdf:resource="https://w3id.org/arco/ontology/movable-property/WoodSample"/>
        <rdfs:range rdf:resource="https://w3id.org/arco/ontology/movable-property/SampleForm"/>
        <rdfs:comment xml:lang="it">Questa proprietà collega un campione alla forma</rdfs:comment>
        <rdfs:comment xml:lang="en">This property relates a specimen to a form</rdfs:comment>
        <rdfs:isDefinedBy rdf:resource="https://w3id.org/arco/ontology/movable-property"/>
        <rdfs:label xml:lang="it">ha forma del reperto</rdfs:label>
        <rdfs:label xml:lang="en">has sample form</rdfs:label>
        <owl:versionInfo xml:lang="it">instabile</owl:versionInfo>
        <owl:versionInfo xml:lang="en">unstable</owl:versionInfo>
        <a-cat:iccdNormTag>Normativa ICCD BNB: DB/DBX/DBXX</a-cat:iccdNormTag>
    </owl:ObjectProperty>
    


    <!-- https://w3id.org/arco/ontology/movable-property/hasShadeTolerance -->

    <owl:ObjectProperty rdf:about="https://w3id.org/arco/ontology/movable-property/hasShadeTolerance">
        <owl:inverseOf rdf:resource="https://w3id.org/arco/ontology/movable-property/isShadeToleranceOf"/>
        <rdfs:domain rdf:resource="https://w3id.org/arco/ontology/movable-property/CollectingSite"/>
        <rdfs:range rdf:resource="https://w3id.org/arco/ontology/movable-property/ShadeTolerance"/>
        <rdfs:comment xml:lang="it">Questa proprietà collega il luogo di raccolta del campione alla caratteristica del popolamento del luogo</rdfs:comment>
        <rdfs:comment xml:lang="en">This property relates the collecting site the individuals&apos; shade tolerance</rdfs:comment>
        <rdfs:isDefinedBy rdf:resource="https://w3id.org/arco/ontology/movable-property"/>
        <rdfs:label xml:lang="it">ha situazione luminosa</rdfs:label>
        <rdfs:label xml:lang="en">has shade tolerance</rdfs:label>
        <owl:versionInfo xml:lang="it">instabile</owl:versionInfo>
        <owl:versionInfo xml:lang="en">unstable</owl:versionInfo>
        <a-cat:iccdNormTag xml:lang="it">ICCD Normativa BNB: LR/LRI/LRIS</a-cat:iccdNormTag>
    </owl:ObjectProperty>
    


    <!-- https://w3id.org/arco/ontology/movable-property/hasSpecimenHarvesting -->

    <owl:ObjectProperty rdf:about="https://w3id.org/arco/ontology/movable-property/hasSpecimenHarvesting">
        <owl:inverseOf rdf:resource="https://w3id.org/arco/ontology/movable-property/isSpecimenHarvestingOf"/>
        <rdf:type rdf:resource="http://www.w3.org/2002/07/owl#FunctionalProperty"/>
        <rdfs:domain rdf:resource="https://w3id.org/italia/onto/l0/Entity"/>
        <rdfs:range rdf:resource="https://w3id.org/arco/ontology/movable-property/SpecimenHarvesting"/>
        <rdfs:comment xml:lang="it">Questa proprietà collega il campione alle informazioni sulla sua raccolta</rdfs:comment>
        <rdfs:comment xml:lang="en">This property relates the specimen to the information about its harvesting</rdfs:comment>
        <rdfs:isDefinedBy rdf:resource="https://w3id.org/arco/ontology/movable-property"/>
        <rdfs:label xml:lang="it">ha raccolta del campione</rdfs:label>
        <rdfs:label xml:lang="en">has specimen harvesting</rdfs:label>
        <owl:versionInfo xml:lang="it">instabile</owl:versionInfo>
        <owl:versionInfo xml:lang="en">unstable</owl:versionInfo>
        <a-cat:iccdNormTag>ICCD Normativa BNB: LR/LRD, LR/LRD</a-cat:iccdNormTag>
    </owl:ObjectProperty>
    


    <!-- https://w3id.org/arco/ontology/movable-property/hasSubstrate -->

    <owl:ObjectProperty rdf:about="https://w3id.org/arco/ontology/movable-property/hasSubstrate">
        <owl:inverseOf rdf:resource="https://w3id.org/arco/ontology/movable-property/isSubstrateOf"/>
        <rdf:type rdf:resource="http://www.w3.org/2002/07/owl#FunctionalProperty"/>
        <rdfs:domain rdf:resource="https://w3id.org/arco/ontology/movable-property/CollectingSite"/>
        <rdfs:range rdf:resource="https://w3id.org/arco/ontology/movable-property/Substrate"/>
        <rdfs:comment xml:lang="it">Questa proprietà collega il luogo di raccolta al substrato</rdfs:comment>
        <rdfs:comment xml:lang="en">This property relates the collecting site to the substrate</rdfs:comment>
        <rdfs:isDefinedBy rdf:resource="https://w3id.org/arco/ontology/movable-property"/>
        <rdfs:label xml:lang="it">ha substrato</rdfs:label>
        <rdfs:label xml:lang="en">has substrate</rdfs:label>
        <owl:versionInfo xml:lang="it">instabile</owl:versionInfo>
        <owl:versionInfo xml:lang="en">unstable</owl:versionInfo>
        <a-cat:iccdNormTag>ICCD Normativa BNB: LR/LRI/LRIR</a-cat:iccdNormTag>
    </owl:ObjectProperty>
    


    <!-- https://w3id.org/arco/ontology/movable-property/hasTaxon -->

    <owl:ObjectProperty rdf:about="https://w3id.org/arco/ontology/movable-property/hasTaxon">
        <owl:inverseOf rdf:resource="https://w3id.org/arco/ontology/movable-property/isTaxonOf"/>
        <rdfs:domain rdf:resource="http://www.w3.org/2002/07/owl#Thing"/>
        <rdfs:range rdf:resource="https://w3id.org/arco/ontology/movable-property/BiologicalTaxon"/>
        <rdfs:comment xml:lang="it">Questa proprietà collega un&apos;entità biologica a un taxon.</rdfs:comment>
        <rdfs:comment xml:lang="en">This property relates a biological entity to a taxon.</rdfs:comment>
        <rdfs:isDefinedBy rdf:resource="https://w3id.org/arco/ontology/movable-property"/>
        <rdfs:label xml:lang="it">ha taxon</rdfs:label>
        <rdfs:label xml:lang="en">has taxon</rdfs:label>
        <owl:versionInfo xml:lang="it">instabile</owl:versionInfo>
        <owl:versionInfo xml:lang="en">unstable</owl:versionInfo>
        <a-cat:iccdNormTag>ICCD Normativa AT: OG/OGS. BNB: SB/SBS/SBSA, SB/NBN/NBNA, SB/NAA, SB/TBI/TBIN, SB/NAT, RB/RBR/RBRN, RB/RBN</a-cat:iccdNormTag>
    </owl:ObjectProperty>
    


    <!-- https://w3id.org/arco/ontology/movable-property/hasTypeSpecimenIdentification -->

    <owl:ObjectProperty rdf:about="https://w3id.org/arco/ontology/movable-property/hasTypeSpecimenIdentification">
        <rdfs:subPropertyOf rdf:resource="https://w3id.org/arco/ontology/core/hasSituation"/>
        <owl:inverseOf rdf:resource="https://w3id.org/arco/ontology/movable-property/isTypeSpecimenIdentificationOf"/>
        <rdfs:domain rdf:resource="http://dati.beniculturali.it/cis/CulturalEntity"/>
        <rdfs:range rdf:resource="https://w3id.org/arco/ontology/movable-property/TypeSpecimenIdentification"/>
        <rdfs:comment xml:lang="it">Questa proprietà collega il campione all&apos;individuazione del tipo nomenclaturale creato a partire dal campione</rdfs:comment>
        <rdfs:comment xml:lang="en">This property relates the specimen to the identification of type specimen</rdfs:comment>
        <rdfs:isDefinedBy rdf:resource="https://w3id.org/arco/ontology/movable-property"/>
        <rdfs:label xml:lang="it">ha identificazione del tipo nomenclaturale</rdfs:label>
        <rdfs:label xml:lang="en">has type specimen identification</rdfs:label>
        <owl:versionInfo xml:lang="it">instabile</owl:versionInfo>
        <owl:versionInfo xml:lang="en">unstable</owl:versionInfo>
        <a-cat:iccdNormTag>ICCD Normativa BNB: SB/TBI</a-cat:iccdNormTag>
    </owl:ObjectProperty>
    


    <!-- https://w3id.org/arco/ontology/movable-property/isAccessionOf -->

    <owl:ObjectProperty rdf:about="https://w3id.org/arco/ontology/movable-property/isAccessionOf">
        <rdfs:domain rdf:resource="https://w3id.org/arco/ontology/movable-property/Accession"/>
        <rdfs:range rdf:resource="http://dati.beniculturali.it/cis/CulturalEntity"/>
        <rdfs:comment xml:lang="it">Questa proprietà collega l&apos;accessione presso l&apos;ente di riferimento al campione</rdfs:comment>
        <rdfs:comment xml:lang="en">This property relates the accession to a specimen</rdfs:comment>
        <rdfs:isDefinedBy rdf:resource="https://w3id.org/arco/ontology/movable-property"/>
        <rdfs:label xml:lang="en">is accession of</rdfs:label>
        <rdfs:label xml:lang="it">è accessione di</rdfs:label>
        <owl:versionInfo xml:lang="it">instabile</owl:versionInfo>
        <owl:versionInfo xml:lang="en">unstable</owl:versionInfo>
    </owl:ObjectProperty>
    


    <!-- https://w3id.org/arco/ontology/movable-property/isAssociatedPreparationOf -->

    <owl:ObjectProperty rdf:about="https://w3id.org/arco/ontology/movable-property/isAssociatedPreparationOf">
        <rdfs:domain rdf:resource="https://w3id.org/arco/ontology/movable-property/Preparation"/>
        <rdfs:range rdf:resource="http://dati.beniculturali.it/cis/CulturalEntity"/>
        <rdfs:comment xml:lang="it">Questa proprietà collega il preparato al campione</rdfs:comment>
        <rdfs:comment xml:lang="en">This property relates  a preparation to a specimen</rdfs:comment>
        <rdfs:isDefinedBy rdf:resource="https://w3id.org/arco/ontology/movable-property"/>
        <rdfs:label xml:lang="en">is associated preparation of</rdfs:label>
        <rdfs:label xml:lang="it">è preparato associato di</rdfs:label>
        <owl:versionInfo xml:lang="it">instabile</owl:versionInfo>
        <owl:versionInfo xml:lang="en">unstable</owl:versionInfo>
    </owl:ObjectProperty>
    


    <!-- https://w3id.org/arco/ontology/movable-property/isBotanicalRevisionOf -->

    <owl:ObjectProperty rdf:about="https://w3id.org/arco/ontology/movable-property/isBotanicalRevisionOf">
        <rdfs:domain rdf:resource="https://w3id.org/arco/ontology/movable-property/BotanicalRevision"/>
        <rdfs:range rdf:resource="http://dati.beniculturali.it/cis/CulturalEntity"/>
        <rdfs:comment xml:lang="it">Questa proprietà collega la revisione botanica al campione</rdfs:comment>
        <rdfs:comment xml:lang="en">This property relates the botanical revision to a specimen</rdfs:comment>
        <rdfs:isDefinedBy rdf:resource="https://w3id.org/arco/ontology/movable-property"/>
        <rdfs:label xml:lang="en">is botanical revision of</rdfs:label>
        <rdfs:label xml:lang="it">è revisione botanica di</rdfs:label>
        <owl:versionInfo xml:lang="it">instabile</owl:versionInfo>
        <owl:versionInfo xml:lang="en">unstable</owl:versionInfo>
    </owl:ObjectProperty>
    


    <!-- https://w3id.org/arco/ontology/movable-property/isClassifiedByOriginalTaxon -->

    <owl:ObjectProperty rdf:about="https://w3id.org/arco/ontology/movable-property/isClassifiedByOriginalTaxon">
        <rdfs:subPropertyOf rdf:resource="https://w3id.org/arco/ontology/core/isClassifiedBy"/>
        <rdfs:domain rdf:resource="http://www.w3.org/2002/07/owl#Thing"/>
        <rdfs:range rdf:resource="https://w3id.org/arco/ontology/movable-property/BiologicalTaxon"/>
        <rdfs:comment xml:lang="it">Questa proprietà collega un&apos;entità al primo taxon che l&apos;ha classificata</rdfs:comment>
        <rdfs:comment xml:lang="en">This property relates an entity to the first taxon assigned to it</rdfs:comment>
        <rdfs:isDefinedBy rdf:resource="https://w3id.org/arco/ontology/movable-property"/>
        <rdfs:label xml:lang="en">is classified by original taxon</rdfs:label>
        <rdfs:label xml:lang="it">è classificato dal taxon originario</rdfs:label>
        <owl:versionInfo xml:lang="it">instabile</owl:versionInfo>
        <owl:versionInfo xml:lang="en">unstable</owl:versionInfo>
    </owl:ObjectProperty>
    


    <!-- https://w3id.org/arco/ontology/movable-property/isCloseIndivisualOf -->

    <owl:ObjectProperty rdf:about="https://w3id.org/arco/ontology/movable-property/isCloseIndivisualOf">
        <rdfs:domain rdf:resource="https://w3id.org/arco/ontology/movable-property/CloseIndividual"/>
        <rdfs:range rdf:resource="http://dati.beniculturali.it/cis/CulturalEntity"/>
        <rdfs:comment xml:lang="it">Questa proprietà collega l&apos;individuo vicino e il campione</rdfs:comment>
        <rdfs:comment xml:lang="en">This property relates the close individual to  the specimen</rdfs:comment>
        <rdfs:isDefinedBy rdf:resource="https://w3id.org/arco/ontology/movable-property"/>
        <rdfs:label xml:lang="en">is close individual of</rdfs:label>
        <rdfs:label xml:lang="it">è individuo vicino di</rdfs:label>
        <owl:versionInfo xml:lang="it">instabile</owl:versionInfo>
        <owl:versionInfo xml:lang="en">unstable</owl:versionInfo>
    </owl:ObjectProperty>
    


    <!-- https://w3id.org/arco/ontology/movable-property/isCollectingSiteOF -->

    <owl:ObjectProperty rdf:about="https://w3id.org/arco/ontology/movable-property/isCollectingSiteOF">
        <rdfs:subPropertyOf rdf:resource="https://w3id.org/arco/ontology/core/isLocationOf"/>
        <rdfs:comment xml:lang="it">Questa proprietà collega il luogo di raccolta al campione</rdfs:comment>
        <rdfs:comment xml:lang="en">This property relates the collecting site to the specimen</rdfs:comment>
        <rdfs:label xml:lang="en">is collecting site of</rdfs:label>
        <rdfs:label xml:lang="it">è luogo di raccolta di</rdfs:label>
        <owl:versionInfo xml:lang="it">instabile</owl:versionInfo>
        <owl:versionInfo xml:lang="en">unstable</owl:versionInfo>
    </owl:ObjectProperty>
    


    <!-- https://w3id.org/arco/ontology/movable-property/isCollectingSiteOf -->

    <owl:ObjectProperty rdf:about="https://w3id.org/arco/ontology/movable-property/isCollectingSiteOf"/>
    


    <!-- https://w3id.org/arco/ontology/movable-property/isFluidDynamismOf -->

    <owl:ObjectProperty rdf:about="https://w3id.org/arco/ontology/movable-property/isFluidDynamismOf">
        <rdfs:domain rdf:resource="https://w3id.org/arco/ontology/movable-property/FluidDynamism"/>
        <rdfs:range rdf:resource="https://w3id.org/arco/ontology/movable-property/CollectingSite"/>
        <rdfs:comment xml:lang="it">Questa proprietà collega l&apos;idrodinamismo al luogo di raccolta</rdfs:comment>
        <rdfs:comment xml:lang="en">This property relates the fluid dynamism to the collecting site</rdfs:comment>
        <rdfs:label xml:lang="en">is fluid dynamism of</rdfs:label>
        <rdfs:label xml:lang="it">è idrodinamismo di</rdfs:label>
        <owl:versionInfo xml:lang="it">instabile</owl:versionInfo>
        <owl:versionInfo xml:lang="en">unstable</owl:versionInfo>
    </owl:ObjectProperty>
    


    <!-- https://w3id.org/arco/ontology/movable-property/isHostIndividualOf -->

    <owl:ObjectProperty rdf:about="https://w3id.org/arco/ontology/movable-property/isHostIndividualOf">
        <rdfs:domain rdf:resource="https://w3id.org/arco/ontology/movable-property/HostIndividual"/>
        <rdfs:range rdf:resource="http://dati.beniculturali.it/cis/CulturalEntity"/>
        <rdfs:comment xml:lang="it">Questa proprietà collega l&apos;indivduo ospite al campione</rdfs:comment>
        <rdfs:comment xml:lang="en">This property relates the host individual to  the specimen</rdfs:comment>
        <rdfs:label xml:lang="en">is host individual of</rdfs:label>
        <rdfs:label xml:lang="it">è individuo ospite di</rdfs:label>
        <owl:versionInfo xml:lang="it">instabile</owl:versionInfo>
        <owl:versionInfo xml:lang="en">unstable</owl:versionInfo>
    </owl:ObjectProperty>
    


    <!-- https://w3id.org/arco/ontology/movable-property/isInclineOf -->

    <owl:ObjectProperty rdf:about="https://w3id.org/arco/ontology/movable-property/isInclineOf">
        <rdfs:domain rdf:resource="https://w3id.org/arco/ontology/movable-property/Incline"/>
        <rdfs:range rdf:resource="https://w3id.org/arco/ontology/movable-property/Substrate"/>
        <rdfs:comment xml:lang="it">Questa proprietà collega l&apos;inclinazione al luogo di raccolta</rdfs:comment>
        <rdfs:comment xml:lang="en">This property relates the incline to the collecting site</rdfs:comment>
        <rdfs:label xml:lang="en">is incline of</rdfs:label>
        <rdfs:label xml:lang="it">è inclinazione di</rdfs:label>
        <owl:versionInfo xml:lang="it">instabile</owl:versionInfo>
        <owl:versionInfo xml:lang="en">unstable</owl:versionInfo>
    </owl:ObjectProperty>
    


    <!-- https://w3id.org/arco/ontology/movable-property/isLabelOf -->

    <owl:ObjectProperty rdf:about="https://w3id.org/arco/ontology/movable-property/isLabelOf">
        <rdfs:domain rdf:resource="https://w3id.org/arco/ontology/movable-property/Label"/>
        <rdfs:range rdf:resource="http://dati.beniculturali.it/cis/CulturalEntity"/>
        <rdfs:comment xml:lang="it">Questa proprietà collega un&apos;etichetta ad un bene culturale</rdfs:comment>
        <rdfs:comment xml:lang="en">This property relates a label to a cultural property.</rdfs:comment>
        <rdfs:label xml:lang="en">is label of</rdfs:label>
        <rdfs:label xml:lang="it">è etichetta di</rdfs:label>
        <owl:versionInfo xml:lang="it">instabile</owl:versionInfo>
        <owl:versionInfo xml:lang="en">unstable</owl:versionInfo>
    </owl:ObjectProperty>
    


    <!-- https://w3id.org/arco/ontology/movable-property/isLanguageOf -->

    <owl:ObjectProperty rdf:about="https://w3id.org/arco/ontology/movable-property/isLanguageOf">
        <rdfs:domain rdf:resource="https://w3id.org/arco/ontology/movable-property/Language"/>
        <rdfs:range rdf:resource="http://www.w3.org/2002/07/owl#Thing"/>
        <rdfs:comment xml:lang="it">Questa proprietà collega la lingua con una cosa</rdfs:comment>
        <rdfs:comment xml:lang="en">This property realtes a language to a thing</rdfs:comment>
        <rdfs:label xml:lang="en">is language of</rdfs:label>
        <rdfs:label xml:lang="it">è lingua di</rdfs:label>
        <owl:versionInfo xml:lang="it">instabile</owl:versionInfo>
        <owl:versionInfo xml:lang="en">unstable</owl:versionInfo>
        <a-cat:iccdNormTag>ICCD Normativa BNB: SB/SBE/SBEL</a-cat:iccdNormTag>
    </owl:ObjectProperty>
    


    <!-- https://w3id.org/arco/ontology/movable-property/isNaturalEnvironmentOf -->

    <owl:ObjectProperty rdf:about="https://w3id.org/arco/ontology/movable-property/isNaturalEnvironmentOf">
        <rdfs:domain rdf:resource="https://w3id.org/arco/ontology/movable-property/NaturalEnvironment"/>
        <rdfs:range rdf:resource="https://w3id.org/arco/ontology/movable-property/Substrate"/>
        <rdfs:comment xml:lang="it">Questa proprietà collega l&apos;ambiente al substrato</rdfs:comment>
        <rdfs:comment xml:lang="en">This property relates the natural environment to  the substrate</rdfs:comment>
        <rdfs:label xml:lang="en">is natural environment of</rdfs:label>
        <rdfs:label xml:lang="it">è ambiente naturale di</rdfs:label>
        <owl:versionInfo xml:lang="it">instabile</owl:versionInfo>
        <owl:versionInfo xml:lang="en">unstable</owl:versionInfo>
    </owl:ObjectProperty>
    


    <!-- https://w3id.org/arco/ontology/movable-property/isPreservationTypeOf -->

    <owl:ObjectProperty rdf:about="https://w3id.org/arco/ontology/movable-property/isPreservationTypeOf">
        <rdfs:subPropertyOf rdf:resource="https://w3id.org/arco/ontology/core/isTypeOf"/>
        <rdfs:domain rdf:resource="https://w3id.org/arco/ontology/movable-property/PreservationType"/>
        <rdfs:range rdf:resource="https://w3id.org/arco/ontology/movable-property/FruitSample"/>
        <rdfs:comment xml:lang="it">Questa proprietà collega il tipo di conservazione al campione</rdfs:comment>
        <rdfs:comment xml:lang="en">This property relates the conservation type to a  specimen</rdfs:comment>
        <rdfs:isDefinedBy rdf:resource="https://w3id.org/arco/ontology/movable-property"/>
        <rdfs:label xml:lang="en">is preservation type of</rdfs:label>
        <rdfs:label xml:lang="it">è tipo di conservazione di</rdfs:label>
        <owl:versionInfo xml:lang="it">instabile</owl:versionInfo>
        <owl:versionInfo xml:lang="en">unstable</owl:versionInfo>
    </owl:ObjectProperty>
    


    <!-- https://w3id.org/arco/ontology/movable-property/isRelatedSampleOf -->

    <owl:ObjectProperty rdf:about="https://w3id.org/arco/ontology/movable-property/isRelatedSampleOf">
        <rdfs:domain rdf:resource="https://w3id.org/arco/ontology/movable-property/Sample"/>
        <rdfs:range rdf:resource="http://dati.beniculturali.it/cis/CulturalEntity"/>
        <rdfs:comment xml:lang="it">Questa proprietà collega il reperto della collezione ancillare al campione di riferimento</rdfs:comment>
        <rdfs:comment xml:lang="en">This property relates a sample belonging to ancillary collection to a specimen</rdfs:comment>
        <rdfs:isDefinedBy rdf:resource="https://w3id.org/arco/ontology/movable-property"/>
        <rdfs:label xml:lang="en">is related sample of</rdfs:label>
        <rdfs:label xml:lang="it">è reperto associato di</rdfs:label>
        <owl:versionInfo xml:lang="it">instabile</owl:versionInfo>
        <owl:versionInfo xml:lang="en">unstable</owl:versionInfo>
    </owl:ObjectProperty>
    


    <!-- https://w3id.org/arco/ontology/movable-property/isSampleFormOf -->

    <owl:ObjectProperty rdf:about="https://w3id.org/arco/ontology/movable-property/isSampleFormOf">
        <rdfs:domain rdf:resource="https://w3id.org/arco/ontology/movable-property/SampleForm"/>
        <rdfs:range rdf:resource="https://w3id.org/arco/ontology/movable-property/WoodSample"/>
        <rdfs:comment xml:lang="it">Questa proprietà collega la forma al campione</rdfs:comment>
        <rdfs:comment xml:lang="en">This property relates the form to a specimen</rdfs:comment>
        <rdfs:isDefinedBy rdf:resource="https://w3id.org/arco/ontology/movable-property"/>
        <rdfs:label xml:lang="en">is sample form of</rdfs:label>
        <rdfs:label xml:lang="it">è forma del reperto di</rdfs:label>
        <owl:versionInfo xml:lang="it">instabile</owl:versionInfo>
        <owl:versionInfo xml:lang="en">unstable</owl:versionInfo>
        <a-cat:iccdNormTag xml:lang="it">ICCD Normativa BNB: DB/DBX/DBXX</a-cat:iccdNormTag>
    </owl:ObjectProperty>
    


    <!-- https://w3id.org/arco/ontology/movable-property/isShadeToleranceOf -->

    <owl:ObjectProperty rdf:about="https://w3id.org/arco/ontology/movable-property/isShadeToleranceOf">
        <rdfs:domain rdf:resource="https://w3id.org/arco/ontology/movable-property/ShadeTolerance"/>
        <rdfs:range rdf:resource="https://w3id.org/arco/ontology/movable-property/CollectingSite"/>
        <rdfs:comment xml:lang="it">Questa proprietà collega la caratteristica del popolamento del luogo di raccolta al il luogo di raccolta del campione</rdfs:comment>
        <rdfs:comment xml:lang="en">This property relates the individuals&apos; shade tolerance the collecting site</rdfs:comment>
        <rdfs:isDefinedBy rdf:resource="https://w3id.org/arco/ontology/movable-property"/>
        <rdfs:label xml:lang="en">is shade tolerance of</rdfs:label>
        <rdfs:label xml:lang="it">è situazione luminosa di</rdfs:label>
        <owl:versionInfo xml:lang="it">instabile</owl:versionInfo>
        <owl:versionInfo xml:lang="en">unstable</owl:versionInfo>
    </owl:ObjectProperty>
    


    <!-- https://w3id.org/arco/ontology/movable-property/isSpecimenHarvestingOf -->

    <owl:ObjectProperty rdf:about="https://w3id.org/arco/ontology/movable-property/isSpecimenHarvestingOf">
        <rdfs:domain rdf:resource="https://w3id.org/arco/ontology/movable-property/SpecimenHarvesting"/>
        <rdfs:range rdf:resource="https://w3id.org/italia/onto/l0/Entity"/>
        <rdfs:comment xml:lang="it">Questa proprietà collega le informazioni sulla raccolta del campione al campione.</rdfs:comment>
        <rdfs:comment xml:lang="en">This property relates the information about harvesting of the specimen to  its specimen</rdfs:comment>
        <rdfs:isDefinedBy rdf:resource="https://w3id.org/arco/ontology/movable-property"/>
        <rdfs:label xml:lang="en">is specimen harvesting of</rdfs:label>
        <rdfs:label xml:lang="it">è raccolta del campione</rdfs:label>
        <owl:versionInfo xml:lang="it">instabile</owl:versionInfo>
        <owl:versionInfo xml:lang="en">unstable</owl:versionInfo>
    </owl:ObjectProperty>
    


    <!-- https://w3id.org/arco/ontology/movable-property/isSubstrateOf -->

    <owl:ObjectProperty rdf:about="https://w3id.org/arco/ontology/movable-property/isSubstrateOf">
        <rdfs:domain rdf:resource="https://w3id.org/arco/ontology/movable-property/Substrate"/>
        <rdfs:range rdf:resource="https://w3id.org/arco/ontology/movable-property/CollectingSite"/>
        <rdfs:comment xml:lang="it">Questa proprietà  collega il substrato al luogo di raccolta</rdfs:comment>
        <rdfs:comment xml:lang="en">This property relates the substrate to the collecting site</rdfs:comment>
        <rdfs:isDefinedBy rdf:resource="https://w3id.org/arco/ontology/movable-property"/>
        <rdfs:label xml:lang="en">is substrate of</rdfs:label>
        <rdfs:label xml:lang="it">è substrato di</rdfs:label>
        <owl:versionInfo xml:lang="it">instabile</owl:versionInfo>
        <owl:versionInfo xml:lang="en">unstable</owl:versionInfo>
        <a-cat:iccdNormTag>ICCD Normativa BNB: LR/LRI/LRIR</a-cat:iccdNormTag>
    </owl:ObjectProperty>
    


    <!-- https://w3id.org/arco/ontology/movable-property/isTaxonOf -->

    <owl:ObjectProperty rdf:about="https://w3id.org/arco/ontology/movable-property/isTaxonOf">
        <rdfs:domain rdf:resource="https://w3id.org/arco/ontology/movable-property/BiologicalTaxon"/>
        <rdfs:range rdf:resource="http://www.w3.org/2002/07/owl#Thing"/>
        <rdfs:comment xml:lang="it">Questa proprietà collega un taxon con un&apos;entità biologica.</rdfs:comment>
        <rdfs:comment xml:lang="it">This property relates a taxon to a biological entity.</rdfs:comment>
        <rdfs:isDefinedBy rdf:resource="https://w3id.org/arco/ontology/movable-property"/>
        <rdfs:label xml:lang="en">is taxon of</rdfs:label>
        <rdfs:label xml:lang="it">è taxon di</rdfs:label>
        <owl:versionInfo xml:lang="it">instabile</owl:versionInfo>
        <owl:versionInfo xml:lang="en">unstable</owl:versionInfo>
    </owl:ObjectProperty>
    


    <!-- https://w3id.org/arco/ontology/movable-property/isTypeSpecimenIdentificationOf -->

    <owl:ObjectProperty rdf:about="https://w3id.org/arco/ontology/movable-property/isTypeSpecimenIdentificationOf">
        <rdfs:subPropertyOf rdf:resource="https://w3id.org/arco/ontology/core/isSituationOf"/>
        <rdfs:domain rdf:resource="https://w3id.org/arco/ontology/movable-property/TypeSpecimenIdentification"/>
        <rdfs:range rdf:resource="http://dati.beniculturali.it/cis/CulturalEntity"/>
        <rdfs:comment xml:lang="it">Questa proprietà collega l&apos;individiazione del tipo nomenclaturale al campione</rdfs:comment>
        <rdfs:comment xml:lang="en">This property relates the type specimen identification to the specimen</rdfs:comment>
        <rdfs:isDefinedBy rdf:resource="https://w3id.org/arco/ontology/movable-property"/>
        <rdfs:label xml:lang="en">is type specimen identification of</rdfs:label>
        <rdfs:label xml:lang="it">è identificazione del tipo nomenclaturale di</rdfs:label>
        <owl:versionInfo xml:lang="it">instabile</owl:versionInfo>
        <owl:versionInfo xml:lang="en">unstable</owl:versionInfo>
        <a-cat:iccdNormTag>ICCD Normativa BNB: SB/TBI</a-cat:iccdNormTag>
    </owl:ObjectProperty>
    


    <!-- 
    ///////////////////////////////////////////////////////////////////////////////////////
    //
    // Data properties
    //
    ///////////////////////////////////////////////////////////////////////////////////////
     -->

    


    <!-- https://w3id.org/arco/ontology/denotative-description/transcript -->

    <owl:DatatypeProperty rdf:about="https://w3id.org/arco/ontology/denotative-description/transcript"/>
    


    <!-- https://w3id.org/arco/ontology/movable-property/bodyTranscript -->

    <owl:DatatypeProperty rdf:about="https://w3id.org/arco/ontology/movable-property/bodyTranscript">
        <rdfs:subPropertyOf rdf:resource="https://w3id.org/arco/ontology/denotative-description/transcript"/>
        <rdfs:domain rdf:resource="https://w3id.org/arco/ontology/movable-property/Label"/>
        <rdfs:range rdf:resource="http://www.w3.org/2000/01/rdf-schema#Literal"/>
        <rdfs:comment xml:lang="it">Questa proprietà rappresenta il testo scritto nel corpo dell&apos;etichetta</rdfs:comment>
        <rdfs:comment xml:lang="en">This property represents the text written in the body of the label</rdfs:comment>
        <rdfs:isDefinedBy rdf:resource="https://w3id.org/arco/ontology/movable-property"/>
        <rdfs:label xml:lang="en">body transcript</rdfs:label>
        <rdfs:label xml:lang="it">trascrizione del corpo</rdfs:label>
        <owl:versionInfo xml:lang="it">instabile</owl:versionInfo>
        <owl:versionInfo xml:lang="en">unstable</owl:versionInfo>
        <a-cat:iccdNormTag>ICCD Normativa BNB: SB/SBE/SBET</a-cat:iccdNormTag>
    </owl:DatatypeProperty>
    


    <!-- https://w3id.org/arco/ontology/movable-property/dateOfLastChangePreservative -->

    <owl:DatatypeProperty rdf:about="https://w3id.org/arco/ontology/movable-property/dateOfLastChangePreservative">
        <rdfs:subPropertyOf rdf:resource="https://w3id.org/italia/onto/TI/date"/>
        <rdfs:domain rdf:resource="https://w3id.org/arco/ontology/movable-property/FruitSample"/>
        <rdfs:range rdf:resource="http://www.w3.org/2000/01/rdf-schema#Literal"/>
        <rdfs:comment xml:lang="it">Questa proprietàrappresenta la data in cui per l’ultima volta il conservante del preparato è stato cambiato</rdfs:comment>
        <rdfs:comment xml:lang="en">This preperty represents the date in which the preservative has been changed for the last time</rdfs:comment>
        <rdfs:isDefinedBy rdf:resource="https://w3id.org/arco/ontology/movable-property"/>
        <rdfs:label xml:lang="it">data ultimo cambio conservante</rdfs:label>
        <rdfs:label xml:lang="en">date of last change preservative</rdfs:label>
        <owl:versionInfo xml:lang="it">instabile</owl:versionInfo>
        <owl:versionInfo xml:lang="en">unstable</owl:versionInfo>
        <a-cat:iccdNormTag xml:lang="en">Normativa BNB: DB/DBC/DBCE</a-cat:iccdNormTag>
    </owl:DatatypeProperty>
    


    <!-- https://w3id.org/arco/ontology/movable-property/genusNumber -->

    <owl:DatatypeProperty rdf:about="https://w3id.org/arco/ontology/movable-property/genusNumber">
        <rdfs:domain rdf:resource="https://w3id.org/arco/ontology/movable-property/Genus"/>
        <rdfs:range rdf:resource="http://www.w3.org/2000/01/rdf-schema#Literal"/>
        <rdfs:comment xml:lang="it">Questa porprietà rappresenta il numero del genere (secondo lo schema sistematico di riferimento)</rdfs:comment>
        <rdfs:comment xml:lang="en">This property represents the genus number (according to the referenced axonomy)</rdfs:comment>
        <rdfs:isDefinedBy rdf:resource="https://w3id.org/arco/ontology/movable-property"/>
        <rdfs:label xml:lang="en">genus number</rdfs:label>
        <rdfs:label xml:lang="it">numero del genere</rdfs:label>
        <owl:versionInfo xml:lang="it">instabile</owl:versionInfo>
        <owl:versionInfo xml:lang="en">unstable</owl:versionInfo>
        <a-cat:iccdNormTag>ICCD Normativa BNB: SB/SBS/SBSN</a-cat:iccdNormTag>
    </owl:DatatypeProperty>
    


    <!-- https://w3id.org/arco/ontology/movable-property/graphicSymbols -->

    <owl:DatatypeProperty rdf:about="https://w3id.org/arco/ontology/movable-property/graphicSymbols">
        <rdfs:domain rdf:resource="https://w3id.org/arco/ontology/movable-property/Label"/>
        <rdfs:range rdf:resource="http://www.w3.org/2000/01/rdf-schema#Literal"/>
        <rdfs:comment xml:lang="it">Questa proprietà rappresenta i simboli grafici scritti nell&apos;etichetta</rdfs:comment>
        <rdfs:comment xml:lang="en">This property represents graphic symbols written in the label</rdfs:comment>
        <rdfs:isDefinedBy rdf:resource="https://w3id.org/arco/ontology/movable-property"/>
        <rdfs:label xml:lang="en">graphic symbols</rdfs:label>
        <rdfs:label xml:lang="it">simboli grafici</rdfs:label>
        <owl:versionInfo xml:lang="it">instabile</owl:versionInfo>
        <owl:versionInfo xml:lang="en">unstable</owl:versionInfo>
        <a-cat:iccdNormTag>ICCD Normativa BNB: SB/SBE/SBEG</a-cat:iccdNormTag>
    </owl:DatatypeProperty>
    


    <!-- https://w3id.org/arco/ontology/movable-property/handWriting -->

    <owl:DatatypeProperty rdf:about="https://w3id.org/arco/ontology/movable-property/handWriting">
        <rdfs:domain rdf:resource="https://w3id.org/arco/ontology/movable-property/Label"/>
        <rdfs:range rdf:resource="http://www.w3.org/2001/XMLSchema#boolean"/>
        <rdfs:comment xml:lang="it">Questa proprietà indica se l&apos;etichetta è autografa o meno</rdfs:comment>
        <rdfs:comment xml:lang="en">This property indicates if the label is handwritten or not</rdfs:comment>
        <rdfs:isDefinedBy rdf:resource="https://w3id.org/arco/ontology/movable-property"/>
        <rdfs:label xml:lang="it">autografa</rdfs:label>
        <rdfs:label xml:lang="en">handwriting</rdfs:label>
        <owl:versionInfo xml:lang="it">instabile</owl:versionInfo>
        <owl:versionInfo xml:lang="en">unstable</owl:versionInfo>
        <a-cat:iccdNormTag>ICCD Normativa BNB: SB/SBE/SBEA</a-cat:iccdNormTag>
    </owl:DatatypeProperty>
    


    <!-- https://w3id.org/arco/ontology/movable-property/headingTranscript -->

    <owl:DatatypeProperty rdf:about="https://w3id.org/arco/ontology/movable-property/headingTranscript">
        <rdfs:subPropertyOf rdf:resource="https://w3id.org/arco/ontology/denotative-description/transcript"/>
        <rdfs:domain rdf:resource="https://w3id.org/arco/ontology/movable-property/Label"/>
        <rdfs:range rdf:resource="http://www.w3.org/2000/01/rdf-schema#Literal"/>
        <rdfs:comment xml:lang="it">Questa proprietà rappresenta il testo scritto nell&apos;intestazione dell&apos;etichetta</rdfs:comment>
        <rdfs:comment xml:lang="en">This property represents the heading of the label</rdfs:comment>
        <rdfs:isDefinedBy rdf:resource="https://w3id.org/arco/ontology/movable-property"/>
        <rdfs:label xml:lang="en">heading transcript</rdfs:label>
        <rdfs:label xml:lang="it">trascrizione dell&apos;intestazione</rdfs:label>
        <owl:versionInfo xml:lang="it">instabile</owl:versionInfo>
        <owl:versionInfo xml:lang="en">unstable</owl:versionInfo>
        <a-cat:iccdNormTag>ICCD Normativa BNB: SB/SBE/SBEI</a-cat:iccdNormTag>
    </owl:DatatypeProperty>
    


    <!-- https://w3id.org/arco/ontology/movable-property/manufacturingDate -->

    <owl:DatatypeProperty rdf:about="https://w3id.org/arco/ontology/movable-property/manufacturingDate">
        <rdfs:subPropertyOf rdf:resource="https://w3id.org/italia/onto/TI/date"/>
        <rdfs:domain rdf:resource="http://www.w3.org/2002/07/owl#Thing"/>
        <rdfs:range rdf:resource="http://www.w3.org/2000/01/rdf-schema#Literal"/>
        <rdfs:comment xml:lang="it">Questa proprietà rappresenta la data di preparazione del reperto o del preparato</rdfs:comment>
        <rdfs:comment xml:lang="en">This property represents the date of manufacturing of the sample or of the preparation</rdfs:comment>
        <rdfs:isDefinedBy rdf:resource="https://w3id.org/arco/ontology/movable-property"/>
        <rdfs:label xml:lang="it">data di preparazione</rdfs:label>
        <rdfs:label xml:lang="en">manufacturing date</rdfs:label>
        <owl:versionInfo xml:lang="it">instabile</owl:versionInfo>
        <owl:versionInfo xml:lang="en">unstable</owl:versionInfo>
        <a-cat:iccdNormTag>ICCD Normativa BNB: DB/DBR/DBRD, DB/DBX/DBXO, DB/DBS/DBSD, DB/DB/DBP/DBPD.</a-cat:iccdNormTag>
    </owl:DatatypeProperty>
    


    <!-- https://w3id.org/arco/ontology/movable-property/numberOfEnvelopes -->

    <owl:DatatypeProperty rdf:about="https://w3id.org/arco/ontology/movable-property/numberOfEnvelopes">
        <rdfs:domain rdf:resource="http://dati.beniculturali.it/cis/CulturalEntity"/>
        <rdfs:range rdf:resource="http://www.w3.org/2001/XMLSchema#positiveInteger"/>
        <rdfs:comment xml:lang="it">Questa proprietà rappresenta il numero di buste che contengono il campione o sue parti se conservate assieme al campione, e non in collezioni ancillari</rdfs:comment>
        <rdfs:comment xml:lang="en">This property represents the numebr of envelopes, containing the specimen or its parts, if they are preserved with the specimen itself and not in ancillar collections</rdfs:comment>
        <rdfs:isDefinedBy>https://w3id.org/arco/ontology/movable-property</rdfs:isDefinedBy>
        <rdfs:label xml:lang="en">numbers of envelopes</rdfs:label>
        <rdfs:label xml:lang="it">numero di buste</rdfs:label>
        <owl:versionInfo xml:lang="it">instabile</owl:versionInfo>
        <owl:versionInfo xml:lang="en">unstable</owl:versionInfo>
        <a-cat:iccdNormTag>ICCD Normativa BNB: SB/CBP/CBPB</a-cat:iccdNormTag>
    </owl:DatatypeProperty>
    


    <!-- https://w3id.org/arco/ontology/movable-property/numberOfLabels -->

    <owl:DatatypeProperty rdf:about="https://w3id.org/arco/ontology/movable-property/numberOfLabels">
        <rdfs:domain rdf:resource="http://dati.beniculturali.it/cis/CulturalEntity"/>
        <rdfs:range rdf:resource="http://www.w3.org/2001/XMLSchema#positiveInteger"/>
        <rdfs:comment xml:lang="it">Questa proprietà rappresenta etichette presenti assieme al campione</rdfs:comment>
        <rdfs:comment xml:lang="en">This property represents the number of labels with the specimen</rdfs:comment>
        <rdfs:isDefinedBy>https://w3id.org/arco/ontology/movable-property</rdfs:isDefinedBy>
        <rdfs:label xml:lang="en">number of labels</rdfs:label>
        <rdfs:label xml:lang="it">numero di etichette</rdfs:label>
        <owl:versionInfo xml:lang="it">instabile</owl:versionInfo>
        <owl:versionInfo xml:lang="en">unstable</owl:versionInfo>
        <a-cat:iccdNormTag>ICCD Normativa BNB: SB/CBP/CBPE</a-cat:iccdNormTag>
    </owl:DatatypeProperty>
    


    <!-- https://w3id.org/arco/ontology/movable-property/originalClassification -->

    <owl:DatatypeProperty rdf:about="https://w3id.org/arco/ontology/movable-property/originalClassification">
        <rdfs:domain rdf:resource="https://w3id.org/arco/ontology/core/ClassificationInTime"/>
        <rdfs:range rdf:resource="http://www.w3.org/2001/XMLSchema#boolean"/>
        <rdfs:comment xml:lang="it">Questa proprietà indica se il taxon associato alla classificazione è stato il primo ad essere associato al campione</rdfs:comment>
        <rdfs:comment xml:lang="en">This property indicates if the taxon of the classification is the first one assigned to the specimen</rdfs:comment>
        <rdfs:label xml:lang="it">classificazione originaria</rdfs:label>
        <rdfs:label xml:lang="en">original classification</rdfs:label>
        <owl:versionInfo xml:lang="it">instabile</owl:versionInfo>
        <owl:versionInfo xml:lang="en">unstable</owl:versionInfo>
    </owl:DatatypeProperty>
    


    <!-- https://w3id.org/arco/ontology/movable-property/sampleLocation -->

    <owl:DatatypeProperty rdf:about="https://w3id.org/arco/ontology/movable-property/sampleLocation">
        <rdfs:domain rdf:resource="https://w3id.org/arco/ontology/movable-property/Sample"/>
        <rdfs:range rdf:resource="http://www.w3.org/2000/01/rdf-schema#Literal"/>
        <rdfs:comment xml:lang="it">Questa proprietà rappresenta la collocazione che l’oggetto ha nella collezione ancillare di cui fa parte</rdfs:comment>
        <rdfs:comment xml:lang="en">This property represents the location of the object inthe ancillar collection</rdfs:comment>
        <rdfs:isDefinedBy rdf:resource="https://w3id.org/arco/ontology/movable-property"/>
        <rdfs:label xml:lang="it">collocazione del reperto</rdfs:label>
        <rdfs:label xml:lang="en">sample location</rdfs:label>
        <owl:versionInfo xml:lang="it">instabile</owl:versionInfo>
        <owl:versionInfo xml:lang="en">unstable</owl:versionInfo>
        <a-cat:iccdNormTag>ICCD Normativa BNB: DB/DBC/DBCC, DB/DBX/DBXC, DB/DBS/DBSC, DB/DB/DBP/DBPC.</a-cat:iccdNormTag>
    </owl:DatatypeProperty>
    


    <!-- https://w3id.org/arco/ontology/movable-property/taxonomicNumber -->

    <owl:DatatypeProperty rdf:about="https://w3id.org/arco/ontology/movable-property/taxonomicNumber">
        <rdfs:domain rdf:resource="https://w3id.org/arco/ontology/movable-property/BiologicalTaxon"/>
        <rdfs:range rdf:resource="http://www.w3.org/2000/01/rdf-schema#Literal"/>
        <rdfs:comment xml:lang="it">Questa proprietà rappresenta il numero che fa riferimento a determinate categorie tassonomiche diverse dal genere, nel caso di erbari antichi (prelinneiani o linneiani antichi, come ad es. l&apos;Erbario Micheli).</rdfs:comment>
        <rdfs:comment xml:lang="en">This property represents the number related to a taxonomic category, different from the genus (expecially for ancient herbaria and prelinnaean herbaria, e.g. Micheli Herbarium)</rdfs:comment>
        <rdfs:isDefinedBy rdf:resource="https://w3id.org/arco/ontology/movable-property"/>
        <rdfs:label xml:lang="it">numero tassonomico</rdfs:label>
        <rdfs:label xml:lang="en">taxonomic number</rdfs:label>
        <owl:versionInfo xml:lang="it">instabile</owl:versionInfo>
        <owl:versionInfo xml:lang="en">unstable</owl:versionInfo>
        <a-cat:iccdNormTag>ICCD Normativa BNB: SB/SBS/SBSG</a-cat:iccdNormTag>
    </owl:DatatypeProperty>
    


    <!-- https://w3id.org/italia/onto/TI/date -->

    <owl:DatatypeProperty rdf:about="https://w3id.org/italia/onto/TI/date"/>
    


    <!-- 
    ///////////////////////////////////////////////////////////////////////////////////////
    //
    // Classes
    //
    ///////////////////////////////////////////////////////////////////////////////////////
     -->

    


    <!-- http://dati.beniculturali.it/cis/CulturalEntity -->

    <owl:Class rdf:about="http://dati.beniculturali.it/cis/CulturalEntity"/>
    


    <!-- https://w3id.org/arco/ontology/core/ClassificationInTime -->

    <rdf:Description rdf:about="https://w3id.org/arco/ontology/core/ClassificationInTime">
        <rdfs:subClassOf>
            <owl:Restriction>
                <owl:onProperty rdf:resource="https://w3id.org/arco/ontology/movable-property/hasTaxon"/>
                <owl:someValuesFrom rdf:resource="https://w3id.org/arco/ontology/movable-property/BiologicalTaxon"/>
            </owl:Restriction>
        </rdfs:subClassOf>
        <rdfs:subClassOf>
            <owl:Restriction>
                <owl:onProperty rdf:resource="https://w3id.org/arco/ontology/context-description/hasBibliography"/>
                <owl:allValuesFrom rdf:resource="https://w3id.org/arco/ontology/context-description/Bibliography"/>
            </owl:Restriction>
        </rdfs:subClassOf>
        <rdfs:subClassOf>
            <owl:Restriction>
                <owl:onProperty rdf:resource="https://w3id.org/arco/ontology/movable-property/originalClassification"/>
                <owl:someValuesFrom rdf:resource="http://www.w3.org/2001/XMLSchema#boolean"/>
            </owl:Restriction>
        </rdfs:subClassOf>
    </rdf:Description>
    


    <!-- https://w3id.org/arco/ontology/core/TimeIndexedEvent -->

    <owl:Class rdf:about="https://w3id.org/arco/ontology/core/TimeIndexedEvent"/>
    


    <!-- https://w3id.org/arco/ontology/core/Type -->

    <owl:Class rdf:about="https://w3id.org/arco/ontology/core/Type"/>
    


    <!-- https://w3id.org/arco/ontology/denotative-description/AffixedElement -->

    <owl:Class rdf:about="https://w3id.org/arco/ontology/denotative-description/AffixedElement"/>
    


    <!-- https://w3id.org/arco/ontology/denotative-description/FontStyle -->

    <owl:Class rdf:about="https://w3id.org/arco/ontology/denotative-description/FontStyle"/>
    


    <!-- https://w3id.org/arco/ontology/denotative-description/MeasurementCollection -->

    <owl:Class rdf:about="https://w3id.org/arco/ontology/denotative-description/MeasurementCollection"/>
    


    <!-- https://w3id.org/arco/ontology/denotative-description/Orientation -->

    <owl:Class rdf:about="https://w3id.org/arco/ontology/denotative-description/Orientation"/>
    


    <!-- https://w3id.org/arco/ontology/location/TimeIndexedTypedLocation -->

    <owl:Class rdf:about="https://w3id.org/arco/ontology/location/TimeIndexedTypedLocation"/>
    


    <!-- https://w3id.org/arco/ontology/movable-property/Accession -->

    <owl:Class rdf:about="https://w3id.org/arco/ontology/movable-property/Accession">
        <rdfs:subClassOf rdf:resource="https://w3id.org/arco/ontology/core/TimeIndexedEvent"/>
        <rdfs:subClassOf>
            <owl:Restriction>
                <owl:onProperty rdf:resource="https://w3id.org/arco/ontology/movable-property/isAccessionOf"/>
                <owl:someValuesFrom rdf:resource="http://dati.beniculturali.it/cis/CulturalEntity"/>
            </owl:Restriction>
        </rdfs:subClassOf>
        <rdfs:subClassOf>
            <owl:Restriction>
                <owl:onProperty rdf:resource="https://w3id.org/arco/ontology/core/involvesAgent"/>
                <owl:allValuesFrom rdf:resource="https://w3id.org/italia/onto/l0/Agent"/>
            </owl:Restriction>
        </rdfs:subClassOf>
        <rdfs:subClassOf>
            <owl:Restriction>
                <owl:onProperty rdf:resource="https://w3id.org/italia/onto/TI/atTime"/>
                <owl:allValuesFrom rdf:resource="https://w3id.org/italia/onto/TI/TimeInterval"/>
            </owl:Restriction>
        </rdfs:subClassOf>
        <rdfs:comment xml:lang="it">Questa classe rappresenta l&apos;informazione (dato) sulla/e persona fisica o giuridica/che che a vario titolo ha/hanno fatto pervenire il bene (campione, raccolta, collezione ecc.) all&apos;Ente di riferimento.</rdfs:comment>
        <rdfs:comment xml:lang="en">This class represents the information about the way in which the cultural property has arrived to the organization</rdfs:comment>
        <rdfs:isDefinedBy rdf:resource="https://w3id.org/arco/ontology/movable-property"/>
        <rdfs:label xml:lang="en">Accession</rdfs:label>
        <rdfs:label xml:lang="it">Accessione</rdfs:label>
        <owl:versionInfo xml:lang="it">instabile</owl:versionInfo>
        <owl:versionInfo xml:lang="en">unstable</owl:versionInfo>
        <a-cat:iccdNormTag>ICCD Normativa BNB: SB/ABC</a-cat:iccdNormTag>
    </owl:Class>
    


    <!-- https://w3id.org/arco/ontology/movable-property/BiologicalTaxon -->

    <owl:Class rdf:about="https://w3id.org/arco/ontology/movable-property/BiologicalTaxon">
        <rdfs:subClassOf rdf:resource="https://w3id.org/arco/ontology/core/Concept"/>
        <rdfs:subClassOf>
            <owl:Restriction>
                <owl:onProperty rdf:resource="https://w3id.org/arco/ontology/context-description/hasAuthor"/>
                <owl:allValuesFrom rdf:resource="https://w3id.org/italia/onto/l0/Agent"/>
            </owl:Restriction>
        </rdfs:subClassOf>
        <rdfs:subClassOf>
            <owl:Restriction>
                <owl:onProperty rdf:resource="https://w3id.org/arco/ontology/context-description/hasBibliography"/>
                <owl:allValuesFrom rdf:resource="https://w3id.org/arco/ontology/context-description/Bibliography"/>
            </owl:Restriction>
        </rdfs:subClassOf>
        <rdfs:subClassOf>
            <owl:Restriction>
                <owl:onProperty rdf:resource="https://w3id.org/arco/ontology/movable-property/taxonomicNumber"/>
                <owl:allValuesFrom rdf:resource="http://www.w3.org/2000/01/rdf-schema#Literal"/>
            </owl:Restriction>
        </rdfs:subClassOf>
        <rdfs:comment xml:lang="en">This class represents a biological taxon.</rdfs:comment>
        <rdfs:isDefinedBy rdf:resource="https://w3id.org/arco/ontology/movable-property"/>
        <rdfs:label xml:lang="en">Biological taxon</rdfs:label>
        <rdfs:label xml:lang="it">Taxon biologico</rdfs:label>
        <owl:versionInfo xml:lang="it">stabile</owl:versionInfo>
        <owl:versionInfo xml:lang="en">stable</owl:versionInfo>
        <a-cat:iccdNormTag>ICCD Normativa AT: OG/OGS. - Normativa BNB: SB/SBS, SB/TBI, RB/RBN</a-cat:iccdNormTag>
    </owl:Class>
    


    <!-- https://w3id.org/arco/ontology/movable-property/BotanicalForm -->

    <owl:Class rdf:about="https://w3id.org/arco/ontology/movable-property/BotanicalForm">
        <rdfs:subClassOf rdf:resource="https://w3id.org/arco/ontology/movable-property/BiologicalTaxon"/>
        <rdfs:subClassOf>
            <owl:Restriction>
                <owl:onProperty rdf:resource="https://w3id.org/arco/ontology/movable-property/hasHigherRank"/>
                <owl:allValuesFrom>
                    <owl:Class>
                        <owl:complementOf>
                            <owl:Class>
                                <owl:unionOf rdf:parseType="Collection">
                                    <rdf:Description rdf:about="https://w3id.org/arco/ontology/movable-property/BotanicalForm"/>
                                    <rdf:Description rdf:about="https://w3id.org/arco/ontology/movable-property/Cultivar"/>
                                    <rdf:Description rdf:about="https://w3id.org/arco/ontology/movable-property/Variety"/>
                                </owl:unionOf>
                            </owl:Class>
                        </owl:complementOf>
                    </owl:Class>
                </owl:allValuesFrom>
            </owl:Restriction>
        </rdfs:subClassOf>
        <owl:disjointWith rdf:resource="https://w3id.org/arco/ontology/movable-property/Cultivar"/>
        <rdfs:comment xml:lang="it">Questa classe rappresenta una varietà dal punto di vista della forma estetica o cromatica</rdfs:comment>
        <rdfs:comment xml:lang="en">This class represents a variety from an aesthetic or chromatic point of view.</rdfs:comment>
        <rdfs:isDefinedBy rdf:resource="https://w3id.org/arco/ontology/movable-property"/>
        <rdfs:label xml:lang="en">Botanical form</rdfs:label>
        <rdfs:label xml:lang="it">Forma botanica</rdfs:label>
        <owl:versionInfo xml:lang="it">instabile</owl:versionInfo>
        <owl:versionInfo xml:lang="en">unstable</owl:versionInfo>
        <a-cat:iccdNormTag>ICCD Normativa BNB: RB/RBN/RBNH; SB/NAA/NAAH; SB/NAT/NATH</a-cat:iccdNormTag>
    </owl:Class>
    


    <!-- https://w3id.org/arco/ontology/movable-property/BotanicalRevision -->

    <owl:Class rdf:about="https://w3id.org/arco/ontology/movable-property/BotanicalRevision">
        <rdfs:subClassOf rdf:resource="https://w3id.org/arco/ontology/context-description/Survey"/>
        <rdfs:subClassOf>
            <owl:Restriction>
                <owl:onProperty rdf:resource="https://w3id.org/arco/ontology/context-description/hasAuthor"/>
                <owl:allValuesFrom rdf:resource="https://w3id.org/italia/onto/l0/Agent"/>
            </owl:Restriction>
        </rdfs:subClassOf>
        <rdfs:subClassOf>
            <owl:Restriction>
                <owl:onProperty rdf:resource="https://w3id.org/arco/ontology/context-description/hasBibliography"/>
                <owl:allValuesFrom rdf:resource="https://w3id.org/arco/ontology/context-description/Bibliography"/>
            </owl:Restriction>
        </rdfs:subClassOf>
        <rdfs:subClassOf>
            <owl:Restriction>
                <owl:onProperty rdf:resource="https://w3id.org/arco/ontology/core/hasType"/>
                <owl:allValuesFrom rdf:resource="https://w3id.org/arco/ontology/movable-property/BotanicalRevisionType"/>
            </owl:Restriction>
        </rdfs:subClassOf>
        <rdfs:comment xml:lang="it">Questa classe rappresenta le informazioni su eventuali revisioni cui il campione  sia andato incontro, compresi i cambi nomenclaturali conseguenti.</rdfs:comment>
        <rdfs:comment xml:lang="en">This class represents a revision made on the specimen</rdfs:comment>
        <rdfs:isDefinedBy rdf:resource="https://w3id.org/arco/ontology/movable-property"/>
        <rdfs:label xml:lang="en">Botanical revision</rdfs:label>
        <rdfs:label xml:lang="it">Revisione botanica</rdfs:label>
        <owl:versionInfo xml:lang="it">instabile</owl:versionInfo>
        <owl:versionInfo xml:lang="en">unstable</owl:versionInfo>
        <a-cat:iccdNormTag>ICCD Normativa BNB: RB/RBR</a-cat:iccdNormTag>
    </owl:Class>
    


    <!-- https://w3id.org/arco/ontology/movable-property/BotanicalRevisionType -->

    <owl:Class rdf:about="https://w3id.org/arco/ontology/movable-property/BotanicalRevisionType">
        <rdfs:subClassOf rdf:resource="https://w3id.org/arco/ontology/core/Type"/>
        <rdfs:comment xml:lang="it">Questa classe rappresenta la tipologia della revisione cui il campione è stato oggetto.</rdfs:comment>
        <rdfs:comment xml:lang="en">This class represents the type of revision of the specimen</rdfs:comment>
        <rdfs:isDefinedBy rdf:resource="https://w3id.org/arco/ontology/movable-property"/>
        <rdfs:label xml:lang="en">Botanical revision type</rdfs:label>
        <rdfs:label xml:lang="it">Tipo di revisione botanica</rdfs:label>
        <owl:versionInfo xml:lang="it">instabile</owl:versionInfo>
        <owl:versionInfo xml:lang="en">unstable</owl:versionInfo>
        <a-cat:iccdNormTag>ICCD Normativa BNB: RB/RBR/RBRT</a-cat:iccdNormTag>
    </owl:Class>
    


    <!-- https://w3id.org/arco/ontology/movable-property/Class -->

    <owl:Class rdf:about="https://w3id.org/arco/ontology/movable-property/Class">
        <rdfs:subClassOf rdf:resource="https://w3id.org/arco/ontology/movable-property/BiologicalTaxon"/>
        <rdfs:subClassOf>
            <owl:Restriction>
                <owl:onProperty rdf:resource="https://w3id.org/arco/ontology/movable-property/hasDirectHigherRank"/>
                <owl:allValuesFrom rdf:resource="https://w3id.org/arco/ontology/movable-property/Phylum"/>
            </owl:Restriction>
        </rdfs:subClassOf>
        <rdfs:subClassOf>
            <owl:Restriction>
                <owl:onProperty rdf:resource="https://w3id.org/arco/ontology/movable-property/hasDirectLowerRank"/>
                <owl:allValuesFrom rdf:resource="https://w3id.org/arco/ontology/movable-property/Order"/>
            </owl:Restriction>
        </rdfs:subClassOf>
        <rdfs:subClassOf>
            <owl:Restriction>
                <owl:onProperty rdf:resource="https://w3id.org/arco/ontology/movable-property/hasHigherRank"/>
                <owl:allValuesFrom>
                    <owl:Class>
                        <owl:unionOf rdf:parseType="Collection">
                            <rdf:Description rdf:about="https://w3id.org/arco/ontology/movable-property/Kingdom"/>
                            <rdf:Description rdf:about="https://w3id.org/arco/ontology/movable-property/Phylum"/>
                        </owl:unionOf>
                    </owl:Class>
                </owl:allValuesFrom>
            </owl:Restriction>
        </rdfs:subClassOf>
        <rdfs:subClassOf>
            <owl:Restriction>
                <owl:onProperty rdf:resource="https://w3id.org/arco/ontology/movable-property/hasLowerRank"/>
                <owl:allValuesFrom>
                    <owl:Class>
                        <owl:complementOf>
                            <owl:Class>
                                <owl:unionOf rdf:parseType="Collection">
                                    <rdf:Description rdf:about="https://w3id.org/arco/ontology/movable-property/Class"/>
                                    <rdf:Description rdf:about="https://w3id.org/arco/ontology/movable-property/Kingdom"/>
                                    <rdf:Description rdf:about="https://w3id.org/arco/ontology/movable-property/Phylum"/>
                                </owl:unionOf>
                            </owl:Class>
                        </owl:complementOf>
                    </owl:Class>
                </owl:allValuesFrom>
            </owl:Restriction>
        </rdfs:subClassOf>
        <rdfs:comment xml:lang="it">Questa classe rappresenta uno dei livelli di classificazione di una tassonomia biologica, ovvero la classe.</rdfs:comment>
        <rdfs:comment xml:lang="en">This class represents one level of a biological taxon, the class</rdfs:comment>
        <rdfs:isDefinedBy rdf:resource="https://w3di.org/arco/ontology/movable-property/"/>
        <rdfs:label xml:lang="en">Class</rdfs:label>
        <rdfs:label xml:lang="it">Classe</rdfs:label>
        <owl:versionInfo xml:lang="it">instabile</owl:versionInfo>
        <owl:versionInfo xml:lang="en">unstable</owl:versionInfo>
    </owl:Class>
    


    <!-- https://w3id.org/arco/ontology/movable-property/CloseIndividual -->

    <owl:Class rdf:about="https://w3id.org/arco/ontology/movable-property/CloseIndividual">
        <rdfs:subClassOf rdf:resource="https://w3id.org/italia/onto/l0/Object"/>
        <rdfs:subClassOf>
            <owl:Restriction>
                <owl:onProperty rdf:resource="https://w3id.org/arco/ontology/movable-property/isCloseIndivisualOf"/>
                <owl:someValuesFrom rdf:resource="http://dati.beniculturali.it/cis/CulturalEntity"/>
            </owl:Restriction>
        </rdfs:subClassOf>
        <rdfs:comment xml:lang="it">Questa classe rappresenta l&apos;individuo vicino al campione</rdfs:comment>
        <rdfs:comment xml:lang="en">This class represents the individual close to the specimen</rdfs:comment>
        <rdfs:isDefinedBy rdf:resource="https://w3id.org/arco/ontology/movable-property"/>
        <rdfs:label xml:lang="en">Close individual</rdfs:label>
        <rdfs:label xml:lang="it">Individuo vicino</rdfs:label>
        <owl:versionInfo xml:lang="it">instabile</owl:versionInfo>
        <owl:versionInfo xml:lang="en">unstable</owl:versionInfo>
        <a-cat:iccdNormTag>ICCD Normativa BNB: LR/LRI/LRIV</a-cat:iccdNormTag>
    </owl:Class>
    


    <!-- https://w3id.org/arco/ontology/movable-property/CollectingSite -->

    <owl:Class rdf:about="https://w3id.org/arco/ontology/movable-property/CollectingSite">
        <rdfs:subClassOf rdf:resource="https://w3id.org/arco/ontology/location/TimeIndexedTypedLocation"/>
        <rdfs:subClassOf>
            <owl:Restriction>
                <owl:onProperty rdf:resource="https://w3id.org/arco/ontology/movable-property/isCollectingSiteOF"/>
                <owl:someValuesFrom rdf:resource="http://dati.beniculturali.it/cis/CulturalEntity"/>
            </owl:Restriction>
        </rdfs:subClassOf>
        <rdfs:subClassOf>
            <owl:Restriction>
                <owl:onProperty rdf:resource="https://w3id.org/arco/ontology/denotative-description/hasMeasurementCollection"/>
                <owl:allValuesFrom rdf:resource="https://w3id.org/arco/ontology/denotative-description/MeasurementCollection"/>
            </owl:Restriction>
        </rdfs:subClassOf>
        <rdfs:subClassOf>
            <owl:Restriction>
                <owl:onProperty rdf:resource="https://w3id.org/arco/ontology/denotative-description/hasOrientation"/>
                <owl:allValuesFrom rdf:resource="https://w3id.org/arco/ontology/denotative-description/Orientation"/>
            </owl:Restriction>
        </rdfs:subClassOf>
        <rdfs:subClassOf>
            <owl:Restriction>
                <owl:onProperty rdf:resource="https://w3id.org/arco/ontology/movable-property/hasFluidDynamism"/>
                <owl:allValuesFrom rdf:resource="https://w3id.org/arco/ontology/movable-property/FluidDynamism"/>
            </owl:Restriction>
        </rdfs:subClassOf>
        <rdfs:subClassOf>
            <owl:Restriction>
                <owl:onProperty rdf:resource="https://w3id.org/arco/ontology/movable-property/hasShadeTolerance"/>
                <owl:allValuesFrom rdf:resource="https://w3id.org/arco/ontology/movable-property/ShadeTolerance"/>
            </owl:Restriction>
        </rdfs:subClassOf>
        <rdfs:subClassOf>
            <owl:Restriction>
                <owl:onProperty rdf:resource="https://w3id.org/arco/ontology/movable-property/hasSubstrate"/>
                <owl:allValuesFrom rdf:resource="https://w3id.org/arco/ontology/movable-property/Substrate"/>
            </owl:Restriction>
        </rdfs:subClassOf>
        <rdfs:comment xml:lang="it">Questa classe rappresenta informazioni specifiche, non relative alla posizione geografica, della località di reperimento dell&apos;oggetto della scheda</rdfs:comment>
        <rdfs:comment xml:lang="en">This class represents non geographical information about the site where the specimen was collected</rdfs:comment>
        <rdfs:isDefinedBy rdf:resource="https://w3id.org/arco/ontology/movable-property"/>
        <rdfs:label xml:lang="en">Collecting site</rdfs:label>
        <rdfs:label xml:lang="it">Luogo di raccolta</rdfs:label>
        <owl:versionInfo xml:lang="it">instabile</owl:versionInfo>
        <owl:versionInfo xml:lang="en">unstable</owl:versionInfo>
        <a-cat:iccdNormTag>ICCD Normativa BNB: LR/LRI</a-cat:iccdNormTag>
    </owl:Class>
    


    <!-- https://w3id.org/arco/ontology/movable-property/Cultivar -->

    <owl:Class rdf:about="https://w3id.org/arco/ontology/movable-property/Cultivar">
        <rdfs:subClassOf rdf:resource="https://w3id.org/arco/ontology/movable-property/BiologicalTaxon"/>
        <rdfs:subClassOf>
            <owl:Restriction>
                <owl:onProperty rdf:resource="https://w3id.org/arco/ontology/movable-property/hasHigherRank"/>
                <owl:allValuesFrom>
                    <owl:Class>
                        <owl:complementOf>
                            <owl:Class>
                                <owl:unionOf rdf:parseType="Collection">
                                    <rdf:Description rdf:about="https://w3id.org/arco/ontology/movable-property/BotanicalForm"/>
                                    <rdf:Description rdf:about="https://w3id.org/arco/ontology/movable-property/Cultivar"/>
                                    <rdf:Description rdf:about="https://w3id.org/arco/ontology/movable-property/Variety"/>
                                </owl:unionOf>
                            </owl:Class>
                        </owl:complementOf>
                    </owl:Class>
                </owl:allValuesFrom>
            </owl:Restriction>
        </rdfs:subClassOf>
        <rdfs:comment xml:lang="it">Questa classe rappresenta una varietà dal punto di vista delle specifiche forme coltivate</rdfs:comment>
        <rdfs:comment xml:lang="en">This class represents is the most basic classification category of cultivated plants in the International Code of Nomenclature for Cultivated Plants</rdfs:comment>
        <rdfs:isDefinedBy rdf:resource="https://w3id.org/arco/ontology/movable-property"/>
        <rdfs:label xml:lang="en">Cultivar</rdfs:label>
        <rdfs:label xml:lang="it">Cultivar</rdfs:label>
        <owl:versionInfo xml:lang="it">instabile</owl:versionInfo>
        <owl:versionInfo xml:lang="en">unstable</owl:versionInfo>
        <a-cat:iccdNormTag>ICCD Normativa BNB: RB/RBN/RBNL; SB/NAA/NAAL; SB/NAT/NATL</a-cat:iccdNormTag>
    </owl:Class>
    


    <!-- https://w3id.org/arco/ontology/movable-property/Family -->

    <owl:Class rdf:about="https://w3id.org/arco/ontology/movable-property/Family">
        <rdfs:subClassOf rdf:resource="https://w3id.org/arco/ontology/movable-property/BiologicalTaxon"/>
        <rdfs:subClassOf>
            <owl:Restriction>
                <owl:onProperty rdf:resource="https://w3id.org/arco/ontology/movable-property/hasDirectHigherRank"/>
                <owl:allValuesFrom rdf:resource="https://w3id.org/arco/ontology/movable-property/Order"/>
            </owl:Restriction>
        </rdfs:subClassOf>
        <rdfs:subClassOf>
            <owl:Restriction>
                <owl:onProperty rdf:resource="https://w3id.org/arco/ontology/movable-property/hasDirectLowerRank"/>
                <owl:allValuesFrom rdf:resource="https://w3id.org/arco/ontology/movable-property/Genus"/>
            </owl:Restriction>
        </rdfs:subClassOf>
        <rdfs:subClassOf>
            <owl:Restriction>
                <owl:onProperty rdf:resource="https://w3id.org/arco/ontology/movable-property/hasHigherRank"/>
                <owl:allValuesFrom>
                    <owl:Class>
                        <owl:complementOf>
                            <owl:Class>
                                <owl:unionOf rdf:parseType="Collection">
                                    <rdf:Description rdf:about="https://w3id.org/arco/ontology/movable-property/BotanicalForm"/>
                                    <rdf:Description rdf:about="https://w3id.org/arco/ontology/movable-property/Cultivar"/>
                                    <rdf:Description rdf:about="https://w3id.org/arco/ontology/movable-property/Family"/>
                                    <rdf:Description rdf:about="https://w3id.org/arco/ontology/movable-property/Genus"/>
                                    <rdf:Description rdf:about="https://w3id.org/arco/ontology/movable-property/Species"/>
                                    <rdf:Description rdf:about="https://w3id.org/arco/ontology/movable-property/Subspecies"/>
                                    <rdf:Description rdf:about="https://w3id.org/arco/ontology/movable-property/Variety"/>
                                </owl:unionOf>
                            </owl:Class>
                        </owl:complementOf>
                    </owl:Class>
                </owl:allValuesFrom>
            </owl:Restriction>
        </rdfs:subClassOf>
        <rdfs:subClassOf>
            <owl:Restriction>
                <owl:onProperty rdf:resource="https://w3id.org/arco/ontology/movable-property/hasLowerRank"/>
                <owl:allValuesFrom>
                    <owl:Class>
                        <owl:unionOf rdf:parseType="Collection">
                            <rdf:Description rdf:about="https://w3id.org/arco/ontology/movable-property/BotanicalForm"/>
                            <rdf:Description rdf:about="https://w3id.org/arco/ontology/movable-property/Cultivar"/>
                            <rdf:Description rdf:about="https://w3id.org/arco/ontology/movable-property/Genus"/>
                            <rdf:Description rdf:about="https://w3id.org/arco/ontology/movable-property/Species"/>
                            <rdf:Description rdf:about="https://w3id.org/arco/ontology/movable-property/Subspecies"/>
                            <rdf:Description rdf:about="https://w3id.org/arco/ontology/movable-property/Variety"/>
                        </owl:unionOf>
                    </owl:Class>
                </owl:allValuesFrom>
            </owl:Restriction>
        </rdfs:subClassOf>
        <rdfs:comment xml:lang="it">Questa classe rappresenta uno dei livelli di classificazione di una tassonomia biologica, ovvero la famiglia</rdfs:comment>
        <rdfs:comment xml:lang="en">This class represents one level of a biological taxon, the family.</rdfs:comment>
        <rdfs:isDefinedBy rdf:resource="https://w3di.org/arco/ontology/movable-property/"/>
        <rdfs:label xml:lang="it">Famiglia</rdfs:label>
        <rdfs:label xml:lang="en">Family</rdfs:label>
        <owl:versionInfo xml:lang="it">instabile</owl:versionInfo>
        <owl:versionInfo xml:lang="en">unstable</owl:versionInfo>
        <a-cat:iccdNormTag>ICCD Normativa BNB: SB/SBS/SBSF</a-cat:iccdNormTag>
    </owl:Class>
    


    <!-- https://w3id.org/arco/ontology/movable-property/FluidDynamism -->

    <owl:Class rdf:about="https://w3id.org/arco/ontology/movable-property/FluidDynamism">
        <rdfs:subClassOf rdf:resource="https://w3id.org/italia/onto/l0/Characteristic"/>
        <rdfs:subClassOf>
            <owl:Restriction>
                <owl:onProperty rdf:resource="https://w3id.org/arco/ontology/movable-property/isFluidDynamismOf"/>
                <owl:someValuesFrom rdf:resource="https://w3id.org/arco/ontology/movable-property/CollectingSite"/>
            </owl:Restriction>
        </rdfs:subClassOf>
        <rdfs:comment xml:lang="en">This class represents the fluid dynamis when the specimenwas collected</rdfs:comment>
        <rdfs:isDefinedBy rdf:resource="https://w3id.org/arco/ontology/movable-property"/>
        <rdfs:label xml:lang="en">Fluid dynamism</rdfs:label>
        <rdfs:label xml:lang="it">Idrodinamismo</rdfs:label>
        <owl:versionInfo xml:lang="it">instabile</owl:versionInfo>
        <owl:versionInfo xml:lang="en">unstable</owl:versionInfo>
        <a-cat:iccdNormTag>ICCD Normativa BNB: LR/LRI/LRID</a-cat:iccdNormTag>
    </owl:Class>
    


    <!-- https://w3id.org/arco/ontology/movable-property/FruitSample -->

    <owl:Class rdf:about="https://w3id.org/arco/ontology/movable-property/FruitSample">
        <rdfs:subClassOf rdf:resource="https://w3id.org/arco/ontology/movable-property/Sample"/>
        <rdfs:subClassOf>
            <owl:Restriction>
                <owl:onProperty rdf:resource="https://w3id.org/arco/ontology/movable-property/hasPreservationType"/>
                <owl:allValuesFrom rdf:resource="https://w3id.org/arco/ontology/movable-property/PreservationType"/>
            </owl:Restriction>
        </rdfs:subClassOf>
        <rdfs:subClassOf>
            <owl:Restriction>
                <owl:onProperty rdf:resource="https://w3id.org/arco/ontology/movable-property/dateOfLastChangePreservative"/>
                <owl:allValuesFrom rdf:resource="http://www.w3.org/2001/XMLSchema#date"/>
            </owl:Restriction>
        </rdfs:subClassOf>
        <rdfs:comment xml:lang="it">Questa classe rappresenta un reperto carpologico (frutti)</rdfs:comment>
        <rdfs:comment xml:lang="en">This class represents a sample from the fruit collection</rdfs:comment>
        <rdfs:isDefinedBy rdf:resource="https://w3id.org/arco/ontology/movable-property"/>
        <rdfs:label xml:lang="en">Fruit  sample</rdfs:label>
        <rdfs:label xml:lang="it">Reperto carpologico</rdfs:label>
        <owl:versionInfo xml:lang="it">instabile</owl:versionInfo>
        <owl:versionInfo xml:lang="en">unstable</owl:versionInfo>
        <a-cat:iccdNormTag>ICCD Normativa BNB: DB/DBC</a-cat:iccdNormTag>
    </owl:Class>
    


    <!-- https://w3id.org/arco/ontology/movable-property/Genus -->

    <owl:Class rdf:about="https://w3id.org/arco/ontology/movable-property/Genus">
        <rdfs:subClassOf rdf:resource="https://w3id.org/arco/ontology/movable-property/BiologicalTaxon"/>
        <rdfs:subClassOf>
            <owl:Restriction>
                <owl:onProperty rdf:resource="https://w3id.org/arco/ontology/movable-property/hasDirectHigherRank"/>
                <owl:allValuesFrom rdf:resource="https://w3id.org/arco/ontology/movable-property/Family"/>
            </owl:Restriction>
        </rdfs:subClassOf>
        <rdfs:subClassOf>
            <owl:Restriction>
                <owl:onProperty rdf:resource="https://w3id.org/arco/ontology/movable-property/hasDirectLowerRank"/>
                <owl:allValuesFrom rdf:resource="https://w3id.org/arco/ontology/movable-property/Species"/>
            </owl:Restriction>
        </rdfs:subClassOf>
        <rdfs:subClassOf>
            <owl:Restriction>
                <owl:onProperty rdf:resource="https://w3id.org/arco/ontology/movable-property/hasHigherRank"/>
                <owl:allValuesFrom>
                    <owl:Class>
                        <owl:complementOf>
                            <owl:Class>
                                <owl:unionOf rdf:parseType="Collection">
                                    <rdf:Description rdf:about="https://w3id.org/arco/ontology/movable-property/BotanicalForm"/>
                                    <rdf:Description rdf:about="https://w3id.org/arco/ontology/movable-property/Cultivar"/>
                                    <rdf:Description rdf:about="https://w3id.org/arco/ontology/movable-property/Genus"/>
                                    <rdf:Description rdf:about="https://w3id.org/arco/ontology/movable-property/Species"/>
                                    <rdf:Description rdf:about="https://w3id.org/arco/ontology/movable-property/Subspecies"/>
                                    <rdf:Description rdf:about="https://w3id.org/arco/ontology/movable-property/Variety"/>
                                </owl:unionOf>
                            </owl:Class>
                        </owl:complementOf>
                    </owl:Class>
                </owl:allValuesFrom>
            </owl:Restriction>
        </rdfs:subClassOf>
        <rdfs:subClassOf>
            <owl:Restriction>
                <owl:onProperty rdf:resource="https://w3id.org/arco/ontology/movable-property/hasLowerRank"/>
                <owl:allValuesFrom>
                    <owl:Class>
                        <owl:unionOf rdf:parseType="Collection">
                            <rdf:Description rdf:about="https://w3id.org/arco/ontology/movable-property/BotanicalForm"/>
                            <rdf:Description rdf:about="https://w3id.org/arco/ontology/movable-property/Cultivar"/>
                            <rdf:Description rdf:about="https://w3id.org/arco/ontology/movable-property/Species"/>
                            <rdf:Description rdf:about="https://w3id.org/arco/ontology/movable-property/Subspecies"/>
                            <rdf:Description rdf:about="https://w3id.org/arco/ontology/movable-property/Variety"/>
                        </owl:unionOf>
                    </owl:Class>
                </owl:allValuesFrom>
            </owl:Restriction>
        </rdfs:subClassOf>
        <rdfs:subClassOf>
            <owl:Restriction>
                <owl:onProperty rdf:resource="https://w3id.org/arco/ontology/movable-property/genusNumber"/>
                <owl:allValuesFrom rdf:resource="http://www.w3.org/2000/01/rdf-schema#Literal"/>
            </owl:Restriction>
        </rdfs:subClassOf>
        <rdfs:comment xml:lang="it">Questa classe rappresenta uno dei livelli di classificazione di una tassonomia biologica, ovvero il genere.</rdfs:comment>
        <rdfs:comment xml:lang="en">This class represents one level of a biological taxon, the genus.</rdfs:comment>
        <rdfs:isDefinedBy rdf:resource="https://w3di.org/arco/ontology/movable-property/"/>
        <rdfs:label xml:lang="it">Genere</rdfs:label>
        <rdfs:label xml:lang="en">Genus</rdfs:label>
        <owl:versionInfo xml:lang="it">instabile</owl:versionInfo>
        <owl:versionInfo xml:lang="en">unstable</owl:versionInfo>
        <a-cat:iccdNormTag>ICCD Normativa AT: OG/OGS/OGSG. - Normativa BNB: RB/RBN/RBNA; SB/NAA/NAAA; SB/NAT/NATA</a-cat:iccdNormTag>
    </owl:Class>
    


    <!-- https://w3id.org/arco/ontology/movable-property/HostIndividual -->

    <owl:Class rdf:about="https://w3id.org/arco/ontology/movable-property/HostIndividual">
        <rdfs:subClassOf rdf:resource="https://w3id.org/italia/onto/l0/Object"/>
        <rdfs:subClassOf>
            <owl:Restriction>
                <owl:onProperty rdf:resource="https://w3id.org/arco/ontology/movable-property/isHostIndividualOf"/>
                <owl:someValuesFrom rdf:resource="http://dati.beniculturali.it/cis/CulturalEntity"/>
            </owl:Restriction>
        </rdfs:subClassOf>
        <rdfs:comment xml:lang="it">Questa classe rappresenta l&apos;individuo ospite del campione</rdfs:comment>
        <rdfs:comment xml:lang="en">This class represents the individual hosting the specimen</rdfs:comment>
        <rdfs:isDefinedBy rdf:resource="https://w3id.org/arco/ontology/movable-property"/>
        <rdfs:label xml:lang="en">Host individual</rdfs:label>
        <rdfs:label xml:lang="it">Individuo ospite</rdfs:label>
        <owl:versionInfo xml:lang="it">instabile</owl:versionInfo>
        <owl:versionInfo xml:lang="en">unstable</owl:versionInfo>
        <a-cat:iccdNormTag>ICCD Normativa BNB: LR/LRI/LRIM</a-cat:iccdNormTag>
    </owl:Class>
    


    <!-- https://w3id.org/arco/ontology/movable-property/Incline -->

    <owl:Class rdf:about="https://w3id.org/arco/ontology/movable-property/Incline">
        <rdfs:subClassOf rdf:resource="https://w3id.org/italia/onto/l0/Characteristic"/>
        <rdfs:subClassOf>
            <owl:Restriction>
                <owl:onProperty rdf:resource="https://w3id.org/arco/ontology/movable-property/isInclineOf"/>
                <owl:someValuesFrom rdf:resource="https://w3id.org/arco/ontology/movable-property/Substrate"/>
            </owl:Restriction>
        </rdfs:subClassOf>
        <rdfs:comment xml:lang="it">Questa classe rappresenta l&apos;inclinazione (qualitativa) del substrato di raccolta del campione</rdfs:comment>
        <rdfs:comment xml:lang="en">This class represents the incline of the substrate where the specimen was collected</rdfs:comment>
        <rdfs:isDefinedBy rdf:resource="https://w3id.org/arco/ontology/movable-property"/>
        <rdfs:label xml:lang="it">Inclinazione</rdfs:label>
        <rdfs:label xml:lang="en">Incline</rdfs:label>
        <owl:versionInfo xml:lang="it">instabile</owl:versionInfo>
        <owl:versionInfo xml:lang="en">unstable</owl:versionInfo>
        <a-cat:iccdNormTag>ICCD Normativa BNB: LR/LRI/LRII</a-cat:iccdNormTag>
    </owl:Class>
    


    <!-- https://w3id.org/arco/ontology/movable-property/Kingdom -->

    <owl:Class rdf:about="https://w3id.org/arco/ontology/movable-property/Kingdom">
        <rdfs:subClassOf rdf:resource="https://w3id.org/arco/ontology/movable-property/BiologicalTaxon"/>
        <rdfs:subClassOf>
            <owl:Restriction>
                <owl:onProperty rdf:resource="https://w3id.org/arco/ontology/movable-property/hasDirectLowerRank"/>
                <owl:allValuesFrom rdf:resource="https://w3id.org/arco/ontology/movable-property/Phylum"/>
            </owl:Restriction>
        </rdfs:subClassOf>
        <rdfs:subClassOf>
            <owl:Restriction>
                <owl:onProperty rdf:resource="https://w3id.org/arco/ontology/movable-property/hasLowerRank"/>
                <owl:allValuesFrom>
                    <owl:Class>
                        <owl:complementOf rdf:resource="https://w3id.org/arco/ontology/movable-property/Kingdom"/>
                    </owl:Class>
                </owl:allValuesFrom>
            </owl:Restriction>
        </rdfs:subClassOf>
        <rdfs:comment xml:lang="it">Questa classe rappresenta uno dei livelli di classificazione di una tassonomia biologica, ovvero il regno.</rdfs:comment>
        <rdfs:comment xml:lang="en">This class represents one level of a biological taxon, the kingdom</rdfs:comment>
        <rdfs:isDefinedBy rdf:resource="https://w3di.org/arco/ontology/movable-property/"/>
        <rdfs:label xml:lang="en">Kingdom</rdfs:label>
        <rdfs:label xml:lang="it">Regno</rdfs:label>
        <owl:versionInfo xml:lang="it">instabile</owl:versionInfo>
        <owl:versionInfo xml:lang="en">unstable</owl:versionInfo>
    </owl:Class>
    


    <!-- https://w3id.org/arco/ontology/movable-property/Label -->

    <owl:Class rdf:about="https://w3id.org/arco/ontology/movable-property/Label">
        <rdfs:subClassOf rdf:resource="https://w3id.org/arco/ontology/denotative-description/AffixedElement"/>
        <rdfs:subClassOf>
            <owl:Restriction>
                <owl:onProperty rdf:resource="https://w3id.org/arco/ontology/movable-property/isLabelOf"/>
                <owl:someValuesFrom rdf:resource="http://dati.beniculturali.it/cis/CulturalEntity"/>
            </owl:Restriction>
        </rdfs:subClassOf>
        <rdfs:subClassOf>
            <owl:Restriction>
                <owl:onProperty rdf:resource="https://w3id.org/arco/ontology/denotative-description/hasFontStyle"/>
                <owl:allValuesFrom rdf:resource="https://w3id.org/arco/ontology/denotative-description/FontStyle"/>
            </owl:Restriction>
        </rdfs:subClassOf>
        <rdfs:subClassOf>
            <owl:Restriction>
                <owl:onProperty rdf:resource="https://w3id.org/arco/ontology/movable-property/hasLanguage"/>
                <owl:allValuesFrom rdf:resource="https://w3id.org/arco/ontology/movable-property/Language"/>
            </owl:Restriction>
        </rdfs:subClassOf>
        <rdfs:subClassOf>
            <owl:Restriction>
                <owl:onProperty rdf:resource="https://w3id.org/arco/ontology/movable-property/bodyTranscript"/>
                <owl:allValuesFrom rdf:resource="http://www.w3.org/2000/01/rdf-schema#Literal"/>
            </owl:Restriction>
        </rdfs:subClassOf>
        <rdfs:subClassOf>
            <owl:Restriction>
                <owl:onProperty rdf:resource="https://w3id.org/arco/ontology/movable-property/graphicSymbols"/>
                <owl:allValuesFrom rdf:resource="http://www.w3.org/2000/01/rdf-schema#Literal"/>
            </owl:Restriction>
        </rdfs:subClassOf>
        <rdfs:subClassOf>
            <owl:Restriction>
                <owl:onProperty rdf:resource="https://w3id.org/arco/ontology/movable-property/handWriting"/>
                <owl:allValuesFrom rdf:resource="http://www.w3.org/2001/XMLSchema#boolean"/>
            </owl:Restriction>
        </rdfs:subClassOf>
        <rdfs:subClassOf>
            <owl:Restriction>
                <owl:onProperty rdf:resource="https://w3id.org/arco/ontology/movable-property/headingTranscript"/>
                <owl:allValuesFrom rdf:resource="http://www.w3.org/2000/01/rdf-schema#Literal"/>
            </owl:Restriction>
        </rdfs:subClassOf>
        <rdfs:comment xml:lang="it">Questa classe rappresenta il cartellino o l&apos;etichetta presente sul o insieme al campione oggetto della scheda o al contenitore.</rdfs:comment>
        <rdfs:comment xml:lang="en">This class represents the label located on a specimen or on a specimen container.</rdfs:comment>
        <rdfs:isDefinedBy rdf:resource="https://w3id.org/arco/ontology/movable-property"/>
        <rdfs:label xml:lang="it">Etichetta</rdfs:label>
        <rdfs:label xml:lang="en">Label</rdfs:label>
        <owl:versionInfo xml:lang="it">instabile</owl:versionInfo>
        <owl:versionInfo xml:lang="en">untable</owl:versionInfo>
        <a-cat:iccdNormTag>ICCD Normativa BNB: SB/SBE</a-cat:iccdNormTag>
    </owl:Class>
    


    <!-- https://w3id.org/arco/ontology/movable-property/Language -->

    <owl:Class rdf:about="https://w3id.org/arco/ontology/movable-property/Language">
        <rdfs:comment xml:lang="en">A natural or artificial language, provided with an alphabet (or vocabulary) and combinatorial rules.</rdfs:comment>
        <rdfs:comment xml:lang="it">Un linguaggio artificiale o naturale, con un alfabeto (o vocabolario) e delle regole per combinare i simboli/suoni.</rdfs:comment>
        <rdfs:isDefinedBy rdf:resource="https://w3id.org/arco/ontology/movable-property"/>
        <rdfs:label xml:lang="en">Language</rdfs:label>
        <rdfs:label xml:lang="it">Lingua</rdfs:label>
        <owl:versionInfo xml:lang="it">instabile</owl:versionInfo>
        <owl:versionInfo xml:lang="en">unstable</owl:versionInfo>
        <a-cat:iccdNormTag>ICCD Normativa BNB: SB/SBE/SBEL</a-cat:iccdNormTag>
    </owl:Class>
    


    <!-- https://w3id.org/arco/ontology/movable-property/NaturalEnvironment -->

    <owl:Class rdf:about="https://w3id.org/arco/ontology/movable-property/NaturalEnvironment">
        <rdfs:subClassOf rdf:resource="https://w3id.org/italia/onto/l0/Characteristic"/>
        <rdfs:subClassOf>
            <owl:Restriction>
                <owl:onProperty rdf:resource="https://w3id.org/arco/ontology/movable-property/isNaturalEnvironmentOf"/>
                <owl:someValuesFrom rdf:resource="https://w3id.org/arco/ontology/movable-property/Substrate"/>
            </owl:Restriction>
        </rdfs:subClassOf>
        <rdfs:comment xml:lang="it">Questa classe rappresenta l&apos;ambiente cui appartiene il substrato su cui è stato raccolto il campione</rdfs:comment>
        <rdfs:comment xml:lang="en">This class represents the natural environment of the substrate where the specimen was collected</rdfs:comment>
        <rdfs:isDefinedBy rdf:resource="https://w3id.org/arco/ontology/movable-property"/>
        <rdfs:label xml:lang="it">Ambiente naturale</rdfs:label>
        <rdfs:label xml:lang="en">Natural environment</rdfs:label>
        <owl:versionInfo xml:lang="it">instabile</owl:versionInfo>
        <owl:versionInfo xml:lang="en">unstable</owl:versionInfo>
        <a-cat:iccdNormTag>ICCD Normativa BNB: LR/LRI/LRIB</a-cat:iccdNormTag>
    </owl:Class>
    


    <!-- https://w3id.org/arco/ontology/movable-property/Order -->

    <owl:Class rdf:about="https://w3id.org/arco/ontology/movable-property/Order">
        <rdfs:subClassOf rdf:resource="https://w3id.org/arco/ontology/movable-property/BiologicalTaxon"/>
        <rdfs:subClassOf>
            <owl:Restriction>
                <owl:onProperty rdf:resource="https://w3id.org/arco/ontology/movable-property/hasDirectHigherRank"/>
                <owl:allValuesFrom rdf:resource="https://w3id.org/arco/ontology/movable-property/Class"/>
            </owl:Restriction>
        </rdfs:subClassOf>
        <rdfs:subClassOf>
            <owl:Restriction>
                <owl:onProperty rdf:resource="https://w3id.org/arco/ontology/movable-property/hasDirectLowerRank"/>
                <owl:allValuesFrom rdf:resource="https://w3id.org/arco/ontology/movable-property/Family"/>
            </owl:Restriction>
        </rdfs:subClassOf>
        <rdfs:subClassOf>
            <owl:Restriction>
                <owl:onProperty rdf:resource="https://w3id.org/arco/ontology/movable-property/hasHigherRank"/>
                <owl:allValuesFrom>
                    <owl:Class>
                        <owl:unionOf rdf:parseType="Collection">
                            <rdf:Description rdf:about="https://w3id.org/arco/ontology/movable-property/Class"/>
                            <rdf:Description rdf:about="https://w3id.org/arco/ontology/movable-property/Kingdom"/>
                            <rdf:Description rdf:about="https://w3id.org/arco/ontology/movable-property/Phylum"/>
                        </owl:unionOf>
                    </owl:Class>
                </owl:allValuesFrom>
            </owl:Restriction>
        </rdfs:subClassOf>
        <rdfs:subClassOf>
            <owl:Restriction>
                <owl:onProperty rdf:resource="https://w3id.org/arco/ontology/movable-property/hasLowerRank"/>
                <owl:allValuesFrom>
                    <owl:Class>
                        <owl:unionOf rdf:parseType="Collection">
                            <rdf:Description rdf:about="https://w3id.org/arco/ontology/movable-property/BotanicalForm"/>
                            <rdf:Description rdf:about="https://w3id.org/arco/ontology/movable-property/Cultivar"/>
                            <rdf:Description rdf:about="https://w3id.org/arco/ontology/movable-property/Family"/>
                            <rdf:Description rdf:about="https://w3id.org/arco/ontology/movable-property/Genus"/>
                            <rdf:Description rdf:about="https://w3id.org/arco/ontology/movable-property/Species"/>
                            <rdf:Description rdf:about="https://w3id.org/arco/ontology/movable-property/Subspecies"/>
                            <rdf:Description rdf:about="https://w3id.org/arco/ontology/movable-property/Variety"/>
                        </owl:unionOf>
                    </owl:Class>
                </owl:allValuesFrom>
            </owl:Restriction>
        </rdfs:subClassOf>
        <rdfs:comment xml:lang="it">Questa classe rappresenta uno dei livelli di classificazione di una tassonomia biologica, ovvero l&apos;ordine</rdfs:comment>
        <rdfs:comment xml:lang="en">This class represents one level of a biological taxon, the order</rdfs:comment>
        <rdfs:isDefinedBy rdf:resource="https://w3di.org/arco/ontology/movable-property/"/>
        <rdfs:label xml:lang="en">Order</rdfs:label>
        <rdfs:label xml:lang="it">Ordine</rdfs:label>
        <owl:versionInfo xml:lang="it">instabile</owl:versionInfo>
        <owl:versionInfo xml:lang="en">unstable</owl:versionInfo>
    </owl:Class>
    


    <!-- https://w3id.org/arco/ontology/movable-property/Phylum -->

    <owl:Class rdf:about="https://w3id.org/arco/ontology/movable-property/Phylum">
        <rdfs:subClassOf rdf:resource="https://w3id.org/arco/ontology/movable-property/BiologicalTaxon"/>
        <rdfs:subClassOf>
            <owl:Restriction>
                <owl:onProperty rdf:resource="https://w3id.org/arco/ontology/movable-property/hasDirectHigherRank"/>
                <owl:allValuesFrom rdf:resource="https://w3id.org/arco/ontology/movable-property/Kingdom"/>
            </owl:Restriction>
        </rdfs:subClassOf>
        <rdfs:subClassOf>
            <owl:Restriction>
                <owl:onProperty rdf:resource="https://w3id.org/arco/ontology/movable-property/hasDirectLowerRank"/>
                <owl:allValuesFrom rdf:resource="https://w3id.org/arco/ontology/movable-property/Class"/>
            </owl:Restriction>
        </rdfs:subClassOf>
        <rdfs:subClassOf>
            <owl:Restriction>
                <owl:onProperty rdf:resource="https://w3id.org/arco/ontology/movable-property/hasHigherRank"/>
                <owl:allValuesFrom rdf:resource="https://w3id.org/arco/ontology/movable-property/Kingdom"/>
            </owl:Restriction>
        </rdfs:subClassOf>
        <rdfs:subClassOf>
            <owl:Restriction>
                <owl:onProperty rdf:resource="https://w3id.org/arco/ontology/movable-property/hasLowerRank"/>
                <owl:allValuesFrom>
                    <owl:Class>
                        <owl:complementOf>
                            <owl:Class>
                                <owl:unionOf rdf:parseType="Collection">
                                    <rdf:Description rdf:about="https://w3id.org/arco/ontology/movable-property/Kingdom"/>
                                    <rdf:Description rdf:about="https://w3id.org/arco/ontology/movable-property/Phylum"/>
                                </owl:unionOf>
                            </owl:Class>
                        </owl:complementOf>
                    </owl:Class>
                </owl:allValuesFrom>
            </owl:Restriction>
        </rdfs:subClassOf>
        <rdfs:comment xml:lang="it">Questa classe rappresenta uno dei livelli di classificazione di una tassonomia biologica, ovvero il phylum.</rdfs:comment>
        <rdfs:comment xml:lang="en">This class represents one level of a biological taxon, the phylum</rdfs:comment>
        <rdfs:isDefinedBy rdf:resource="https://w3id.org/arco/ontology/movable-property"/>
        <rdfs:label xml:lang="en">Phylum</rdfs:label>
        <rdfs:label xml:lang="it">Phylum</rdfs:label>
        <owl:versionInfo xml:lang="it">instabile</owl:versionInfo>
        <owl:versionInfo xml:lang="en">unstable</owl:versionInfo>
    </owl:Class>
    


    <!-- https://w3id.org/arco/ontology/movable-property/PollenSample -->

    <owl:Class rdf:about="https://w3id.org/arco/ontology/movable-property/PollenSample">
        <rdfs:subClassOf rdf:resource="https://w3id.org/arco/ontology/movable-property/Sample"/>
        <rdfs:subClassOf>
            <owl:Restriction>
                <owl:onProperty rdf:resource="https://w3id.org/arco/ontology/denotative-description/hasTechnique"/>
                <owl:allValuesFrom rdf:resource="https://w3id.org/arco/ontology/denotative-description/TechnicalCharacteristic"/>
            </owl:Restriction>
        </rdfs:subClassOf>
        <rdfs:comment xml:lang="it">Questa classe rappresenta un reperto palinologico (pollini)</rdfs:comment>
        <rdfs:comment xml:lang="en">This class represents sample from the pollen collection</rdfs:comment>
        <rdfs:isDefinedBy rdf:resource="https://w3id.org/arco/ontology/movable-property"/>
        <rdfs:label xml:lang="en">Pollen sample</rdfs:label>
        <rdfs:label xml:lang="it">Reperto palinologico</rdfs:label>
        <owl:versionInfo xml:lang="it">instabile</owl:versionInfo>
        <owl:versionInfo xml:lang="en">unstable</owl:versionInfo>
        <a-cat:iccdNormTag>ICCD Normativa BNB: DB/DBP</a-cat:iccdNormTag>
    </owl:Class>
    


    <!-- https://w3id.org/arco/ontology/movable-property/Preparation -->

    <owl:Class rdf:about="https://w3id.org/arco/ontology/movable-property/Preparation">
        <rdfs:subClassOf rdf:resource="https://w3id.org/italia/onto/l0/Object"/>
        <rdfs:subClassOf>
            <owl:Restriction>
                <owl:onProperty rdf:resource="https://w3id.org/arco/ontology/context-description/hasAuthor"/>
                <owl:allValuesFrom rdf:resource="https://w3id.org/italia/onto/l0/Agent"/>
            </owl:Restriction>
        </rdfs:subClassOf>
        <rdfs:subClassOf>
            <owl:Restriction>
                <owl:onProperty rdf:resource="https://w3id.org/arco/ontology/core/hasType"/>
                <owl:allValuesFrom rdf:resource="https://w3id.org/arco/ontology/movable-property/PreparationType"/>
            </owl:Restriction>
        </rdfs:subClassOf>
        <rdfs:subClassOf>
            <owl:Restriction>
                <owl:onProperty rdf:resource="https://w3id.org/arco/ontology/movable-property/manufacturingDate"/>
                <owl:allValuesFrom rdf:resource="http://www.w3.org/2000/01/rdf-schema#Literal"/>
            </owl:Restriction>
        </rdfs:subClassOf>
        <rdfs:comment xml:lang="it">Questa classe rappresenta informazioni sul preparato (es. vetrini, provette, risultati di analisi) associato o conservato con l&apos;oggetto della scheda e non in una collezione ancillare</rdfs:comment>
        <rdfs:comment xml:lang="en">This class represents information about the preparation, associated to the specimen and not belonging to an ancillary collection</rdfs:comment>
        <rdfs:isDefinedBy rdf:resource="https://w3id.org/arco/ontology/movable-property"/>
        <rdfs:label xml:lang="en">Preparation</rdfs:label>
        <rdfs:label xml:lang="it">Preparato</rdfs:label>
        <owl:versionInfo xml:lang="it">instabile</owl:versionInfo>
        <owl:versionInfo xml:lang="en">unstable</owl:versionInfo>
        <a-cat:iccdNormTag>ICCD Normativa BNB: DB/DBR</a-cat:iccdNormTag>
    </owl:Class>
    


    <!-- https://w3id.org/arco/ontology/movable-property/PreparationType -->

    <owl:Class rdf:about="https://w3id.org/arco/ontology/movable-property/PreparationType">
        <rdfs:subClassOf rdf:resource="https://w3id.org/arco/ontology/core/Type"/>
        <rdfs:comment xml:lang="it">Questa classe rappresenta il tipo di preparato</rdfs:comment>
        <rdfs:comment xml:lang="en">This class represents the type of te preparation</rdfs:comment>
        <rdfs:isDefinedBy rdf:resource="https://w3id.org/arco/ontology/movable-property"/>
        <rdfs:label xml:lang="en">Preparation type</rdfs:label>
        <rdfs:label xml:lang="it">Tipo di preparato</rdfs:label>
        <owl:versionInfo xml:lang="it">instabile</owl:versionInfo>
        <owl:versionInfo xml:lang="en">unstable</owl:versionInfo>
        <a-cat:iccdNormTag>ICCD Normativa BNB: DB/DBR/DBRT</a-cat:iccdNormTag>
    </owl:Class>
    


    <!-- https://w3id.org/arco/ontology/movable-property/PreservationType -->

    <owl:Class rdf:about="https://w3id.org/arco/ontology/movable-property/PreservationType">
        <rdfs:subClassOf rdf:resource="https://w3id.org/arco/ontology/core/Type"/>
        <rdfs:comment xml:lang="it">Questa classe rappresenta il tipo di conservazione di un campione</rdfs:comment>
        <rdfs:comment xml:lang="en">This class represents the preparation type of a sample</rdfs:comment>
        <rdfs:isDefinedBy rdf:resource="https://w3id.org/arco/ontology/movable-property"/>
        <rdfs:label xml:lang="en">Preservation type</rdfs:label>
        <rdfs:label xml:lang="it">Tipo di conservazione</rdfs:label>
        <a-cat:iccdNormTag xml:lang="en">Normativa ICCD BNB: DB/DBC/DBCX</a-cat:iccdNormTag>
    </owl:Class>
    


    <!-- https://w3id.org/arco/ontology/movable-property/Sample -->

    <owl:Class rdf:about="https://w3id.org/arco/ontology/movable-property/Sample">
        <rdfs:subClassOf rdf:resource="https://w3id.org/italia/onto/l0/Object"/>
        <rdfs:subClassOf>
            <owl:Restriction>
                <owl:onProperty rdf:resource="https://w3id.org/arco/ontology/movable-property/isRelatedSampleOf"/>
                <owl:someValuesFrom rdf:resource="http://dati.beniculturali.it/cis/CulturalEntity"/>
            </owl:Restriction>
        </rdfs:subClassOf>
        <rdfs:subClassOf>
            <owl:Restriction>
                <owl:onProperty rdf:resource="https://w3id.org/arco/ontology/context-description/hasAuthor"/>
                <owl:allValuesFrom rdf:resource="https://w3id.org/italia/onto/l0/Agent"/>
            </owl:Restriction>
        </rdfs:subClassOf>
        <rdfs:subClassOf>
            <owl:Restriction>
                <owl:onProperty rdf:resource="https://w3id.org/arco/ontology/movable-property/manufacturingDate"/>
                <owl:allValuesFrom rdf:resource="http://www.w3.org/2000/01/rdf-schema#Literal"/>
            </owl:Restriction>
        </rdfs:subClassOf>
        <rdfs:subClassOf>
            <owl:Restriction>
                <owl:onProperty rdf:resource="https://w3id.org/arco/ontology/movable-property/sampleLocation"/>
                <owl:allValuesFrom rdf:resource="http://www.w3.org/2000/01/rdf-schema#Literal"/>
            </owl:Restriction>
        </rdfs:subClassOf>
        <rdfs:comment xml:lang="it">Questa classe rappresenta il reperto appartenente alle collezioni ancillari</rdfs:comment>
        <rdfs:comment xml:lang="en">This class represents a sample belonging to ancillar collections</rdfs:comment>
        <rdfs:isDefinedBy rdf:resource="https://w3id.org/arco/ontology/movable-property"/>
        <rdfs:label xml:lang="it">Reperto di collezione ancillare</rdfs:label>
        <rdfs:label xml:lang="en">Sample</rdfs:label>
        <owl:versionInfo xml:lang="it">instabile</owl:versionInfo>
        <owl:versionInfo xml:lang="en">unstable</owl:versionInfo>
    </owl:Class>
    


    <!-- https://w3id.org/arco/ontology/movable-property/SampleForm -->

    <owl:Class rdf:about="https://w3id.org/arco/ontology/movable-property/SampleForm">
        <rdfs:subClassOf rdf:resource="https://w3id.org/italia/onto/l0/Characteristic"/>
        <rdfs:subClassOf>
            <owl:Restriction>
                <owl:onProperty rdf:resource="https://w3id.org/arco/ontology/movable-property/isSampleFormOf"/>
                <owl:someValuesFrom rdf:resource="https://w3id.org/arco/ontology/movable-property/WoodSample"/>
            </owl:Restriction>
        </rdfs:subClassOf>
        <rdfs:comment xml:lang="it">Questa classe rappresenta la forma del reperto</rdfs:comment>
        <rdfs:comment xml:lang="en">This class represents the form of the sample</rdfs:comment>
        <rdfs:label xml:lang="it">Forma del reperto</rdfs:label>
        <rdfs:label xml:lang="en">Sample form</rdfs:label>
        <owl:versionInfo xml:lang="it">instabile</owl:versionInfo>
        <owl:versionInfo xml:lang="en">unstable</owl:versionInfo>
        <a-cat:iccdNormTag xml:lang="en">Normativa ICCD BNB: DB/DBX/DBXX</a-cat:iccdNormTag>
    </owl:Class>
    


    <!-- https://w3id.org/arco/ontology/movable-property/SeedSample -->

    <owl:Class rdf:about="https://w3id.org/arco/ontology/movable-property/SeedSample">
        <rdfs:subClassOf rdf:resource="https://w3id.org/arco/ontology/movable-property/Sample"/>
        <rdfs:comment xml:lang="it">Questa classe rappresenta un reperto spermologico (semi)</rdfs:comment>
        <rdfs:comment xml:lang="en">This class represents a sample from the seed collection</rdfs:comment>
        <rdfs:isDefinedBy rdf:resource="https://w3id.org/arco/ontology/movable-property"/>
        <rdfs:label xml:lang="it">Reperto spermologico</rdfs:label>
        <rdfs:label xml:lang="en">Seed  sample</rdfs:label>
        <owl:versionInfo xml:lang="it">instabile</owl:versionInfo>
        <owl:versionInfo xml:lang="en">unstable</owl:versionInfo>
        <a-cat:iccdNormTag>ICCD Normativa BNB: DB/DBS</a-cat:iccdNormTag>
    </owl:Class>
    


    <!-- https://w3id.org/arco/ontology/movable-property/ShadeTolerance -->

    <owl:Class rdf:about="https://w3id.org/arco/ontology/movable-property/ShadeTolerance">
        <rdfs:subClassOf rdf:resource="https://w3id.org/italia/onto/l0/Characteristic"/>
        <rdfs:subClassOf>
            <owl:Restriction>
                <owl:onProperty rdf:resource="https://w3id.org/arco/ontology/movable-property/isShadeToleranceOf"/>
                <owl:someValuesFrom rdf:resource="https://w3id.org/arco/ontology/movable-property/CollectingSite"/>
            </owl:Restriction>
        </rdfs:subClassOf>
        <rdfs:comment xml:lang="it">Questa classe rappresenta la tolleranza alla luminosità del popolamento ove il campione è stato raccolto</rdfs:comment>
        <rdfs:comment xml:lang="en">This class represents the shade tolerance of the individuals in the collecting location</rdfs:comment>
        <rdfs:isDefinedBy rdf:resource="https://w3id.org/arco/ontology/movable-property"/>
        <rdfs:label xml:lang="en">Shade tolerance</rdfs:label>
        <rdfs:label xml:lang="it">Situazione luminosa</rdfs:label>
        <owl:versionInfo xml:lang="it">instabile</owl:versionInfo>
        <owl:versionInfo xml:lang="en">unstable</owl:versionInfo>
        <core:iccdNormTag xml:lang="en">ICCD Normativa BNB: LR/LRI/LRIS</core:iccdNormTag>
    </owl:Class>
    


    <!-- https://w3id.org/arco/ontology/movable-property/Species -->

    <owl:Class rdf:about="https://w3id.org/arco/ontology/movable-property/Species">
        <rdfs:subClassOf rdf:resource="https://w3id.org/arco/ontology/movable-property/BiologicalTaxon"/>
        <rdfs:subClassOf>
            <owl:Restriction>
                <owl:onProperty rdf:resource="https://w3id.org/arco/ontology/movable-property/hasDirectHigherRank"/>
                <owl:allValuesFrom rdf:resource="https://w3id.org/arco/ontology/movable-property/Genus"/>
            </owl:Restriction>
        </rdfs:subClassOf>
        <rdfs:subClassOf>
            <owl:Restriction>
                <owl:onProperty rdf:resource="https://w3id.org/arco/ontology/movable-property/hasDirectLowerRank"/>
                <owl:allValuesFrom rdf:resource="https://w3id.org/arco/ontology/movable-property/Subspecies"/>
            </owl:Restriction>
        </rdfs:subClassOf>
        <rdfs:subClassOf>
            <owl:Restriction>
                <owl:onProperty rdf:resource="https://w3id.org/arco/ontology/movable-property/hasHigherRank"/>
                <owl:allValuesFrom>
                    <owl:Class>
                        <owl:complementOf>
                            <owl:Class>
                                <owl:unionOf rdf:parseType="Collection">
                                    <rdf:Description rdf:about="https://w3id.org/arco/ontology/movable-property/BotanicalForm"/>
                                    <rdf:Description rdf:about="https://w3id.org/arco/ontology/movable-property/Cultivar"/>
                                    <rdf:Description rdf:about="https://w3id.org/arco/ontology/movable-property/Species"/>
                                    <rdf:Description rdf:about="https://w3id.org/arco/ontology/movable-property/Subspecies"/>
                                    <rdf:Description rdf:about="https://w3id.org/arco/ontology/movable-property/Variety"/>
                                </owl:unionOf>
                            </owl:Class>
                        </owl:complementOf>
                    </owl:Class>
                </owl:allValuesFrom>
            </owl:Restriction>
        </rdfs:subClassOf>
        <rdfs:subClassOf>
            <owl:Restriction>
                <owl:onProperty rdf:resource="https://w3id.org/arco/ontology/movable-property/hasLowerRank"/>
                <owl:allValuesFrom>
                    <owl:Class>
                        <owl:unionOf rdf:parseType="Collection">
                            <rdf:Description rdf:about="https://w3id.org/arco/ontology/movable-property/BotanicalForm"/>
                            <rdf:Description rdf:about="https://w3id.org/arco/ontology/movable-property/Cultivar"/>
                            <rdf:Description rdf:about="https://w3id.org/arco/ontology/movable-property/Subspecies"/>
                            <rdf:Description rdf:about="https://w3id.org/arco/ontology/movable-property/Variety"/>
                        </owl:unionOf>
                    </owl:Class>
                </owl:allValuesFrom>
            </owl:Restriction>
        </rdfs:subClassOf>
        <rdfs:comment xml:lang="it">Questa classe rappresenta uno dei livelli di classificazione di una tassonomia biologica, ovvero la specie.</rdfs:comment>
        <rdfs:comment xml:lang="en">This class represents one level of a biological taxon, the species.</rdfs:comment>
        <rdfs:isDefinedBy rdf:resource="https://w3di.org/arco/ontology/movable-property/"/>
        <rdfs:label xml:lang="it">Specie</rdfs:label>
        <rdfs:label xml:lang="en">Species</rdfs:label>
        <owl:versionInfo xml:lang="it">instabile</owl:versionInfo>
        <owl:versionInfo xml:lang="en">unstable</owl:versionInfo>
        <a-cat:iccdNormTag>ICCD Normativa AT: OG/OGS/OGSN. - Normativa BNB: RB/RBN/RBNB; SB/NAA/NAAB; SB/NAT/NATB</a-cat:iccdNormTag>
    </owl:Class>
    


    <!-- https://w3id.org/arco/ontology/movable-property/SpecimenHarvesting -->

    <owl:Class rdf:about="https://w3id.org/arco/ontology/movable-property/SpecimenHarvesting">
        <rdfs:subClassOf rdf:resource="https://w3id.org/arco/ontology/core/TimeIndexedEvent"/>
        <rdfs:subClassOf>
            <owl:Restriction>
                <owl:onProperty rdf:resource="https://w3id.org/arco/ontology/core/involvesAgent"/>
                <owl:allValuesFrom rdf:resource="https://w3id.org/italia/onto/l0/Agent"/>
            </owl:Restriction>
        </rdfs:subClassOf>
        <rdfs:subClassOf>
            <owl:Restriction>
                <owl:onProperty rdf:resource="https://w3id.org/arco/ontology/movable-property/hasCollectingSite"/>
                <owl:allValuesFrom rdf:resource="https://w3id.org/arco/ontology/movable-property/CollectingSite"/>
            </owl:Restriction>
        </rdfs:subClassOf>
        <rdfs:subClassOf>
            <owl:Restriction>
                <owl:onProperty rdf:resource="https://w3id.org/italia/onto/TI/atTime"/>
                <owl:allValuesFrom rdf:resource="https://w3id.org/italia/onto/TI/TimeInterval"/>
            </owl:Restriction>
        </rdfs:subClassOf>
        <rdfs:comment xml:lang="it">Questa classe rappresenta l&apos;informazione sulla raccolta del campione</rdfs:comment>
        <rdfs:comment xml:lang="en">This class represents the information about the harvesting of the specimen</rdfs:comment>
        <rdfs:label xml:lang="it">Raccolta del campione</rdfs:label>
        <rdfs:label xml:lang="en">Specimen harvesting</rdfs:label>
        <owl:versionInfo xml:lang="it">instabile</owl:versionInfo>
        <owl:versionInfo xml:lang="en">unstable</owl:versionInfo>
    </owl:Class>
    


    <!-- https://w3id.org/arco/ontology/movable-property/Subspecies -->

    <owl:Class rdf:about="https://w3id.org/arco/ontology/movable-property/Subspecies">
        <rdfs:subClassOf rdf:resource="https://w3id.org/arco/ontology/movable-property/BiologicalTaxon"/>
        <rdfs:subClassOf>
            <owl:Restriction>
                <owl:onProperty rdf:resource="https://w3id.org/arco/ontology/movable-property/hasDirectHigherRank"/>
                <owl:allValuesFrom rdf:resource="https://w3id.org/arco/ontology/movable-property/Species"/>
            </owl:Restriction>
        </rdfs:subClassOf>
        <rdfs:subClassOf>
            <owl:Restriction>
                <owl:onProperty rdf:resource="https://w3id.org/arco/ontology/movable-property/hasHigherRank"/>
                <owl:allValuesFrom>
                    <owl:Class>
                        <owl:complementOf>
                            <owl:Class>
                                <owl:unionOf rdf:parseType="Collection">
                                    <rdf:Description rdf:about="https://w3id.org/arco/ontology/movable-property/BotanicalForm"/>
                                    <rdf:Description rdf:about="https://w3id.org/arco/ontology/movable-property/Cultivar"/>
                                    <rdf:Description rdf:about="https://w3id.org/arco/ontology/movable-property/Subspecies"/>
                                    <rdf:Description rdf:about="https://w3id.org/arco/ontology/movable-property/Variety"/>
                                </owl:unionOf>
                            </owl:Class>
                        </owl:complementOf>
                    </owl:Class>
                </owl:allValuesFrom>
            </owl:Restriction>
        </rdfs:subClassOf>
        <rdfs:subClassOf>
            <owl:Restriction>
                <owl:onProperty rdf:resource="https://w3id.org/arco/ontology/movable-property/hasLowerRank"/>
                <owl:allValuesFrom>
                    <owl:Class>
                        <owl:unionOf rdf:parseType="Collection">
                            <rdf:Description rdf:about="https://w3id.org/arco/ontology/movable-property/BotanicalForm"/>
                            <rdf:Description rdf:about="https://w3id.org/arco/ontology/movable-property/Cultivar"/>
                            <rdf:Description rdf:about="https://w3id.org/arco/ontology/movable-property/Variety"/>
                        </owl:unionOf>
                    </owl:Class>
                </owl:allValuesFrom>
            </owl:Restriction>
        </rdfs:subClassOf>
        <rdfs:comment xml:lang="it">Questa classe rappresenta uno dei livelli di classificazione di una tassonomia biologica, ovvero la sottospecie.</rdfs:comment>
        <rdfs:comment xml:lang="en">This class represents one level of a biological taxon, the subspecies.</rdfs:comment>
        <rdfs:isDefinedBy rdf:resource="https://w3di.org/arco/ontology/movable-property/"/>
        <rdfs:label xml:lang="it">Sottospecie</rdfs:label>
        <rdfs:label xml:lang="en">Subspecies</rdfs:label>
        <owl:versionInfo xml:lang="it">instabile</owl:versionInfo>
        <owl:versionInfo xml:lang="en">unstable</owl:versionInfo>
        <a-cat:iccdNormTag>ICCD Normativa AT: OG/OGS/OGST. -  Normativa BNB: RB/RBN/RBND; SB/NAA/NAAD; SB/NAT/NATD</a-cat:iccdNormTag>
    </owl:Class>
    


    <!-- https://w3id.org/arco/ontology/movable-property/Substrate -->

    <owl:Class rdf:about="https://w3id.org/arco/ontology/movable-property/Substrate">
        <rdfs:subClassOf rdf:resource="https://w3id.org/italia/onto/l0/Object"/>
        <rdfs:subClassOf>
            <owl:Restriction>
                <owl:onProperty rdf:resource="https://w3id.org/arco/ontology/core/hasType"/>
                <owl:allValuesFrom rdf:resource="https://w3id.org/arco/ontology/movable-property/SubstrateType"/>
            </owl:Restriction>
        </rdfs:subClassOf>
        <rdfs:subClassOf>
            <owl:Restriction>
                <owl:onProperty rdf:resource="https://w3id.org/arco/ontology/movable-property/hasIncline"/>
                <owl:allValuesFrom rdf:resource="https://w3id.org/arco/ontology/movable-property/Incline"/>
            </owl:Restriction>
        </rdfs:subClassOf>
        <rdfs:subClassOf>
            <owl:Restriction>
                <owl:onProperty rdf:resource="https://w3id.org/arco/ontology/movable-property/hasNaturalEnvironment"/>
                <owl:allValuesFrom rdf:resource="https://w3id.org/arco/ontology/movable-property/NaturalEnvironment"/>
            </owl:Restriction>
        </rdfs:subClassOf>
        <rdfs:comment xml:lang="it">Questa classe rappresenta substrato specifico sul quale è stato raccolto il campione</rdfs:comment>
        <rdfs:comment xml:lang="en">This class represents  the specific substrate where the specimen was collected</rdfs:comment>
        <rdfs:isDefinedBy rdf:resource="https://w3id.org/arco/ontology/movable-property"/>
        <rdfs:label xml:lang="en">Substrate</rdfs:label>
        <rdfs:label xml:lang="it">Substrato</rdfs:label>
        <owl:versionInfo xml:lang="it">instabile</owl:versionInfo>
        <owl:versionInfo xml:lang="en">unstable</owl:versionInfo>
        <a-cat:iccdNormTag>ICCD Normativa BNB: LR/LRI/LRIR</a-cat:iccdNormTag>
    </owl:Class>
    


    <!-- https://w3id.org/arco/ontology/movable-property/SubstrateType -->

    <owl:Class rdf:about="https://w3id.org/arco/ontology/movable-property/SubstrateType">
        <rdfs:subClassOf rdf:resource="https://w3id.org/arco/ontology/core/Type"/>
        <rdfs:comment xml:lang="it">Questa classe rappresenta la categoria cui appartiene il substrato su cui è stato raccolto il campione</rdfs:comment>
        <rdfs:comment xml:lang="en">This class represents the category of the substrate where the specimen was collected</rdfs:comment>
        <rdfs:isDefinedBy rdf:resource="https://w3id.org/arco/ontology/movable-property"/>
        <rdfs:label xml:lang="en">Substrate Type</rdfs:label>
        <rdfs:label xml:lang="it">Tipo di substrato</rdfs:label>
        <owl:versionInfo xml:lang="it">instabile</owl:versionInfo>
        <owl:versionInfo xml:lang="en">unstable</owl:versionInfo>
        <a-cat:iccdNormTag>ICCD Normativa BNB: LR/LRI/LRIJ</a-cat:iccdNormTag>
    </owl:Class>
    


    <!-- https://w3id.org/arco/ontology/movable-property/TypeOfTypeSpecimen -->

    <owl:Class rdf:about="https://w3id.org/arco/ontology/movable-property/TypeOfTypeSpecimen">
        <rdfs:subClassOf rdf:resource="https://w3id.org/arco/ontology/core/Type"/>
        <rdfs:comment xml:lang="it">Questa classe rappresenta il tipo del campione che è servito a denominare un taxon specifico o infraspecifico</rdfs:comment>
        <rdfs:comment xml:lang="en">This class represents the type of a specimen used to produce a specific taxon</rdfs:comment>
        <rdfs:isDefinedBy rdf:resource="https://w3id.org/arco/ontology/movable-property"/>
        <rdfs:label xml:lang="it">Tipo di campione</rdfs:label>
        <rdfs:label xml:lang="en">Type of specimen</rdfs:label>
        <owl:versionInfo xml:lang="it">instabile</owl:versionInfo>
        <owl:versionInfo xml:lang="en">unstable</owl:versionInfo>
        <a-cat:iccdNormTag>ICCD Normativa BNB: SB/TBI/TBIT</a-cat:iccdNormTag>
    </owl:Class>
    


    <!-- https://w3id.org/arco/ontology/movable-property/TypeSpecimenIdentification -->

    <owl:Class rdf:about="https://w3id.org/arco/ontology/movable-property/TypeSpecimenIdentification">
        <rdfs:subClassOf rdf:resource="https://w3id.org/arco/ontology/core/Situation"/>
        <rdfs:subClassOf>
            <owl:Restriction>
                <owl:onProperty rdf:resource="https://w3id.org/arco/ontology/context-description/hasBibliography"/>
                <owl:allValuesFrom rdf:resource="https://w3id.org/arco/ontology/context-description/Bibliography"/>
            </owl:Restriction>
        </rdfs:subClassOf>
        <rdfs:subClassOf>
            <owl:Restriction>
                <owl:onProperty rdf:resource="https://w3id.org/arco/ontology/core/hasConsequence"/>
                <owl:allValuesFrom rdf:resource="https://w3id.org/arco/ontology/core/ClassificationInTime"/>
            </owl:Restriction>
        </rdfs:subClassOf>
        <rdfs:subClassOf>
            <owl:Restriction>
                <owl:onProperty rdf:resource="https://w3id.org/arco/ontology/core/hasType"/>
                <owl:allValuesFrom rdf:resource="https://w3id.org/arco/ontology/movable-property/TypeOfTypeSpecimen"/>
            </owl:Restriction>
        </rdfs:subClassOf>
        <rdfs:comment xml:lang="it">Questa classe rappresenta l&apos;identificazione di un campione vegetale che è servito a produrne la prima descrizione e a denominare un taxon specifico o infraspecifico considerato nuovo.</rdfs:comment>
        <rdfs:comment xml:lang="en">This class represents the identification of a specimen used to produce the first description an to produce the new taxon</rdfs:comment>
        <rdfs:isDefinedBy rdf:resource="https://w3id.org/arco/ontology/movable-property"/>
        <rdfs:label xml:lang="it">Identificazione del tipo nomenclaturale</rdfs:label>
        <rdfs:label xml:lang="en">Type specimen identification</rdfs:label>
        <owl:versionInfo xml:lang="it">instabile</owl:versionInfo>
        <owl:versionInfo xml:lang="en">unstable</owl:versionInfo>
        <a-cat:iccdNormTag>ICCD Normativa BNB: SB/TBI</a-cat:iccdNormTag>
    </owl:Class>
    


    <!-- https://w3id.org/arco/ontology/movable-property/Variety -->

    <owl:Class rdf:about="https://w3id.org/arco/ontology/movable-property/Variety">
        <rdfs:subClassOf rdf:resource="https://w3id.org/arco/ontology/movable-property/BiologicalTaxon"/>
        <rdfs:subClassOf>
            <owl:Restriction>
                <owl:onProperty rdf:resource="https://w3id.org/arco/ontology/movable-property/hasHigherRank"/>
                <owl:allValuesFrom>
                    <owl:Class>
                        <owl:complementOf>
                            <owl:Class>
                                <owl:unionOf rdf:parseType="Collection">
                                    <rdf:Description rdf:about="https://w3id.org/arco/ontology/movable-property/BotanicalForm"/>
                                    <rdf:Description rdf:about="https://w3id.org/arco/ontology/movable-property/Cultivar"/>
                                    <rdf:Description rdf:about="https://w3id.org/arco/ontology/movable-property/Variety"/>
                                </owl:unionOf>
                            </owl:Class>
                        </owl:complementOf>
                    </owl:Class>
                </owl:allValuesFrom>
            </owl:Restriction>
        </rdfs:subClassOf>
        <rdfs:comment xml:lang="it">Questa classe rappresenta uno dei livelli di classificazione di una tassonomia biologica, ovvero la varietà.</rdfs:comment>
        <rdfs:comment xml:lang="en">This class represents one level of a biological taxon, the variety</rdfs:comment>
        <rdfs:isDefinedBy rdf:resource="https://w3di.org/arco/ontology/movable-property/"/>
        <rdfs:label xml:lang="en">Variety</rdfs:label>
        <rdfs:label xml:lang="it">Varietà</rdfs:label>
        <owl:versionInfo xml:lang="it">instabile</owl:versionInfo>
        <owl:versionInfo xml:lang="en">unstable</owl:versionInfo>
        <a-cat:iccdNormTag>ICCD Normativa BNB: RB/RBN/RBNF; SB/NAA/NAAF; SB/NAT/NATF</a-cat:iccdNormTag>
    </owl:Class>
    


    <!-- https://w3id.org/arco/ontology/movable-property/WoodSample -->

    <owl:Class rdf:about="https://w3id.org/arco/ontology/movable-property/WoodSample">
        <rdfs:subClassOf rdf:resource="https://w3id.org/arco/ontology/movable-property/Sample"/>
        <rdfs:subClassOf>
            <owl:Restriction>
                <owl:onProperty rdf:resource="https://w3id.org/arco/ontology/denotative-description/hasMeasurementCollection"/>
                <owl:allValuesFrom rdf:resource="https://w3id.org/arco/ontology/denotative-description/MeasurementCollection"/>
            </owl:Restriction>
        </rdfs:subClassOf>
        <rdfs:subClassOf>
            <owl:Restriction>
                <owl:onProperty rdf:resource="https://w3id.org/arco/ontology/movable-property/hasSampleForm"/>
                <owl:allValuesFrom rdf:resource="https://w3id.org/arco/ontology/movable-property/SampleForm"/>
            </owl:Restriction>
        </rdfs:subClassOf>
        <rdfs:comment xml:lang="it">Questa classe rappresenta un reperto xilologico (legni)</rdfs:comment>
        <rdfs:comment xml:lang="en">This class represents sample from the wood collection</rdfs:comment>
        <rdfs:isDefinedBy rdf:resource="https://w3id.org/arco/ontology/movable-property"/>
        <rdfs:label xml:lang="it">Reperto xilologico</rdfs:label>
        <rdfs:label xml:lang="en">Wood sample</rdfs:label>
        <owl:versionInfo xml:lang="it">instabile</owl:versionInfo>
        <owl:versionInfo xml:lang="en">unstable</owl:versionInfo>
        <a-cat:iccdNormTag>ICCD Normativa BNB: DB/DBX</a-cat:iccdNormTag>
    </owl:Class>
    


    <!-- https://w3id.org/italia/onto/l0/Characteristic -->

    <owl:Class rdf:about="https://w3id.org/italia/onto/l0/Characteristic"/>
    


    <!-- https://w3id.org/italia/onto/l0/Object -->

    <owl:Class rdf:about="https://w3id.org/italia/onto/l0/Object"/>
    


    <!-- 
    ///////////////////////////////////////////////////////////////////////////////////////
    //
    // General axioms
    //
    ///////////////////////////////////////////////////////////////////////////////////////
     -->

    <rdf:Description>
        <rdf:type rdf:resource="http://www.w3.org/2002/07/owl#AllDisjointClasses"/>
        <owl:members rdf:parseType="Collection">
            <rdf:Description rdf:about="https://w3id.org/arco/ontology/movable-property/Class"/>
            <rdf:Description rdf:about="https://w3id.org/arco/ontology/movable-property/Family"/>
            <rdf:Description rdf:about="https://w3id.org/arco/ontology/movable-property/Genus"/>
            <rdf:Description rdf:about="https://w3id.org/arco/ontology/movable-property/Kingdom"/>
            <rdf:Description rdf:about="https://w3id.org/arco/ontology/movable-property/Order"/>
            <rdf:Description rdf:about="https://w3id.org/arco/ontology/movable-property/Phylum"/>
            <rdf:Description rdf:about="https://w3id.org/arco/ontology/movable-property/Species"/>
            <rdf:Description rdf:about="https://w3id.org/arco/ontology/movable-property/Subspecies"/>
            <rdf:Description rdf:about="https://w3id.org/arco/ontology/movable-property/Variety"/>
        </owl:members>
    </rdf:Description>
</rdf:RDF>



<!-- Generated by the OWL API (version 4.5.9.2019-02-01T07:24:44Z) https://github.com/owlcs/owlapi -->

