<?xml version="1.0"?>
<rdf:RDF xmlns="https://w3id.org/arco/ontology/arco/"
     xml:base="https://w3id.org/arco/ontology/arco/"
     xmlns:dc="http://purl.org/dc/elements/1.1/"
     xmlns:l0="https://w3id.org/italia/onto/l0/"
     xmlns:ns="http://www.w3.org/2006/vcard/ns#"
     xmlns:CLV="https://w3id.org/italia/onto/CLV/"
     xmlns:cis="http://dati.beniculturali.it/cis/"
     xmlns:owl="http://www.w3.org/2002/07/owl#"
     xmlns:rdf="http://www.w3.org/1999/02/22-rdf-syntax-ns#"
     xmlns:xml="http://www.w3.org/XML/1998/namespace"
     xmlns:xsd="http://www.w3.org/2001/XMLSchema#"
     xmlns:a-cd="https://w3id.org/arco/ontology/context-description/"
     xmlns:a-ce="https://w3id.org/arco/ontology/cultural-event/"
     xmlns:a-dd="https://w3id.org/arco/ontology/denotative-description/"
     xmlns:adms="https://w3id.org/italia/onto/ADMS/"
     xmlns:arco="https://w3id.org/arco/ontology/arco/"
     xmlns:core="https://w3id.org/arco/ontology/core/"
     xmlns:dcat="http://www.w3.org/ns/dcat#"
     xmlns:foaf="http://xmlns.com/foaf/0.1/"
     xmlns:opla="http://ontologydesignpatterns.org/opla/"
     xmlns:prov="http://www.w3.org/ns/prov#"
     xmlns:rdfs="http://www.w3.org/2000/01/rdf-schema#"
     xmlns:a-cat="https://w3id.org/arco/ontology/catalogue/"
     xmlns:a-loc="https://w3id.org/arco/ontology/location/"
     xmlns:opla1="http://www.ontologydesignpatterns.org/opla/"
     xmlns:terms="http://purl.org/dc/terms/"
     xmlns:roapit="https://w3id.org/italia/onto/RO/"
     xmlns:tiapit="https://w3id.org/italia/onto/TI/">
    <owl:Ontology rdf:about="https://w3id.org/arco/ontology/arco">
        <owl:versionIRI rdf:resource="https://w3id.org/arco/ontology/arco/1.2"/>
        <owl:imports rdf:resource="https://w3id.org/arco/ontology/catalogue/1.2"/>
        <owl:imports rdf:resource="https://w3id.org/arco/ontology/cataloguing-campaign/0.1"/>
        <owl:imports rdf:resource="https://w3id.org/arco/ontology/context-description/1.2"/>
        <owl:imports rdf:resource="https://w3id.org/arco/ontology/core/1.2"/>
        <owl:imports rdf:resource="https://w3id.org/arco/ontology/cultural-event/1.1"/>
        <owl:imports rdf:resource="https://w3id.org/arco/ontology/denotative-description/1.2"/>
        <owl:imports rdf:resource="https://w3id.org/arco/ontology/immovable-property/0.2"/>
        <owl:imports rdf:resource="https://w3id.org/arco/ontology/location/1.2"/>
        <owl:imports rdf:resource="https://w3id.org/arco/ontology/movable-property/0.2"/>
        <opla:reusesPatternAsTemplate rdf:resource="http://www.ontologydesignpatterns.org/cp/owl/classification.owl"/>
        <opla:reusesPatternAsTemplate rdf:resource="http://www.ontologydesignpatterns.org/cp/owl/collectionentity.owl"/>
        <opla:reusesPatternAsTemplate rdf:resource="http://www.ontologydesignpatterns.org/cp/owl/componency.owl"/>
        <opla:reusesPatternAsTemplate rdf:resource="http://www.ontologydesignpatterns.org/cp/owl/partof.owl"/>
        <opla:reusesPatternAsTemplate rdf:resource="http://www.ontologydesignpatterns.org/cp/owl/situation.owl"/>
        <dc:creator>Aldo Gangemi (ISTC-CNR, STLab)</dc:creator>
        <dc:creator>Andrea Nuzzolese (ISTC-CNR, STLab)</dc:creator>
        <dc:creator>Chiara Veninata (MiBAC, ICCD)</dc:creator>
        <dc:creator>Ludovica Marinucci (ISTC-CNR, STLab)</dc:creator>
        <dc:creator>Luigi Asprino (ISTC-CNR, STLab)</dc:creator>
        <dc:creator>Margherita Porena (ISTC-CNR, STLab)</dc:creator>
        <dc:creator>Maria Letizia Mancinelli (MiBAC, ICCD)</dc:creator>
        <dc:creator>Valentina Carriero (ISTC-CNR, STLab)</dc:creator>
        <dc:creator>Valentina Presutti (ISTC-CNR, STLab)</dc:creator>
        <dc:description xml:lang="it">Questo è il modulo centrale della rete di ontologie di ArCo - Architettura della Conoscenza. Qui si modellano informazioni, relative al dominio dei beni culturali, considerate top-level. Vengono importati tutti gli altri moduli della rete.</dc:description>
        <dc:description xml:lang="en">The ArCo module is the root of the network ArCo - Architecture of Knowledge. It imports all the other modules and models top-level distinctions from the cultural heritage domain.</dc:description>
        <dc:language rdf:resource="http://publications.europa.eu/resource/authority/language/ENG"/>
        <dc:language rdf:resource="http://publications.europa.eu/resource/authority/language/ITA"/>
        <dc:title xml:lang="en">ArCo Ontology (ArCo network)</dc:title>
        <dc:title xml:lang="it">Ontologia ArCo (ArCo network)</dc:title>
        <terms:issued>2019-03-05</terms:issued>
        <terms:license rdf:resource="https://creativecommons.org/licenses/by-sa/4.0/"/>
        <terms:license rdf:resource="https://w3id.org/italia/controlled-vocabulary/licences/A31_CCBYSA40"/>
        <terms:modified>2020-03-27</terms:modified>
        <rdfs:comment xml:lang="it">Questo è il modulo centrale della rete di ontologie di ArCo - Architettura della Conoscenza. Qui si modellano informazioni, relative al dominio dei beni culturali, considerate top-level. Vengono importati tutti gli altri moduli della rete.
In questo modulo sono riusati come template i seguenti Ontology Design Patterns:
- http://www.ontologydesignpatterns.org/cp/owl/classification.owl
- http://www.ontologydesignpatterns.org/cp/owl/collectionentity.owl
- http://www.ontologydesignpatterns.org/cp/owl/componency.owl
- http://www.ontologydesignpatterns.org/cp/owl/partof.owl
- http://www.ontologydesignpatterns.org/cp/owl/situation.owl</rdfs:comment>
        <rdfs:comment xml:lang="en">The ArCo module is the root of the network ArCo - Architecture of Knowledge. It imports all the other modules and models top-level distinctions from the cultural heritage domain.
In this module the following Ontology Design Patterns have been used:
- http://www.ontologydesignpatterns.org/cp/owl/classification.owl
- http://www.ontologydesignpatterns.org/cp/owl/collectionentity.owl
- http://www.ontologydesignpatterns.org/cp/owl/componency.owl
- http://www.ontologydesignpatterns.org/cp/owl/partof.owl
- http://www.ontologydesignpatterns.org/cp/owl/situation.owl</rdfs:comment>
        <rdfs:label xml:lang="en">ArCo Ontology (ArCo network)</rdfs:label>
        <rdfs:label xml:lang="it">Ontologia ArCo (ArCo network)</rdfs:label>
        <owl:versionInfo xml:lang="en">Version 1.2</owl:versionInfo>
        <owl:versionInfo xml:lang="it">Versione 1.2</owl:versionInfo>
    </owl:Ontology>
    


    <!-- 
    ///////////////////////////////////////////////////////////////////////////////////////
    //
    // Annotation properties
    //
    ///////////////////////////////////////////////////////////////////////////////////////
     -->

    


    <!-- http://ontologydesignpatterns.org/opla/isNativeTo -->

    <owl:AnnotationProperty rdf:about="http://ontologydesignpatterns.org/opla/isNativeTo"/>
    


    <!-- http://ontologydesignpatterns.org/opla/reusesPatternAsTemplate -->

    <owl:AnnotationProperty rdf:about="http://ontologydesignpatterns.org/opla/reusesPatternAsTemplate"/>
    


    <!-- http://purl.org/dc/elements/1.1/language -->

    <owl:AnnotationProperty rdf:about="http://purl.org/dc/elements/1.1/language"/>
    


    <!-- http://purl.org/dc/elements/1.1/title -->

    <owl:AnnotationProperty rdf:about="http://purl.org/dc/elements/1.1/title"/>
    


    <!-- http://purl.org/dc/terms/issued -->

    <owl:AnnotationProperty rdf:about="http://purl.org/dc/terms/issued"/>
    


    <!-- http://purl.org/dc/terms/license -->

    <owl:AnnotationProperty rdf:about="http://purl.org/dc/terms/license"/>
    


    <!-- http://purl.org/dc/terms/modified -->

    <owl:AnnotationProperty rdf:about="http://purl.org/dc/terms/modified"/>
    


    <!-- https://w3id.org/arco/ontology/catalogue/iccdNormTag -->

    <owl:AnnotationProperty rdf:about="https://w3id.org/arco/ontology/catalogue/iccdNormTag"/>
    


    <!-- 
    ///////////////////////////////////////////////////////////////////////////////////////
    //
    // Object Properties
    //
    ///////////////////////////////////////////////////////////////////////////////////////
     -->

    


    <!-- http://dati.beniculturali.it/cis/isRelatedToRiT -->

    <owl:ObjectProperty rdf:about="http://dati.beniculturali.it/cis/isRelatedToRiT"/>
    


    <!-- https://w3id.org/arco/ontology/arco/hasAlternativeDiscipline -->

    <owl:ObjectProperty rdf:about="https://w3id.org/arco/ontology/arco/hasAlternativeDiscipline">
        <owl:inverseOf rdf:resource="https://w3id.org/arco/ontology/arco/isAlternativeDisciplineOf"/>
        <rdfs:domain rdf:resource="https://w3id.org/arco/ontology/arco/CulturalProperty"/>
        <rdfs:range rdf:resource="http://dati.beniculturali.it/cis/SubjectDiscipline"/>
        <rdfs:comment xml:lang="it">Questa proprietà permette di associare un bene culturale a discipline scientifiche, alternative a quella principale, cui fa riferimento.</rdfs:comment>
        <rdfs:comment xml:lang="en">This property relates a cultural property to a related scientific discipline, alternative to the main one.</rdfs:comment>
        <rdfs:isDefinedBy rdf:resource="https://w3id.org/arco/ontology/arco"/>
        <rdfs:label xml:lang="it">ha altra disciplina</rdfs:label>
        <rdfs:label xml:lang="en">has alternative discipline</rdfs:label>
        <owl:versionInfo xml:lang="it">stabile</owl:versionInfo>
        <owl:versionInfo xml:lang="en">stable</owl:versionInfo>
        <a-cat:iccdNormTag>ICCD Normativa PST: CT/CTA, versione 4.00: OG/CTA</a-cat:iccdNormTag>
    </owl:ObjectProperty>
    


    <!-- https://w3id.org/arco/ontology/arco/hasArchaeologicalMaterialCategory -->

    <owl:ObjectProperty rdf:about="https://w3id.org/arco/ontology/arco/hasArchaeologicalMaterialCategory">
        <rdfs:subPropertyOf rdf:resource="https://w3id.org/arco/ontology/core/hasCategory"/>
        <owl:inverseOf rdf:resource="https://w3id.org/arco/ontology/arco/isArchaeologicalMaterialCategoryOf"/>
        <rdfs:domain rdf:resource="https://w3id.org/arco/ontology/arco/ArchaeologicalMaterial"/>
        <rdfs:range rdf:resource="https://w3id.org/arco/ontology/arco/ArchaeologicalMaterialCategory"/>
        <rdfs:comment xml:lang="it">Questa proprietà collega un materiale archeologico alla sua categoria (es.: ceramiche, industria litica, intonaco, legno, etc.)</rdfs:comment>
        <rdfs:comment xml:lang="en">This property relates the archaeological material to its category (e.g.: ceramics, plaster, lithic materials, etc.)</rdfs:comment>
        <rdfs:isDefinedBy rdf:resource="https://w3id.org/arco/ontology/arco"/>
        <rdfs:label xml:lang="it">ha categoria di materiale archeologico</rdfs:label>
        <rdfs:label xml:lang="en">has archaeological material category</rdfs:label>
        <owl:versionInfo xml:lang="it">stabile</owl:versionInfo>
        <owl:versionInfo xml:lang="en">stable</owl:versionInfo>
        <a-cat:iccdNormTag>ICCD Normativa TMA: MA/MAC/MACC</a-cat:iccdNormTag>
    </owl:ObjectProperty>
    


    <!-- https://w3id.org/arco/ontology/arco/hasCartographicClassification -->

    <owl:ObjectProperty rdf:about="https://w3id.org/arco/ontology/arco/hasCartographicClassification">
        <rdfs:subPropertyOf rdf:resource="https://w3id.org/arco/ontology/core/hasClassification"/>
        <owl:inverseOf rdf:resource="https://w3id.org/arco/ontology/arco/isCartographicClassificationOf"/>
        <rdfs:domain rdf:resource="https://w3id.org/arco/ontology/arco/CulturalProperty"/>
        <rdfs:range rdf:resource="https://w3id.org/arco/ontology/arco/CartographicClassification"/>
        <rdfs:comment xml:lang="it">Questa proprietà collega un bene culturale alla sua classificazione cartografica.</rdfs:comment>
        <rdfs:comment xml:lang="en">This property relates a cultural property to its cartographic classification.</rdfs:comment>
        <rdfs:isDefinedBy rdf:resource="https://w3id.org/arco/ontology/arco"/>
        <rdfs:label xml:lang="it">ha classificazione cartografica</rdfs:label>
        <rdfs:label xml:lang="en">has cartographic classification</rdfs:label>
        <owl:versionInfo xml:lang="it">stabile</owl:versionInfo>
        <owl:versionInfo xml:lang="en">stable</owl:versionInfo>
        <a-cat:iccdNormTag>ICCD Normativa Trasversale 4.00: CT</a-cat:iccdNormTag>
    </owl:ObjectProperty>
    


    <!-- https://w3id.org/arco/ontology/arco/hasCartographicSymbol -->

    <owl:ObjectProperty rdf:about="https://w3id.org/arco/ontology/arco/hasCartographicSymbol">
        <rdfs:subPropertyOf rdf:resource="https://w3id.org/arco/ontology/core/hasConcept"/>
        <owl:inverseOf rdf:resource="https://w3id.org/arco/ontology/arco/isCartographicSymbolOf"/>
        <rdfs:domain rdf:resource="https://w3id.org/arco/ontology/arco/CartographicClassification"/>
        <rdfs:range rdf:resource="https://w3id.org/arco/ontology/arco/CartographicSymbol"/>
        <rdfs:comment xml:lang="it">Questa proprietà collega una classificazione cartografica di un bene cultural al simbolo cartografico, in riferimento al tema.</rdfs:comment>
        <rdfs:comment xml:lang="en">This property relates a cartographic classification of a cultural property to the cartographic symbol related to the theme.</rdfs:comment>
        <rdfs:isDefinedBy rdf:resource="https://w3id.org/arco/ontology/arco"/>
        <rdfs:label xml:lang="it">ha simbolo cartografico</rdfs:label>
        <rdfs:label xml:lang="en">has cartographic symbol</rdfs:label>
        <owl:versionInfo xml:lang="it">stabile</owl:versionInfo>
        <owl:versionInfo xml:lang="en">stable</owl:versionInfo>
        <a-cat:iccdNormTag>ICCD Normativa Trasversale 4.00: CT/CTM/CTMD</a-cat:iccdNormTag>
    </owl:ObjectProperty>
    


    <!-- https://w3id.org/arco/ontology/arco/hasCartographicTheme -->

    <owl:ObjectProperty rdf:about="https://w3id.org/arco/ontology/arco/hasCartographicTheme">
        <rdfs:subPropertyOf rdf:resource="https://w3id.org/arco/ontology/core/hasConcept"/>
        <owl:inverseOf rdf:resource="https://w3id.org/arco/ontology/arco/isCartographicThemeOf"/>
        <rdfs:domain rdf:resource="https://w3id.org/arco/ontology/arco/CartographicClassification"/>
        <rdfs:range rdf:resource="https://w3id.org/arco/ontology/arco/CartographicTheme"/>
        <rdfs:comment xml:lang="it">Questa proprietà collega una classificazione cartografica di un bene culturale al tema di riferimento.</rdfs:comment>
        <rdfs:comment xml:lang="en">This property relates a cartographic classification of a cultural property to the cartographic theme.</rdfs:comment>
        <rdfs:isDefinedBy rdf:resource="https://w3id.org/arco/ontology/arco"/>
        <rdfs:label xml:lang="it">ha tema cartografico</rdfs:label>
        <rdfs:label xml:lang="en">has cartographic theme</rdfs:label>
        <owl:versionInfo xml:lang="it">stabile</owl:versionInfo>
        <owl:versionInfo xml:lang="en">stable</owl:versionInfo>
        <a-cat:iccdNormTag>ICCD Normativa Trasversale 4.00: CT/CTM/CTMT</a-cat:iccdNormTag>
    </owl:ObjectProperty>
    


    <!-- https://w3id.org/arco/ontology/arco/hasCataloguingAgency -->

    <owl:ObjectProperty rdf:about="https://w3id.org/arco/ontology/arco/hasCataloguingAgency">
        <rdfs:subPropertyOf rdf:resource="https://w3id.org/arco/ontology/arco/hasRelatedAgency"/>
        <owl:inverseOf rdf:resource="https://w3id.org/arco/ontology/arco/isCataloguingAgencyOf"/>
        <rdfs:domain rdf:resource="https://w3id.org/arco/ontology/arco/CulturalProperty"/>
        <rdfs:range rdf:resource="https://w3id.org/italia/onto/l0/Agent"/>
        <rdfs:comment xml:lang="it">Questa proprietà rappresenta la relazione che collega un bene culturale al relativo ente schedatore. La relazione tra il ruolo e l&apos;ente che lo riveste è espressa nel nome della proprietà, che quindi ne fornisce una rappresentazione semplificata, con ridotta espressività. Nell&apos;ontologia questa relazione è modellata anche, in maniera più espressiva, dalla classe AgentRole, che permette di collegare l&apos;ente e il suo ruolo.</rdfs:comment>
        <rdfs:comment xml:lang="en">This property relates a cultural property to its cagaloguing agency. The relation is declared in the name of the property, but within the ontology this relation is also modeled, in a more expressive way, through the class AgentRole.</rdfs:comment>
        <rdfs:isDefinedBy rdf:resource="https://w3id.org/arco/ontology/arco"/>
        <rdfs:label xml:lang="it">ha ente schedatore</rdfs:label>
        <rdfs:label xml:lang="en">has cataloguing agency</rdfs:label>
        <owl:versionInfo xml:lang="it">stabile</owl:versionInfo>
        <owl:versionInfo xml:lang="en">stable</owl:versionInfo>
        <a-cat:iccdNormTag>ICCD Normativa Trasversale 4.00: CD/ESC</a-cat:iccdNormTag>
    </owl:ObjectProperty>
    


    <!-- https://w3id.org/arco/ontology/arco/hasCulturalPropertyCataloguingCategory -->

    <owl:ObjectProperty rdf:about="https://w3id.org/arco/ontology/arco/hasCulturalPropertyCataloguingCategory">
        <rdfs:subPropertyOf rdf:resource="https://w3id.org/arco/ontology/core/hasCategory"/>
        <owl:inverseOf rdf:resource="https://w3id.org/arco/ontology/arco/isCulturalPropertyCataloguingCategoryOf"/>
        <rdfs:domain rdf:resource="https://w3id.org/arco/ontology/arco/CulturalProperty"/>
        <rdfs:range rdf:resource="https://w3id.org/arco/ontology/arco/CulturalPropertyCataloguingCategory"/>
        <rdfs:comment xml:lang="it">Questa proprietà collega un bene culturale a una categoria basata su una valutazione soggettiva del catalogatore durante il processo di catalogazione.</rdfs:comment>
        <rdfs:comment xml:lang="en">This property relates a cultural property to a category based on a subjective evaluation of the cataloguing agent, during the cataloguing process.</rdfs:comment>
        <rdfs:isDefinedBy rdf:resource="https://w3id.org/arco/ontology/arco"/>
        <rdfs:label xml:lang="it">ha categoria di bene culturale basata su catalogazione</rdfs:label>
        <rdfs:label xml:lang="en">has cultural property cataloguing category</rdfs:label>
        <owl:versionInfo xml:lang="it">stabile</owl:versionInfo>
        <owl:versionInfo xml:lang="en">stable</owl:versionInfo>
        <a-cat:iccdNormTag>ICCD Normativa Trasversale 4.00: OG/OGT/OGTV</a-cat:iccdNormTag>
    </owl:ObjectProperty>
    


    <!-- https://w3id.org/arco/ontology/arco/hasCulturalPropertyCategory -->

    <owl:ObjectProperty rdf:about="https://w3id.org/arco/ontology/arco/hasCulturalPropertyCategory">
        <rdfs:subPropertyOf rdf:resource="https://w3id.org/arco/ontology/core/hasCategory"/>
        <owl:inverseOf rdf:resource="https://w3id.org/arco/ontology/arco/isCulturalPropertyCategoryOf"/>
        <rdfs:domain rdf:resource="https://w3id.org/arco/ontology/arco/CulturalProperty"/>
        <rdfs:range rdf:resource="https://w3id.org/arco/ontology/arco/CulturalPropertyCategory"/>
        <rdfs:comment xml:lang="it">Questa proprietà collega un bene culturale alla sua categoria.</rdfs:comment>
        <rdfs:comment xml:lang="en">This property relates a cultural property to its category.</rdfs:comment>
        <rdfs:isDefinedBy rdf:resource="https://w3id.org/arco/ontology/arco"/>
        <rdfs:label xml:lang="it">ha categoria</rdfs:label>
        <rdfs:label xml:lang="en">has cultural property category</rdfs:label>
        <owl:versionInfo xml:lang="it">stabile</owl:versionInfo>
        <owl:versionInfo xml:lang="en">stable</owl:versionInfo>
        <a-cat:iccdNormTag>ICCD Normativa Trasversale 4.00: OG/CTG -  Normativa AT: OG/OGT/OGTP - Normativa RA: OG/CLS - Normative CA e MA e Normativa VeAC: OG/OGT/OGTC</a-cat:iccdNormTag>
    </owl:ObjectProperty>
    


    <!-- https://w3id.org/arco/ontology/arco/hasCulturalPropertyComponent -->

    <owl:ObjectProperty rdf:about="https://w3id.org/arco/ontology/arco/hasCulturalPropertyComponent">
        <rdfs:subPropertyOf rdf:resource="https://w3id.org/arco/ontology/core/hasComponent"/>
        <owl:inverseOf rdf:resource="https://w3id.org/arco/ontology/arco/isCulturalPropertyComponentOf"/>
        <rdfs:domain rdf:resource="https://w3id.org/arco/ontology/arco/ComplexCulturalProperty"/>
        <rdfs:range rdf:resource="https://w3id.org/arco/ontology/arco/CulturalPropertyComponent"/>
        <rdfs:comment xml:lang="it">Questa proprietà collega un bene culturale complesso a una delle sue parti componenti.</rdfs:comment>
        <rdfs:comment xml:lang="en">This property relates a cultural property to its components.</rdfs:comment>
        <rdfs:isDefinedBy rdf:resource="https://w3id.org/arco/ontology/arco"/>
        <rdfs:label xml:lang="it">ha parte componente di bene culturale</rdfs:label>
        <rdfs:label xml:lang="en">has cultural property component</rdfs:label>
        <owl:versionInfo xml:lang="it">stabile</owl:versionInfo>
        <owl:versionInfo xml:lang="en">stable</owl:versionInfo>
        <a-cat:iccdNormTag>OG/OGT/OGTP</a-cat:iccdNormTag>
    </owl:ObjectProperty>
    


    <!-- https://w3id.org/arco/ontology/arco/hasCulturalPropertyInventoryCategory -->

    <owl:ObjectProperty rdf:about="https://w3id.org/arco/ontology/arco/hasCulturalPropertyInventoryCategory">
        <rdfs:subPropertyOf rdf:resource="https://w3id.org/arco/ontology/core/hasCategory"/>
        <owl:inverseOf rdf:resource="https://w3id.org/arco/ontology/arco/isCulturalPropertyInventoryCategoryOf"/>
        <rdfs:domain rdf:resource="https://w3id.org/arco/ontology/arco/CulturalProperty"/>
        <rdfs:range rdf:resource="https://w3id.org/arco/ontology/arco/CulturalPropertyInventoryCategory"/>
        <rdfs:comment xml:lang="it">Questa proprietà collega un bene culturale a una categoria basata su una classificazione relativa a un repertorio riconosciuto dallo specifico ambito disciplinare.</rdfs:comment>
        <rdfs:comment xml:lang="en">This property relates a cultural property to a category based on a classification related to an inventory approved by the specific subject area.</rdfs:comment>
        <rdfs:isDefinedBy rdf:resource="https://w3id.org/arco/ontology/arco"/>
        <rdfs:label xml:lang="it">ha categoria basata su repertorio</rdfs:label>
        <rdfs:label xml:lang="en">has cultural property inventory category</rdfs:label>
        <owl:versionInfo xml:lang="it">stabile</owl:versionInfo>
        <owl:versionInfo xml:lang="en">stable</owl:versionInfo>
        <a-cat:iccdNormTag>ICCD Normativa Trasversale 4.00: OG/OGT/OGTS</a-cat:iccdNormTag>
    </owl:ObjectProperty>
    


    <!-- https://w3id.org/arco/ontology/arco/hasCulturalPropertyResidual -->

    <owl:ObjectProperty rdf:about="https://w3id.org/arco/ontology/arco/hasCulturalPropertyResidual">
        <rdfs:subPropertyOf rdf:resource="https://w3id.org/arco/ontology/core/hasPart"/>
        <owl:inverseOf rdf:resource="https://w3id.org/arco/ontology/arco/isCulturalPropertyResidualOf"/>
        <rdfs:domain rdf:resource="https://w3id.org/arco/ontology/arco/CulturalProperty"/>
        <rdfs:range rdf:resource="https://w3id.org/arco/ontology/arco/CulturalPropertyResidual"/>
        <rdfs:comment xml:lang="it">Questa proprietà collega un bene culturale alla/alle sua/e parte/i residuale/i.</rdfs:comment>
        <rdfs:comment xml:lang="en">This property relates a cultural property to its residual.</rdfs:comment>
        <rdfs:isDefinedBy rdf:resource="https://w3id.org/arco/ontology/arco"/>
        <rdfs:label xml:lang="it">ha parte residuale di bene culturale</rdfs:label>
        <rdfs:label xml:lang="en">has cultural property residual</rdfs:label>
        <owl:versionInfo xml:lang="it">stabile</owl:versionInfo>
        <owl:versionInfo xml:lang="en">stable</owl:versionInfo>
        <a-cat:iccdNormTag>OG/OGT/OGTW</a-cat:iccdNormTag>
    </owl:ObjectProperty>
    


    <!-- https://w3id.org/arco/ontology/arco/hasHeritageProtectionAgency -->

    <owl:ObjectProperty rdf:about="https://w3id.org/arco/ontology/arco/hasHeritageProtectionAgency">
        <rdfs:subPropertyOf rdf:resource="https://w3id.org/arco/ontology/arco/hasRelatedAgency"/>
        <owl:inverseOf rdf:resource="https://w3id.org/arco/ontology/arco/isHeritageProtectionAgencyOf"/>
        <rdfs:domain rdf:resource="https://w3id.org/arco/ontology/arco/CulturalProperty"/>
        <rdfs:range rdf:resource="https://w3id.org/italia/onto/l0/Agent"/>
        <rdfs:comment xml:lang="it">Questa proprietà rappresenta la relazione che collega un bene culturale al relativo ente competente per la tutela. La relazione tra il ruolo e l&apos;ente che lo riveste è espressa nel nome della proprietà, che quindi ne fornisce una rappresentazione semplificata, con ridotta espressività. Nell&apos;ontologia questa relazione è modellata anche, in maniera più espressiva, dalla classe AgentRole, che permette di collegare l&apos;ente e il suo ruolo.</rdfs:comment>
        <rdfs:comment xml:lang="en">This property relates a cultural property to its heritage protection agency. The relation is declared in the name of the property, but within the ontology this relation is also modeled, in a more expressive way, through the class AgentRole.</rdfs:comment>
        <rdfs:isDefinedBy rdf:resource="https://w3id.org/arco/ontology/arco"/>
        <rdfs:label xml:lang="it">ha ente competente per la tutela</rdfs:label>
        <rdfs:label xml:lang="en">has heritage protection agency</rdfs:label>
        <owl:versionInfo xml:lang="it">stabile</owl:versionInfo>
        <owl:versionInfo xml:lang="en">stable</owl:versionInfo>
        <a-cat:iccdNormTag>ICCD Normativa Trasversale 4.00: CD/ECP</a-cat:iccdNormTag>
    </owl:ObjectProperty>
    


    <!-- https://w3id.org/arco/ontology/arco/hasMainDiscipline -->

    <owl:ObjectProperty rdf:about="https://w3id.org/arco/ontology/arco/hasMainDiscipline">
        <owl:inverseOf rdf:resource="https://w3id.org/arco/ontology/arco/isMainDisciplineOf"/>
        <rdfs:domain rdf:resource="https://w3id.org/arco/ontology/arco/CulturalProperty"/>
        <rdfs:range rdf:resource="http://dati.beniculturali.it/cis/SubjectDiscipline"/>
        <rdfs:comment xml:lang="it">Questa proprietà permette di associare un bene culturale alla disciplina scientifica più importante, o storicamente riconosciuta, cui fa riferimento.</rdfs:comment>
        <rdfs:comment xml:lang="en">This property relates a cultural property to the main related scientific discipline.</rdfs:comment>
        <rdfs:isDefinedBy rdf:resource="https://w3id.org/arco/ontology/arco"/>
        <rdfs:label xml:lang="it">ha disciplina principale</rdfs:label>
        <rdfs:label xml:lang="en">has main discipline</rdfs:label>
        <owl:versionInfo xml:lang="it">stabile</owl:versionInfo>
        <owl:versionInfo xml:lang="en">stable</owl:versionInfo>
        <a-cat:iccdNormTag>ICCD Normativa PST: CT/CTP</a-cat:iccdNormTag>
    </owl:ObjectProperty>
    


    <!-- https://w3id.org/arco/ontology/arco/hasMibacScopeOfProtection -->

    <owl:ObjectProperty rdf:about="https://w3id.org/arco/ontology/arco/hasMibacScopeOfProtection">
        <owl:inverseOf rdf:resource="https://w3id.org/arco/ontology/arco/isMibacScopeOfProtectionOf"/>
        <rdfs:domain rdf:resource="https://w3id.org/arco/ontology/arco/CulturalProperty"/>
        <rdfs:range rdf:resource="https://w3id.org/arco/ontology/arco/MibacScopeOfProtection"/>
        <rdfs:comment xml:lang="it">Questa proprietà associa un bene culturale all&apos;ambito di tutela nel quale ricade.</rdfs:comment>
        <rdfs:comment xml:lang="en">This property relates a cultural property to ist MiBAC scope of protection</rdfs:comment>
        <rdfs:isDefinedBy rdf:resource="https://w3id.org/arco/ontology/arco"/>
        <rdfs:label xml:lang="it">ha ambito di tutela</rdfs:label>
        <rdfs:label xml:lang="en">has MiBAC scope of protection</rdfs:label>
        <owl:versionInfo xml:lang="it">stabile</owl:versionInfo>
        <owl:versionInfo xml:lang="en">stable</owl:versionInfo>
        <a-cat:iccdNormTag>ICCD Normativa Trasversale 4.00: OG/AMB</a-cat:iccdNormTag>
    </owl:ObjectProperty>
    


    <!-- https://w3id.org/arco/ontology/arco/hasMusicalInstrumentClassification -->

    <owl:ObjectProperty rdf:about="https://w3id.org/arco/ontology/arco/hasMusicalInstrumentClassification">
        <rdfs:subPropertyOf rdf:resource="https://w3id.org/arco/ontology/core/hasClassification"/>
        <owl:inverseOf rdf:resource="https://w3id.org/arco/ontology/arco/isMusicalInstrumentClassificationOf"/>
        <rdfs:domain rdf:resource="https://w3id.org/arco/ontology/arco/MusicHeritage"/>
        <rdfs:range rdf:resource="https://w3id.org/arco/ontology/arco/MusicalInstrumentClassification"/>
        <rdfs:comment xml:lang="it">Questa proprietà collega un bene musicale a una classificazione con cui lo strumento può essere codificato.</rdfs:comment>
        <rdfs:comment xml:lang="en">This property connects a cultural entity to a classification through which the instrument can be coded.</rdfs:comment>
        <rdfs:isDefinedBy rdf:resource="https://w3id.org/arco/arco/"/>
        <rdfs:label xml:lang="it">ha classificazione di strumento musicale</rdfs:label>
        <rdfs:label xml:lang="en">has musical instrument classification</rdfs:label>
        <owl:versionInfo xml:lang="it">stabile</owl:versionInfo>
        <owl:versionInfo xml:lang="en">stable</owl:versionInfo>
    </owl:ObjectProperty>
    


    <!-- https://w3id.org/arco/ontology/arco/hasNumismaticPropertyCategory -->

    <owl:ObjectProperty rdf:about="https://w3id.org/arco/ontology/arco/hasNumismaticPropertyCategory">
        <rdfs:subPropertyOf rdf:resource="https://w3id.org/arco/ontology/core/hasCategory"/>
        <owl:inverseOf rdf:resource="https://w3id.org/arco/ontology/arco/isNumismaticPropertyCategoryOf"/>
        <rdfs:domain rdf:resource="https://w3id.org/arco/ontology/arco/NumismaticProperty"/>
        <rdfs:range rdf:resource="https://w3id.org/arco/ontology/arco/NumismaticPropertyCategory"/>
        <rdfs:comment xml:lang="it">Questa proprietà collega un bene numismatico a una sua categoria.</rdfs:comment>
        <rdfs:comment xml:lang="en">This property relates a numismatic property to one of its categories.</rdfs:comment>
        <rdfs:isDefinedBy rdf:resource="https://w3id.org/arco/ontology/arco"/>
        <rdfs:label xml:lang="it">ha categoria di bene numismatico</rdfs:label>
        <rdfs:label xml:lang="en">has numismatic property category</rdfs:label>
        <owl:versionInfo xml:lang="it">stabile</owl:versionInfo>
        <owl:versionInfo xml:lang="en">stable</owl:versionInfo>
        <a-cat:iccdNormTag>ICCD Normativa NU 4.00: OG/OGT/OGTH</a-cat:iccdNormTag>
    </owl:ObjectProperty>
    


    <!-- https://w3id.org/arco/ontology/arco/hasPhotographicHeritageClassification -->

    <owl:ObjectProperty rdf:about="https://w3id.org/arco/ontology/arco/hasPhotographicHeritageClassification">
        <rdfs:subPropertyOf rdf:resource="https://w3id.org/arco/ontology/core/hasClassification"/>
        <owl:inverseOf rdf:resource="https://w3id.org/arco/ontology/arco/isPhotographicHeritageClassificationOf"/>
        <rdfs:domain rdf:resource="https://w3id.org/arco/ontology/arco/PhotographicHeritage"/>
        <rdfs:range rdf:resource="https://w3id.org/arco/ontology/arco/PhotographicHeritageClassification"/>
        <rdfs:comment xml:lang="it">Questa proprietà collega un bene fotografico a una classificazione di un bene fotografico secondo un sistema di classificazione alternativo a Iconclass, che sia comunque riconosciuto e utilizzato a livello nazionale, o preferibilmente internazionale.</rdfs:comment>
        <rdfs:comment xml:lang="en">This property connects a photographic property to a photographic property&apos;s classification, according to to other classification systems as Iconclass. The system has to be recognised and used at national or preferably international level.</rdfs:comment>
        <rdfs:isDefinedBy rdf:resource="https://w3id.org/arco/ontology/arco"/>
        <rdfs:label xml:lang="it">ha classificazione di bene fotografico</rdfs:label>
        <rdfs:label xml:lang="en">has photographic heritage classification</rdfs:label>
        <owl:versionInfo xml:lang="it">stabile</owl:versionInfo>
        <owl:versionInfo xml:lang="en">stable</owl:versionInfo>
        <a-cat:iccdNormTag>ICCD Normativa F 4.00: SG/CLF</a-cat:iccdNormTag>
    </owl:ObjectProperty>
    


    <!-- https://w3id.org/arco/ontology/arco/hasPhotographicHeritageClassificationType -->

    <owl:ObjectProperty rdf:about="https://w3id.org/arco/ontology/arco/hasPhotographicHeritageClassificationType">
        <rdfs:subPropertyOf rdf:resource="https://w3id.org/arco/ontology/core/hasType"/>
        <owl:inverseOf rdf:resource="https://w3id.org/arco/ontology/arco/isPhotographicHeritageClassificationTypeOf"/>
        <rdfs:domain rdf:resource="https://w3id.org/arco/ontology/arco/PhotographicHeritageClassification"/>
        <rdfs:range rdf:resource="https://w3id.org/arco/ontology/arco/PhotographicHeritageClassificationType"/>
        <rdfs:comment xml:lang="it">Questa proprietà collega una classificazione di un bene fotografico al tipo di classificazione, relativamente a un sistema di classificazione alternativo a Iconclass, che sia comunque riconosciuto e utilizzato a livello nazionale, o preferibilmente internazionale.</rdfs:comment>
        <rdfs:comment xml:lang="en">This property connects a photographic property&apos;s classification to the classification type, according to to other classification systems as Iconclass. The system has to be recognised and used at national or preferably international level.</rdfs:comment>
        <rdfs:isDefinedBy rdf:resource="https://w3id.org/arco/ontology/arco"/>
        <rdfs:label xml:lang="it">ha tipo di classificazione di bene fotografico</rdfs:label>
        <rdfs:label xml:lang="en">has photographic heritage classification type</rdfs:label>
        <owl:versionInfo xml:lang="it">stabile</owl:versionInfo>
        <owl:versionInfo xml:lang="en">stable</owl:versionInfo>
        <a-cat:iccdNormTag>ICCD Normativa F: SG/CLF/CLFT</a-cat:iccdNormTag>
    </owl:ObjectProperty>
    


    <!-- https://w3id.org/arco/ontology/arco/hasRFId -->

    <owl:ObjectProperty rdf:about="https://w3id.org/arco/ontology/arco/hasRFId">
        <owl:inverseOf rdf:resource="https://w3id.org/arco/ontology/arco/isRFIdOf"/>
        <rdfs:domain rdf:resource="http://www.w3.org/2002/07/owl#Thing"/>
        <rdfs:range rdf:resource="https://w3id.org/arco/ontology/arco/RFId"/>
        <rdfs:comment xml:lang="it">Questa proprietà collega un oggetto a un identificatore a radiofrequenza RFId.</rdfs:comment>
        <rdfs:comment xml:lang="en">This property relates an object to an RFId.</rdfs:comment>
        <rdfs:isDefinedBy rdf:resource="https://w3id.org/arco/ontology/arco"/>
        <rdfs:label xml:lang="it">ha identificativo RFId</rdfs:label>
        <rdfs:label xml:lang="en">has RFId identifier</rdfs:label>
        <owl:versionInfo xml:lang="it">stabile</owl:versionInfo>
        <owl:versionInfo xml:lang="en">stable</owl:versionInfo>
    </owl:ObjectProperty>
    


    <!-- https://w3id.org/arco/ontology/arco/hasReferenceCoinLegend -->

    <owl:ObjectProperty rdf:about="https://w3id.org/arco/ontology/arco/hasReferenceCoinLegend">
        <rdfs:subPropertyOf rdf:resource="https://w3id.org/arco/ontology/core/hasConcept"/>
        <owl:inverseOf rdf:resource="https://w3id.org/arco/ontology/arco/isReferenceCoinLegendOf"/>
        <rdf:type rdf:resource="http://www.w3.org/2002/07/owl#FunctionalProperty"/>
        <rdfs:domain rdf:resource="https://w3id.org/arco/ontology/arco/NumismaticProperty"/>
        <rdfs:range rdf:resource="https://w3id.org/arco/ontology/arco/ReferenceCoinLegend"/>
        <rdfs:comment xml:lang="it">Questa proprietà collega un bene numismatico alla sua legenda tipo.</rdfs:comment>
        <rdfs:comment xml:lang="en">This property relates a numismatic property with its reference coin legend.</rdfs:comment>
        <rdfs:isDefinedBy rdf:resource="https://w3id.org/arco/ontology/arco"/>
        <rdfs:label xml:lang="it">ha legenda tipo</rdfs:label>
        <rdfs:label xml:lang="en">has reference coin legend</rdfs:label>
        <owl:versionInfo xml:lang="it">stabile</owl:versionInfo>
        <owl:versionInfo xml:lang="en">stable</owl:versionInfo>
        <a-cat:iccdNormTag>ICCD Normativa NU: OG/OGT/OGTL</a-cat:iccdNormTag>
    </owl:ObjectProperty>
    


    <!-- https://w3id.org/arco/ontology/arco/hasRelatedAgency -->

    <owl:ObjectProperty rdf:about="https://w3id.org/arco/ontology/arco/hasRelatedAgency">
        <owl:inverseOf rdf:resource="https://w3id.org/arco/ontology/arco/isRelatedAgencyOf"/>
        <rdfs:domain rdf:resource="https://w3id.org/arco/ontology/arco/CulturalProperty"/>
        <rdfs:range rdf:resource="https://w3id.org/italia/onto/l0/Agent"/>
        <owl:propertyChainAxiom rdf:parseType="Collection">
            <rdf:Description rdf:about="https://w3id.org/arco/ontology/core/hasAgentRole"/>
            <rdf:Description rdf:about="https://w3id.org/arco/ontology/core/hasAgent"/>
        </owl:propertyChainAxiom>
        <rdfs:comment xml:lang="it">Questa proprietà rappresenta la relazione che collega un bene culturale a un ente che riveste un ruolo nei suoi confronti. La relazione tra il ruolo e l&apos;ente che lo riveste è espressa, in maniera generica, nel nome della proprietà, che quindi ne fornisce una rappresentazione semplificata, con ridotta espressività. La proprietà è specializzata per mezzo di sottoproprietà. Nell&apos;ontologia questa relazione è modellata anche, in maniera più espressiva, dalla classe AgentRole, che permette di collegare l&apos;ente e il suo ruolo.</rdfs:comment>
        <rdfs:comment xml:lang="en">This property relates a cultural property to an agency that plays a role related to the cultural property. The relation is declared in the name of the property, but within the ontology this relation is also modeled, in a more expressive way, through the class AgentRole.</rdfs:comment>
        <rdfs:isDefinedBy rdf:resource="https://w3id.org/arco/ontology/arco"/>
        <rdfs:label xml:lang="it">ha ente collegato</rdfs:label>
        <rdfs:label xml:lang="en">has related agency</rdfs:label>
        <owl:versionInfo xml:lang="it">stabile</owl:versionInfo>
        <owl:versionInfo xml:lang="en">stable</owl:versionInfo>
    </owl:ObjectProperty>
    


    <!-- https://w3id.org/arco/ontology/arco/hasThematicCategory -->

    <owl:ObjectProperty rdf:about="https://w3id.org/arco/ontology/arco/hasThematicCategory">
        <rdfs:subPropertyOf rdf:resource="https://w3id.org/arco/ontology/core/hasCategory"/>
        <owl:inverseOf rdf:resource="https://w3id.org/arco/ontology/arco/isThematicCategoryOf"/>
        <rdfs:domain rdf:resource="https://w3id.org/arco/ontology/arco/CartographicClassification"/>
        <rdfs:range rdf:resource="https://w3id.org/arco/ontology/arco/ThematicCategory"/>
        <rdfs:comment xml:lang="it">Questa proprietà collega una classificazione cartografica di un bene culturale alla categoria tematica.</rdfs:comment>
        <rdfs:comment xml:lang="en">This property relates a cartographic classification of a cultural property to the thematic category.</rdfs:comment>
        <rdfs:isDefinedBy rdf:resource="https://w3id.org/arco/ontology/arco"/>
        <rdfs:label xml:lang="it">ha categoria tematica</rdfs:label>
        <rdfs:label xml:lang="en">has thematic category</rdfs:label>
        <owl:versionInfo xml:lang="it">stabile</owl:versionInfo>
        <owl:versionInfo xml:lang="en">stable</owl:versionInfo>
        <a-cat:iccdNormTag>ICCD Normativa Trasversale 4.00: CT/CTM/CTMC</a-cat:iccdNormTag>
    </owl:ObjectProperty>
    


    <!-- https://w3id.org/arco/ontology/arco/isAlternativeDisciplineOf -->

    <owl:ObjectProperty rdf:about="https://w3id.org/arco/ontology/arco/isAlternativeDisciplineOf">
        <rdfs:domain rdf:resource="http://dati.beniculturali.it/cis/SubjectDiscipline"/>
        <rdfs:range rdf:resource="https://w3id.org/arco/ontology/arco/CulturalProperty"/>
        <rdfs:comment xml:lang="it">Questa proprietà permette di associare discipline scientifiche, alternative a quella principale, cui un bene culturale fa riferimento, al bene culturale stesso.</rdfs:comment>
        <rdfs:comment xml:lang="en">This property relates a scientific discipline, alternative to the main one, related to a cultural property to that cultural property.</rdfs:comment>
        <rdfs:isDefinedBy rdf:resource="https://w3id.org/arco/ontology/arco"/>
        <rdfs:label xml:lang="en">is alternative discipline of</rdfs:label>
        <rdfs:label xml:lang="it">è altra disciplina di</rdfs:label>
        <owl:versionInfo xml:lang="it">stabile</owl:versionInfo>
        <owl:versionInfo xml:lang="en">stable</owl:versionInfo>
    </owl:ObjectProperty>
    


    <!-- https://w3id.org/arco/ontology/arco/isArchaeologicalMaterialCategoryOf -->

    <owl:ObjectProperty rdf:about="https://w3id.org/arco/ontology/arco/isArchaeologicalMaterialCategoryOf">
        <rdfs:subPropertyOf rdf:resource="https://w3id.org/arco/ontology/core/isCategoryOf"/>
        <rdfs:domain rdf:resource="https://w3id.org/arco/ontology/arco/ArchaeologicalMaterialCategory"/>
        <rdfs:range rdf:resource="https://w3id.org/arco/ontology/arco/ArchaeologicalMaterial"/>
        <rdfs:comment xml:lang="it">Questa è la proprietà inversa di &quot;ha categoria di materiale archeologico&quot;.</rdfs:comment>
        <rdfs:comment xml:lang="en">This is the inverse property of &quot;has archaeological material category of&quot;.</rdfs:comment>
        <rdfs:isDefinedBy rdf:resource="https://w3id.org/arco/ontology/arco"/>
        <rdfs:label xml:lang="en">is archaeological material category of</rdfs:label>
        <rdfs:label xml:lang="it">è categoria di materiale archeologico</rdfs:label>
        <owl:versionInfo xml:lang="it">stabile</owl:versionInfo>
        <owl:versionInfo xml:lang="en">stable</owl:versionInfo>
    </owl:ObjectProperty>
    


    <!-- https://w3id.org/arco/ontology/arco/isCartographicClassificationOf -->

    <owl:ObjectProperty rdf:about="https://w3id.org/arco/ontology/arco/isCartographicClassificationOf">
        <rdfs:subPropertyOf rdf:resource="https://w3id.org/arco/ontology/core/isClassificationOf"/>
        <rdfs:domain rdf:resource="https://w3id.org/arco/ontology/arco/CartographicClassification"/>
        <rdfs:range rdf:resource="https://w3id.org/arco/ontology/arco/CulturalProperty"/>
        <rdfs:comment xml:lang="it">Questa è la proprietà inversa di &quot;ha classificazione cartografica&quot;.</rdfs:comment>
        <rdfs:comment xml:lang="en">This is the inverse property of &quot;has cartographic classification&quot;.</rdfs:comment>
        <rdfs:isDefinedBy rdf:resource="https://w3id.org/arco/ontology/arco"/>
        <rdfs:label xml:lang="en">is cartographic classification of</rdfs:label>
        <rdfs:label xml:lang="it">è classificazione cartografica di</rdfs:label>
        <owl:versionInfo xml:lang="it">stabile</owl:versionInfo>
        <owl:versionInfo xml:lang="en">stable</owl:versionInfo>
    </owl:ObjectProperty>
    


    <!-- https://w3id.org/arco/ontology/arco/isCartographicSymbolOf -->

    <owl:ObjectProperty rdf:about="https://w3id.org/arco/ontology/arco/isCartographicSymbolOf">
        <rdfs:subPropertyOf rdf:resource="https://w3id.org/arco/ontology/core/isConceptOf"/>
        <rdfs:domain rdf:resource="https://w3id.org/arco/ontology/arco/CartographicSymbol"/>
        <rdfs:range rdf:resource="https://w3id.org/arco/ontology/arco/CartographicClassification"/>
        <rdfs:comment xml:lang="it">Questa è la proprietà inversa di &quot;ha simbolo cartografico&quot;.</rdfs:comment>
        <rdfs:comment xml:lang="en">This is the inverse property of &quot;has cartographic symbol&quot;.</rdfs:comment>
        <rdfs:isDefinedBy rdf:resource="https://w3id.org/arco/ontology/arco"/>
        <rdfs:label xml:lang="en">is cartographic symbol of</rdfs:label>
        <rdfs:label xml:lang="it">è simbolo cartografico di</rdfs:label>
        <owl:versionInfo xml:lang="it">stabile</owl:versionInfo>
        <owl:versionInfo xml:lang="en">stable</owl:versionInfo>
    </owl:ObjectProperty>
    


    <!-- https://w3id.org/arco/ontology/arco/isCartographicThemeOf -->

    <owl:ObjectProperty rdf:about="https://w3id.org/arco/ontology/arco/isCartographicThemeOf">
        <rdfs:subPropertyOf rdf:resource="https://w3id.org/arco/ontology/core/isConceptOf"/>
        <rdfs:domain rdf:resource="https://w3id.org/arco/ontology/arco/CartographicTheme"/>
        <rdfs:range rdf:resource="https://w3id.org/arco/ontology/arco/CartographicClassification"/>
        <rdfs:comment xml:lang="it">Questa è la proprietà inversa di &quot;ha tema cartografico&quot;.</rdfs:comment>
        <rdfs:comment xml:lang="en">This is the inverse property of &quot;has cartographic theme&quot;.</rdfs:comment>
        <rdfs:isDefinedBy rdf:resource="https://w3id.org/arco/ontology/arco"/>
        <rdfs:label xml:lang="en">is cartographic theme of</rdfs:label>
        <rdfs:label xml:lang="it">è tema cartografico di</rdfs:label>
        <owl:versionInfo xml:lang="it">stabile</owl:versionInfo>
        <owl:versionInfo xml:lang="en">stable</owl:versionInfo>
    </owl:ObjectProperty>
    


    <!-- https://w3id.org/arco/ontology/arco/isCataloguingAgencyOf -->

    <owl:ObjectProperty rdf:about="https://w3id.org/arco/ontology/arco/isCataloguingAgencyOf">
        <rdfs:subPropertyOf rdf:resource="https://w3id.org/arco/ontology/arco/isRelatedAgencyOf"/>
        <rdfs:domain rdf:resource="https://w3id.org/italia/onto/l0/Agent"/>
        <rdfs:range rdf:resource="https://w3id.org/arco/ontology/arco/CulturalProperty"/>
        <rdfs:comment xml:lang="it">Questa proprietà rappresenta la relazione che collega un ente schedatore al relativo bene culturale che ha schedato. La relazione tra il ruolo e l&apos;ente che lo riveste è espressa nel nome della proprietà, che quindi ne fornisce una rappresentazione semplificata, con ridotta espressività. Nell&apos;ontologia questa relazione è modellata anche, in maniera più espressiva, dalla classe AgentRole, che permette di collegare l&apos;ente e il suo ruolo.</rdfs:comment>
        <rdfs:comment xml:lang="en">This property relates a cagaloguing agency to the catalogued cultural property. The relation is declared in the name of the property, but within the ontology this relation is also modeled, in a more expressive way, through the class AgentRole.</rdfs:comment>
        <rdfs:isDefinedBy rdf:resource="https://w3id.org/arco/ontology/arco"/>
        <rdfs:label xml:lang="en">is cataloguing agency of</rdfs:label>
        <rdfs:label xml:lang="it">è ente schedatore di</rdfs:label>
        <owl:versionInfo xml:lang="it">stabile</owl:versionInfo>
        <owl:versionInfo xml:lang="en">stable</owl:versionInfo>
        <a-cat:iccdNormTag>ICCD Normativa Trasversale 4.00: CD/ESC</a-cat:iccdNormTag>
    </owl:ObjectProperty>
    


    <!-- https://w3id.org/arco/ontology/arco/isCulturalPropertyCataloguingCategoryOf -->

    <owl:ObjectProperty rdf:about="https://w3id.org/arco/ontology/arco/isCulturalPropertyCataloguingCategoryOf">
        <rdfs:subPropertyOf rdf:resource="https://w3id.org/arco/ontology/core/isCategoryOf"/>
        <rdfs:domain rdf:resource="https://w3id.org/arco/ontology/arco/CulturalPropertyCataloguingCategory"/>
        <rdfs:range rdf:resource="https://w3id.org/arco/ontology/arco/CulturalProperty"/>
        <rdfs:comment xml:lang="it">Questa è la proprietà inversa a &quot;ha categoria di bene culturale basata su catalogazione&quot;.</rdfs:comment>
        <rdfs:comment xml:lang="en">This is the inverse property of &quot;has cultural property cataloguing category of&quot;.</rdfs:comment>
        <rdfs:isDefinedBy rdf:resource="https://w3id.org/arco/ontology/arco"/>
        <rdfs:label xml:lang="en">is cultural property cataloguing category of</rdfs:label>
        <rdfs:label xml:lang="it">è categoria di bene culturale basata su catalogazione di</rdfs:label>
        <owl:versionInfo xml:lang="it">stabile</owl:versionInfo>
        <owl:versionInfo xml:lang="en">stable</owl:versionInfo>
    </owl:ObjectProperty>
    


    <!-- https://w3id.org/arco/ontology/arco/isCulturalPropertyCategoryOf -->

    <owl:ObjectProperty rdf:about="https://w3id.org/arco/ontology/arco/isCulturalPropertyCategoryOf">
        <rdfs:subPropertyOf rdf:resource="https://w3id.org/arco/ontology/core/isCategoryOf"/>
        <rdfs:domain rdf:resource="https://w3id.org/arco/ontology/arco/CulturalPropertyCategory"/>
        <rdfs:range rdf:resource="https://w3id.org/arco/ontology/arco/CulturalProperty"/>
        <rdfs:comment xml:lang="it">Questa è la proprietà inversa di &quot;ha categoria&quot;.</rdfs:comment>
        <rdfs:comment xml:lang="en">This is the inverse property of &quot;has cultural property category&quot;.</rdfs:comment>
        <rdfs:isDefinedBy rdf:resource="https://w3id.org/arco/ontology/arco"/>
        <rdfs:label xml:lang="en">is cultural property category of</rdfs:label>
        <rdfs:label xml:lang="it">è categoria di bene culturale</rdfs:label>
        <owl:versionInfo xml:lang="it">stabile</owl:versionInfo>
        <owl:versionInfo xml:lang="en">stable</owl:versionInfo>
    </owl:ObjectProperty>
    


    <!-- https://w3id.org/arco/ontology/arco/isCulturalPropertyComponentOf -->

    <owl:ObjectProperty rdf:about="https://w3id.org/arco/ontology/arco/isCulturalPropertyComponentOf">
        <rdfs:subPropertyOf rdf:resource="https://w3id.org/arco/ontology/core/isPartOf"/>
        <rdfs:domain rdf:resource="https://w3id.org/arco/ontology/arco/CulturalPropertyComponent"/>
        <rdfs:range rdf:resource="https://w3id.org/arco/ontology/arco/ComplexCulturalProperty"/>
        <rdfs:comment xml:lang="it">Questa proprietà, inversa a &quot;ha componente&quot;, collega una delle parti componenti di un bene culturale complesso al bene complesso stesso.</rdfs:comment>
        <rdfs:comment xml:lang="en">This property, inverse of &quot;has component&quot;, relates a component of a complex cultural property to the complex cultural property.</rdfs:comment>
        <rdfs:isDefinedBy rdf:resource="https://w3id.org/arco/ontology/arco"/>
        <rdfs:label xml:lang="en">is cultural property component of</rdfs:label>
        <rdfs:label xml:lang="it">è parte componente di bene culturale</rdfs:label>
        <owl:versionInfo xml:lang="it">stabile</owl:versionInfo>
        <owl:versionInfo xml:lang="en">stable</owl:versionInfo>
        <a-cat:iccdNormTag>OG/OGT/OGTP</a-cat:iccdNormTag>
    </owl:ObjectProperty>
    


    <!-- https://w3id.org/arco/ontology/arco/isCulturalPropertyInventoryCategoryOf -->

    <owl:ObjectProperty rdf:about="https://w3id.org/arco/ontology/arco/isCulturalPropertyInventoryCategoryOf">
        <rdfs:subPropertyOf rdf:resource="https://w3id.org/arco/ontology/core/isCategoryOf"/>
        <rdfs:domain rdf:resource="https://w3id.org/arco/ontology/arco/CulturalPropertyInventoryCategory"/>
        <rdfs:range rdf:resource="https://w3id.org/arco/ontology/arco/CulturalProperty"/>
        <rdfs:comment xml:lang="it">Questa proprietà collega una categoria basata su una classificazione relativa a un repertorio riconosciuto dallo specifico ambito disciplinare a un bene culturale.</rdfs:comment>
        <rdfs:comment xml:lang="en">This property relates a category based on a classification related to an inventory approved by the specific subject area to a cultural property.</rdfs:comment>
        <rdfs:isDefinedBy rdf:resource="https://w3id.org/arco/ontology/arco"/>
        <rdfs:label xml:lang="en">is cultural property inventory category of</rdfs:label>
        <rdfs:label xml:lang="it">è categoria basata su repertorio di</rdfs:label>
        <owl:versionInfo xml:lang="it">stabile</owl:versionInfo>
        <owl:versionInfo xml:lang="en">stable</owl:versionInfo>
        <a-cat:iccdNormTag>ICCD Normativa Trasversale 4.00: OG/OGT/OGTS</a-cat:iccdNormTag>
    </owl:ObjectProperty>
    


    <!-- https://w3id.org/arco/ontology/arco/isCulturalPropertyResidualOf -->

    <owl:ObjectProperty rdf:about="https://w3id.org/arco/ontology/arco/isCulturalPropertyResidualOf">
        <rdfs:subPropertyOf rdf:resource="https://w3id.org/arco/ontology/core/isPartOf"/>
        <rdfs:domain rdf:resource="https://w3id.org/arco/ontology/arco/CulturalPropertyResidual"/>
        <rdfs:range rdf:resource="https://w3id.org/arco/ontology/arco/CulturalProperty"/>
        <rdfs:comment xml:lang="it">Questa proprietà, inversa a &quot;ha parte residuale&quot;, collega una parte residuale di un bene culturale al bene culturale stesso.</rdfs:comment>
        <rdfs:comment xml:lang="en">This property, inverse of &quot;has residual&quot;, relates a residual of a cultural property to the cultural property.</rdfs:comment>
        <rdfs:isDefinedBy rdf:resource="https://w3id.org/arco/ontology/arco"/>
        <rdfs:label xml:lang="en">is cultural property residual of</rdfs:label>
        <rdfs:label xml:lang="it">è parte residuale di bene culturale</rdfs:label>
        <owl:versionInfo xml:lang="it">stabile</owl:versionInfo>
        <owl:versionInfo xml:lang="en">stable</owl:versionInfo>
        <a-cat:iccdNormTag>OG/OGT/OGTW</a-cat:iccdNormTag>
    </owl:ObjectProperty>
    


    <!-- https://w3id.org/arco/ontology/arco/isHeritageProtectionAgencyOf -->

    <owl:ObjectProperty rdf:about="https://w3id.org/arco/ontology/arco/isHeritageProtectionAgencyOf">
        <rdfs:subPropertyOf rdf:resource="https://w3id.org/arco/ontology/arco/isRelatedAgencyOf"/>
        <rdfs:domain rdf:resource="https://w3id.org/italia/onto/l0/Agent"/>
        <rdfs:range rdf:resource="https://w3id.org/arco/ontology/arco/CulturalProperty"/>
        <rdfs:comment xml:lang="it">Questa proprietà rappresenta la relazione che collega un ente competente per la tutela al relativo bene culturale della cui tutela è competente. La relazione tra il ruolo e l&apos;ente che lo riveste è espressa nel nome della proprietà, che quindi ne fornisce una rappresentazione semplificata, con ridotta espressività. Nell&apos;ontologia questa relazione è modellata anche, in maniera più espressiva, dalla classe AgentRole, che permette di collegare l&apos;ente e il suo ruolo.</rdfs:comment>
        <rdfs:comment xml:lang="en">This property relates an heritage protection agency to the cultural property. The relation is declared in the name of the property, but within the ontology this relation is also modeled, in a more expressive way, through the class AgentRole.</rdfs:comment>
        <rdfs:isDefinedBy rdf:resource="https://w3id.org/arco/ontology/arco"/>
        <rdfs:label xml:lang="en">is heritage protection agency of</rdfs:label>
        <rdfs:label xml:lang="it">è ente competente per la tutela di</rdfs:label>
        <owl:versionInfo xml:lang="it">stabile</owl:versionInfo>
        <owl:versionInfo xml:lang="en">stable</owl:versionInfo>
        <a-cat:iccdNormTag>ICCD Normativa Trasversale 4.00: CD/ECP</a-cat:iccdNormTag>
    </owl:ObjectProperty>
    


    <!-- https://w3id.org/arco/ontology/arco/isMainDisciplineOf -->

    <owl:ObjectProperty rdf:about="https://w3id.org/arco/ontology/arco/isMainDisciplineOf">
        <rdfs:domain rdf:resource="http://dati.beniculturali.it/cis/SubjectDiscipline"/>
        <rdfs:range rdf:resource="https://w3id.org/arco/ontology/arco/CulturalProperty"/>
        <rdfs:comment xml:lang="it">Questa proprietà permette di associare la disciplina scientifica principale, cui un bene culturale fa riferimento, al bene culturale stesso.</rdfs:comment>
        <rdfs:comment xml:lang="en">This property relates the main scientific discipline related to a cultural property to that cultural property.</rdfs:comment>
        <rdfs:isDefinedBy rdf:resource="https://w3id.org/arco/ontology/arco"/>
        <rdfs:label xml:lang="en">is main discipline of</rdfs:label>
        <rdfs:label xml:lang="it">è disciplina principale di</rdfs:label>
        <owl:versionInfo xml:lang="it">stabile</owl:versionInfo>
        <owl:versionInfo xml:lang="en">stable</owl:versionInfo>
    </owl:ObjectProperty>
    


    <!-- https://w3id.org/arco/ontology/arco/isMibacScopeOfProtectionOf -->

    <owl:ObjectProperty rdf:about="https://w3id.org/arco/ontology/arco/isMibacScopeOfProtectionOf">
        <rdfs:domain rdf:resource="https://w3id.org/arco/ontology/arco/MibacScopeOfProtection"/>
        <rdfs:range rdf:resource="https://w3id.org/arco/ontology/arco/CulturalProperty"/>
        <rdfs:comment xml:lang="it">Questa è la proprietà inversa di &quot;ha ambito di tutela&quot;.</rdfs:comment>
        <rdfs:comment xml:lang="en">This is the inverse property of &quot;has MiBAC scope of protection&quot;.</rdfs:comment>
        <rdfs:isDefinedBy rdf:resource="https://w3id.org/arco/ontology/arco"/>
        <rdfs:label xml:lang="en">is MiBAC scope of protection of</rdfs:label>
        <rdfs:label xml:lang="it">è ambito di tutela di</rdfs:label>
        <owl:versionInfo xml:lang="it">stabile</owl:versionInfo>
        <owl:versionInfo xml:lang="en">stable</owl:versionInfo>
    </owl:ObjectProperty>
    


    <!-- https://w3id.org/arco/ontology/arco/isMusicalInstrumentClassificationOf -->

    <owl:ObjectProperty rdf:about="https://w3id.org/arco/ontology/arco/isMusicalInstrumentClassificationOf">
        <rdfs:subPropertyOf rdf:resource="https://w3id.org/arco/ontology/core/isClassificationOf"/>
        <rdfs:domain rdf:resource="https://w3id.org/arco/ontology/arco/MusicalInstrumentClassification"/>
        <rdfs:range rdf:resource="https://w3id.org/arco/ontology/arco/MusicHeritage"/>
        <rdfs:comment xml:lang="it">Questa proprietà, inversa a &quot;ha classificazione di bene musicale&quot;, collega un una classificazione con cui uno strumento musicale può essere codificato al bene musicale.</rdfs:comment>
        <rdfs:isDefinedBy rdf:resource="https://w3id.org/arco/ontology/arco"/>
        <rdfs:label xml:lang="en">is musical instrument classification of</rdfs:label>
        <rdfs:label xml:lang="it">è classificazione di strumento musicale di</rdfs:label>
        <owl:versionInfo xml:lang="it">stabile</owl:versionInfo>
        <owl:versionInfo xml:lang="en">stable</owl:versionInfo>
    </owl:ObjectProperty>
    


    <!-- https://w3id.org/arco/ontology/arco/isNumismaticPropertyCategoryOf -->

    <owl:ObjectProperty rdf:about="https://w3id.org/arco/ontology/arco/isNumismaticPropertyCategoryOf">
        <rdfs:subPropertyOf rdf:resource="https://w3id.org/arco/ontology/core/isCategoryOf"/>
        <rdfs:domain rdf:resource="https://w3id.org/arco/ontology/arco/NumismaticPropertyCategory"/>
        <rdfs:range rdf:resource="https://w3id.org/arco/ontology/arco/NumismaticProperty"/>
        <rdfs:comment xml:lang="it">Questa proprietà collega una categoria di bene numismatico al bene numismatico cui si riferisce.</rdfs:comment>
        <rdfs:isDefinedBy rdf:resource="https://w3id.org/arco/ontology/arco"/>
        <rdfs:label xml:lang="en">is numismatic property category of</rdfs:label>
        <rdfs:label xml:lang="it">è categoria di bene numismatico</rdfs:label>
        <owl:versionInfo xml:lang="it">stabile</owl:versionInfo>
        <owl:versionInfo xml:lang="en">stable</owl:versionInfo>
        <a-cat:iccdNormTag>ICCD Normativa NU 4.00: OG/OGT/OGTH</a-cat:iccdNormTag>
    </owl:ObjectProperty>
    


    <!-- https://w3id.org/arco/ontology/arco/isPhotographicHeritageClassificationOf -->

    <owl:ObjectProperty rdf:about="https://w3id.org/arco/ontology/arco/isPhotographicHeritageClassificationOf">
        <rdfs:subPropertyOf rdf:resource="https://w3id.org/arco/ontology/core/isClassificationOf"/>
        <rdfs:domain rdf:resource="https://w3id.org/arco/ontology/arco/PhotographicHeritageClassification"/>
        <rdfs:range rdf:resource="https://w3id.org/arco/ontology/arco/PhotographicHeritage"/>
        <rdfs:isDefinedBy rdf:resource="https://w3id.org/arco/ontology/arco"/>
        <rdfs:label xml:lang="en">is photographic heritage classification of</rdfs:label>
        <rdfs:label xml:lang="it">è classificazione di bene fotografico di</rdfs:label>
        <owl:versionInfo xml:lang="it">Questa proprietà, inversa a &quot;ha classificazione di bene fotografico&quot;, collega una classificazione di un bene fotografico secondo un sistema di classificazione alternativo a Iconclass, a un bene fotografico.</owl:versionInfo>
        <owl:versionInfo xml:lang="it">stabile</owl:versionInfo>
        <owl:versionInfo xml:lang="en">stable</owl:versionInfo>
    </owl:ObjectProperty>
    


    <!-- https://w3id.org/arco/ontology/arco/isPhotographicHeritageClassificationTypeOf -->

    <owl:ObjectProperty rdf:about="https://w3id.org/arco/ontology/arco/isPhotographicHeritageClassificationTypeOf">
        <rdfs:subPropertyOf rdf:resource="https://w3id.org/arco/ontology/core/isTypeOf"/>
        <rdfs:domain rdf:resource="https://w3id.org/arco/ontology/arco/PhotographicHeritageClassificationType"/>
        <rdfs:range rdf:resource="https://w3id.org/arco/ontology/arco/PhotographicHeritageClassification"/>
        <rdfs:comment xml:lang="it">Questa è la proprietà inversa di &quot;ha tipo di classificazione di bene fotografico&quot;.</rdfs:comment>
        <rdfs:comment xml:lang="en">This is the inverse property of &quot;has photographic heritage classification type&quot;.</rdfs:comment>
        <rdfs:isDefinedBy rdf:resource="https://w3id.org/arco/ontology/arco"/>
        <rdfs:label xml:lang="en">is photographic heritage classification type of</rdfs:label>
        <rdfs:label xml:lang="it">è tipo di classificazione di bene fotografico</rdfs:label>
        <owl:versionInfo xml:lang="it">stabile</owl:versionInfo>
        <owl:versionInfo xml:lang="en">stable</owl:versionInfo>
    </owl:ObjectProperty>
    


    <!-- https://w3id.org/arco/ontology/arco/isRFIdOf -->

    <owl:ObjectProperty rdf:about="https://w3id.org/arco/ontology/arco/isRFIdOf">
        <rdfs:domain rdf:resource="https://w3id.org/arco/ontology/arco/RFId"/>
        <rdfs:range rdf:resource="http://www.w3.org/2002/07/owl#Thing"/>
        <rdfs:comment xml:lang="it">Questa proprietà collega un identificatore a radiofrequenza RFId a un oggetto.</rdfs:comment>
        <rdfs:comment xml:lang="en">This property relates a radio-frequency identification (RFID) to an object.</rdfs:comment>
        <rdfs:isDefinedBy rdf:resource="https://w3id.org/arco/ontology/arco"/>
        <rdfs:label xml:lang="en">is RFId identifier of</rdfs:label>
        <rdfs:label xml:lang="it">è identificativo RFId di</rdfs:label>
        <owl:versionInfo xml:lang="it">stabile</owl:versionInfo>
        <owl:versionInfo xml:lang="en">stable</owl:versionInfo>
    </owl:ObjectProperty>
    


    <!-- https://w3id.org/arco/ontology/arco/isReferenceCoinLegendOf -->

    <owl:ObjectProperty rdf:about="https://w3id.org/arco/ontology/arco/isReferenceCoinLegendOf">
        <rdfs:subPropertyOf rdf:resource="https://w3id.org/arco/ontology/core/isConceptOf"/>
        <rdfs:domain rdf:resource="https://w3id.org/arco/ontology/arco/ReferenceCoinLegend"/>
        <rdfs:range rdf:resource="https://w3id.org/arco/ontology/arco/NumismaticProperty"/>
        <rdfs:comment xml:lang="it">Questa è la proprietà inversa di &quot;ha legenda tipo&quot;.</rdfs:comment>
        <rdfs:comment xml:lang="en">This is the inverse property of &quot;ha reference coin legend&quot;.</rdfs:comment>
        <rdfs:isDefinedBy rdf:resource="https://w3id.org/arco/ontology/arco"/>
        <rdfs:label xml:lang="en">is reference coin legend of</rdfs:label>
        <rdfs:label xml:lang="it">è legenda tipo di</rdfs:label>
        <owl:versionInfo xml:lang="it">stabile</owl:versionInfo>
        <owl:versionInfo xml:lang="en">stable</owl:versionInfo>
    </owl:ObjectProperty>
    


    <!-- https://w3id.org/arco/ontology/arco/isRelatedAgencyOf -->

    <owl:ObjectProperty rdf:about="https://w3id.org/arco/ontology/arco/isRelatedAgencyOf">
        <rdfs:domain rdf:resource="https://w3id.org/italia/onto/l0/Agent"/>
        <rdfs:range rdf:resource="https://w3id.org/arco/ontology/arco/CulturalProperty"/>
        <rdfs:comment xml:lang="it">Questa proprietà, inversa a &quot;ha ente collegato&quot;, rappresenta la relazione che collega un ente che riveste un ruolo nei confronti di un bene culturale al bene culturale stesso. La relazione tra il ruolo e l&apos;ente che lo riveste è espressa, in maniera generica, nel nome della proprietà, che quindi ne fornisce una rappresentazione semplificata, con ridotta espressività. La proprietà è specializzata per mezzo di sottoproprietà. Nell&apos;ontologia questa relazione è modellata anche, in maniera più espressiva, dalla classe TimeIndexedRole, che permette di collegare l&apos;ente, il suo ruolo e la sua corrispondente estensione temporale.</rdfs:comment>
        <rdfs:comment xml:lang="en">This property, inverse of &quot;has related agency&quot;, relates an agency that plays a role related to a cultural property to that cultural property. The relation is declared in the name of the property, but within the ontology this relation is also modeled, in a more expressive way, through the class AgentRole.</rdfs:comment>
        <rdfs:isDefinedBy rdf:resource="https://w3id.org/arco/ontology/arco"/>
        <rdfs:label xml:lang="en">is related agency of</rdfs:label>
        <rdfs:label xml:lang="it">è ente collegato a</rdfs:label>
        <owl:versionInfo xml:lang="it">stabile</owl:versionInfo>
        <owl:versionInfo xml:lang="en">stable</owl:versionInfo>
    </owl:ObjectProperty>
    


    <!-- https://w3id.org/arco/ontology/arco/isThematicCategoryOf -->

    <owl:ObjectProperty rdf:about="https://w3id.org/arco/ontology/arco/isThematicCategoryOf">
        <rdfs:subPropertyOf rdf:resource="https://w3id.org/arco/ontology/core/isCategoryOf"/>
        <rdfs:domain rdf:resource="https://w3id.org/arco/ontology/arco/ThematicCategory"/>
        <rdfs:range rdf:resource="https://w3id.org/arco/ontology/arco/CartographicClassification"/>
        <rdfs:comment xml:lang="it">Questa è la proprietà inversa di &quot;ha categoria tematica&quot;.</rdfs:comment>
        <rdfs:comment xml:lang="en">This is the inverse property of &quot;has thematic category&quot;.</rdfs:comment>
        <rdfs:isDefinedBy rdf:resource="https://w3id.org/arco/ontology/arco"/>
        <rdfs:label xml:lang="en">is thematic category of</rdfs:label>
        <rdfs:label xml:lang="it">è categoria tematica di</rdfs:label>
        <owl:versionInfo xml:lang="it">stabile</owl:versionInfo>
        <owl:versionInfo xml:lang="en">stable</owl:versionInfo>
    </owl:ObjectProperty>
    


    <!-- https://w3id.org/arco/ontology/catalogue/isRelatedToAdditionalForm -->

    <owl:ObjectProperty rdf:about="https://w3id.org/arco/ontology/catalogue/isRelatedToAdditionalForm"/>
    


    <!-- https://w3id.org/arco/ontology/catalogue/isRelatedToInformationForm -->

    <owl:ObjectProperty rdf:about="https://w3id.org/arco/ontology/catalogue/isRelatedToInformationForm"/>
    


    <!-- https://w3id.org/arco/ontology/context-description/hasAcquisition -->

    <owl:ObjectProperty rdf:about="https://w3id.org/arco/ontology/context-description/hasAcquisition"/>
    


    <!-- https://w3id.org/arco/ontology/context-description/hasAuthor -->

    <owl:ObjectProperty rdf:about="https://w3id.org/arco/ontology/context-description/hasAuthor"/>
    


    <!-- https://w3id.org/arco/ontology/context-description/hasAuthorshipAttribution -->

    <owl:ObjectProperty rdf:about="https://w3id.org/arco/ontology/context-description/hasAuthorshipAttribution"/>
    


    <!-- https://w3id.org/arco/ontology/context-description/hasBibliography -->

    <owl:ObjectProperty rdf:about="https://w3id.org/arco/ontology/context-description/hasBibliography"/>
    


    <!-- https://w3id.org/arco/ontology/context-description/hasBiologicalTaxonomy -->

    <owl:ObjectProperty rdf:about="https://w3id.org/arco/ontology/context-description/hasBiologicalTaxonomy"/>
    


    <!-- https://w3id.org/arco/ontology/context-description/hasChangeOfAvailability -->

    <owl:ObjectProperty rdf:about="https://w3id.org/arco/ontology/context-description/hasChangeOfAvailability"/>
    


    <!-- https://w3id.org/arco/ontology/context-description/hasCoinIssuance -->

    <owl:ObjectProperty rdf:about="https://w3id.org/arco/ontology/context-description/hasCoinIssuance"/>
    


    <!-- https://w3id.org/arco/ontology/context-description/hasCommission -->

    <owl:ObjectProperty rdf:about="https://w3id.org/arco/ontology/context-description/hasCommission"/>
    


    <!-- https://w3id.org/arco/ontology/context-description/hasDating -->

    <owl:ObjectProperty rdf:about="https://w3id.org/arco/ontology/context-description/hasDating"/>
    


    <!-- https://w3id.org/arco/ontology/context-description/hasDetectionMethod -->

    <owl:ObjectProperty rdf:about="https://w3id.org/arco/ontology/context-description/hasDetectionMethod"/>
    


    <!-- https://w3id.org/arco/ontology/context-description/hasDocumentation -->

    <owl:ObjectProperty rdf:about="https://w3id.org/arco/ontology/context-description/hasDocumentation"/>
    


    <!-- https://w3id.org/arco/ontology/context-description/hasEstimate -->

    <owl:ObjectProperty rdf:about="https://w3id.org/arco/ontology/context-description/hasEstimate"/>
    


    <!-- https://w3id.org/arco/ontology/context-description/hasExportImportCertification -->

    <owl:ObjectProperty rdf:about="https://w3id.org/arco/ontology/context-description/hasExportImportCertification"/>
    


    <!-- https://w3id.org/arco/ontology/context-description/hasFindingContext -->

    <owl:ObjectProperty rdf:about="https://w3id.org/arco/ontology/context-description/hasFindingContext"/>
    


    <!-- https://w3id.org/arco/ontology/context-description/hasFruition -->

    <owl:ObjectProperty rdf:about="https://w3id.org/arco/ontology/context-description/hasFruition"/>
    


    <!-- https://w3id.org/arco/ontology/context-description/hasIntervention -->

    <owl:ObjectProperty rdf:about="https://w3id.org/arco/ontology/context-description/hasIntervention"/>
    


    <!-- https://w3id.org/arco/ontology/context-description/hasInventory -->

    <owl:ObjectProperty rdf:about="https://w3id.org/arco/ontology/context-description/hasInventory"/>
    


    <!-- https://w3id.org/arco/ontology/context-description/hasLegalSituation -->

    <owl:ObjectProperty rdf:about="https://w3id.org/arco/ontology/context-description/hasLegalSituation"/>
    


    <!-- https://w3id.org/arco/ontology/context-description/hasMusicalEnsemble -->

    <owl:ObjectProperty rdf:about="https://w3id.org/arco/ontology/context-description/hasMusicalEnsemble"/>
    


    <!-- https://w3id.org/arco/ontology/context-description/hasMusician -->

    <owl:ObjectProperty rdf:about="https://w3id.org/arco/ontology/context-description/hasMusician"/>
    


    <!-- https://w3id.org/arco/ontology/context-description/hasPrimaryDocumentation -->

    <owl:ObjectProperty rdf:about="https://w3id.org/arco/ontology/context-description/hasPrimaryDocumentation"/>
    


    <!-- https://w3id.org/arco/ontology/context-description/hasProtectiveMeasure -->

    <owl:ObjectProperty rdf:about="https://w3id.org/arco/ontology/context-description/hasProtectiveMeasure"/>
    


    <!-- https://w3id.org/arco/ontology/context-description/hasRelatedWorkSituation -->

    <owl:ObjectProperty rdf:about="https://w3id.org/arco/ontology/context-description/hasRelatedWorkSituation"/>
    


    <!-- https://w3id.org/arco/ontology/context-description/hasResearch -->

    <owl:ObjectProperty rdf:about="https://w3id.org/arco/ontology/context-description/hasResearch"/>
    


    <!-- https://w3id.org/arco/ontology/context-description/hasResponsibility -->

    <owl:ObjectProperty rdf:about="https://w3id.org/arco/ontology/context-description/hasResponsibility"/>
    


    <!-- https://w3id.org/arco/ontology/context-description/hasSubject -->

    <owl:ObjectProperty rdf:about="https://w3id.org/arco/ontology/context-description/hasSubject"/>
    


    <!-- https://w3id.org/arco/ontology/context-description/hasSurvey -->

    <owl:ObjectProperty rdf:about="https://w3id.org/arco/ontology/context-description/hasSurvey"/>
    


    <!-- https://w3id.org/arco/ontology/context-description/hasTitle -->

    <owl:ObjectProperty rdf:about="https://w3id.org/arco/ontology/context-description/hasTitle"/>
    


    <!-- https://w3id.org/arco/ontology/context-description/hasUrbanPlanningInstrument -->

    <owl:ObjectProperty rdf:about="https://w3id.org/arco/ontology/context-description/hasUrbanPlanningInstrument"/>
    


    <!-- https://w3id.org/arco/ontology/context-description/hasUse -->

    <owl:ObjectProperty rdf:about="https://w3id.org/arco/ontology/context-description/hasUse"/>
    


    <!-- https://w3id.org/arco/ontology/context-description/isCoinMemberOf -->

    <owl:ObjectProperty rdf:about="https://w3id.org/arco/ontology/context-description/isCoinMemberOf"/>
    


    <!-- https://w3id.org/arco/ontology/context-description/isMemberOfCollection -->

    <owl:ObjectProperty rdf:about="https://w3id.org/arco/ontology/context-description/isMemberOfCollection"/>
    


    <!-- https://w3id.org/arco/ontology/context-description/isMemberOfPhotographicSeries -->

    <owl:ObjectProperty rdf:about="https://w3id.org/arco/ontology/context-description/isMemberOfPhotographicSeries"/>
    


    <!-- https://w3id.org/arco/ontology/core/hasAgent -->

    <owl:ObjectProperty rdf:about="https://w3id.org/arco/ontology/core/hasAgent"/>
    


    <!-- https://w3id.org/arco/ontology/core/hasAgentRole -->

    <owl:ObjectProperty rdf:about="https://w3id.org/arco/ontology/core/hasAgentRole"/>
    


    <!-- https://w3id.org/arco/ontology/core/hasCategory -->

    <owl:ObjectProperty rdf:about="https://w3id.org/arco/ontology/core/hasCategory"/>
    


    <!-- https://w3id.org/arco/ontology/core/hasClassification -->

    <owl:ObjectProperty rdf:about="https://w3id.org/arco/ontology/core/hasClassification"/>
    


    <!-- https://w3id.org/arco/ontology/core/hasComponent -->

    <owl:ObjectProperty rdf:about="https://w3id.org/arco/ontology/core/hasComponent">
        <rdfs:subPropertyOf rdf:resource="https://w3id.org/arco/ontology/arco/hasCulturalPropertyResidual"/>
    </owl:ObjectProperty>
    


    <!-- https://w3id.org/arco/ontology/core/hasConcept -->

    <owl:ObjectProperty rdf:about="https://w3id.org/arco/ontology/core/hasConcept"/>
    


    <!-- https://w3id.org/arco/ontology/core/hasPart -->

    <owl:ObjectProperty rdf:about="https://w3id.org/arco/ontology/core/hasPart"/>
    


    <!-- https://w3id.org/arco/ontology/core/hasType -->

    <owl:ObjectProperty rdf:about="https://w3id.org/arco/ontology/core/hasType"/>
    


    <!-- https://w3id.org/arco/ontology/core/isCategoryOf -->

    <owl:ObjectProperty rdf:about="https://w3id.org/arco/ontology/core/isCategoryOf"/>
    


    <!-- https://w3id.org/arco/ontology/core/isClassificationOf -->

    <owl:ObjectProperty rdf:about="https://w3id.org/arco/ontology/core/isClassificationOf"/>
    


    <!-- https://w3id.org/arco/ontology/core/isConceptOf -->

    <owl:ObjectProperty rdf:about="https://w3id.org/arco/ontology/core/isConceptOf"/>
    


    <!-- https://w3id.org/arco/ontology/core/isPartOf -->

    <owl:ObjectProperty rdf:about="https://w3id.org/arco/ontology/core/isPartOf"/>
    


    <!-- https://w3id.org/arco/ontology/core/isTypeOf -->

    <owl:ObjectProperty rdf:about="https://w3id.org/arco/ontology/core/isTypeOf"/>
    


    <!-- https://w3id.org/arco/ontology/denotative-description/hasAccessory -->

    <owl:ObjectProperty rdf:about="https://w3id.org/arco/ontology/denotative-description/hasAccessory"/>
    


    <!-- https://w3id.org/arco/ontology/denotative-description/hasAffixedElement -->

    <owl:ObjectProperty rdf:about="https://w3id.org/arco/ontology/denotative-description/hasAffixedElement"/>
    


    <!-- https://w3id.org/arco/ontology/denotative-description/hasConservationStatus -->

    <owl:ObjectProperty rdf:about="https://w3id.org/arco/ontology/denotative-description/hasConservationStatus"/>
    


    <!-- https://w3id.org/arco/ontology/denotative-description/hasCulturalPropertyAccessibility -->

    <owl:ObjectProperty rdf:about="https://w3id.org/arco/ontology/denotative-description/hasCulturalPropertyAccessibility"/>
    


    <!-- https://w3id.org/arco/ontology/denotative-description/hasCulturalPropertyAvailability -->

    <owl:ObjectProperty rdf:about="https://w3id.org/arco/ontology/denotative-description/hasCulturalPropertyAvailability"/>
    


    <!-- https://w3id.org/arco/ontology/denotative-description/hasCulturalPropertyType -->

    <owl:ObjectProperty rdf:about="https://w3id.org/arco/ontology/denotative-description/hasCulturalPropertyType"/>
    


    <!-- https://w3id.org/arco/ontology/denotative-description/hasDesignationInTime -->

    <owl:ObjectProperty rdf:about="https://w3id.org/arco/ontology/denotative-description/hasDesignationInTime"/>
    


    <!-- https://w3id.org/arco/ontology/denotative-description/hasFunctionalPurpose -->

    <owl:ObjectProperty rdf:about="https://w3id.org/arco/ontology/denotative-description/hasFunctionalPurpose"/>
    


    <!-- https://w3id.org/arco/ontology/denotative-description/hasIconographicOrDecorativeApparatus -->

    <owl:ObjectProperty rdf:about="https://w3id.org/arco/ontology/denotative-description/hasIconographicOrDecorativeApparatus"/>
    


    <!-- https://w3id.org/arco/ontology/denotative-description/hasLocationSubject -->

    <owl:ObjectProperty rdf:about="https://w3id.org/arco/ontology/denotative-description/hasLocationSubject"/>
    


    <!-- https://w3id.org/arco/ontology/denotative-description/hasMeasurementCollection -->

    <owl:ObjectProperty rdf:about="https://w3id.org/arco/ontology/denotative-description/hasMeasurementCollection"/>
    


    <!-- https://w3id.org/arco/ontology/denotative-description/hasOrientation -->

    <owl:ObjectProperty rdf:about="https://w3id.org/arco/ontology/denotative-description/hasOrientation"/>
    


    <!-- https://w3id.org/arco/ontology/denotative-description/hasSampleCollected -->

    <owl:ObjectProperty rdf:about="https://w3id.org/arco/ontology/denotative-description/hasSampleCollected"/>
    


    <!-- https://w3id.org/arco/ontology/denotative-description/hasTechnicalStatus -->

    <owl:ObjectProperty rdf:about="https://w3id.org/arco/ontology/denotative-description/hasTechnicalStatus"/>
    


    <!-- https://w3id.org/arco/ontology/location/hasCadastralIdentity -->

    <owl:ObjectProperty rdf:about="https://w3id.org/arco/ontology/location/hasCadastralIdentity"/>
    


    <!-- https://w3id.org/arco/ontology/location/hasCulturalPropertyAddress -->

    <owl:ObjectProperty rdf:about="https://w3id.org/arco/ontology/location/hasCulturalPropertyAddress"/>
    


    <!-- https://w3id.org/arco/ontology/location/hasStratigraphicArea -->

    <owl:ObjectProperty rdf:about="https://w3id.org/arco/ontology/location/hasStratigraphicArea"/>
    


    <!-- https://w3id.org/arco/ontology/location/hasStratigraphicRoom -->

    <owl:ObjectProperty rdf:about="https://w3id.org/arco/ontology/location/hasStratigraphicRoom"/>
    


    <!-- https://w3id.org/arco/ontology/location/hasStratigraphicSquare -->

    <owl:ObjectProperty rdf:about="https://w3id.org/arco/ontology/location/hasStratigraphicSquare"/>
    


    <!-- https://w3id.org/arco/ontology/location/hasTimeIndexedTypedLocation -->

    <owl:ObjectProperty rdf:about="https://w3id.org/arco/ontology/location/hasTimeIndexedTypedLocation"/>
    


    <!-- https://w3id.org/arco/ontology/location/hasTypeOfContext -->

    <owl:ObjectProperty rdf:about="https://w3id.org/arco/ontology/location/hasTypeOfContext"/>
    


    <!-- https://w3id.org/arco/ontology/movable-property/hasAccession -->

    <owl:ObjectProperty rdf:about="https://w3id.org/arco/ontology/movable-property/hasAccession"/>
    


    <!-- https://w3id.org/italia/onto/CLV/hasGeometry -->

    <owl:ObjectProperty rdf:about="https://w3id.org/italia/onto/CLV/hasGeometry"/>
    


    <!-- https://w3id.org/italia/onto/RO/isRoleInTimeOf -->

    <owl:ObjectProperty rdf:about="https://w3id.org/italia/onto/RO/isRoleInTimeOf"/>
    


    <!-- 
    ///////////////////////////////////////////////////////////////////////////////////////
    //
    // Data properties
    //
    ///////////////////////////////////////////////////////////////////////////////////////
     -->

    


    <!-- https://w3id.org/arco/ontology/arco/HSDefinition -->

    <owl:DatatypeProperty rdf:about="https://w3id.org/arco/ontology/arco/HSDefinition">
        <rdfs:domain rdf:resource="https://w3id.org/arco/ontology/arco/HornbostelSachsClassification"/>
        <rdfs:range rdf:resource="http://www.w3.org/2000/01/rdf-schema#Literal"/>
        <rdfs:comment xml:lang="it">Questa proprietà rappresenta la definizione associata allo strumento musicale, secondo la classificazione Hornbostel-Sachs.</rdfs:comment>
        <rdfs:comment xml:lang="en">This property represents the definition associated to a musical instrument, according to the Hornbostel-Sachs classification.</rdfs:comment>
        <rdfs:isDefinedBy rdf:resource="https://w3id.org/arco/ontology/arco"/>
        <rdfs:label xml:lang="en">Hornbostel-Sachs definition</rdfs:label>
        <rdfs:label xml:lang="it">definizione Hornbostel-Sachs</rdfs:label>
        <owl:versionInfo xml:lang="it">stabile</owl:versionInfo>
        <owl:versionInfo xml:lang="en">stable</owl:versionInfo>
        <a-cat:iccdNormTag>Normativa SM 4.00: CL/CHS/CHSD</a-cat:iccdNormTag>
    </owl:DatatypeProperty>
    


    <!-- https://w3id.org/arco/ontology/arco/HSEdition -->

    <owl:DatatypeProperty rdf:about="https://w3id.org/arco/ontology/arco/HSEdition">
        <rdfs:domain rdf:resource="https://w3id.org/arco/ontology/arco/HornbostelSachsClassification"/>
        <rdfs:range rdf:resource="http://www.w3.org/2000/01/rdf-schema#Literal"/>
        <rdfs:comment xml:lang="it">Questa proprietà rappresenta l&apos;indicazione bibliografica dell&apos;edizione Hornbostel-Sachs utilizzata per la classificazione dello strumento musicale.</rdfs:comment>
        <rdfs:comment xml:lang="en">This property represents the edition Horbonstel-Sachs used for classifying a musical instrument.</rdfs:comment>
        <rdfs:isDefinedBy rdf:resource="https://w3id.org/arco/ontology/arco"/>
        <rdfs:label xml:lang="en">Hornbostel-Sachs edition</rdfs:label>
        <rdfs:label xml:lang="it">edizione Hornbostel-Sachs</rdfs:label>
        <owl:versionInfo xml:lang="it">stabile</owl:versionInfo>
        <owl:versionInfo xml:lang="en">stable</owl:versionInfo>
        <a-cat:iccdNormTag>Normativa SM 4.00: CL/CHS/CHSE</a-cat:iccdNormTag>
    </owl:DatatypeProperty>
    


    <!-- https://w3id.org/arco/ontology/arco/HSNumber -->

    <owl:DatatypeProperty rdf:about="https://w3id.org/arco/ontology/arco/HSNumber">
        <rdfs:subPropertyOf rdf:resource="https://w3id.org/italia/onto/l0/identifier"/>
        <rdf:type rdf:resource="http://www.w3.org/2002/07/owl#FunctionalProperty"/>
        <rdfs:domain rdf:resource="https://w3id.org/arco/ontology/arco/HornbostelSachsClassification"/>
        <rdfs:range rdf:resource="http://www.w3.org/2000/01/rdf-schema#Literal"/>
        <rdfs:comment xml:lang="it">Questa proprietà rappresenta il codice numerico, secondo l&apos;edizione specifica Hornbostel-Sachs, associato allo strumento musicale nell&apos;ambito della classificazione Hornbostel-Sachs.</rdfs:comment>
        <rdfs:comment xml:lang="en">This property represents the numerical code associated to a musical instrument according to a specific edition of the Hornbostel-Sachs classification.</rdfs:comment>
        <rdfs:isDefinedBy rdf:resource="https://w3id.org/arco/ontology/arco"/>
        <rdfs:label xml:lang="it">Codice numerico Hornbostel-Sachs</rdfs:label>
        <rdfs:label xml:lang="en">Hornbostel-Sachs number</rdfs:label>
        <owl:versionInfo xml:lang="it">stabile</owl:versionInfo>
        <owl:versionInfo xml:lang="en">stable</owl:versionInfo>
        <a-cat:iccdNormTag>Normativa SM 4.00: CL/CHS/CHSN</a-cat:iccdNormTag>
    </owl:DatatypeProperty>
    


    <!-- https://w3id.org/arco/ontology/arco/RVERidentifier -->

    <owl:DatatypeProperty rdf:about="https://w3id.org/arco/ontology/arco/RVERidentifier">
        <rdfs:subPropertyOf rdf:resource="https://w3id.org/italia/onto/l0/identifier"/>
    </owl:DatatypeProperty>
    


    <!-- https://w3id.org/arco/ontology/arco/archaeologicalSiteIdentifier -->

    <owl:DatatypeProperty rdf:about="https://w3id.org/arco/ontology/arco/archaeologicalSiteIdentifier">
        <rdfs:subPropertyOf rdf:resource="https://w3id.org/italia/onto/l0/identifier"/>
        <rdf:type rdf:resource="http://www.w3.org/2002/07/owl#FunctionalProperty"/>
        <rdfs:domain rdf:resource="https://w3id.org/arco/ontology/arco/ArchaeologicalProperty"/>
        <rdfs:range rdf:resource="http://www.w3.org/2000/01/rdf-schema#Literal"/>
        <rdfs:comment xml:lang="it">Questa proprietà rappresenta la sigla del saggio stratigrafico.</rdfs:comment>
        <rdfs:comment xml:lang="en">This property represents the archaeological site identifier.</rdfs:comment>
        <rdfs:isDefinedBy rdf:resource="https://w3id.org/arco/ontology/arco"/>
        <rdfs:label xml:lang="en">archaeological site identifier</rdfs:label>
        <rdfs:label xml:lang="it">sigla identificativa del saggio stratigrafico</rdfs:label>
        <owl:versionInfo xml:lang="it">stabile</owl:versionInfo>
        <owl:versionInfo xml:lang="en">stable</owl:versionInfo>
        <a-cat:iccdNormTag>ICCD Normativa SAS: OG/OGT/OGTI</a-cat:iccdNormTag>
    </owl:DatatypeProperty>
    


    <!-- https://w3id.org/arco/ontology/arco/cartographicSymbolIdentifier -->

    <owl:DatatypeProperty rdf:about="https://w3id.org/arco/ontology/arco/cartographicSymbolIdentifier">
        <rdfs:subPropertyOf rdf:resource="https://w3id.org/italia/onto/l0/identifier"/>
        <rdfs:domain rdf:resource="https://w3id.org/arco/ontology/arco/CartographicSymbol"/>
        <rdfs:range rdf:resource="http://www.w3.org/2000/01/rdf-schema#Literal"/>
        <rdfs:comment xml:lang="it">Questa proprietà rappresenta il codice identificativo attribuito al simbolo cartografico.</rdfs:comment>
        <rdfs:comment xml:lang="en">This property represents the identifier associated to the cartographic symbol.</rdfs:comment>
        <rdfs:isDefinedBy rdf:resource="https://w3id.org/arco/ontology/arco"/>
        <rdfs:label xml:lang="en">cartographic symbol identifier</rdfs:label>
        <rdfs:label xml:lang="it">identificativo del simbolo cartografico</rdfs:label>
        <owl:versionInfo xml:lang="it">stabile</owl:versionInfo>
        <owl:versionInfo xml:lang="en">stable</owl:versionInfo>
        <a-cat:iccdNormTag>ICCD Normativa Trasversale 4.00: CT/CTM/CTMS</a-cat:iccdNormTag>
    </owl:DatatypeProperty>
    


    <!-- https://w3id.org/arco/ontology/arco/catalogueNumber -->

    <owl:DatatypeProperty rdf:about="https://w3id.org/arco/ontology/arco/catalogueNumber">
        <rdfs:subPropertyOf rdf:resource="https://w3id.org/italia/onto/l0/identifier"/>
        <rdf:type rdf:resource="http://www.w3.org/2002/07/owl#FunctionalProperty"/>
        <rdfs:domain rdf:resource="https://w3id.org/arco/ontology/arco/CulturalProperty"/>
        <rdfs:range rdf:resource="http://www.w3.org/2000/01/rdf-schema#Literal"/>
        <rdfs:comment xml:lang="it">Questa proprietà permette di associare il numero di catalogo generale a un bene culturale descritto in una scheda catalografica.</rdfs:comment>
        <rdfs:comment xml:lang="en">This property represents the general catalogue number associated to a cultural property described by a catalogue record.</rdfs:comment>
        <rdfs:isDefinedBy rdf:resource="https://w3id.org/arco/ontology/arco"/>
        <rdfs:label xml:lang="en">catalogue number</rdfs:label>
        <rdfs:label xml:lang="it">numero catalogo generale</rdfs:label>
        <owl:versionInfo xml:lang="it">stabile</owl:versionInfo>
        <owl:versionInfo xml:lang="en">stable</owl:versionInfo>
        <a-cat:iccdNormTag>ICCD Normativa Trasversale 4.00: CD/NCT/NCTN</a-cat:iccdNormTag>
    </owl:DatatypeProperty>
    


    <!-- https://w3id.org/arco/ontology/arco/classifiedSubject -->

    <owl:DatatypeProperty rdf:about="https://w3id.org/arco/ontology/arco/classifiedSubject">
        <rdf:type rdf:resource="http://www.w3.org/2002/07/owl#FunctionalProperty"/>
        <rdfs:domain rdf:resource="https://w3id.org/arco/ontology/arco/PhotographicHeritageClassification"/>
        <rdfs:range rdf:resource="http://www.w3.org/2000/01/rdf-schema#Literal"/>
        <rdfs:comment xml:lang="it">Questa proprietà rappresenta la descrizione codificata del/i soggetto/i raffigurato/i nell&apos;opera secondo il sistema di classificazione scelto dall&apos;Ente schedatore, in alternativa e/o in aggiunta ad Iconclass.</rdfs:comment>
        <rdfs:comment xml:lang="en">This property represents the subject of a photographic heritage as described in a photographic heritage classification other than Iconclass.</rdfs:comment>
        <rdfs:isDefinedBy rdf:resource="https://w3id.org/arco/ontology/arco"/>
        <rdfs:label xml:lang="en">classified subject</rdfs:label>
        <rdfs:label xml:lang="it">soggetto classificato</rdfs:label>
        <owl:versionInfo xml:lang="it">stabile</owl:versionInfo>
        <owl:versionInfo xml:lang="en">stable</owl:versionInfo>
        <a-cat:iccdNormTag>ICCD Normativa F 4.00: SG/CLF/CLFS</a-cat:iccdNormTag>
    </owl:DatatypeProperty>
    


    <!-- https://w3id.org/arco/ontology/arco/completedCollection -->

    <owl:DatatypeProperty rdf:about="https://w3id.org/arco/ontology/arco/completedCollection">
        <rdf:type rdf:resource="http://www.w3.org/2002/07/owl#FunctionalProperty"/>
        <rdfs:domain rdf:resource="https://w3id.org/arco/ontology/arco/CulturalPropertyCollection"/>
        <rdfs:range rdf:resource="http://www.w3.org/2001/XMLSchema#boolean"/>
        <rdfs:comment xml:lang="it">Questa proprietà segnala se la serie risulta completa o incompleta</rdfs:comment>
        <rdfs:comment xml:lang="en">This property indicates if the collection is completed or not</rdfs:comment>
        <rdfs:label xml:lang="it">collezione completa</rdfs:label>
        <rdfs:label xml:lang="en">completed collection</rdfs:label>
        <owl:versionInfo xml:lang="it">instabile</owl:versionInfo>
        <owl:versionInfo xml:lang="en">unstable</owl:versionInfo>
        <a-cat:iccdNormTag>ICCD normative F, MI, S: OG/QNT/QNTC</a-cat:iccdNormTag>
    </owl:DatatypeProperty>
    


    <!-- https://w3id.org/arco/ontology/arco/containerSequence -->

    <owl:DatatypeProperty rdf:about="https://w3id.org/arco/ontology/arco/containerSequence">
        <rdfs:comment xml:lang="it">Questa proprietà rappresenta il codice che definisce la sequenza dei contenitori.</rdfs:comment>
        <rdfs:comment xml:lang="en">Thisproperty represents the code defining the container sequence.</rdfs:comment>
        <rdfs:isDefinedBy rdf:resource="https://w3id.org/arco/ontology/arco"/>
        <rdfs:label xml:lang="it">codice sequenza</rdfs:label>
        <rdfs:label xml:lang="en">container sequence</rdfs:label>
        <owl:versionInfo xml:lang="it">instabile</owl:versionInfo>
        <owl:versionInfo xml:lang="en">unstable</owl:versionInfo>
        <a-cat:iccdNormTag>ICCD Normativa BNB: AC/ACZ</a-cat:iccdNormTag>
    </owl:DatatypeProperty>
    


    <!-- https://w3id.org/arco/ontology/arco/definitionAndPositionOfComponents -->

    <owl:DatatypeProperty rdf:about="https://w3id.org/arco/ontology/arco/definitionAndPositionOfComponents">
        <rdfs:domain rdf:resource="https://w3id.org/arco/ontology/arco/ComplexCulturalProperty"/>
        <rdfs:range rdf:resource="http://www.w3.org/2000/01/rdf-schema#Literal"/>
        <rdfs:comment xml:lang="it">Questa proprietà rappresenta le informazioni sulla definizione e posizione delle parti componenti di un bene culturale complesso.</rdfs:comment>
        <rdfs:comment xml:lang="en">This property represents information on definition and position of the components of a complex cultural property.</rdfs:comment>
        <rdfs:isDefinedBy rdf:resource="https://w3id.org/arco/ontology/arco"/>
        <rdfs:label xml:lang="en">definition and position of components</rdfs:label>
        <rdfs:label xml:lang="it">definizione e posizione delle parti componenti</rdfs:label>
        <owl:versionInfo xml:lang="it">stabile</owl:versionInfo>
        <owl:versionInfo xml:lang="en">stable</owl:versionInfo>
        <a-cat:iccdNormTag>ICCD Normativa Trasversale 4.00: OG/OGC/OGCD</a-cat:iccdNormTag>
    </owl:DatatypeProperty>
    


    <!-- https://w3id.org/arco/ontology/arco/digitalPhotographNote -->

    <owl:DatatypeProperty rdf:about="https://w3id.org/arco/ontology/arco/digitalPhotographNote">
        <rdfs:subPropertyOf rdf:resource="https://w3id.org/arco/ontology/core/note"/>
        <rdf:type rdf:resource="http://www.w3.org/2002/07/owl#FunctionalProperty"/>
        <rdfs:domain rdf:resource="https://w3id.org/arco/ontology/arco/PhotographicHeritage"/>
        <rdfs:range rdf:resource="http://www.w3.org/2000/01/rdf-schema#Literal"/>
        <rdfs:comment xml:lang="it">Questa proprietà rappresenta le note relative alla fotografia digitale. Può rappresentare informazioni utili a identificare le intenzioni dell&apos;autore in relazione alla visualizzazione o rioggettivazione della fotografia digitale, come la dimensione del quadro, la risoluzione di stampa e relativa unità di misura, altre indicazioni per la stampa (tipo stampante, correzioni cromatiche, ecc.), categoria, URL, ecc.</rdfs:comment>
        <rdfs:comment xml:lang="en">This property represents notes on a digital photograph.</rdfs:comment>
        <rdfs:isDefinedBy rdf:resource="https://w3id.org/arco/ontology/arco"/>
        <rdfs:label xml:lang="en">digital photograph note</rdfs:label>
        <rdfs:label xml:lang="it">note sulla fotografia digitale</rdfs:label>
        <owl:versionInfo xml:lang="it">stabile</owl:versionInfo>
        <owl:versionInfo xml:lang="en">stable</owl:versionInfo>
        <a-cat:iccdNormTag>ICCD Normativa F: MT/FVC/FVCV</a-cat:iccdNormTag>
    </owl:DatatypeProperty>
    


    <!-- https://w3id.org/arco/ontology/arco/endTime -->

    <owl:DatatypeProperty rdf:about="https://w3id.org/arco/ontology/arco/endTime">
        <rdfs:subPropertyOf rdf:resource="https://w3id.org/italia/onto/TI/time"/>
        <rdfs:domain rdf:resource="https://w3id.org/italia/onto/TI/TimeInterval"/>
        <rdfs:range rdf:resource="http://www.w3.org/2000/01/rdf-schema#Literal"/>
        <rdfs:comment xml:lang="it">Questa proprietà rappresenta la data di fine di un intervallo temporale, che può essere espressa secondo criteri diversi e a diverso livello di dettaglio (secolo, intervallo di secoli, anno, intervallo di anni, aaaa/mm/gg, periodo storico, etc.)</rdfs:comment>
        <rdfs:comment xml:lang="en">This property represents the end time of a time interval, according to different criteria and level of detail (century, century interval, year, yyyy/mm/dd, historical period, etc.).</rdfs:comment>
        <rdfs:isDefinedBy rdf:resource="https://w3id.org/arco/ontology/arco"/>
        <rdfs:label xml:lang="it">data di fine</rdfs:label>
        <rdfs:label xml:lang="en">end time</rdfs:label>
        <owl:versionInfo xml:lang="it">stabile</owl:versionInfo>
        <owl:versionInfo xml:lang="en">stable</owl:versionInfo>
    </owl:DatatypeProperty>
    


    <!-- https://w3id.org/arco/ontology/arco/internationalIdentifier -->

    <owl:DatatypeProperty rdf:about="https://w3id.org/arco/ontology/arco/internationalIdentifier">
        <rdfs:subPropertyOf rdf:resource="https://w3id.org/italia/onto/l0/identifier"/>
        <rdf:type rdf:resource="http://www.w3.org/2002/07/owl#FunctionalProperty"/>
        <rdfs:domain rdf:resource="https://w3id.org/arco/ontology/arco/CulturalProperty"/>
        <rdfs:range rdf:resource="http://www.w3.org/2000/01/rdf-schema#Literal"/>
        <rdfs:comment xml:lang="it">Questa proprietà rappresenta il numero di codice internazionale che identifica un bene scientifico e tecnologico. All&apos;indirizzo http://www.isin.org/ è possibile reperire tutte le specifiche per l&apos;adesione al progetto e l&apos;attribuzione del codice internazionale. Il Registro Online è un database che raccoglie informazioni su strumenti scientifici di interesse storico promosso dal Museum of the History of Science di Oxford in collaborazione con la Commissione Strumenti Scientifici dell&apos;International Union of the History and Philosophy of Science.</rdfs:comment>
        <rdfs:comment xml:lang="en">This property represents the international identifier of a scientific or technological heritage. More info can be found at https://www.isin.org/</rdfs:comment>
        <rdfs:isDefinedBy rdf:resource="https://w3id.org/arco/ontology/arco"/>
        <rdfs:label xml:lang="it">codice internazionale</rdfs:label>
        <rdfs:label xml:lang="en">international identifier</rdfs:label>
        <owl:versionInfo xml:lang="it">stabile</owl:versionInfo>
        <owl:versionInfo xml:lang="en">stable</owl:versionInfo>
        <a-cat:iccdNormTag>ICCD Normativa PST: AC/ACI</a-cat:iccdNormTag>
    </owl:DatatypeProperty>
    


    <!-- https://w3id.org/arco/ontology/arco/musicalInstrumentNote -->

    <owl:DatatypeProperty rdf:about="https://w3id.org/arco/ontology/arco/musicalInstrumentNote">
        <rdfs:subPropertyOf rdf:resource="https://w3id.org/arco/ontology/core/note"/>
        <rdf:type rdf:resource="http://www.w3.org/2002/07/owl#FunctionalProperty"/>
        <rdfs:domain rdf:resource="https://w3id.org/arco/ontology/arco/MusicHeritage"/>
        <rdfs:range rdf:resource="http://www.w3.org/2000/01/rdf-schema#Literal"/>
        <rdfs:comment xml:lang="it">Questa proprietà rappresenta le note relative agli aspetti acustici di uno strumento musicale, ed eventualmente anche relative ai rilevamenti e ai criteri adottati in sede di restauro.</rdfs:comment>
        <rdfs:comment xml:lang="en">This property represents notes on a musical instrument.</rdfs:comment>
        <rdfs:isDefinedBy rdf:resource="https://w3id.org/arco/ontology/arco"/>
        <rdfs:label xml:lang="en">musical instrument note</rdfs:label>
        <rdfs:label xml:lang="it">note sullo strumento musicale</rdfs:label>
        <owl:versionInfo xml:lang="it">stabile</owl:versionInfo>
        <owl:versionInfo xml:lang="en">stable</owl:versionInfo>
        <a-cat:iccdNormTag>ICCD Normativa SM 4.00: AA/AAS</a-cat:iccdNormTag>
    </owl:DatatypeProperty>
    


    <!-- https://w3id.org/arco/ontology/arco/numberOfArchaeologicalMaterials -->

    <owl:DatatypeProperty rdf:about="https://w3id.org/arco/ontology/arco/numberOfArchaeologicalMaterials">
        <rdfs:subPropertyOf rdf:resource="https://w3id.org/arco/ontology/arco/numberOfParts"/>
        <rdf:type rdf:resource="http://www.w3.org/2002/07/owl#FunctionalProperty"/>
        <rdfs:domain rdf:resource="https://w3id.org/arco/ontology/arco/ArchaeologicalMaterial"/>
        <rdfs:range rdf:resource="http://www.w3.org/2001/XMLSchema#integer"/>
        <rdfs:comment xml:lang="it">Questa proprietà rappresenta la quantità complessiva di uno stesso materiale archeologico componente di un lotto di materiali.</rdfs:comment>
        <rdfs:comment xml:lang="en">This property represents the total quantity of an archaeological material that is part of a lot of archaeological materials.</rdfs:comment>
        <rdfs:comment xml:lang="it">numero di materiali archeologici componenti</rdfs:comment>
        <rdfs:isDefinedBy rdf:resource="https://w3id.org/arco/ontology/arco"/>
        <rdfs:label xml:lang="en">number of archeological materials</rdfs:label>
        <owl:versionInfo xml:lang="it">stabile</owl:versionInfo>
        <owl:versionInfo xml:lang="en">stable</owl:versionInfo>
        <a-cat:iccdNormTag>ICCD Normativa TMA: MA/MAC/MACQ</a-cat:iccdNormTag>
    </owl:DatatypeProperty>
    


    <!-- https://w3id.org/arco/ontology/arco/numberOfComponents -->

    <owl:DatatypeProperty rdf:about="https://w3id.org/arco/ontology/arco/numberOfComponents">
        <rdfs:subPropertyOf rdf:resource="https://w3id.org/arco/ontology/arco/numberOfParts"/>
        <rdf:type rdf:resource="http://www.w3.org/2002/07/owl#FunctionalProperty"/>
        <rdfs:domain rdf:resource="https://w3id.org/arco/ontology/arco/ComplexCulturalProperty"/>
        <rdfs:range rdf:resource="http://www.w3.org/2000/01/rdf-schema#Literal"/>
        <rdfs:comment xml:lang="it">Questa proprietà rappresenta il numero di oggetti componenti di un bene culturale identificato come serie o come insieme.</rdfs:comment>
        <rdfs:comment xml:lang="en">This property represents the number of components of a complex cultural property.</rdfs:comment>
        <rdfs:isDefinedBy rdf:resource="https://w3id.org/arco/ontology/arco"/>
        <rdfs:label xml:lang="en">number of components</rdfs:label>
        <rdfs:label xml:lang="it">numero di componenti</rdfs:label>
        <owl:versionInfo xml:lang="it">stabile</owl:versionInfo>
        <owl:versionInfo xml:lang="en">stable</owl:versionInfo>
        <a-cat:iccdNormTag>ICCD Normativa Trasversale 4.00: OG/QNT/QNTN; OG/QNT/QNTS</a-cat:iccdNormTag>
    </owl:DatatypeProperty>
    


    <!-- https://w3id.org/arco/ontology/arco/numberOfCulturalPropertyParts -->

    <owl:DatatypeProperty rdf:about="https://w3id.org/arco/ontology/arco/numberOfCulturalPropertyParts">
        <rdfs:subPropertyOf rdf:resource="https://w3id.org/arco/ontology/arco/numberOfParts"/>
        <rdf:type rdf:resource="http://www.w3.org/2002/07/owl#FunctionalProperty"/>
        <rdfs:domain rdf:resource="https://w3id.org/arco/ontology/arco/CulturalPropertyPart"/>
        <rdfs:range rdf:resource="http://www.w3.org/2001/XMLSchema#integer"/>
        <rdfs:comment xml:lang="it">Questa proprietà rappresenta il numero di esemplari di una stessa parte di un bene culturale (es.: il numero di denti di un reperto antropologico)</rdfs:comment>
        <rdfs:comment xml:lang="en">This property represents the number of specimens of the same cultural property part (es.: the number of the teeth of an anthropological material).</rdfs:comment>
        <rdfs:isDefinedBy rdf:resource="https://w3id.org/arco/ontology/arco"/>
        <rdfs:label xml:lang="en">number of cultural property part</rdfs:label>
        <rdfs:label xml:lang="it">numero di parte di bene culturale</rdfs:label>
        <owl:versionInfo xml:lang="it">stabile</owl:versionInfo>
        <owl:versionInfo xml:lang="en">stable</owl:versionInfo>
        <a-cat:iccdNormTag>ICCD Normativa AT 3.01: EL/ELE/ELEM</a-cat:iccdNormTag>
    </owl:DatatypeProperty>
    


    <!-- https://w3id.org/arco/ontology/arco/numberOfElements -->

    <owl:DatatypeProperty rdf:about="https://w3id.org/arco/ontology/arco/numberOfElements">
        <rdfs:subPropertyOf rdf:resource="https://w3id.org/arco/ontology/arco/numberOfParts"/>
        <rdf:type rdf:resource="http://www.w3.org/2002/07/owl#FunctionalProperty"/>
        <rdfs:domain rdf:resource="https://w3id.org/arco/ontology/arco/ComplexCulturalProperty"/>
        <rdfs:range rdf:resource="http://www.w3.org/2001/XMLSchema#positiveInteger"/>
        <rdfs:comment xml:lang="it">Questa propietà rappresenta  il numero complessivo, espresso in cifre, degli elementi che costituiscono il bene catalogato, nel caso esso sia un insieme o una serie i cui esemplari/oggetti componenti comprendono ciascuno più elementi.</rdfs:comment>
        <rdfs:label xml:lang="en">This property represents the total number of elements of a complex cultural property, when it is composed by parts containing more elements.</rdfs:label>
        <rdfs:label xml:lang="en">number of elements</rdfs:label>
        <rdfs:label xml:lang="it">numero di elementi</rdfs:label>
        <owl:versionInfo xml:lang="it">instabile</owl:versionInfo>
        <owl:versionInfo xml:lang="en">unstable</owl:versionInfo>
        <a-cat:iccdNormTag>ICCD Normativa Trasversale 4.00: OG/QNT/QNTI; OG/QNT/QNTS</a-cat:iccdNormTag>
    </owl:DatatypeProperty>
    


    <!-- https://w3id.org/arco/ontology/arco/numberOfMembers -->

    <owl:DatatypeProperty rdf:about="https://w3id.org/arco/ontology/arco/numberOfMembers">
        <rdfs:subPropertyOf rdf:resource="https://w3id.org/arco/ontology/arco/numberOfParts"/>
        <rdf:type rdf:resource="http://www.w3.org/2002/07/owl#FunctionalProperty"/>
        <rdfs:domain rdf:resource="https://w3id.org/arco/ontology/arco/CulturalPropertyCollection"/>
        <rdfs:range rdf:resource="http://www.w3.org/2000/01/rdf-schema#Literal"/>
        <rdfs:comment xml:lang="it">Questa proprietà rappresenta il numero di membri di un bene culturale che si identifica come una collezione (es.: serie)</rdfs:comment>
        <rdfs:comment xml:lang="en">This property represents the number of members of a cultural property that is a collection (e.g.: series)</rdfs:comment>
        <rdfs:isDefinedBy rdf:resource="https://w3id.org/arco/ontology/arco"/>
        <rdfs:label xml:lang="en">number of members</rdfs:label>
        <rdfs:label xml:lang="it">numero di membri</rdfs:label>
        <owl:versionInfo xml:lang="it">stabile</owl:versionInfo>
        <owl:versionInfo xml:lang="en">stable</owl:versionInfo>
        <a-cat:iccdNormTag>ICCD Normativa Trasversale 4.00: OG/QNT/QNTN; OG/QNT/QNTI; OG/QNT/QNTS</a-cat:iccdNormTag>
    </owl:DatatypeProperty>
    


    <!-- https://w3id.org/arco/ontology/arco/numberOfParts -->

    <owl:DatatypeProperty rdf:about="https://w3id.org/arco/ontology/arco/numberOfParts">
        <rdf:type rdf:resource="http://www.w3.org/2002/07/owl#FunctionalProperty"/>
        <rdfs:domain rdf:resource="http://www.w3.org/2002/07/owl#Thing"/>
        <rdfs:range rdf:resource="http://www.w3.org/2001/XMLSchema#integer"/>
        <rdfs:comment xml:lang="it">Questa proprietà rappresenta il numero di parti di un&apos;entità.</rdfs:comment>
        <rdfs:comment xml:lang="en">This property represents the number of parts of an entity.</rdfs:comment>
        <rdfs:isDefinedBy rdf:resource="https://w3id.org/arco/ontology/arco"/>
        <rdfs:label xml:lang="en">number of parts</rdfs:label>
        <rdfs:label xml:lang="it">numero di parti</rdfs:label>
        <owl:versionInfo xml:lang="it">stabile</owl:versionInfo>
        <owl:versionInfo xml:lang="en">stable</owl:versionInfo>
    </owl:DatatypeProperty>
    


    <!-- https://w3id.org/arco/ontology/arco/numberOfResiduals -->

    <owl:DatatypeProperty rdf:about="https://w3id.org/arco/ontology/arco/numberOfResiduals">
        <rdfs:subPropertyOf rdf:resource="https://w3id.org/arco/ontology/arco/numberOfParts"/>
        <rdf:type rdf:resource="http://www.w3.org/2002/07/owl#FunctionalProperty"/>
        <rdfs:domain rdf:resource="https://w3id.org/arco/ontology/arco/CulturalPropertyResidual"/>
        <rdfs:range rdf:resource="http://www.w3.org/2001/XMLSchema#integer"/>
        <rdfs:comment xml:lang="it">Questa proprietà rappresenta il numero di parti residuali, nel caso in cui si stia descrivendo un bene di cui si conservano più parti residuali.</rdfs:comment>
        <rdfs:comment xml:lang="en">This property represents the number of residuals (only if more than one) of a cultural property.</rdfs:comment>
        <rdfs:isDefinedBy rdf:resource="https://w3id.org/arco/ontology/arco"/>
        <rdfs:label xml:lang="en">number of cultural property residual parts</rdfs:label>
        <rdfs:label xml:lang="it">numero di parti residuali di bene culturale</rdfs:label>
        <owl:versionInfo xml:lang="it">stabile</owl:versionInfo>
        <owl:versionInfo xml:lang="en">stable</owl:versionInfo>
        <a-cat:iccdNormTag>OG/QNT/QNTR</a-cat:iccdNormTag>
    </owl:DatatypeProperty>
    


    <!-- https://w3id.org/arco/ontology/arco/positionInSequence -->

    <owl:DatatypeProperty rdf:about="https://w3id.org/arco/ontology/arco/positionInSequence">
        <rdf:type rdf:resource="http://www.w3.org/2002/07/owl#FunctionalProperty"/>
        <rdfs:domain rdf:resource="https://w3id.org/arco/ontology/arco/CulturalPropertyComponent"/>
        <rdfs:range rdf:resource="http://www.w3.org/2001/XMLSchema#nonNegativeInteger"/>
        <rdfs:comment xml:lang="it">Questa proprietà rappresenta la posizione o il numero d’ordine dell’elemento all’interno del bene preso in considerazione.</rdfs:comment>
        <rdfs:comment xml:lang="en">This property represents the position of a cultural property component in the sequence to which it belogns.</rdfs:comment>
        <rdfs:isDefinedBy rdf:resource="https://w3id.org/arco/ontology/"/>
        <rdfs:label xml:lang="it">numero d&apos;ordine</rdfs:label>
        <rdfs:label xml:lang="en">position in sequence</rdfs:label>
        <owl:versionInfo xml:lang="it">instabile</owl:versionInfo>
        <owl:versionInfo xml:lang="en">unstable</owl:versionInfo>
        <a-cat:iccdNormTag>ICCD normative F, MI, OAC, S: OG/QNT/QNTO</a-cat:iccdNormTag>
    </owl:DatatypeProperty>
    


    <!-- https://w3id.org/arco/ontology/arco/previousIdentifier -->

    <owl:DatatypeProperty rdf:about="https://w3id.org/arco/ontology/arco/previousIdentifier">
        <rdfs:subPropertyOf rdf:resource="https://w3id.org/italia/onto/l0/identifier"/>
        <rdfs:range rdf:resource="http://www.w3.org/2000/01/rdf-schema#Literal"/>
        <rdfs:comment xml:lang="it">Questa proprietà rappresenta qualsiasi codice precedente a quello attuale che identifica il campione.</rdfs:comment>
        <rdfs:comment xml:lang="en">This property represents any previous identifier of the specimen.</rdfs:comment>
        <rdfs:isDefinedBy rdf:resource="https://w3id.org/arco/ontology/arco"/>
        <rdfs:label xml:lang="it">identificativo precedente</rdfs:label>
        <rdfs:label xml:lang="en">previous identifier</rdfs:label>
        <owl:versionInfo xml:lang="it">Instabile</owl:versionInfo>
        <owl:versionInfo xml:lang="en">unstable</owl:versionInfo>
        <a-cat:iccdNormTag>ICCD Normativa BNB: AC/ACN</a-cat:iccdNormTag>
    </owl:DatatypeProperty>
    


    <!-- https://w3id.org/arco/ontology/arco/regionIdentifier -->

    <owl:DatatypeProperty rdf:about="https://w3id.org/arco/ontology/arco/regionIdentifier">
        <rdfs:subPropertyOf rdf:resource="https://w3id.org/italia/onto/l0/identifier"/>
        <rdf:type rdf:resource="http://www.w3.org/2002/07/owl#FunctionalProperty"/>
        <rdfs:domain rdf:resource="https://w3id.org/arco/ontology/arco/CulturalProperty"/>
        <rdfs:range rdf:resource="http://www.w3.org/2000/01/rdf-schema#Literal"/>
        <rdfs:comment xml:lang="it">Questa proprietà permette di associare il codice regione a un bene culturale descritto in una scheda catalografica.</rdfs:comment>
        <rdfs:comment xml:lang="en">This property represents the &quot;region identifier&quot; associated to a cultural property described by a catalogue record.</rdfs:comment>
        <rdfs:isDefinedBy rdf:resource="https://w3id.org/arco/ontology/arco"/>
        <rdfs:label xml:lang="it">codice regione</rdfs:label>
        <rdfs:label xml:lang="en">region identifier</rdfs:label>
        <owl:versionInfo xml:lang="it">stabile</owl:versionInfo>
        <owl:versionInfo xml:lang="en">stable</owl:versionInfo>
        <a-cat:iccdNormTag>ICCD Normativa Trasversale 4.00: CD/NCT/NCTR</a-cat:iccdNormTag>
    </owl:DatatypeProperty>
    


    <!-- https://w3id.org/arco/ontology/arco/startTime -->

    <owl:DatatypeProperty rdf:about="https://w3id.org/arco/ontology/arco/startTime">
        <rdfs:subPropertyOf rdf:resource="https://w3id.org/italia/onto/TI/time"/>
        <rdfs:domain rdf:resource="https://w3id.org/italia/onto/TI/TimeInterval"/>
        <rdfs:range rdf:resource="http://www.w3.org/2000/01/rdf-schema#Literal"/>
        <rdfs:comment xml:lang="it">Questa proprietà rappresenta la data di inizio di un intervallo temporale, che può essere espressa secondo criteri diversi e a diverso livello di dettaglio (secolo, intervallo di secoli, anno, intervallo di anni, aaaa/mm/gg, periodo storico, etc.)</rdfs:comment>
        <rdfs:comment xml:lang="en">This property represents the start time of a time interval, according to different criteria and level of detail (century, century interval, year, yyyy/mm/dd, historical period, etc.).</rdfs:comment>
        <rdfs:isDefinedBy rdf:resource="https://w3id.org/arco/ontology/arco"/>
        <rdfs:label xml:lang="it">data di inizio</rdfs:label>
        <rdfs:label xml:lang="en">start time</rdfs:label>
        <owl:versionInfo xml:lang="it">stabile</owl:versionInfo>
        <owl:versionInfo xml:lang="en">stable</owl:versionInfo>
    </owl:DatatypeProperty>
    


    <!-- https://w3id.org/arco/ontology/arco/suffix -->

    <owl:DatatypeProperty rdf:about="https://w3id.org/arco/ontology/arco/suffix">
        <rdfs:subPropertyOf rdf:resource="https://w3id.org/italia/onto/l0/identifier"/>
        <rdf:type rdf:resource="http://www.w3.org/2002/07/owl#FunctionalProperty"/>
        <rdfs:domain rdf:resource="https://w3id.org/arco/ontology/arco/CulturalProperty"/>
        <rdfs:range rdf:resource="http://www.w3.org/2000/01/rdf-schema#Literal"/>
        <rdfs:comment xml:lang="it">Questa proprietà permette di associare il suffisso a un bene culturale descritto in una scheda catalografica.</rdfs:comment>
        <rdfs:comment xml:lang="en">This property represents the &quot;suffix&quot; associated to a cultural property described by a catalogue record.</rdfs:comment>
        <rdfs:isDefinedBy rdf:resource="https://w3id.org/arco/ontology/arco"/>
        <rdfs:label xml:lang="it">suffisso</rdfs:label>
        <rdfs:label xml:lang="en">suffix</rdfs:label>
        <owl:versionInfo xml:lang="it">stabile</owl:versionInfo>
        <owl:versionInfo xml:lang="en">stable</owl:versionInfo>
        <a-cat:iccdNormTag>ICCD Normativa Trasversale 4.00: CD/NCT/NCTS</a-cat:iccdNormTag>
    </owl:DatatypeProperty>
    


    <!-- https://w3id.org/arco/ontology/arco/taxon -->

    <owl:DatatypeProperty rdf:about="https://w3id.org/arco/ontology/arco/taxon">
        <rdfs:domain rdf:resource="https://w3id.org/arco/ontology/arco/AlternativeMusicalInstrumentClassification"/>
        <rdfs:range rdf:resource="http://www.w3.org/2000/01/rdf-schema#Literal"/>
        <rdfs:comment xml:lang="it">Questa proprietà rappresenta il codice tassonomico e la definizione attribuiti allo strumento musicale schedato nell&apos;ambito del sistema di classificazione preso in considerazione.</rdfs:comment>
        <rdfs:comment xml:lang="en">This property represents the taxon code and the taxon definition associated to the musical instrument, according to a musical instrument classification.</rdfs:comment>
        <rdfs:isDefinedBy rdf:resource="https://w3id.org/arco/ontology/arco"/>
        <rdfs:label xml:lang="en">taxon</rdfs:label>
        <rdfs:label xml:lang="it">taxon</rdfs:label>
        <owl:versionInfo xml:lang="it">stabile</owl:versionInfo>
        <owl:versionInfo xml:lang="en">stable</owl:versionInfo>
        <a-cat:iccdNormTag>Normativa SM 4.00: CL/CLA/CLAT</a-cat:iccdNormTag>
    </owl:DatatypeProperty>
    


    <!-- https://w3id.org/arco/ontology/arco/uniqueIdentifier -->

    <owl:DatatypeProperty rdf:about="https://w3id.org/arco/ontology/arco/uniqueIdentifier">
        <rdfs:subPropertyOf rdf:resource="https://w3id.org/italia/onto/l0/identifier"/>
        <rdf:type rdf:resource="http://www.w3.org/2002/07/owl#FunctionalProperty"/>
        <rdfs:domain rdf:resource="https://w3id.org/arco/ontology/arco/CulturalProperty"/>
        <rdfs:range rdf:resource="http://www.w3.org/2000/01/rdf-schema#Literal"/>
        <rdfs:comment xml:lang="it">Questa proprietà permette di associare il codice univoco (ricavato dalla concatenazione di codice regione, numero di catalogo generale ed eventuale suffisso) a un bene culturale descritto in una scheda catalografica.</rdfs:comment>
        <rdfs:comment xml:lang="en">This property represents the unique identifier (derived as the concatenation of the region identifier, the catalogue number and the suffix) of a cultural property describey by a catalogue record.</rdfs:comment>
        <rdfs:isDefinedBy rdf:resource="https://w3id.org/arco/ontology/arco"/>
        <rdfs:label xml:lang="it">codice univoco</rdfs:label>
        <rdfs:label xml:lang="en">unique identifier</rdfs:label>
        <owl:versionInfo xml:lang="it">stabile</owl:versionInfo>
        <owl:versionInfo xml:lang="en">stable</owl:versionInfo>
        <a-cat:iccdNormTag>ICCD Normativa Trasversale 4.00: concat(CD/NCT/NCTR + CD/NCT/NCTN + CD/NCT/NCTS); RV/RVE/RVER (identificativo univoco delle schede collegate); scheda A e PG, v. 1 e v. 2: RV/RVE/RVES (identificativo univoco delle schede collegate). RV/RSE/RSEC (identificativo univoco delle schede collegate)</a-cat:iccdNormTag>
    </owl:DatatypeProperty>
    


    <!-- https://w3id.org/arco/ontology/context-description/historicalInformation -->

    <owl:DatatypeProperty rdf:about="https://w3id.org/arco/ontology/context-description/historicalInformation"/>
    


    <!-- https://w3id.org/arco/ontology/context-description/informationGatheredOnSite -->

    <owl:DatatypeProperty rdf:about="https://w3id.org/arco/ontology/context-description/informationGatheredOnSite"/>
    


    <!-- https://w3id.org/arco/ontology/context-description/numberInCirculation -->

    <owl:DatatypeProperty rdf:about="https://w3id.org/arco/ontology/context-description/numberInCirculation"/>
    


    <!-- https://w3id.org/arco/ontology/context-description/numberOfEnvelopes -->

    <owl:DatatypeProperty rdf:about="https://w3id.org/arco/ontology/context-description/numberOfEnvelopes"/>
    


    <!-- https://w3id.org/arco/ontology/context-description/numberOfLabels -->

    <owl:DatatypeProperty rdf:about="https://w3id.org/arco/ontology/context-description/numberOfLabels"/>
    


    <!-- https://w3id.org/arco/ontology/context-description/rights -->

    <owl:DatatypeProperty rdf:about="https://w3id.org/arco/ontology/context-description/rights"/>
    


    <!-- https://w3id.org/arco/ontology/context-description/subject -->

    <owl:DatatypeProperty rdf:about="https://w3id.org/arco/ontology/context-description/subject"/>
    


    <!-- https://w3id.org/arco/ontology/context-description/title -->

    <owl:DatatypeProperty rdf:about="https://w3id.org/arco/ontology/context-description/title"/>
    


    <!-- https://w3id.org/arco/ontology/core/note -->

    <owl:DatatypeProperty rdf:about="https://w3id.org/arco/ontology/core/note"/>
    


    <!-- https://w3id.org/arco/ontology/denotative-description/anthropologicalMaterialMorphology -->

    <owl:DatatypeProperty rdf:about="https://w3id.org/arco/ontology/denotative-description/anthropologicalMaterialMorphology"/>
    


    <!-- https://w3id.org/arco/ontology/denotative-description/positionInComplexCulturalProperty -->

    <owl:DatatypeProperty rdf:about="https://w3id.org/arco/ontology/denotative-description/positionInComplexCulturalProperty"/>
    


    <!-- https://w3id.org/arco/ontology/denotative-description/proposedIntervention -->

    <owl:DatatypeProperty rdf:about="https://w3id.org/arco/ontology/denotative-description/proposedIntervention"/>
    


    <!-- https://w3id.org/arco/ontology/denotative-description/storageConditions -->

    <owl:DatatypeProperty rdf:about="https://w3id.org/arco/ontology/denotative-description/storageConditions"/>
    


    <!-- https://w3id.org/italia/onto/TI/time -->

    <owl:DatatypeProperty rdf:about="https://w3id.org/italia/onto/TI/time"/>
    


    <!-- https://w3id.org/italia/onto/l0/identifier -->

    <owl:DatatypeProperty rdf:about="https://w3id.org/italia/onto/l0/identifier"/>
    


    <!-- https://w3id.org/italia/onto/l0/name -->

    <owl:DatatypeProperty rdf:about="https://w3id.org/italia/onto/l0/name"/>
    


    <!-- 
    ///////////////////////////////////////////////////////////////////////////////////////
    //
    // Classes
    //
    ///////////////////////////////////////////////////////////////////////////////////////
     -->

    


    <!-- http://dati.beniculturali.it/cis/CulturalEntity -->

    <owl:Class rdf:about="http://dati.beniculturali.it/cis/CulturalEntity"/>
    


    <!-- http://dati.beniculturali.it/cis/GeographicalFeature -->

    <owl:Class rdf:about="http://dati.beniculturali.it/cis/GeographicalFeature"/>
    


    <!-- http://dati.beniculturali.it/cis/SubjectDiscipline -->

    <owl:Class rdf:about="http://dati.beniculturali.it/cis/SubjectDiscipline"/>
    


    <!-- https://w3id.org/arco/ontology/arco/AlternativeMusicalInstrumentClassification -->

    <owl:Class rdf:about="https://w3id.org/arco/ontology/arco/AlternativeMusicalInstrumentClassification">
        <rdfs:subClassOf rdf:resource="https://w3id.org/arco/ontology/arco/MusicalInstrumentClassification"/>
        <rdfs:subClassOf>
            <owl:Restriction>
                <owl:onProperty rdf:resource="https://w3id.org/arco/ontology/context-description/hasAuthor"/>
                <owl:someValuesFrom rdf:resource="https://w3id.org/italia/onto/l0/Agent"/>
            </owl:Restriction>
        </rdfs:subClassOf>
        <rdfs:subClassOf>
            <owl:Restriction>
                <owl:onProperty rdf:resource="https://w3id.org/arco/ontology/context-description/hasBibliography"/>
                <owl:allValuesFrom rdf:resource="https://w3id.org/arco/ontology/context-description/Bibliography"/>
            </owl:Restriction>
        </rdfs:subClassOf>
        <rdfs:subClassOf>
            <owl:Restriction>
                <owl:onProperty rdf:resource="https://w3id.org/arco/ontology/arco/taxon"/>
                <owl:someValuesFrom rdf:resource="http://www.w3.org/2000/01/rdf-schema#Literal"/>
            </owl:Restriction>
        </rdfs:subClassOf>
        <owl:disjointWith rdf:resource="https://w3id.org/arco/ontology/arco/HornbostelSachsClassification"/>
        <rdfs:comment xml:lang="it">Questa classe rappresenta un sistema di classificazione diverso da quello Hornbostel-Sachs, con cui può essere codificato uno strumento musicale.</rdfs:comment>
        <rdfs:comment xml:lang="en">This class represents a classification different from the Hornbostel-Sachs classification.</rdfs:comment>
        <rdfs:isDefinedBy rdf:resource="https://w3id.org/arco/ontology/arco"/>
        <rdfs:label xml:lang="en">Alternative musical instrument classification</rdfs:label>
        <rdfs:label xml:lang="it">Classificazione alternativa di strumento musicale</rdfs:label>
        <owl:versionInfo xml:lang="it">stabile</owl:versionInfo>
        <owl:versionInfo xml:lang="en">stable</owl:versionInfo>
        <a-cat:iccdNormTag>Normativa SM 4.00: CL/CLA</a-cat:iccdNormTag>
    </owl:Class>
    


    <!-- https://w3id.org/arco/ontology/arco/ArchaeologicalMaterial -->

    <owl:Class rdf:about="https://w3id.org/arco/ontology/arco/ArchaeologicalMaterial">
        <rdfs:subClassOf rdf:resource="https://w3id.org/arco/ontology/arco/CulturalPropertyPart"/>
        <rdfs:subClassOf>
            <owl:Restriction>
                <owl:onProperty rdf:resource="https://w3id.org/arco/ontology/arco/hasArchaeologicalMaterialCategory"/>
                <owl:someValuesFrom rdf:resource="https://w3id.org/arco/ontology/arco/ArchaeologicalMaterialCategory"/>
            </owl:Restriction>
        </rdfs:subClassOf>
        <rdfs:subClassOf>
            <owl:Restriction>
                <owl:onProperty rdf:resource="https://w3id.org/arco/ontology/arco/numberOfArchaeologicalMaterials"/>
                <owl:someValuesFrom rdf:resource="http://www.w3.org/2001/XMLSchema#integer"/>
            </owl:Restriction>
        </rdfs:subClassOf>
        <rdfs:comment xml:lang="it">Questa classe rappresenta un materiale archeologico, che è una parte di un lotto di materiali archeologici.</rdfs:comment>
        <rdfs:comment xml:lang="en">This class represents an archaeological material, that is a part of a lot of archaeological materials.</rdfs:comment>
        <rdfs:isDefinedBy rdf:resource="https://w3id.org/arco/ontology/arco"/>
        <rdfs:label xml:lang="en">Archaeological material</rdfs:label>
        <rdfs:label xml:lang="it">Materiale archeologico</rdfs:label>
        <owl:versionInfo xml:lang="it">stabile</owl:versionInfo>
        <owl:versionInfo xml:lang="en">stable</owl:versionInfo>
        <a-cat:iccdNormTag>ICCD Normativa TMA: MA</a-cat:iccdNormTag>
    </owl:Class>
    


    <!-- https://w3id.org/arco/ontology/arco/ArchaeologicalMaterialCategory -->

    <owl:Class rdf:about="https://w3id.org/arco/ontology/arco/ArchaeologicalMaterialCategory">
        <rdfs:subClassOf rdf:resource="https://w3id.org/arco/ontology/core/Category"/>
        <rdfs:subClassOf>
            <owl:Restriction>
                <owl:onProperty rdf:resource="https://w3id.org/arco/ontology/arco/isArchaeologicalMaterialCategoryOf"/>
                <owl:someValuesFrom rdf:resource="https://w3id.org/arco/ontology/arco/ArchaeologicalMaterial"/>
            </owl:Restriction>
        </rdfs:subClassOf>
        <rdfs:comment xml:lang="it">Questa classe rappresenta la categoria di materiale, parte di un lotto di materiali archeologici. (es.: ceramiche, industria litica, intonaco, legno, etc.)</rdfs:comment>
        <rdfs:comment xml:lang="en">This class represents the category of an archaeological material, that is part of a lot of archaeological materials (e.g.: ceramics, plaster, lithic materials, etc.)</rdfs:comment>
        <rdfs:isDefinedBy rdf:resource="https://w3id.org/arco/ontology/arco"/>
        <rdfs:label xml:lang="en">Archaeological material category</rdfs:label>
        <rdfs:label xml:lang="it">Categoria del materiale archeologico</rdfs:label>
        <owl:versionInfo xml:lang="it">stabile</owl:versionInfo>
        <owl:versionInfo xml:lang="en">stable</owl:versionInfo>
        <a-cat:iccdNormTag>ICCD Normativa TMA: MA/MAC/MACC</a-cat:iccdNormTag>
    </owl:Class>
    


    <!-- https://w3id.org/arco/ontology/arco/ArchaeologicalProperty -->

    <owl:Class rdf:about="https://w3id.org/arco/ontology/arco/ArchaeologicalProperty">
        <rdfs:subClassOf rdf:resource="https://w3id.org/arco/ontology/arco/TangibleCulturalProperty"/>
        <rdfs:subClassOf>
            <owl:Restriction>
                <owl:onProperty rdf:resource="https://w3id.org/arco/ontology/context-description/hasAgeOfDeathInterpretation"/>
                <owl:allValuesFrom rdf:resource="https://w3id.org/arco/ontology/context-description/AgeOfDeathInterpretation"/>
            </owl:Restriction>
        </rdfs:subClassOf>
        <rdfs:subClassOf>
            <owl:Restriction>
                <owl:onProperty rdf:resource="https://w3id.org/arco/ontology/context-description/hasBiologicalTaxonomy"/>
                <owl:allValuesFrom rdf:resource="https://w3id.org/arco/ontology/context-description/BiologicalTaxonomy"/>
            </owl:Restriction>
        </rdfs:subClassOf>
        <rdfs:subClassOf>
            <owl:Restriction>
                <owl:onProperty rdf:resource="https://w3id.org/arco/ontology/context-description/hasFindingContext"/>
                <owl:allValuesFrom rdf:resource="https://w3id.org/arco/ontology/context-description/FindingContext"/>
            </owl:Restriction>
        </rdfs:subClassOf>
        <rdfs:subClassOf>
            <owl:Restriction>
                <owl:onProperty rdf:resource="https://w3id.org/arco/ontology/context-description/hasSexInterpretation"/>
                <owl:allValuesFrom rdf:resource="https://w3id.org/arco/ontology/context-description/SexInterpretation"/>
            </owl:Restriction>
        </rdfs:subClassOf>
        <rdfs:subClassOf>
            <owl:Restriction>
                <owl:onProperty rdf:resource="https://w3id.org/arco/ontology/denotative-description/hasSampleCollected"/>
                <owl:allValuesFrom rdf:resource="https://w3id.org/arco/ontology/denotative-description/SampleCollected"/>
            </owl:Restriction>
        </rdfs:subClassOf>
        <rdfs:subClassOf>
            <owl:Restriction>
                <owl:onProperty rdf:resource="https://w3id.org/arco/ontology/location/hasStratigraphicArea"/>
                <owl:allValuesFrom rdf:resource="https://w3id.org/italia/onto/l0/Location"/>
            </owl:Restriction>
        </rdfs:subClassOf>
        <rdfs:subClassOf>
            <owl:Restriction>
                <owl:onProperty rdf:resource="https://w3id.org/arco/ontology/location/hasStratigraphicRoom"/>
                <owl:allValuesFrom rdf:resource="https://w3id.org/italia/onto/l0/Location"/>
            </owl:Restriction>
        </rdfs:subClassOf>
        <rdfs:subClassOf>
            <owl:Restriction>
                <owl:onProperty rdf:resource="https://w3id.org/arco/ontology/location/hasStratigraphicSquare"/>
                <owl:allValuesFrom rdf:resource="https://w3id.org/italia/onto/l0/Location"/>
            </owl:Restriction>
        </rdfs:subClassOf>
        <rdfs:subClassOf>
            <owl:Restriction>
                <owl:onProperty rdf:resource="https://w3id.org/arco/ontology/denotative-description/anthropologicalMaterialMorphology"/>
                <owl:allValuesFrom rdf:resource="http://www.w3.org/2000/01/rdf-schema#Literal"/>
            </owl:Restriction>
        </rdfs:subClassOf>
        <rdfs:comment xml:lang="it">Questa classe rappresenta un bene culturale archeologico, che può essere un complesso archeologico, un monumento archeologico, un reperto archeologico, un reperto antropologico, un saggio stratigrafico, un sito archeologico, o una tabella materiali archeologici. Complessi archeologici: complessi monumentali costituiti da più unità edilizie (abitati, centri fortificati, santuari, complessi termali, ecc.), catalogati a prescindere dal loro attuale stato di conservazione. Monumenti archeologici: singole unità edilizie (una torre, una domus, un tempio, ecc.) catalogate a prescindere dal loro attuale stato di conservazione. Reperti antropologici: testimonianze biologiche in relazione con contesti archeologici e paleontologici. Reperti archeologici: beni mobili di provenienza archeologica (gioielli e monili, vestimenti, arredi, elementi architettonici, opere di pittura, reperti archeobotanici e archeozoologici, scultura, strumenti e oggetti d’uso, ecc.). Saggi stratigrafici: sequenze stratigrafiche rinvenute in contesti di scavo archeologico. Siti archeologici: porzioni di territorio che conservano testimonianze archeologiche. Tabella materiali archeologici: lotti di materiali di provenienza archeologica</rdfs:comment>
        <rdfs:comment xml:lang="en">This class represents an archaeological cultural property, consisting of archaeological complexes, archaeological monuments, anthropological materials, archaeological objects, stratigraphic records, archaeological sites, archaeological materials tables. Archaeological complexes: monumental complexes consisting of several building units (inhabited areas, fortified centers, sanctuaries, thermal complexes, etc.), catalogued regardless of their current conservation status. Archaeological monuments: single building units (a tower, a domus, a temple, etc.) catalogued regardless of their current conservation status. Anthropological materials: biological evidence related to archaeological and paleontological contexts. Archaeological objects: movable properties of archaeological origin (jewelry and jewelry, clothing, furnishings, architectural elements, paintings, archeobotanical and archeozoological objects, sculpture, tools and everyday objects, etc.). Stratigraphic records: stratigraphic sequences found in archaeological excavation contexts. Archaeological sites: portions of territory that preserve archaeological evidence. Archaeological materials tables: lots of archaeological materials.</rdfs:comment>
        <rdfs:isDefinedBy rdf:resource="https://w3id.org/arco/ontology/arco"/>
        <rdfs:label xml:lang="en">Archaeological Property</rdfs:label>
        <rdfs:label xml:lang="it">Bene Archeologico</rdfs:label>
        <owl:versionInfo xml:lang="it">stabile</owl:versionInfo>
        <owl:versionInfo xml:lang="en">stable</owl:versionInfo>
    </owl:Class>
    


    <!-- https://w3id.org/arco/ontology/arco/ArchitecturalOrLandscapeHeritage -->

    <owl:Class rdf:about="https://w3id.org/arco/ontology/arco/ArchitecturalOrLandscapeHeritage">
        <rdfs:subClassOf rdf:resource="https://w3id.org/arco/ontology/arco/ImmovableCulturalProperty"/>
        <rdfs:comment xml:lang="it">Questa classe rappresenta un bene culturale architettonico e paesaggistico. Architettura: complessi monumentali, edifici pubblici e di culto, dimore gentilizie, architetture fortificate, edifici privati, edilizia rurale, fabbricati di archeologia industriale caratterizzati da particolare rilevanza storico artistica. Centri/nuclei storici: strutture insediative urbane più antiche dei territori comunali, caratterizzate da testimonianze storico artistiche di particolare rilevanza. Parchi e giardini: spazi verdi di particolare rilevanza  storica, artistica e ambientale. Esempi di questa tipologia di beni culturali sono i giardini e i parchi annessi alle proprietà nobiliari, gli orti e i giardini botanici, i parchi urbani, le aree verdi comprese nei siti archeologici, ma anche i piccoli giardini privati, i chiostri e i cortili, i cimiteri, sempre se caratterizzati da particolare rilevanza storico artistica.</rdfs:comment>
        <rdfs:comment xml:lang="en">This class represents an architectural or landscape heritage. Architecture: monumental complexes, public and religious buildings, noble residences, fortified architectures, private buildings, rural buildings, industrial archeology buildings characterized by particular historical and artistic importance. Historical centers: urban settlement structures older than the municipal territories, characterized by particularly important historical artistic testimonies. Parks and gardens: green spaces of particular historical, artistic and environmental importance. Examples of this type of cultural heritage are gardens and parks annexed to noble properties, vegetable gardens and botanical gardens, urban parks, green areas included in archaeological sites, but also small private gardens, cloisters and courtyards, cemeteries, always if characterized by particular historical and artistic relevance.</rdfs:comment>
        <rdfs:isDefinedBy rdf:resource="https://w3id.org/arco/ontology/arco"/>
        <rdfs:label xml:lang="en">Architectural or Landscape Heritage</rdfs:label>
        <rdfs:label xml:lang="it">Bene Architettonico o Paesaggistico</rdfs:label>
        <owl:versionInfo xml:lang="it">stabile</owl:versionInfo>
        <owl:versionInfo xml:lang="en">stable</owl:versionInfo>
    </owl:Class>
    


    <!-- https://w3id.org/arco/ontology/arco/BotanicalHeritage -->

    <owl:Class rdf:about="https://w3id.org/arco/ontology/arco/BotanicalHeritage">
        <rdfs:subClassOf rdf:resource="https://w3id.org/arco/ontology/arco/NaturalHeritage"/>
        <rdfs:subClassOf>
            <owl:Restriction>
                <owl:onProperty rdf:resource="https://w3id.org/arco/ontology/movable-property/hasAccession"/>
                <owl:allValuesFrom rdf:resource="https://w3id.org/arco/ontology/movable-property/Accession"/>
            </owl:Restriction>
        </rdfs:subClassOf>
        <rdfs:subClassOf>
            <owl:Restriction>
                <owl:onProperty rdf:resource="https://w3id.org/italia/onto/l0/identifier"/>
                <owl:allValuesFrom rdf:resource="http://www.w3.org/2000/01/rdf-schema#Literal"/>
            </owl:Restriction>
        </rdfs:subClassOf>
        <rdfs:comment xml:lang="it">Questa classe rappresenta esemplari del mondo vegetale provenienti da collezioni di botanica  (raccolte di piante essiccate: erbari)</rdfs:comment>
        <rdfs:comment xml:lang="en">This class represents specimens of the plant world from botanical collections (collections of dried plants: herbaria)</rdfs:comment>
        <rdfs:label xml:lang="it">Bene Botanico</rdfs:label>
        <rdfs:label xml:lang="en">Botanical Heritage</rdfs:label>
        <owl:versionInfo xml:lang="it">instabile</owl:versionInfo>
        <owl:versionInfo xml:lang="en">unstable</owl:versionInfo>
    </owl:Class>
    


    <!-- https://w3id.org/arco/ontology/arco/CartographicClassification -->

    <owl:Class rdf:about="https://w3id.org/arco/ontology/arco/CartographicClassification">
        <rdfs:subClassOf rdf:resource="https://w3id.org/arco/ontology/core/CulturalEntityClassification"/>
        <rdfs:subClassOf>
            <owl:Restriction>
                <owl:onProperty rdf:resource="https://w3id.org/arco/ontology/arco/hasCartographicSymbol"/>
                <owl:someValuesFrom rdf:resource="https://w3id.org/arco/ontology/arco/CartographicSymbol"/>
            </owl:Restriction>
        </rdfs:subClassOf>
        <rdfs:subClassOf>
            <owl:Restriction>
                <owl:onProperty rdf:resource="https://w3id.org/arco/ontology/arco/hasCartographicTheme"/>
                <owl:someValuesFrom rdf:resource="https://w3id.org/arco/ontology/arco/CartographicTheme"/>
            </owl:Restriction>
        </rdfs:subClassOf>
        <rdfs:subClassOf>
            <owl:Restriction>
                <owl:onProperty rdf:resource="https://w3id.org/arco/ontology/arco/isCartographicClassificationOf"/>
                <owl:someValuesFrom rdf:resource="https://w3id.org/arco/ontology/arco/CulturalProperty"/>
            </owl:Restriction>
        </rdfs:subClassOf>
        <rdfs:subClassOf>
            <owl:Restriction>
                <owl:onProperty rdf:resource="https://w3id.org/arco/ontology/arco/hasThematicCategory"/>
                <owl:allValuesFrom rdf:resource="https://w3id.org/arco/ontology/arco/ThematicCategory"/>
            </owl:Restriction>
        </rdfs:subClassOf>
        <rdfs:comment xml:lang="it">Questa classe rappresenta una classificazione di un bene culturale relativamente alla rappresentazione cartografica del bene su specifici livelli tematici, con riferimento a uno standard oppure a un&apos;organizzazione logica predefinita dall&apos;Ente responsabile dell&apos;attività di catalogazione.</rdfs:comment>
        <rdfs:comment xml:lang="en">This class represents a cartographic classification of a cultural property, referring to the cartographic representation on specific thematic levels, based on a standard or a classification defined by the cataloguing agency.</rdfs:comment>
        <rdfs:isDefinedBy rdf:resource="https://w3id.org/arco/ontology/arco"/>
        <rdfs:label xml:lang="en">Cartographic classification</rdfs:label>
        <rdfs:label xml:lang="it">Classificazione cartografica</rdfs:label>
        <owl:versionInfo xml:lang="it">stabile</owl:versionInfo>
        <owl:versionInfo xml:lang="en">stable</owl:versionInfo>
        <a-cat:iccdNormTag>ICCD Normativa Trasversale: CT</a-cat:iccdNormTag>
    </owl:Class>
    


    <!-- https://w3id.org/arco/ontology/arco/CartographicSymbol -->

    <owl:Class rdf:about="https://w3id.org/arco/ontology/arco/CartographicSymbol">
        <rdfs:subClassOf rdf:resource="https://w3id.org/arco/ontology/core/Concept"/>
        <rdfs:subClassOf>
            <owl:Restriction>
                <owl:onProperty rdf:resource="https://w3id.org/arco/ontology/arco/isCartographicSymbolOf"/>
                <owl:someValuesFrom rdf:resource="https://w3id.org/arco/ontology/arco/CartographicClassification"/>
            </owl:Restriction>
        </rdfs:subClassOf>
        <rdfs:subClassOf>
            <owl:Restriction>
                <owl:onProperty rdf:resource="https://w3id.org/arco/ontology/arco/cartographicSymbolIdentifier"/>
                <owl:allValuesFrom rdf:resource="http://www.w3.org/2000/01/rdf-schema#Literal"/>
            </owl:Restriction>
        </rdfs:subClassOf>
        <rdfs:comment xml:lang="it">Questa classe rappresenta il simbolo con cui si rappresenta il bene su una base cartografica in relazione al tema di interesse.</rdfs:comment>
        <rdfs:comment xml:lang="en">This class represents the symbol used to represent the cultural property on a cartographic base map, referring to the cartographic theme.</rdfs:comment>
        <rdfs:isDefinedBy rdf:resource="https://w3id.org/arco/ontology/arco"/>
        <rdfs:label xml:lang="en">Cartographic symbol</rdfs:label>
        <rdfs:label xml:lang="it">Simbolo cartografico</rdfs:label>
        <owl:versionInfo xml:lang="it">stabile</owl:versionInfo>
        <owl:versionInfo xml:lang="en">stable</owl:versionInfo>
        <a-cat:iccdNormTag>ICCD Normativa Trasversale 4.00: CT/CTM/CTMD</a-cat:iccdNormTag>
    </owl:Class>
    


    <!-- https://w3id.org/arco/ontology/arco/CartographicTheme -->

    <owl:Class rdf:about="https://w3id.org/arco/ontology/arco/CartographicTheme">
        <rdfs:subClassOf rdf:resource="https://w3id.org/arco/ontology/core/Concept"/>
        <rdfs:subClassOf>
            <owl:Restriction>
                <owl:onProperty rdf:resource="https://w3id.org/arco/ontology/arco/isCartographicThemeOf"/>
                <owl:someValuesFrom rdf:resource="https://w3id.org/arco/ontology/arco/CartographicTheme"/>
            </owl:Restriction>
        </rdfs:subClassOf>
        <rdfs:comment xml:lang="it">Questa classe rappresenta il tema di riferimento associato a una classificazione cartografica di un bene culturale.</rdfs:comment>
        <rdfs:comment xml:lang="en">This class represents the cartographic theme associated to a cartographic classification of a cultural property.</rdfs:comment>
        <rdfs:isDefinedBy rdf:resource="https://w3id.org/arco/ontology/arco"/>
        <rdfs:label xml:lang="en">Cartographic theme</rdfs:label>
        <rdfs:label xml:lang="it">Tema cartografico</rdfs:label>
        <owl:versionInfo xml:lang="it">stabile</owl:versionInfo>
        <owl:versionInfo xml:lang="en">stable</owl:versionInfo>
        <a-cat:iccdNormTag>ICCD Normativa Trasversale 4.00: CT/CTM/CTMT</a-cat:iccdNormTag>
    </owl:Class>
    


    <!-- https://w3id.org/arco/ontology/arco/ComplexCulturalProperty -->

    <owl:Class rdf:about="https://w3id.org/arco/ontology/arco/ComplexCulturalProperty">
        <owl:equivalentClass>
            <owl:Class>
                <owl:unionOf rdf:parseType="Collection">
                    <rdf:Description rdf:about="https://w3id.org/arco/ontology/arco/CulturalPropertyCollection"/>
                    <owl:Restriction>
                        <owl:onProperty rdf:resource="https://w3id.org/arco/ontology/arco/hasCulturalPropertyComponent"/>
                        <owl:someValuesFrom rdf:resource="https://w3id.org/arco/ontology/arco/CulturalPropertyComponent"/>
                    </owl:Restriction>
                </owl:unionOf>
            </owl:Class>
        </owl:equivalentClass>
        <rdfs:subClassOf rdf:resource="https://w3id.org/arco/ontology/arco/CulturalProperty"/>
        <rdfs:comment xml:lang="it">Questa classe rappresenta un bene culturale complesso, cioè costituito da più parti componenti.</rdfs:comment>
        <rdfs:comment xml:lang="en">This class represents a complex cultural property, that consists of different components.</rdfs:comment>
        <rdfs:isDefinedBy rdf:resource="https://w3id.org/arco/ontology/arco"/>
        <rdfs:label xml:lang="it">Bene Culturale Complesso</rdfs:label>
        <rdfs:label xml:lang="en">Complex Cultural Property</rdfs:label>
        <owl:versionInfo xml:lang="it">stabile</owl:versionInfo>
        <owl:versionInfo xml:lang="en">stable</owl:versionInfo>
        <a-cat:iccdNormTag xml:lang="it">ICCD Normativa Trasversale 4.00: se viene valorizzato il campo OG/OGT/OGTP, i valori dei campi OGTD e OGTT si riferiscono a un bene culturale complesso, rappresentato quindi per mezzo di questa classe, di cui OGTP è parte componente.</a-cat:iccdNormTag>
    </owl:Class>
    


    <!-- https://w3id.org/arco/ontology/arco/CulturalProperty -->

    <owl:Class rdf:about="https://w3id.org/arco/ontology/arco/CulturalProperty">
        <owl:equivalentClass>
            <owl:Class>
                <owl:unionOf rdf:parseType="Collection">
                    <rdf:Description rdf:about="https://w3id.org/arco/ontology/arco/IntangibleCulturalProperty"/>
                    <rdf:Description rdf:about="https://w3id.org/arco/ontology/arco/TangibleCulturalProperty"/>
                </owl:unionOf>
            </owl:Class>
        </owl:equivalentClass>
        <rdfs:subClassOf rdf:resource="http://dati.beniculturali.it/cis/CulturalEntity"/>
        <rdfs:subClassOf>
            <owl:Restriction>
                <owl:onProperty rdf:resource="https://w3id.org/arco/ontology/context-description/hasDocumentation"/>
                <owl:someValuesFrom rdf:resource="https://w3id.org/arco/ontology/context-description/Documentation"/>
            </owl:Restriction>
        </rdfs:subClassOf>
        <rdfs:subClassOf>
            <owl:Restriction>
                <owl:onProperty rdf:resource="https://w3id.org/arco/ontology/arco/hasCulturalPropertyComponent"/>
                <owl:allValuesFrom rdf:resource="https://w3id.org/arco/ontology/arco/CulturalPropertyComponent"/>
            </owl:Restriction>
        </rdfs:subClassOf>
        <rdfs:subClassOf>
            <owl:Restriction>
                <owl:onProperty rdf:resource="https://w3id.org/arco/ontology/arco/hasCulturalPropertyResidual"/>
                <owl:allValuesFrom rdf:resource="https://w3id.org/arco/ontology/arco/CulturalPropertyResidual"/>
            </owl:Restriction>
        </rdfs:subClassOf>
        <rdfs:subClassOf>
            <owl:Restriction>
                <owl:onProperty rdf:resource="https://w3id.org/arco/ontology/catalogue/isRelatedToAdditionalForm"/>
                <owl:allValuesFrom rdf:resource="https://w3id.org/arco/ontology/catalogue/AdditionalForm"/>
            </owl:Restriction>
        </rdfs:subClassOf>
        <rdfs:subClassOf>
            <owl:Restriction>
                <owl:onProperty rdf:resource="https://w3id.org/arco/ontology/catalogue/isRelatedToInformationForm"/>
                <owl:allValuesFrom rdf:resource="https://w3id.org/arco/ontology/catalogue/InformationForm"/>
            </owl:Restriction>
        </rdfs:subClassOf>
        <rdfs:subClassOf>
            <owl:Restriction>
                <owl:onProperty rdf:resource="https://w3id.org/arco/ontology/context-description/hasAcquisition"/>
                <owl:allValuesFrom rdf:resource="https://w3id.org/arco/ontology/context-description/Acquisition"/>
            </owl:Restriction>
        </rdfs:subClassOf>
        <rdfs:subClassOf>
            <owl:Restriction>
                <owl:onProperty rdf:resource="https://w3id.org/arco/ontology/context-description/hasAuthorshipAttribution"/>
                <owl:allValuesFrom rdf:resource="https://w3id.org/arco/ontology/context-description/AuthorshipAttribution"/>
            </owl:Restriction>
        </rdfs:subClassOf>
        <rdfs:subClassOf>
            <owl:Restriction>
                <owl:onProperty rdf:resource="https://w3id.org/arco/ontology/context-description/hasBibliography"/>
                <owl:allValuesFrom rdf:resource="https://w3id.org/arco/ontology/context-description/Bibliography"/>
            </owl:Restriction>
        </rdfs:subClassOf>
        <rdfs:subClassOf>
            <owl:Restriction>
                <owl:onProperty rdf:resource="https://w3id.org/arco/ontology/context-description/hasChangeOfAvailability"/>
                <owl:allValuesFrom rdf:resource="https://w3id.org/arco/ontology/context-description/ChangeOfAvailability"/>
            </owl:Restriction>
        </rdfs:subClassOf>
        <rdfs:subClassOf>
            <owl:Restriction>
                <owl:onProperty rdf:resource="https://w3id.org/arco/ontology/context-description/hasCommission"/>
                <owl:allValuesFrom rdf:resource="https://w3id.org/arco/ontology/context-description/Commission"/>
            </owl:Restriction>
        </rdfs:subClassOf>
        <rdfs:subClassOf>
            <owl:Restriction>
                <owl:onProperty rdf:resource="https://w3id.org/arco/ontology/context-description/hasDating"/>
                <owl:allValuesFrom rdf:resource="https://w3id.org/arco/ontology/context-description/Dating"/>
            </owl:Restriction>
        </rdfs:subClassOf>
        <rdfs:subClassOf>
            <owl:Restriction>
                <owl:onProperty rdf:resource="https://w3id.org/arco/ontology/context-description/hasDetectionMethod"/>
                <owl:allValuesFrom rdf:resource="https://w3id.org/arco/ontology/context-description/DetectionMethod"/>
            </owl:Restriction>
        </rdfs:subClassOf>
        <rdfs:subClassOf>
            <owl:Restriction>
                <owl:onProperty rdf:resource="https://w3id.org/arco/ontology/context-description/hasExportImportCertification"/>
                <owl:allValuesFrom rdf:resource="https://w3id.org/arco/ontology/context-description/ExportImportCertification"/>
            </owl:Restriction>
        </rdfs:subClassOf>
        <rdfs:subClassOf>
            <owl:Restriction>
                <owl:onProperty rdf:resource="https://w3id.org/arco/ontology/context-description/hasIntervention"/>
                <owl:allValuesFrom rdf:resource="https://w3id.org/arco/ontology/context-description/Intervention"/>
            </owl:Restriction>
        </rdfs:subClassOf>
        <rdfs:subClassOf>
            <owl:Restriction>
                <owl:onProperty rdf:resource="https://w3id.org/arco/ontology/context-description/hasInventory"/>
                <owl:allValuesFrom rdf:resource="https://w3id.org/arco/ontology/context-description/Inventory"/>
            </owl:Restriction>
        </rdfs:subClassOf>
        <rdfs:subClassOf>
            <owl:Restriction>
                <owl:onProperty rdf:resource="https://w3id.org/arco/ontology/context-description/hasLegalSituation"/>
                <owl:allValuesFrom rdf:resource="https://w3id.org/arco/ontology/context-description/LegalSituation"/>
            </owl:Restriction>
        </rdfs:subClassOf>
        <rdfs:subClassOf>
            <owl:Restriction>
                <owl:onProperty rdf:resource="https://w3id.org/arco/ontology/context-description/hasProtectiveMeasure"/>
                <owl:allValuesFrom rdf:resource="https://w3id.org/arco/ontology/context-description/ProtectiveMeasure"/>
            </owl:Restriction>
        </rdfs:subClassOf>
        <rdfs:subClassOf>
            <owl:Restriction>
                <owl:onProperty rdf:resource="https://w3id.org/arco/ontology/context-description/hasRelatedWorkSituation"/>
                <owl:allValuesFrom rdf:resource="https://w3id.org/arco/ontology/context-description/RelatedWorkSituation"/>
            </owl:Restriction>
        </rdfs:subClassOf>
        <rdfs:subClassOf>
            <owl:Restriction>
                <owl:onProperty rdf:resource="https://w3id.org/arco/ontology/context-description/hasSubject"/>
                <owl:allValuesFrom rdf:resource="https://w3id.org/arco/ontology/context-description/Subject"/>
            </owl:Restriction>
        </rdfs:subClassOf>
        <rdfs:subClassOf>
            <owl:Restriction>
                <owl:onProperty rdf:resource="https://w3id.org/arco/ontology/context-description/hasSurvey"/>
                <owl:allValuesFrom rdf:resource="https://w3id.org/arco/ontology/context-description/Survey"/>
            </owl:Restriction>
        </rdfs:subClassOf>
        <rdfs:subClassOf>
            <owl:Restriction>
                <owl:onProperty rdf:resource="https://w3id.org/arco/ontology/context-description/hasTitle"/>
                <owl:allValuesFrom rdf:resource="https://w3id.org/arco/ontology/context-description/Title"/>
            </owl:Restriction>
        </rdfs:subClassOf>
        <rdfs:subClassOf>
            <owl:Restriction>
                <owl:onProperty rdf:resource="https://w3id.org/arco/ontology/context-description/hasUrbanPlanningInstrument"/>
                <owl:allValuesFrom rdf:resource="https://w3id.org/arco/ontology/context-description/UrbanPlanningInstrument"/>
            </owl:Restriction>
        </rdfs:subClassOf>
        <rdfs:subClassOf>
            <owl:Restriction>
                <owl:onProperty rdf:resource="https://w3id.org/arco/ontology/context-description/hasUse"/>
                <owl:allValuesFrom rdf:resource="https://w3id.org/arco/ontology/context-description/Use"/>
            </owl:Restriction>
        </rdfs:subClassOf>
        <rdfs:subClassOf>
            <owl:Restriction>
                <owl:onProperty rdf:resource="https://w3id.org/arco/ontology/context-description/isMemberOfCollection"/>
                <owl:allValuesFrom rdf:resource="https://w3id.org/arco/ontology/context-description/CollectionMembership"/>
            </owl:Restriction>
        </rdfs:subClassOf>
        <rdfs:subClassOf>
            <owl:Restriction>
                <owl:onProperty rdf:resource="https://w3id.org/arco/ontology/denotative-description/hasAffixedElement"/>
                <owl:allValuesFrom rdf:resource="https://w3id.org/arco/ontology/denotative-description/AffixedElement"/>
            </owl:Restriction>
        </rdfs:subClassOf>
        <rdfs:subClassOf>
            <owl:Restriction>
                <owl:onProperty rdf:resource="https://w3id.org/arco/ontology/denotative-description/hasConservationStatus"/>
                <owl:allValuesFrom rdf:resource="https://w3id.org/arco/ontology/denotative-description/ConservationStatus"/>
            </owl:Restriction>
        </rdfs:subClassOf>
        <rdfs:subClassOf>
            <owl:Restriction>
                <owl:onProperty rdf:resource="https://w3id.org/arco/ontology/denotative-description/hasCulturalPropertyAccessibility"/>
                <owl:allValuesFrom rdf:resource="https://w3id.org/arco/ontology/denotative-description/CulturalPropertyAccessibility"/>
            </owl:Restriction>
        </rdfs:subClassOf>
        <rdfs:subClassOf>
            <owl:Restriction>
                <owl:onProperty rdf:resource="https://w3id.org/arco/ontology/denotative-description/hasCulturalPropertyAvailability"/>
                <owl:allValuesFrom rdf:resource="https://w3id.org/arco/ontology/denotative-description/CulturalPropertyAvailability"/>
            </owl:Restriction>
        </rdfs:subClassOf>
        <rdfs:subClassOf>
            <owl:Restriction>
                <owl:onProperty rdf:resource="https://w3id.org/arco/ontology/denotative-description/hasCulturalPropertyType"/>
                <owl:allValuesFrom rdf:resource="https://w3id.org/arco/ontology/denotative-description/CulturalPropertyType"/>
            </owl:Restriction>
        </rdfs:subClassOf>
        <rdfs:subClassOf>
            <owl:Restriction>
                <owl:onProperty rdf:resource="https://w3id.org/arco/ontology/denotative-description/hasDesignationInTime"/>
                <owl:allValuesFrom rdf:resource="https://w3id.org/arco/ontology/denotative-description/DesignationInTime"/>
            </owl:Restriction>
        </rdfs:subClassOf>
        <rdfs:subClassOf>
            <owl:Restriction>
                <owl:onProperty rdf:resource="https://w3id.org/arco/ontology/denotative-description/hasFunctionalPurpose"/>
                <owl:allValuesFrom rdf:resource="https://w3id.org/arco/ontology/denotative-description/FunctionalPurpose"/>
            </owl:Restriction>
        </rdfs:subClassOf>
        <rdfs:subClassOf>
            <owl:Restriction>
                <owl:onProperty rdf:resource="https://w3id.org/arco/ontology/denotative-description/hasIconographicOrDecorativeApparatus"/>
                <owl:allValuesFrom rdf:resource="https://w3id.org/arco/ontology/denotative-description/IconographicOrDecorativeApparatus"/>
            </owl:Restriction>
        </rdfs:subClassOf>
        <rdfs:subClassOf>
            <owl:Restriction>
                <owl:onProperty rdf:resource="https://w3id.org/arco/ontology/denotative-description/hasLocationSubject"/>
                <owl:allValuesFrom rdf:resource="https://w3id.org/arco/ontology/location/TimeIndexedTypedLocation"/>
            </owl:Restriction>
        </rdfs:subClassOf>
        <rdfs:subClassOf>
            <owl:Restriction>
                <owl:onProperty rdf:resource="https://w3id.org/arco/ontology/denotative-description/hasMeasurementCollection"/>
                <owl:allValuesFrom rdf:resource="https://w3id.org/arco/ontology/denotative-description/MeasurementCollection"/>
            </owl:Restriction>
        </rdfs:subClassOf>
        <rdfs:subClassOf>
            <owl:Restriction>
                <owl:onProperty rdf:resource="https://w3id.org/arco/ontology/denotative-description/hasOrientation"/>
                <owl:allValuesFrom rdf:resource="https://w3id.org/arco/ontology/denotative-description/Orientation"/>
            </owl:Restriction>
        </rdfs:subClassOf>
        <rdfs:subClassOf>
            <owl:Restriction>
                <owl:onProperty rdf:resource="https://w3id.org/arco/ontology/denotative-description/hasTechnicalStatus"/>
                <owl:allValuesFrom rdf:resource="https://w3id.org/arco/ontology/denotative-description/CulturalEntityTechnicalStatus"/>
            </owl:Restriction>
        </rdfs:subClassOf>
        <rdfs:subClassOf>
            <owl:Restriction>
                <owl:onProperty rdf:resource="https://w3id.org/arco/ontology/location/hasCadastralIdentity"/>
                <owl:allValuesFrom rdf:resource="https://w3id.org/arco/ontology/location/CadastralIdentity"/>
            </owl:Restriction>
        </rdfs:subClassOf>
        <rdfs:subClassOf>
            <owl:Restriction>
                <owl:onProperty rdf:resource="https://w3id.org/arco/ontology/location/hasCulturalPropertyAddress"/>
                <owl:allValuesFrom rdf:resource="https://w3id.org/italia/onto/CLV/Address"/>
            </owl:Restriction>
        </rdfs:subClassOf>
        <rdfs:subClassOf>
            <owl:Restriction>
                <owl:onProperty rdf:resource="https://w3id.org/arco/ontology/location/hasTimeIndexedTypedLocation"/>
                <owl:allValuesFrom rdf:resource="https://w3id.org/arco/ontology/location/TimeIndexedTypedLocation"/>
            </owl:Restriction>
        </rdfs:subClassOf>
        <rdfs:subClassOf>
            <owl:Restriction>
                <owl:onProperty rdf:resource="https://w3id.org/arco/ontology/location/hasTypeOfContext"/>
                <owl:allValuesFrom rdf:resource="https://w3id.org/arco/ontology/location/TypeOfContext"/>
            </owl:Restriction>
        </rdfs:subClassOf>
        <rdfs:subClassOf>
            <owl:Restriction>
                <owl:onProperty rdf:resource="https://w3id.org/italia/onto/CLV/hasGeometry"/>
                <owl:allValuesFrom rdf:resource="https://w3id.org/italia/onto/CLV/Geometry"/>
            </owl:Restriction>
        </rdfs:subClassOf>
        <rdfs:subClassOf>
            <owl:Restriction>
                <owl:onProperty rdf:resource="https://w3id.org/arco/ontology/arco/numberOfComponents"/>
                <owl:allValuesFrom rdf:resource="http://www.w3.org/2000/01/rdf-schema#Literal"/>
            </owl:Restriction>
        </rdfs:subClassOf>
        <rdfs:subClassOf>
            <owl:Restriction>
                <owl:onProperty rdf:resource="https://w3id.org/arco/ontology/context-description/historicalInformation"/>
                <owl:allValuesFrom rdf:resource="http://www.w3.org/2000/01/rdf-schema#Literal"/>
            </owl:Restriction>
        </rdfs:subClassOf>
        <rdfs:subClassOf>
            <owl:Restriction>
                <owl:onProperty rdf:resource="https://w3id.org/arco/ontology/context-description/informationGatheredOnSite"/>
                <owl:allValuesFrom rdf:resource="http://www.w3.org/2000/01/rdf-schema#Literal"/>
            </owl:Restriction>
        </rdfs:subClassOf>
        <rdfs:subClassOf>
            <owl:Restriction>
                <owl:onProperty rdf:resource="https://w3id.org/arco/ontology/context-description/rights"/>
                <owl:allValuesFrom rdf:resource="http://www.w3.org/2000/01/rdf-schema#Literal"/>
            </owl:Restriction>
        </rdfs:subClassOf>
        <rdfs:subClassOf>
            <owl:Restriction>
                <owl:onProperty rdf:resource="https://w3id.org/arco/ontology/context-description/subject"/>
                <owl:allValuesFrom rdf:resource="http://www.w3.org/2000/01/rdf-schema#Literal"/>
            </owl:Restriction>
        </rdfs:subClassOf>
        <rdfs:subClassOf>
            <owl:Restriction>
                <owl:onProperty rdf:resource="https://w3id.org/arco/ontology/context-description/title"/>
                <owl:allValuesFrom rdf:resource="http://www.w3.org/2000/01/rdf-schema#Literal"/>
            </owl:Restriction>
        </rdfs:subClassOf>
        <rdfs:subClassOf>
            <owl:Restriction>
                <owl:onProperty rdf:resource="https://w3id.org/arco/ontology/denotative-description/proposedIntervention"/>
                <owl:allValuesFrom rdf:resource="http://www.w3.org/2000/01/rdf-schema#Literal"/>
            </owl:Restriction>
        </rdfs:subClassOf>
        <rdfs:subClassOf>
            <owl:Restriction>
                <owl:onProperty rdf:resource="https://w3id.org/arco/ontology/denotative-description/storageConditions"/>
                <owl:allValuesFrom rdf:resource="http://www.w3.org/2000/01/rdf-schema#Literal"/>
            </owl:Restriction>
        </rdfs:subClassOf>
        <rdfs:subClassOf>
            <owl:Restriction>
                <owl:onProperty rdf:resource="https://w3id.org/arco/ontology/arco/catalogueNumber"/>
                <owl:maxCardinality rdf:datatype="http://www.w3.org/2001/XMLSchema#nonNegativeInteger">1</owl:maxCardinality>
            </owl:Restriction>
        </rdfs:subClassOf>
        <rdfs:subClassOf>
            <owl:Restriction>
                <owl:onProperty rdf:resource="https://w3id.org/arco/ontology/arco/regionIdentifier"/>
                <owl:maxCardinality rdf:datatype="http://www.w3.org/2001/XMLSchema#nonNegativeInteger">1</owl:maxCardinality>
            </owl:Restriction>
        </rdfs:subClassOf>
        <rdfs:subClassOf>
            <owl:Restriction>
                <owl:onProperty rdf:resource="https://w3id.org/arco/ontology/arco/suffix"/>
                <owl:maxCardinality rdf:datatype="http://www.w3.org/2001/XMLSchema#nonNegativeInteger">1</owl:maxCardinality>
            </owl:Restriction>
        </rdfs:subClassOf>
        <rdfs:subClassOf>
            <owl:Restriction>
                <owl:onProperty rdf:resource="https://w3id.org/arco/ontology/arco/uniqueIdentifier"/>
                <owl:maxCardinality rdf:datatype="http://www.w3.org/2001/XMLSchema#nonNegativeInteger">1</owl:maxCardinality>
            </owl:Restriction>
        </rdfs:subClassOf>
        <rdfs:comment xml:lang="it">Questa classe rappresenta un bene culturale, sia materiale che immateriale. Un bene culturale è una testimonianza materiale o immateriale, riconosciuta come parte del patrimonio culturale nazionale in quanto utile alla conoscenza e alla ricostruzione della storia e del paesaggio.</rdfs:comment>
        <rdfs:comment xml:lang="en">This class represents a cultural property, both tangible and intangible. A cultural property is the legacy, tangible or intangible, recognised as part of the national cultural heritage, since it helps know and reconstruct the history and the landscape.</rdfs:comment>
        <rdfs:isDefinedBy rdf:resource="https://w3id.org/arco/ontology/arco"/>
        <rdfs:label xml:lang="it">Bene culturale</rdfs:label>
        <rdfs:label xml:lang="en">Cultural Property</rdfs:label>
        <owl:versionInfo xml:lang="it">stabile</owl:versionInfo>
        <owl:versionInfo xml:lang="en">stable</owl:versionInfo>
    </owl:Class>
    


    <!-- https://w3id.org/arco/ontology/arco/CulturalPropertyCataloguingCategory -->

    <owl:Class rdf:about="https://w3id.org/arco/ontology/arco/CulturalPropertyCataloguingCategory">
        <rdfs:subClassOf rdf:resource="https://w3id.org/arco/ontology/core/Category"/>
        <rdfs:subClassOf>
            <owl:Restriction>
                <owl:onProperty rdf:resource="https://w3id.org/arco/ontology/arco/isCulturalPropertyCataloguingCategoryOf"/>
                <owl:someValuesFrom rdf:resource="https://w3id.org/arco/ontology/arco/CulturalProperty"/>
            </owl:Restriction>
        </rdfs:subClassOf>
        <rdfs:comment xml:lang="it">Questa classe rappresenta una categoria di un bene culturale basata su una valutazione soggettiva del catalogatore durante il processo di catalogazione.</rdfs:comment>
        <rdfs:comment xml:lang="en">This class represents a cultural property category based on a subjective evaluation of the cataloguing agent, during the cataloguing process.</rdfs:comment>
        <rdfs:isDefinedBy rdf:resource="https://w3id.org/arco/ontology/arco"/>
        <rdfs:label xml:lang="it">Categoria di bene culturale basata su catalogazione</rdfs:label>
        <rdfs:label xml:lang="en">Cultural property cataloguing category</rdfs:label>
        <owl:versionInfo xml:lang="it">stabile</owl:versionInfo>
        <owl:versionInfo xml:lang="en">stable</owl:versionInfo>
        <a-cat:iccdNormTag>ICCD Normativa Trasversale 4.00: OG/OGT/OGTV</a-cat:iccdNormTag>
    </owl:Class>
    


    <!-- https://w3id.org/arco/ontology/arco/CulturalPropertyCategory -->

    <owl:Class rdf:about="https://w3id.org/arco/ontology/arco/CulturalPropertyCategory">
        <rdfs:subClassOf rdf:resource="https://w3id.org/arco/ontology/core/Category"/>
        <rdfs:subClassOf>
            <owl:Restriction>
                <owl:onProperty rdf:resource="https://w3id.org/arco/ontology/arco/isCulturalPropertyCategoryOf"/>
                <owl:someValuesFrom rdf:resource="https://w3id.org/arco/ontology/arco/CulturalProperty"/>
            </owl:Restriction>
        </rdfs:subClassOf>
        <rdfs:subClassOf>
            <owl:Restriction>
                <owl:onProperty rdf:resource="https://w3id.org/italia/onto/l0/name"/>
                <owl:allValuesFrom rdf:resource="http://www.w3.org/2000/01/rdf-schema#Literal"/>
            </owl:Restriction>
        </rdfs:subClassOf>
        <rdfs:comment xml:lang="it">Questa classe rappresenta la categoria di un bene culturale, che contiene le indicazioni che consentono di inquadrare l&apos;individuazione terminologica del bene catalogato nell&apos;ambito di una più ampia e complessa organizzazione semantica.</rdfs:comment>
        <rdfs:comment xml:lang="en">This class represents the category of a cultural property, which contains the information that allows us to frame the terminological identification of the properties catalogued in the context of a wider and more complex semantic structure.</rdfs:comment>
        <rdfs:isDefinedBy rdf:resource="https://w3id.org/arco/ontology/arco"/>
        <rdfs:label xml:lang="it">Categoria del bene</rdfs:label>
        <rdfs:label xml:lang="en">Cultural Property Category</rdfs:label>
        <owl:versionInfo xml:lang="it">stabile</owl:versionInfo>
        <owl:versionInfo xml:lang="en">stable</owl:versionInfo>
        <a-cat:iccdNormTag xml:lang="it">ICCD Normativa Trasversale 4.00: OG/CTG -  Normativa AT: OG/OGT/OGTP - Normativa RA: OG/CLS - Normative CA e MA e Normativa VeAC: OG/OGT/OGTC, Normativa BDM: OG/OGT/OGTG</a-cat:iccdNormTag>
    </owl:Class>
    


    <!-- https://w3id.org/arco/ontology/arco/CulturalPropertyCollection -->

    <owl:Class rdf:about="https://w3id.org/arco/ontology/arco/CulturalPropertyCollection">
        <rdfs:subClassOf rdf:resource="https://w3id.org/italia/onto/l0/Collection"/>
        <rdfs:subClassOf>
            <owl:Restriction>
                <owl:onProperty rdf:resource="https://w3id.org/arco/ontology/arco/numberOfMembers"/>
                <owl:allValuesFrom rdf:resource="http://www.w3.org/2000/01/rdf-schema#Literal"/>
            </owl:Restriction>
        </rdfs:subClassOf>
        <rdfs:comment xml:lang="it">Questa classe rappresenta un bene culturale complesso, quando questo si configuri come una serie o un insieme.</rdfs:comment>
        <rdfs:comment xml:lang="en">This class represents a complex cultural property, when it is a series or a set.</rdfs:comment>
        <rdfs:isDefinedBy rdf:resource="https://w3id.org/arco/ontology/arco"/>
        <rdfs:label xml:lang="en">Cultural Property Collection</rdfs:label>
        <rdfs:label xml:lang="it">Insieme di beni culturali</rdfs:label>
        <owl:versionInfo xml:lang="it">stabile</owl:versionInfo>
        <owl:versionInfo xml:lang="en">stable</owl:versionInfo>
    </owl:Class>
    


    <!-- https://w3id.org/arco/ontology/arco/CulturalPropertyComponent -->

    <owl:Class rdf:about="https://w3id.org/arco/ontology/arco/CulturalPropertyComponent">
        <rdfs:subClassOf rdf:resource="https://w3id.org/arco/ontology/arco/CulturalProperty"/>
        <rdfs:subClassOf>
            <owl:Restriction>
                <owl:onProperty rdf:resource="https://w3id.org/arco/ontology/arco/isCulturalPropertyComponentOf"/>
                <owl:someValuesFrom rdf:resource="https://w3id.org/arco/ontology/arco/ComplexCulturalProperty"/>
            </owl:Restriction>
        </rdfs:subClassOf>
        <rdfs:subClassOf>
            <owl:Restriction>
                <owl:onProperty rdf:resource="https://w3id.org/arco/ontology/denotative-description/positionInComplexCulturalProperty"/>
                <owl:allValuesFrom rdf:resource="http://www.w3.org/2000/01/rdf-schema#Literal"/>
            </owl:Restriction>
        </rdfs:subClassOf>
        <rdfs:comment xml:lang="it">Questa classe rappresenta una parte componente di un bene culturale complesso.</rdfs:comment>
        <rdfs:comment xml:lang="en">This class represents a component of a complex cultural property.</rdfs:comment>
        <rdfs:isDefinedBy rdf:resource="https://w3id.org/arco/ontology/arco"/>
        <rdfs:label xml:lang="en">Cultural Property Component</rdfs:label>
        <rdfs:label xml:lang="it">Parte Componente di Bene Culturale</rdfs:label>
        <owl:versionInfo xml:lang="it">stabile</owl:versionInfo>
        <owl:versionInfo xml:lang="en">stable</owl:versionInfo>
        <a-cat:iccdNormTag>OG/OGT/OGTP</a-cat:iccdNormTag>
    </owl:Class>
    


    <!-- https://w3id.org/arco/ontology/arco/CulturalPropertyInventoryCategory -->

    <owl:Class rdf:about="https://w3id.org/arco/ontology/arco/CulturalPropertyInventoryCategory">
        <rdfs:subClassOf rdf:resource="https://w3id.org/arco/ontology/core/Category"/>
        <rdfs:subClassOf>
            <owl:Restriction>
                <owl:onProperty rdf:resource="https://w3id.org/arco/ontology/arco/isCulturalPropertyInventoryCategoryOf"/>
                <owl:someValuesFrom rdf:resource="https://w3id.org/arco/ontology/arco/CulturalProperty"/>
            </owl:Restriction>
        </rdfs:subClassOf>
        <rdfs:comment xml:lang="it">Questa classe rappresenta la categoria di un bene numismatico, in riferimento a una classificazione che si basa su un repertorio riconosciuto nello specifico ambito disciplinare.</rdfs:comment>
        <rdfs:comment xml:lang="en">This class represents a category of a numismatic property, related to a classification based on an inventory approved by the specific subject area.</rdfs:comment>
        <rdfs:isDefinedBy rdf:resource="https://w3id.org/arco/ontology/arco"/>
        <rdfs:label xml:lang="it">Categoria di bene culturale basata su repertorio</rdfs:label>
        <rdfs:label xml:lang="en">Cultural property inventory category</rdfs:label>
        <owl:versionInfo xml:lang="it">stabile</owl:versionInfo>
        <owl:versionInfo xml:lang="en">stable</owl:versionInfo>
        <a-cat:iccdNormTag>ICCD Normativa Trasversale 4.00: OG/OGT/OGTS</a-cat:iccdNormTag>
    </owl:Class>
    


    <!-- https://w3id.org/arco/ontology/arco/CulturalPropertyPart -->

    <owl:Class rdf:about="https://w3id.org/arco/ontology/arco/CulturalPropertyPart">
        <rdfs:subClassOf rdf:resource="http://dati.beniculturali.it/cis/CulturalEntity"/>
        <rdfs:subClassOf>
            <owl:Restriction>
                <owl:onProperty rdf:resource="https://w3id.org/arco/ontology/arco/numberOfCulturalPropertyParts"/>
                <owl:allValuesFrom rdf:resource="http://www.w3.org/2001/XMLSchema#integer"/>
            </owl:Restriction>
        </rdfs:subClassOf>
        <rdfs:comment xml:lang="it">Questa classe rappresenta, a un livello generico, una parte di un bene culturale descritto in una scheda cui si possono riferire informazioni specifiche.</rdfs:comment>
        <rdfs:comment xml:lang="en">This class represents a generic part of a cultural property, to which some specific information is referred.</rdfs:comment>
        <rdfs:isDefinedBy rdf:resource="https://w3id.org/arco/ontology/arco"/>
        <rdfs:label xml:lang="en">Cultural Property Part</rdfs:label>
        <rdfs:label xml:lang="it">Parte di Bene Culturale</rdfs:label>
        <owl:versionInfo xml:lang="it">stabile</owl:versionInfo>
        <owl:versionInfo xml:lang="en">stable</owl:versionInfo>
        <a-cat:iccdNormTag xml:lang="it">&quot;Riferimento alla parte&quot;, presente in molti campi strutturati delle normative ICCD - ICCD Normativa AT 3.01: EL/ELE</a-cat:iccdNormTag>
    </owl:Class>
    


    <!-- https://w3id.org/arco/ontology/arco/CulturalPropertyResidual -->

    <owl:Class rdf:about="https://w3id.org/arco/ontology/arco/CulturalPropertyResidual">
        <rdfs:subClassOf rdf:resource="https://w3id.org/arco/ontology/arco/CulturalProperty"/>
        <rdfs:subClassOf>
            <owl:Restriction>
                <owl:onProperty rdf:resource="https://w3id.org/arco/ontology/arco/isCulturalPropertyResidualOf"/>
                <owl:someValuesFrom rdf:resource="https://w3id.org/arco/ontology/arco/CulturalProperty"/>
            </owl:Restriction>
        </rdfs:subClassOf>
        <rdfs:subClassOf>
            <owl:Restriction>
                <owl:onProperty rdf:resource="https://w3id.org/arco/ontology/arco/numberOfResiduals"/>
                <owl:allValuesFrom rdf:resource="http://www.w3.org/2001/XMLSchema#integer"/>
            </owl:Restriction>
        </rdfs:subClassOf>
        <rdfs:comment xml:lang="it">Questa classe rappresenta la parte residuale di un bene culturale, cioè la parte che si conserva del bene culturale originale.</rdfs:comment>
        <rdfs:comment xml:lang="en">This class represents the residual part of a cultural property, that is what&apos;s left of the original cultural property.</rdfs:comment>
        <rdfs:isDefinedBy rdf:resource="https://w3id.org/arco/ontology/arco"/>
        <rdfs:label xml:lang="en">Cultural Property Residual</rdfs:label>
        <rdfs:label xml:lang="it">Parte Residuale di Bene Culturale</rdfs:label>
        <owl:versionInfo xml:lang="it">stabile</owl:versionInfo>
        <owl:versionInfo xml:lang="en">stable</owl:versionInfo>
        <a-cat:iccdNormTag>OG/OGT/OGTW</a-cat:iccdNormTag>
    </owl:Class>
    


    <!-- https://w3id.org/arco/ontology/arco/DemoEthnoAnthropologicalHeritage -->

    <owl:Class rdf:about="https://w3id.org/arco/ontology/arco/DemoEthnoAnthropologicalHeritage">
        <rdfs:subClassOf rdf:resource="https://w3id.org/arco/ontology/arco/CulturalProperty"/>
        <rdfs:subClassOf>
            <owl:Restriction>
                <owl:onProperty rdf:resource="https://w3id.org/arco/ontology/context-description/hasPrimaryDocumentation"/>
                <owl:allValuesFrom rdf:resource="https://w3id.org/arco/ontology/context-description/Documentation"/>
            </owl:Restriction>
        </rdfs:subClassOf>
        <rdfs:subClassOf>
            <owl:Restriction>
                <owl:onProperty rdf:resource="https://w3id.org/arco/ontology/context-description/hasResearch"/>
                <owl:allValuesFrom rdf:resource="https://w3id.org/arco/ontology/context-description/Research"/>
            </owl:Restriction>
        </rdfs:subClassOf>
        <rdfs:comment xml:lang="it">Questa classe rappresenta un bene culturale demoetnoantropologico, che può essere di tipo immateriale e materiale. I beni demoetnoantropologici immateriali sono beni consistenti in performance uniche e irrepetibili strutturalmente connesse al territorio e a prassi socialmente condivise trasmesse attraverso l’oralità e le tecniche corporali, tanto in ambito italiano quanto in ambito europeo ed extra-europeo (comunicazioni non verbali, danze, feste e cerimonie, giochi, letterature orali, musiche, norme consuetudinarie, rappresentazioni e spettacoli, saperi, tecniche). I beni demoetnoantropologici materiali sono beni la cui costruzione e/o il cui uso sono strutturalmente associati a prassi socialmente condivise, trasmesse attraverso l&apos;oralità e le tecniche corporali, tanto in ambito italiano quanto in ambito europeo ed extra-europeo (abbigliamento e ornamenti del corpo, arredi e suppellettili, mezzi di trasporto, ritualità, strumenti e accessori, beni sul territorio).</rdfs:comment>
        <rdfs:comment xml:lang="en">This class represents a demo-ethno-anthropological heritage, both tangible and intangible. The intangible demoetnoanthropological properties are cultural properties consisting of unique and unrepeatable performances, structurally connected to the territory and to socially shared custom, transmitted through orality and bodily techniques, both in Italy and in Europe and beyond Europe (non-verbal communications, dances, parties and ceremonies, games, oral letters, music, customary norms, performances and shows, knowledge, techniques). Demo-ethno-anthropological tangible properties are cultural properties whose construction and/or use are structurally associated with a socially shared custom, transmitted through orality and bodily techniques, both in the Italian and European and extra-European areas (clothing and body ornaments, furnishings and furnishings, means of transport, rituals, instruments and accessories, properties on the territory).</rdfs:comment>
        <rdfs:isDefinedBy rdf:resource="https://w3id.org/arco/ontology/arco"/>
        <rdfs:label xml:lang="it">Bene Demoetnoantropologico</rdfs:label>
        <rdfs:label xml:lang="en">Demo-ethno-anthropological Heritage</rdfs:label>
        <owl:versionInfo xml:lang="it">stabile</owl:versionInfo>
        <owl:versionInfo xml:lang="en">stable</owl:versionInfo>
    </owl:Class>
    


    <!-- https://w3id.org/arco/ontology/arco/HistoricOrArtisticProperty -->

    <owl:Class rdf:about="https://w3id.org/arco/ontology/arco/HistoricOrArtisticProperty">
        <rdfs:subClassOf rdf:resource="https://w3id.org/arco/ontology/arco/MovableCulturalProperty"/>
        <rdfs:subClassOf>
            <owl:Restriction>
                <owl:onProperty rdf:resource="https://w3id.org/arco/ontology/context-description/hasFruition"/>
                <owl:allValuesFrom rdf:resource="https://w3id.org/arco/ontology/context-description/Fruition"/>
            </owl:Restriction>
        </rdfs:subClassOf>
        <rdfs:subClassOf>
            <owl:Restriction>
                <owl:onProperty rdf:resource="https://w3id.org/arco/ontology/context-description/numberInCirculation"/>
                <owl:allValuesFrom rdf:resource="http://www.w3.org/2000/01/rdf-schema#Literal"/>
            </owl:Restriction>
        </rdfs:subClassOf>
        <rdfs:comment xml:lang="it">Questa classe rappresenta un bene culturale storico e artistico, che può essere un disegno, una matrice incisa, un&apos;opera o oggetto d&apos;arte (contemporanea e non), una stampa, un vestimento antico o contemporaneo. Disegni: opere fatte a mano su qualsiasi supporto (carta, cartoncino, cartone, intonaco, legno, pergamena, pietra, seta, tavola, tela ecc.) e con particolari strumenti (carboncino, gessetto, inchiostro, lapis, matita, pastello, penna ecc.) e specifiche tecniche (acquarellatura, sanguigna ecc.). Matrici incise: lastre di vario materiale (acciaio, legno, linoleum, ottone, pietra, zinco rame ecc.) su cui vengono tracciate rappresentazioni pittoriche con particolari strumenti (bulino, punte di acciaio o di diamante, punzoni, raschietti ecc.) e con specifiche tecniche di incisione (acquaforte, acquatinta, litografia, mezzatinta, serigrafia, silografia, zincografia ecc.). Opere e oggetti d&apos;arte: beni mobili costituenti parte integrante di monumenti artistici e storici o provenienti dallo smembramento dei monumenti stessi, conservati in collezioni, musei e pinacoteche (armi ed armature, arredi civili e religiosi, oggetti per il culto, oggetti d&apos;uso, opere di pittura, tessuti e arazzi, sulture, ecc.). Opere e oggetti d&apos;arte contemporanea: opere rappresentative  delle nuove correnti artistiche dei secc. XX e  XXI (assemblaggio, computer art, istallazione, istallazione ambientale, istallazione audio, istallazione video, istallazione multimediale interattiva, opera cinetico-visuale, performance, ready made, realtà virtuale, video arte ecc.). Stampe: esemplari prodotti dall&apos;operazione mediante la quale da una matrice di incisione si ottengono copie uguali di rappresentazioni pittoriche su carta, cartoncino, cuoio,  pergamena, seta ecc. con varie tecniche di incisione (acquaforte, acquatinta, litografia, zincografia ecc.). Vestimenti antichi e contemporanei: abiti e costumi riguardanti l’abbigliamento maschile, femminile e infantile ad uso civile, connessi alle principali finalità d’uso e alle diverse occasioni della vita privata e sociale,  secondo le tipologie storiche dei secoli XVIII, XIX, XX  (abiti, biancheria intima, calzetteria, calzoni, camicie, costumi, cuffie, gonne, giacche, grembiuli, livree, maglie, mantelli, scialli, sciarpe, veli ecc.).</rdfs:comment>
        <rdfs:comment xml:lang="en">This class represents an historic or artistic property: drawing, printing plate, (contemporary) artworks, print, historic and contemporary garment. Drawings: works done by hand on any support (paper, cardboard, plaster, wood, parchment, stone, silk, table, canvas, etc.) and with special tools (charcoal, chalk, ink, pencil, pastel, pen etc.) and technical specifications (watercolor, blood, etc.). Printing plates: plates of various materials (steel, wood, linoleum, brass, stone, copper zinc, etc.) on which pictorial representations are traced with particular tools (burin, steel or diamond points, punches, scrapers, etc.) and with technical specifications for etching (etching, aquatint, lithography, halftone, screen printing, silica, zincography, etc.). Artworks: movable cultural properties that are integral part of artistic and historical monuments or coming from the dismemberment of the monuments themselves, preserved in collections, museums and art galleries (weapons and armor, civil and religious furnishings, objects for worship, everyday objects, paintings, fabrics and tapestries, walls, etc.). Contemporary artworks: cultural properties representative of the new artistic currents of the centuries XX and XXI (assembly, computer art, installation, environmental installation, audio installation, video installation, interactive multimedia installation, kinetic-visual work, performance, ready-made, virtual reality, video art, etc.). Prints: specimens created through this process: equal copies of pictorial representations on paper, cardboard, leather, parchment, silk, etc. are obtained from a printing plate, with various engraving techniques (etching, aquatint, lithography, zincography, etc.). Historic and contemporary garments: clothes and costumes for men&apos;s, women&apos;s and children&apos;s clothing for civil use, connected to the main intended use and to different occasions of private and social life, according to the historical typologies of the XVIII, XIX and XX centuries (dresses, underwear, hosiery, trousers, shirts, costumes, headphones, skirts, jackets, aprons, liveries, sweaters, cloaks, shawls, scarves, veils, etc.).</rdfs:comment>
        <rdfs:isDefinedBy rdf:resource="https://w3id.org/arco/ontology/arco"/>
        <rdfs:label xml:lang="it">Bene Storico o Artistico</rdfs:label>
        <rdfs:label xml:lang="en">Historic Or Artistic Property</rdfs:label>
        <owl:versionInfo xml:lang="it">stabile</owl:versionInfo>
        <owl:versionInfo xml:lang="en">stable</owl:versionInfo>
    </owl:Class>
    


    <!-- https://w3id.org/arco/ontology/arco/HornbostelSachsClassification -->

    <owl:Class rdf:about="https://w3id.org/arco/ontology/arco/HornbostelSachsClassification">
        <rdfs:subClassOf rdf:resource="https://w3id.org/arco/ontology/arco/MusicalInstrumentClassification"/>
        <rdfs:subClassOf>
            <owl:Restriction>
                <owl:onProperty rdf:resource="https://w3id.org/arco/ontology/arco/HSNumber"/>
                <owl:someValuesFrom rdf:resource="http://www.w3.org/2000/01/rdf-schema#Literal"/>
            </owl:Restriction>
        </rdfs:subClassOf>
        <rdfs:subClassOf>
            <owl:Restriction>
                <owl:onProperty rdf:resource="https://w3id.org/arco/ontology/arco/HSDefinition"/>
                <owl:allValuesFrom rdf:resource="http://www.w3.org/2000/01/rdf-schema#Literal"/>
            </owl:Restriction>
        </rdfs:subClassOf>
        <rdfs:subClassOf>
            <owl:Restriction>
                <owl:onProperty rdf:resource="https://w3id.org/arco/ontology/arco/HSEdition"/>
                <owl:allValuesFrom rdf:resource="http://www.w3.org/2000/01/rdf-schema#Literal"/>
            </owl:Restriction>
        </rdfs:subClassOf>
        <rdfs:comment xml:lang="it">Questa classe rappresenta la classificazione Hornbostel-Sachs di uno strumento musicale.</rdfs:comment>
        <rdfs:comment xml:lang="en">This class represents the Hornbostel-Sachs classification of a musical instrument.</rdfs:comment>
        <rdfs:isDefinedBy rdf:resource="https://w3id.org/arco/ontology/arco"/>
        <rdfs:label xml:lang="it">Classificazione Hornbostel-Sachs</rdfs:label>
        <rdfs:label xml:lang="en">Hornbostel-Sachs classification</rdfs:label>
        <owl:versionInfo xml:lang="it">stabile</owl:versionInfo>
        <owl:versionInfo xml:lang="en">stable</owl:versionInfo>
        <a-cat:iccdNormTag>Normativa SM 4.00: CL/CHS</a-cat:iccdNormTag>
    </owl:Class>
    


    <!-- https://w3id.org/arco/ontology/arco/ImmovableCulturalProperty -->

    <owl:Class rdf:about="https://w3id.org/arco/ontology/arco/ImmovableCulturalProperty">
        <rdfs:subClassOf rdf:resource="https://w3id.org/arco/ontology/arco/TangibleCulturalProperty"/>
        <owl:disjointWith rdf:resource="https://w3id.org/arco/ontology/arco/MovableCulturalProperty"/>
        <rdfs:comment xml:lang="it">Questa classe rappresenta un bene materiale immobile, cioè un bene agganciato e/o incorporato al suolo (edifici, complessi monumentali, spazi territoriali, ecc.) che presentano, in genere, un consistente sviluppo spaziale. Si intende come un particolare tipo di Site (contenitore fisico), in quanto luogo fisico georeferenziato che possiede esso stesso un interesse culturale.</rdfs:comment>
        <rdfs:comment xml:lang="en">This class represents an immovable cultural property, a property fastened and/or incorporated into the ground (buildings, monumental complexes, territorial areas, etc.) which generally has a significant spatial extent.</rdfs:comment>
        <rdfs:isDefinedBy rdf:resource="https://w3id.org/arco/ontology/arco"/>
        <rdfs:label xml:lang="it">Bene immobile</rdfs:label>
        <rdfs:label xml:lang="en">Immovable Cultural Property</rdfs:label>
        <owl:versionInfo xml:lang="it">stabile</owl:versionInfo>
        <owl:versionInfo xml:lang="en">stable</owl:versionInfo>
    </owl:Class>
    


    <!-- https://w3id.org/arco/ontology/arco/IntangibleCulturalProperty -->

    <owl:Class rdf:about="https://w3id.org/arco/ontology/arco/IntangibleCulturalProperty">
        <rdfs:subClassOf rdf:resource="https://w3id.org/arco/ontology/arco/CulturalProperty"/>
        <owl:disjointWith rdf:resource="https://w3id.org/arco/ontology/arco/TangibleCulturalProperty"/>
        <rdfs:comment xml:lang="it">Questa classe rappresenta un bene immateriale, cioè quella parte del patrimonio culturale rappresentata da performance effimere di manifestazioni tradizionali, tecniche, saperi (feste, esecuzioni musicali e coreutiche, rappresentazioni teatrali, tecniche artigianali, letteratura orale, ecc.), colte nel momento in cui avvengono e di cui è possibile mantenere memoria solo attraverso la ripresa audio-visiva che le fissa stabilmente, cristallizzandole.</rdfs:comment>
        <rdfs:comment xml:lang="en">This class represents an intangible cultural property, that part of cultural heritage represented by ephemeral performances of traditional manifestations, techniques, knowledge (festivals, musical and dance performances, theatrical performances, craft techniques, oral literature, etc.), when they occur and of which it is possible to keep memory only through the audio-visual recording that fixes them permanently, crystallizing them.</rdfs:comment>
        <rdfs:isDefinedBy rdf:resource="https://w3id.org/arco/ontology/arco"/>
        <rdfs:label xml:lang="it">Bene immateriale</rdfs:label>
        <rdfs:label xml:lang="en">Intangible Cultural Property</rdfs:label>
        <owl:versionInfo xml:lang="it">stabile</owl:versionInfo>
        <owl:versionInfo xml:lang="en">stable</owl:versionInfo>
    </owl:Class>
    


    <!-- https://w3id.org/arco/ontology/arco/MibacScopeOfProtection -->

    <owl:Class rdf:about="https://w3id.org/arco/ontology/arco/MibacScopeOfProtection">
        <owl:equivalentClass>
            <owl:Class>
                <owl:oneOf rdf:parseType="Collection">
                    <rdf:Description rdf:about="https://w3id.org/arco/ontology/arco/ArchaeologicalScope"/>
                    <rdf:Description rdf:about="https://w3id.org/arco/ontology/arco/ArchitecturalLandscapeScope"/>
                    <rdf:Description rdf:about="https://w3id.org/arco/ontology/arco/EthnoAnthropologicalScope"/>
                    <rdf:Description rdf:about="https://w3id.org/arco/ontology/arco/HistoricalArtisticScope"/>
                </owl:oneOf>
            </owl:Class>
        </owl:equivalentClass>
        <rdfs:subClassOf>
            <owl:Restriction>
                <owl:onProperty rdf:resource="https://w3id.org/arco/ontology/arco/isMibacScopeOfProtectionOf"/>
                <owl:someValuesFrom rdf:resource="https://w3id.org/arco/ontology/arco/CulturalProperty"/>
            </owl:Restriction>
        </rdfs:subClassOf>
        <rdfs:comment xml:lang="it">Questa classe rappresenta l&apos;ambito di tutela del MiBAC (archeologico, architettonico e paesaggistico, etnoantropologico, storico artistico), nel quale ricade il bene culturale in esame.</rdfs:comment>
        <rdfs:comment xml:lang="en">This class represents the MiBAC scope of protection (historical artistic, ethnoanthropological, architectural landscape, archaeological) of a cultural property.</rdfs:comment>
        <rdfs:isDefinedBy rdf:resource="https://w3id.org/arco/ontology/arco"/>
        <rdfs:label xml:lang="it">Ambito di tutela MiBAC</rdfs:label>
        <rdfs:label xml:lang="en">MiBAC Scope of protection</rdfs:label>
        <owl:versionInfo xml:lang="it">stabile</owl:versionInfo>
        <owl:versionInfo xml:lang="en">stable</owl:versionInfo>
    </owl:Class>
    


    <!-- https://w3id.org/arco/ontology/arco/MineralHeritage -->

    <owl:Class rdf:about="https://w3id.org/arco/ontology/arco/MineralHeritage">
        <rdfs:subClassOf rdf:resource="https://w3id.org/arco/ontology/arco/NaturalHeritage"/>
        <rdfs:comment xml:lang="it">Questa classe rappresenta esemplari di minerali provenienti da collezioni di mineralogia (Augite, Goethite, scatola di quarzi ecc. ).</rdfs:comment>
        <rdfs:comment xml:lang="en">This class represents specimens of minerals from collections of mineralogy (Augite, Goethite, box of quartz etc.).</rdfs:comment>
        <rdfs:label xml:lang="it">Bene Minerale</rdfs:label>
        <rdfs:label xml:lang="en">Mineral Heritage</rdfs:label>
        <owl:versionInfo xml:lang="it">instabile</owl:versionInfo>
        <owl:versionInfo xml:lang="en">unstable</owl:versionInfo>
    </owl:Class>
    


    <!-- https://w3id.org/arco/ontology/arco/MovableCulturalProperty -->

    <owl:Class rdf:about="https://w3id.org/arco/ontology/arco/MovableCulturalProperty">
        <rdfs:subClassOf rdf:resource="https://w3id.org/arco/ontology/arco/TangibleCulturalProperty"/>
        <rdfs:subClassOf>
            <owl:Restriction>
                <owl:onProperty rdf:resource="https://w3id.org/arco/ontology/context-description/hasEstimate"/>
                <owl:allValuesFrom rdf:resource="https://w3id.org/arco/ontology/context-description/Estimate"/>
            </owl:Restriction>
        </rdfs:subClassOf>
        <rdfs:subClassOf>
            <owl:Restriction>
                <owl:onProperty rdf:resource="https://w3id.org/arco/ontology/context-description/isMemberOfCollection"/>
                <owl:allValuesFrom rdf:resource="https://w3id.org/arco/ontology/context-description/CollectionMembership"/>
            </owl:Restriction>
        </rdfs:subClassOf>
        <rdfs:comment xml:lang="it">Questa classe rappresenta un bene materiale mobile, cioè un oggetto o un manufatto che può essere movimentato in vario modo. I beni mobili possono risultare &quot;immobilizzati per destinazione&quot;, cioè incorporati saldamente nel contesto in cui si trovano.</rdfs:comment>
        <rdfs:comment xml:lang="en">This class represents a movable cultural property, that is, an object or an artefact that can be moved in various ways. Movable cultural properties may be &quot;immobilized by destination&quot;, i.e. incorporated firmly in the context in which they are located.</rdfs:comment>
        <rdfs:isDefinedBy rdf:resource="https://w3id.org/arco/ontology/arco"/>
        <rdfs:label xml:lang="it">Bene mobile</rdfs:label>
        <rdfs:label xml:lang="en">Movable Cultural Property</rdfs:label>
        <owl:versionInfo xml:lang="en">stable</owl:versionInfo>
        <owl:versionInfo xml:lang="it">stable</owl:versionInfo>
    </owl:Class>
    


    <!-- https://w3id.org/arco/ontology/arco/MusicHeritage -->

    <owl:Class rdf:about="https://w3id.org/arco/ontology/arco/MusicHeritage">
        <rdfs:subClassOf rdf:resource="https://w3id.org/arco/ontology/arco/MovableCulturalProperty"/>
        <rdfs:subClassOf>
            <owl:Restriction>
                <owl:onProperty rdf:resource="https://w3id.org/arco/ontology/arco/hasMusicalInstrumentClassification"/>
                <owl:allValuesFrom rdf:resource="https://w3id.org/arco/ontology/arco/MusicalInstrumentClassification"/>
            </owl:Restriction>
        </rdfs:subClassOf>
        <rdfs:subClassOf>
            <owl:Restriction>
                <owl:onProperty rdf:resource="https://w3id.org/arco/ontology/context-description/hasMusicalEnsemble"/>
                <owl:allValuesFrom rdf:resource="https://w3id.org/italia/onto/l0/Agent"/>
            </owl:Restriction>
        </rdfs:subClassOf>
        <rdfs:subClassOf>
            <owl:Restriction>
                <owl:onProperty rdf:resource="https://w3id.org/arco/ontology/context-description/hasMusician"/>
                <owl:allValuesFrom rdf:resource="https://w3id.org/italia/onto/l0/Agent"/>
            </owl:Restriction>
        </rdfs:subClassOf>
        <rdfs:subClassOf>
            <owl:Restriction>
                <owl:onProperty rdf:resource="https://w3id.org/arco/ontology/context-description/hasResearch"/>
                <owl:allValuesFrom rdf:resource="https://w3id.org/arco/ontology/context-description/Research"/>
            </owl:Restriction>
        </rdfs:subClassOf>
        <rdfs:subClassOf>
            <owl:Restriction>
                <owl:onProperty rdf:resource="https://w3id.org/arco/ontology/denotative-description/hasAccessory"/>
                <owl:allValuesFrom rdf:resource="https://w3id.org/arco/ontology/denotative-description/Accessory"/>
            </owl:Restriction>
        </rdfs:subClassOf>
        <rdfs:comment xml:lang="it">Questa classe rappresenta un bene culturale musicale. Strumenti musicali: oggetti nati appositamente per produrre suoni organizzati secondo le diverse culture musicali, senza limiti spazio-temporali (strumenti e accessori di interesse archeologico, storico artistico, etnoantropologico). Strumenti musicali-Organo: oggetto nato per produrre suoni,  costituito da una serie di canne metalliche,  di forma, lunghezza e diametro diversi, nelle quali viene immessa, per mezzo di un mantice o altro meccanismo, una quantità d’aria regolata da una o più tastiere e da una pedaliera (corredato da accessori), caratterizzato da specifici aspetti  morfologici-decorativi e fonico-strumentali (organo idraulico, organo positivo, organo portativo, organo elettronico ecc.)</rdfs:comment>
        <rdfs:comment xml:lang="en">This class represents a music heritage. Musical instruments: objects created specifically to produce sounds according to different musical cultures, without space-time limits (instruments and accessories of archaeological, artistic, ethno-anthropological interest). Musical instruments-Organ: an object created to produce sounds, consisting of a series of metal rods, of different shape, length and diameter, in which a quantity of air is introduced, by means of a bellows or other mechanism, regulated by one or more keyboards and a pedal board (accompanied by accessories), characterized by specific morphological-decorative and phonic-instrumental aspects (hydraulic organ, positive organ, portative organ, electronic organ, etc.)</rdfs:comment>
        <rdfs:isDefinedBy rdf:resource="https://w3id.org/arco/ontology/arco"/>
        <rdfs:label xml:lang="it">Bene Musicale</rdfs:label>
        <rdfs:label xml:lang="en">Music Heritage</rdfs:label>
        <owl:versionInfo xml:lang="it">stabile</owl:versionInfo>
        <owl:versionInfo xml:lang="en">stable</owl:versionInfo>
    </owl:Class>
    


    <!-- https://w3id.org/arco/ontology/arco/MusicalInstrumentClassification -->

    <owl:Class rdf:about="https://w3id.org/arco/ontology/arco/MusicalInstrumentClassification">
        <rdfs:subClassOf rdf:resource="https://w3id.org/arco/ontology/core/CulturalEntityClassification"/>
        <rdfs:subClassOf>
            <owl:Restriction>
                <owl:onProperty rdf:resource="https://w3id.org/arco/ontology/arco/isMusicalInstrumentClassificationOf"/>
                <owl:someValuesFrom rdf:resource="https://w3id.org/arco/ontology/arco/MusicHeritage"/>
            </owl:Restriction>
        </rdfs:subClassOf>
        <rdfs:comment xml:lang="it">Questa classe rappresenta una classificazione relativa a uno strumento musicale, secondo la classificazione di Hornbostel-Sachs ed eventualmente anche secondo altre classificazioni.</rdfs:comment>
        <rdfs:comment xml:lang="en">This class represents a classification concerning a musical instrument, concerning the Hornbostel-Sachs classification or possibily other classifications.</rdfs:comment>
        <rdfs:isDefinedBy rdf:resource="https://w3id.org/arco/ontology/arco"/>
        <rdfs:label xml:lang="it">Classificazione di strumento musicale</rdfs:label>
        <rdfs:label xml:lang="en">Musical instrument classification</rdfs:label>
        <owl:versionInfo xml:lang="it">stabile</owl:versionInfo>
        <owl:versionInfo xml:lang="en">stable</owl:versionInfo>
        <a-cat:iccdNormTag>Normativa SM 4.00: CL</a-cat:iccdNormTag>
    </owl:Class>
    


    <!-- https://w3id.org/arco/ontology/arco/NaturalHeritage -->

    <owl:Class rdf:about="https://w3id.org/arco/ontology/arco/NaturalHeritage">
        <rdfs:subClassOf rdf:resource="https://w3id.org/arco/ontology/arco/MovableCulturalProperty"/>
        <rdfs:comment xml:lang="it">Questa classe rappresenta un bene culturale naturalistico, relativo ai campi della botanica, della mineralogia, della paleontologia, della petrologia, della planetologia, della zoologia. Botanica: esemplari del mondo vegetale provenienti da collezioni di botanica  (raccolte di piante essiccate: erbari). Mineralogia: esemplari di minerali provenienti da collezioni di mineralogia (Augite, Goethite, scatola di quarzi ecc. ). Paleontologia: reperti fossili (animali, vegetali, ichnofossili, campioni e preparati per microscopio, ecc.). Petrologia: esemplari di rocce provenienti da collezioni (Riolite, Trachiandesite ecc). Planetologia: esemplari di meteoriti provenienti da collezioni ( Aubrite, Ureilite, Eucrite ecc.). Zoologia: esemplari del mondo animale provenienti da collezioni di zoologia (ustiolo, toporagno, mammifero, artropode, scatola di farfalle, collezione elmintologica, ecc.)</rdfs:comment>
        <rdfs:comment xml:lang="en">This class represents a natural heritage, related to botany, mineralogy, paleontology, petrology, planetary science, zoology. Botany: specimens of the plant world from botanical collections (collections of dried plants: herbaria). Mineralogy: specimens of minerals from collections of mineralogy (Augite, Goethite, box of quartz etc.). Paleontology: fossil finds (animals, plants, ichnofossils, samples and microscope preparations, etc.). Petrology: specimens of rocks from collections (Riolite, Trachiandesite etc.). Planetology: meteorites from collections (Aubrite, Ureilite, Eucrite, etc.). Zoology: specimens of the animal world from zoology collections (ustiolo, shrew, mammal, arthropod, butterfly box, elmintological collection, etc.)</rdfs:comment>
        <rdfs:isDefinedBy rdf:resource="https://w3id.org/arco/ontology/arco"/>
        <rdfs:label xml:lang="it">Bene Naturalistico</rdfs:label>
        <rdfs:label xml:lang="en">Natural Heritage</rdfs:label>
        <owl:versionInfo xml:lang="it">stabile</owl:versionInfo>
        <owl:versionInfo xml:lang="en">stable</owl:versionInfo>
    </owl:Class>
    


    <!-- https://w3id.org/arco/ontology/arco/NumismaticProperty -->

    <owl:Class rdf:about="https://w3id.org/arco/ontology/arco/NumismaticProperty">
        <rdfs:subClassOf rdf:resource="https://w3id.org/arco/ontology/arco/MovableCulturalProperty"/>
        <rdfs:subClassOf>
            <owl:Restriction>
                <owl:onProperty rdf:resource="https://w3id.org/arco/ontology/arco/hasNumismaticPropertyCategory"/>
                <owl:allValuesFrom rdf:resource="https://w3id.org/arco/ontology/arco/NumismaticProperty"/>
            </owl:Restriction>
        </rdfs:subClassOf>
        <rdfs:subClassOf>
            <owl:Restriction>
                <owl:onProperty rdf:resource="https://w3id.org/arco/ontology/context-description/hasCoinIssuance"/>
                <owl:allValuesFrom rdf:resource="https://w3id.org/arco/ontology/context-description/CoinIssuance"/>
            </owl:Restriction>
        </rdfs:subClassOf>
        <rdfs:subClassOf>
            <owl:Restriction>
                <owl:onProperty rdf:resource="https://w3id.org/arco/ontology/context-description/isCoinMemberOf"/>
                <owl:allValuesFrom rdf:resource="https://w3id.org/arco/ontology/context-description/NumismaticSeries"/>
            </owl:Restriction>
        </rdfs:subClassOf>
        <rdfs:comment xml:lang="it">Questa classe rappresenta un bene culturale numismatico, ovvero monete e altri oggetti di interesse numismatico (reperti premonetali e paramonetali, conii e punzoni monetali, pesi per il controllo monetale, sigilli e medaglie), pertinenti a  qualsiasi epoca.</rdfs:comment>
        <rdfs:comment xml:lang="en">This class represents a numismatic property, that is coins and other objects of numismatic interest (premonetal and paramonetal finds, coinage and monetary punches, weights for monetary control, seals and medals), pertinent to any age.</rdfs:comment>
        <rdfs:isDefinedBy rdf:resource="https://w3id.org/arco/ontology/arco"/>
        <rdfs:label xml:lang="it">Bene Numismatico</rdfs:label>
        <rdfs:label xml:lang="en">Numismatic Property</rdfs:label>
        <owl:versionInfo xml:lang="it">stabile</owl:versionInfo>
        <owl:versionInfo xml:lang="en">stable</owl:versionInfo>
    </owl:Class>
    


    <!-- https://w3id.org/arco/ontology/arco/NumismaticPropertyCategory -->

    <owl:Class rdf:about="https://w3id.org/arco/ontology/arco/NumismaticPropertyCategory">
        <rdfs:subClassOf rdf:resource="https://w3id.org/arco/ontology/core/Category"/>
        <rdfs:subClassOf>
            <owl:Restriction>
                <owl:onProperty rdf:resource="https://w3id.org/arco/ontology/arco/isNumismaticPropertyCategoryOf"/>
                <owl:someValuesFrom rdf:resource="https://w3id.org/arco/ontology/arco/NumismaticProperty"/>
            </owl:Restriction>
        </rdfs:subClassOf>
        <rdfs:comment xml:lang="it">Questa classe rappresenta la categoria di un bene numismatico, in riferimento a una classificazione relativa alla tipologia, alla funzione, alla destinazione, o alla committenza del bene catalogato, secondo le classificazioni più consuete.</rdfs:comment>
        <rdfs:comment xml:lang="en">This class represents a category of a numismatic property, referring to a classification related to the type or the function or the commission of the cultural property, according to the most common classifications.</rdfs:comment>
        <rdfs:isDefinedBy rdf:resource="https://w3id.org/arco/ontology/arco"/>
        <rdfs:label xml:lang="it">Classificazione di bene numismatico</rdfs:label>
        <rdfs:label xml:lang="en">Numismatic property classification</rdfs:label>
        <owl:versionInfo xml:lang="it">stabile</owl:versionInfo>
        <owl:versionInfo xml:lang="en">stable</owl:versionInfo>
    </owl:Class>
    


    <!-- https://w3id.org/arco/ontology/arco/NumismaticPropertyFunctionalCategory -->

    <owl:Class rdf:about="https://w3id.org/arco/ontology/arco/NumismaticPropertyFunctionalCategory">
        <rdfs:subClassOf rdf:resource="https://w3id.org/arco/ontology/arco/NumismaticPropertyCategory"/>
        <rdfs:subClassOf>
            <owl:Restriction>
                <owl:onProperty rdf:resource="https://w3id.org/arco/ontology/arco/isNumismaticPropertyCategoryOf"/>
                <owl:someValuesFrom rdf:resource="https://w3id.org/arco/ontology/arco/NumismaticProperty"/>
            </owl:Restriction>
        </rdfs:subClassOf>
        <rdfs:comment xml:lang="it">Questa classe rappresenta la categoria funzionale di un bene numismatico, in riferimento a una classificazione relativa alla funzione, o alla destinazione, o alla committenza del bene catalogato, secondo le classificazioni più consuete.</rdfs:comment>
        <rdfs:comment xml:lang="en">This class represents a functional category of a numismatic property, referring to a classification related to the function or the commission of the cultural property, according to the most common classifications.</rdfs:comment>
        <rdfs:label xml:lang="it">Classificazione funzionale di bene numismatico</rdfs:label>
        <rdfs:label xml:lang="en">Numismatic property functional category</rdfs:label>
        <owl:versionInfo xml:lang="it">stabile</owl:versionInfo>
        <owl:versionInfo xml:lang="en">stable</owl:versionInfo>
        <a-cat:iccdNormTag>ICCD Normativa NU 4.00: OG/OGT/OGTH</a-cat:iccdNormTag>
    </owl:Class>
    


    <!-- https://w3id.org/arco/ontology/arco/NumismaticPropertyTypologicalCategory -->

    <owl:Class rdf:about="https://w3id.org/arco/ontology/arco/NumismaticPropertyTypologicalCategory">
        <rdfs:subClassOf rdf:resource="https://w3id.org/arco/ontology/arco/NumismaticPropertyCategory"/>
        <rdfs:subClassOf>
            <owl:Restriction>
                <owl:onProperty rdf:resource="https://w3id.org/arco/ontology/arco/isNumismaticPropertyCategoryOf"/>
                <owl:someValuesFrom rdf:resource="https://w3id.org/arco/ontology/arco/NumismaticProperty"/>
            </owl:Restriction>
        </rdfs:subClassOf>
        <rdfs:comment xml:lang="it">Questa classe rappresenta la categoria di un bene numismatico, in riferimento a una classificazione relativa alla tipologia, secondo le classificazioni più consuete.</rdfs:comment>
        <rdfs:comment xml:lang="en">This class represents a category of a numismatic property, referring to a classification related to the type, according to the most common classifications.</rdfs:comment>
        <rdfs:label xml:lang="it">Classificazione tipologica di bene numismatico</rdfs:label>
        <rdfs:label xml:lang="en">Numismatic property typological category</rdfs:label>
        <owl:versionInfo xml:lang="it">stabile</owl:versionInfo>
        <owl:versionInfo xml:lang="en">stable</owl:versionInfo>
    </owl:Class>
    


    <!-- https://w3id.org/arco/ontology/arco/PalaeontologicalHeritage -->

    <owl:Class rdf:about="https://w3id.org/arco/ontology/arco/PalaeontologicalHeritage">
        <rdfs:subClassOf rdf:resource="https://w3id.org/arco/ontology/arco/NaturalHeritage"/>
        <rdfs:comment xml:lang="it">Questa classe rappresenta eperti fossili (animali, vegetali, ichnofossili, campioni e preparati per microscopio, ecc.)</rdfs:comment>
        <rdfs:comment xml:lang="en">This class represents fossil finds (animals, plants, ichnofossils, samples and microscope preparations, etc.).</rdfs:comment>
        <rdfs:label xml:lang="it">Bene Paleontologico</rdfs:label>
        <rdfs:label xml:lang="en">Palaeontological Heritage</rdfs:label>
        <owl:versionInfo xml:lang="it">instabile</owl:versionInfo>
        <owl:versionInfo xml:lang="en">unstable</owl:versionInfo>
    </owl:Class>
    


    <!-- https://w3id.org/arco/ontology/arco/PetrologicHeritage -->

    <owl:Class rdf:about="https://w3id.org/arco/ontology/arco/PetrologicHeritage">
        <rdfs:subClassOf rdf:resource="https://w3id.org/arco/ontology/arco/NaturalHeritage"/>
        <rdfs:comment xml:lang="it">Questa classe rappresenta esemplari di rocce provenienti da collezioni (Riolite, Trachiandesite ecc).</rdfs:comment>
        <rdfs:comment xml:lang="en">This class represents specimens of rocks from collections (Riolite, Trachiandesite etc.).</rdfs:comment>
        <rdfs:label xml:lang="it">Bene Petrologico</rdfs:label>
        <rdfs:label xml:lang="en">Pertologic Heritage</rdfs:label>
        <owl:versionInfo xml:lang="it">instabile</owl:versionInfo>
        <owl:versionInfo xml:lang="en">unstable</owl:versionInfo>
    </owl:Class>
    


    <!-- https://w3id.org/arco/ontology/arco/PhotographicHeritage -->

    <owl:Class rdf:about="https://w3id.org/arco/ontology/arco/PhotographicHeritage">
        <rdfs:subClassOf rdf:resource="https://w3id.org/arco/ontology/arco/MovableCulturalProperty"/>
        <rdfs:subClassOf>
            <owl:Restriction>
                <owl:onProperty rdf:resource="https://w3id.org/arco/ontology/arco/hasPhotographicHeritageClassification"/>
                <owl:allValuesFrom rdf:resource="https://w3id.org/arco/ontology/arco/PhotographicHeritageClassification"/>
            </owl:Restriction>
        </rdfs:subClassOf>
        <rdfs:subClassOf>
            <owl:Restriction>
                <owl:onProperty rdf:resource="https://w3id.org/arco/ontology/context-description/hasResponsibility"/>
                <owl:allValuesFrom rdf:resource="https://w3id.org/arco/ontology/context-description/Responsibility"/>
            </owl:Restriction>
        </rdfs:subClassOf>
        <rdfs:subClassOf>
            <owl:Restriction>
                <owl:onProperty rdf:resource="https://w3id.org/arco/ontology/context-description/isMemberOfPhotographicSeries"/>
                <owl:allValuesFrom rdf:resource="https://w3id.org/arco/ontology/context-description/PhotographicSeriesMembership"/>
            </owl:Restriction>
        </rdfs:subClassOf>
        <rdfs:subClassOf>
            <owl:Restriction>
                <owl:onProperty rdf:resource="https://w3id.org/arco/ontology/core/hasPart"/>
                <owl:allValuesFrom>
                    <owl:Class>
                        <owl:unionOf rdf:parseType="Collection">
                            <rdf:Description rdf:about="https://w3id.org/arco/ontology/context-description/ArchivalRecord"/>
                            <rdf:Description rdf:about="https://w3id.org/arco/ontology/context-description/ArchivalRecordSet"/>
                        </owl:unionOf>
                    </owl:Class>
                </owl:allValuesFrom>
            </owl:Restriction>
        </rdfs:subClassOf>
        <rdfs:subClassOf>
            <owl:Restriction>
                <owl:onProperty rdf:resource="https://w3id.org/arco/ontology/context-description/numberInCirculation"/>
                <owl:allValuesFrom rdf:resource="http://www.w3.org/2000/01/rdf-schema#Literal"/>
            </owl:Restriction>
        </rdfs:subClassOf>
        <rdfs:comment xml:lang="it">Questa classe rappresenta un bene culturale fotografico, che può essere una fotografia o un fondo fotografico. Beni fotografici: negativi, positivi, processi fotografici che danno origine a prodotti unici (dagherrotipi, ferrotipi, polaroid, chimigrammi, ecc.), fotografia digitale; elementi complessi come album, cartelle, fotomontaggi, panorami, porfolii. Fondi fotografici: entità concettuali che si caratterizzano per l&apos;accumulo di più unità fisiche omogenee o eterogenee dal punto di vista dei materiali che li compongono e che acquisiscono nella loro totalità valenza di bene culturale.</rdfs:comment>
        <rdfs:comment xml:lang="en">This class represents a photographic heritage. Photographs: negative, positive, photographic processes that give rise to unique products (daguerreotypes, ferrotypes, polaroids, chimigrams, etc.), digital photography; complex elements like albums, folders, photomontages, panoramas, porfolii. Photographic funds: conceptual entities that are characterized by the accumulation of multiple homogeneous or heterogeneous physical units from the point of view of the materials that compose them and which represent in their totality a cultural heritage.</rdfs:comment>
        <rdfs:isDefinedBy rdf:resource="https://w3id.org/arco/ontology/arco"/>
        <rdfs:label xml:lang="it">Bene Fotografico</rdfs:label>
        <rdfs:label xml:lang="en">Photographic Heritage</rdfs:label>
        <owl:versionInfo xml:lang="it">stabile</owl:versionInfo>
        <owl:versionInfo xml:lang="en">stable</owl:versionInfo>
    </owl:Class>
    


    <!-- https://w3id.org/arco/ontology/arco/PhotographicHeritageClassification -->

    <owl:Class rdf:about="https://w3id.org/arco/ontology/arco/PhotographicHeritageClassification">
        <rdfs:subClassOf rdf:resource="https://w3id.org/arco/ontology/core/CulturalEntityClassification"/>
        <rdfs:subClassOf>
            <owl:Restriction>
                <owl:onProperty rdf:resource="https://w3id.org/arco/ontology/arco/hasPhotographicHeritageClassificationType"/>
                <owl:someValuesFrom rdf:resource="https://w3id.org/arco/ontology/arco/PhotographicHeritageClassificationType"/>
            </owl:Restriction>
        </rdfs:subClassOf>
        <rdfs:subClassOf>
            <owl:Restriction>
                <owl:onProperty rdf:resource="https://w3id.org/arco/ontology/arco/isPhotographicHeritageClassificationOf"/>
                <owl:someValuesFrom rdf:resource="https://w3id.org/arco/ontology/arco/PhotographicHeritage"/>
            </owl:Restriction>
        </rdfs:subClassOf>
        <rdfs:subClassOf>
            <owl:Restriction>
                <owl:onProperty rdf:resource="https://w3id.org/arco/ontology/arco/classifiedSubject"/>
                <owl:someValuesFrom rdf:resource="http://www.w3.org/2000/01/rdf-schema#Literal"/>
            </owl:Restriction>
        </rdfs:subClassOf>
        <rdfs:comment xml:lang="it">Questa classe rappresenta una classificazione di un bene fotografico secondo un sistema di classificazione alternativo a Iconclass, che sia comunque riconosciuto e utilizzato a livello nazionale, o preferibilmente internazionale.</rdfs:comment>
        <rdfs:comment xml:lang="en">This class represents a photographic entity&apos;s classification according to other classification systems as Iconclass. The system has to be recognised and used at national or preferably international level.</rdfs:comment>
        <rdfs:isDefinedBy rdf:resource="https://w3id.org/arco/ontology/arco"/>
        <rdfs:label xml:lang="it">Classificazione di bene fotografico</rdfs:label>
        <rdfs:label xml:lang="en">Photographic heritage classification</rdfs:label>
        <owl:versionInfo xml:lang="it">stabile</owl:versionInfo>
        <owl:versionInfo xml:lang="en">stable</owl:versionInfo>
        <a-cat:iccdNormTag>ICCD Normativa F 4.00: SG/CLF</a-cat:iccdNormTag>
    </owl:Class>
    


    <!-- https://w3id.org/arco/ontology/arco/PhotographicHeritageClassificationType -->

    <owl:Class rdf:about="https://w3id.org/arco/ontology/arco/PhotographicHeritageClassificationType">
        <rdfs:subClassOf rdf:resource="https://w3id.org/arco/ontology/core/Type"/>
        <rdfs:subClassOf>
            <owl:Restriction>
                <owl:onProperty rdf:resource="https://w3id.org/arco/ontology/arco/isPhotographicHeritageClassificationTypeOf"/>
                <owl:someValuesFrom rdf:resource="https://w3id.org/arco/ontology/arco/PhotographicHeritageClassification"/>
            </owl:Restriction>
        </rdfs:subClassOf>
        <rdfs:comment xml:lang="it">Questa classe rappresenta il tipo di classificazione di un bene fotografico, relativamente a un sistema di classificazione alternativo a Iconclass, che sia comunque riconosciuto e utilizzato a livello nazionale, o preferibilmente internazionale.</rdfs:comment>
        <rdfs:comment xml:lang="en">This class represents photographic property&apos;s classification type,, according to to other classification systems as Iconclass. The system has to be recognised and used at national or preferably international level.</rdfs:comment>
        <rdfs:isDefinedBy rdf:resource="https://w3id.org/arco/ontology/arco"/>
        <rdfs:label xml:lang="en">Photographic heritage classification type</rdfs:label>
        <rdfs:label xml:lang="it">Tipo di classificazione di bene fotografico</rdfs:label>
        <owl:versionInfo xml:lang="it">stabile</owl:versionInfo>
        <owl:versionInfo xml:lang="en">stable</owl:versionInfo>
        <a-cat:iccdNormTag>ICCD Normativa F: SG/CLF/CLFT</a-cat:iccdNormTag>
    </owl:Class>
    


    <!-- https://w3id.org/arco/ontology/arco/PlanetaryScienceHeritage -->

    <owl:Class rdf:about="https://w3id.org/arco/ontology/arco/PlanetaryScienceHeritage">
        <rdfs:subClassOf rdf:resource="https://w3id.org/arco/ontology/arco/NaturalHeritage"/>
        <rdfs:comment xml:lang="it">Questa classe rappresenta esemplari di meteoriti provenienti da collezioni ( Aubrite, Ureilite, Eucrite ecc.).</rdfs:comment>
        <rdfs:comment xml:lang="en">This class represents meteorites from collections (Aubrite, Ureilite, Eucrite, etc.).</rdfs:comment>
        <rdfs:label xml:lang="it">Bene della Scienza Planetaria</rdfs:label>
        <rdfs:label xml:lang="en">Planetary Science Heritage</rdfs:label>
        <owl:versionInfo xml:lang="it">instabile</owl:versionInfo>
        <owl:versionInfo xml:lang="en">unstable</owl:versionInfo>
    </owl:Class>
    


    <!-- https://w3id.org/arco/ontology/arco/RFId -->

    <owl:Class rdf:about="https://w3id.org/arco/ontology/arco/RFId">
        <rdfs:subClassOf>
            <owl:Restriction>
                <owl:onProperty rdf:resource="https://w3id.org/arco/ontology/arco/isRFIdOf"/>
                <owl:someValuesFrom rdf:resource="http://www.w3.org/2002/07/owl#Thing"/>
            </owl:Restriction>
        </rdfs:subClassOf>
        <rdfs:subClassOf>
            <owl:Restriction>
                <owl:onProperty rdf:resource="https://w3id.org/arco/ontology/core/note"/>
                <owl:allValuesFrom rdf:resource="http://www.w3.org/2000/01/rdf-schema#Literal"/>
            </owl:Restriction>
        </rdfs:subClassOf>
        <rdfs:comment xml:lang="it">Questa classe rappresenta l&apos;identificatore a radiofrequenza RFId.</rdfs:comment>
        <rdfs:comment xml:lang="en">This class represents the radio-frequency identification (RFID).</rdfs:comment>
        <rdfs:isDefinedBy rdf:resource="https://w3id.org/arco/ontology/arco"/>
        <rdfs:label xml:lang="it">Identificativo RFId</rdfs:label>
        <rdfs:label xml:lang="en">RFId Identifier</rdfs:label>
        <owl:versionInfo xml:lang="it">stabile</owl:versionInfo>
        <owl:versionInfo xml:lang="en">stable</owl:versionInfo>
        <a-cat:iccdNormTag>ICCD Normativa Trasversale 4.00: RF/RFI</a-cat:iccdNormTag>
    </owl:Class>
    


    <!-- https://w3id.org/arco/ontology/arco/ReferenceCoinLegend -->

    <owl:Class rdf:about="https://w3id.org/arco/ontology/arco/ReferenceCoinLegend">
        <rdfs:subClassOf rdf:resource="https://w3id.org/arco/ontology/core/Concept"/>
        <rdfs:subClassOf>
            <owl:Restriction>
                <owl:onProperty rdf:resource="https://w3id.org/arco/ontology/arco/isReferenceCoinLegendOf"/>
                <owl:someValuesFrom rdf:resource="https://w3id.org/arco/ontology/arco/NumismaticProperty"/>
            </owl:Restriction>
        </rdfs:subClassOf>
        <rdfs:comment xml:lang="it">Questa classe rappresenta la legenda tipo di un bene numismatico, inteso come parametro di classificazione attestato nei repertori di riferimento.</rdfs:comment>
        <rdfs:comment xml:lang="en">This class represents the reference coin legend.</rdfs:comment>
        <rdfs:isDefinedBy rdf:resource="https://w3id.org/arco/ontology/arco"/>
        <rdfs:label xml:lang="it">Legenda tipo</rdfs:label>
        <rdfs:label xml:lang="en">Reference coin legend</rdfs:label>
        <owl:versionInfo xml:lang="it">stabile</owl:versionInfo>
        <owl:versionInfo xml:lang="en">stable</owl:versionInfo>
        <a-cat:iccdNormTag>ICCD Normativa NU: OG/OGT/OGTL</a-cat:iccdNormTag>
    </owl:Class>
    


    <!-- https://w3id.org/arco/ontology/arco/ScientificOrTechnologicalHeritage -->

    <owl:Class rdf:about="https://w3id.org/arco/ontology/arco/ScientificOrTechnologicalHeritage">
        <rdfs:subClassOf rdf:resource="https://w3id.org/arco/ontology/arco/MovableCulturalProperty"/>
        <rdfs:comment xml:lang="it">Questa classe rappresenta un bene culturale scientifico e tecnologico, ovvero strumenti di interesse per la storia della scienza e della tecnica (strumenti astronomici, di laboratorio, di misurazione ecc.) pertinenti a qualsiasi epoca e afferenti a specifiche discipline scientifiche ( apparecchio a specchi a piani rotanti, apparecchio per gli anelli colorati di Newton, campana di Savart, orologio di Farina, orologio solare, pendola, sestante, telescopio ecc.); macchine e macchinari, mezzi di trasporto ecc.</rdfs:comment>
        <rdfs:comment xml:lang="en">This class represents a scientific and technological heritage, that is instruments of interest to the history of science and technology (astronomical, laboratory, measurement, etc.) relevant to any age and related to specific scientific disciplines (flat-mirror luminaire rotating, apparatus for the colored rings of Newton, bell of Savart, Farina clock, solar clock, pendulum, sextant, telescope, etc.); machines and machinery, means of transport, etc.</rdfs:comment>
        <rdfs:isDefinedBy rdf:resource="https://w3id.org/arco/ontology/arco"/>
        <rdfs:label xml:lang="it">Bene Scientifico o Tecnologico</rdfs:label>
        <rdfs:label xml:lang="en">Scientific Or Technological Heritage</rdfs:label>
        <owl:versionInfo xml:lang="it">stabile</owl:versionInfo>
        <owl:versionInfo xml:lang="en">stable</owl:versionInfo>
    </owl:Class>
    


    <!-- https://w3id.org/arco/ontology/arco/TangibleCulturalProperty -->

    <owl:Class rdf:about="https://w3id.org/arco/ontology/arco/TangibleCulturalProperty">
        <rdfs:subClassOf rdf:resource="https://w3id.org/arco/ontology/arco/CulturalProperty"/>
        <rdfs:comment xml:lang="it">Questa classe rappresenta un bene materiale, cioè fisicamente tangibile, sia mobile che immobile.</rdfs:comment>
        <rdfs:comment xml:lang="en">This class represents a tangible cultural property, either immovable or movable.</rdfs:comment>
        <rdfs:isDefinedBy rdf:resource="https://w3id.org/arco/ontology/arco"/>
        <rdfs:label xml:lang="it">Bene materiale</rdfs:label>
        <rdfs:label xml:lang="en">Tangible Cultural Property</rdfs:label>
        <owl:versionInfo xml:lang="it">stabile</owl:versionInfo>
        <owl:versionInfo xml:lang="en">stable</owl:versionInfo>
    </owl:Class>
    


    <!-- https://w3id.org/arco/ontology/arco/ThematicCategory -->

    <owl:Class rdf:about="https://w3id.org/arco/ontology/arco/ThematicCategory">
        <rdfs:subClassOf rdf:resource="https://w3id.org/arco/ontology/core/Category"/>
        <rdfs:subClassOf>
            <owl:Restriction>
                <owl:onProperty rdf:resource="https://w3id.org/arco/ontology/arco/isThematicCategoryOf"/>
                <owl:someValuesFrom rdf:resource="https://w3id.org/arco/ontology/arco/CartographicClassification"/>
            </owl:Restriction>
        </rdfs:subClassOf>
        <rdfs:comment xml:lang="it">Questa classe rappresenta la categoria tematica associata alla classificazione cartografica di un bene culturale (es.: Architetture, Emergenze Archeologiche)</rdfs:comment>
        <rdfs:comment xml:lang="en">This class represents the thematic category associated to a cartographic classification of a cultural property (e.g.: Architecture).</rdfs:comment>
        <rdfs:isDefinedBy rdf:resource="https://w3id.org/arco/ontology/arco"/>
        <rdfs:label xml:lang="it">Categoria tematica</rdfs:label>
        <rdfs:label xml:lang="en">Thematic category</rdfs:label>
        <owl:versionInfo xml:lang="it">stabile</owl:versionInfo>
        <owl:versionInfo xml:lang="en">stable</owl:versionInfo>
        <a-cat:iccdNormTag>ICCD Normativa Trasversale 4.00: CT/CTM/CTMC</a-cat:iccdNormTag>
    </owl:Class>
    


    <!-- https://w3id.org/arco/ontology/arco/ZoologicalHeritage -->

    <owl:Class rdf:about="https://w3id.org/arco/ontology/arco/ZoologicalHeritage">
        <rdfs:subClassOf rdf:resource="https://w3id.org/arco/ontology/arco/NaturalHeritage"/>
        <rdfs:comment xml:lang="it">Questa classe rappresenta esemplari del mondo animale provenienti da collezioni di zoologia (ustiolo, toporagno, mammifero, artropode, scatola di farfalle, collezione elmintologica, ecc.)</rdfs:comment>
        <rdfs:comment xml:lang="en">This class represents specimens of the animal world from zoology collections (ustiolo, shrew, mammal, arthropod, butterfly box, elmintological collection, etc.)</rdfs:comment>
        <rdfs:label xml:lang="it">Bene Zoologico</rdfs:label>
        <rdfs:label xml:lang="en">Zoological Heritage</rdfs:label>
        <owl:versionInfo xml:lang="it">instabile</owl:versionInfo>
        <owl:versionInfo xml:lang="en">unstable</owl:versionInfo>
    </owl:Class>
    


    <!-- https://w3id.org/arco/ontology/catalogue/AdditionalForm -->

    <owl:Class rdf:about="https://w3id.org/arco/ontology/catalogue/AdditionalForm"/>
    


    <!-- https://w3id.org/arco/ontology/catalogue/InformationForm -->

    <owl:Class rdf:about="https://w3id.org/arco/ontology/catalogue/InformationForm"/>
    


    <!-- https://w3id.org/arco/ontology/context-description/Acquisition -->

    <owl:Class rdf:about="https://w3id.org/arco/ontology/context-description/Acquisition"/>
    


    <!-- https://w3id.org/arco/ontology/context-description/AnomalyOrigin -->

    <owl:Class rdf:about="https://w3id.org/arco/ontology/context-description/AnomalyOrigin"/>
    


    <!-- https://w3id.org/arco/ontology/context-description/ArchivalRecord -->

    <owl:Class rdf:about="https://w3id.org/arco/ontology/context-description/ArchivalRecord"/>
    


    <!-- https://w3id.org/arco/ontology/context-description/ArchivalRecordSet -->

    <owl:Class rdf:about="https://w3id.org/arco/ontology/context-description/ArchivalRecordSet"/>
    


    <!-- https://w3id.org/arco/ontology/context-description/AuthorshipAttribution -->

    <owl:Class rdf:about="https://w3id.org/arco/ontology/context-description/AuthorshipAttribution"/>
    


    <!-- https://w3id.org/arco/ontology/context-description/Bibliography -->

    <owl:Class rdf:about="https://w3id.org/arco/ontology/context-description/Bibliography"/>
    


    <!-- https://w3id.org/arco/ontology/context-description/BiologicalTaxonomy -->

    <owl:Class rdf:about="https://w3id.org/arco/ontology/context-description/BiologicalTaxonomy"/>
    


    <!-- https://w3id.org/arco/ontology/context-description/ChangeOfAvailability -->

    <owl:Class rdf:about="https://w3id.org/arco/ontology/context-description/ChangeOfAvailability"/>
    


    <!-- https://w3id.org/arco/ontology/context-description/CoinIssuance -->

    <owl:Class rdf:about="https://w3id.org/arco/ontology/context-description/CoinIssuance"/>
    


    <!-- https://w3id.org/arco/ontology/context-description/CollectionMembership -->

    <owl:Class rdf:about="https://w3id.org/arco/ontology/context-description/CollectionMembership"/>
    


    <!-- https://w3id.org/arco/ontology/context-description/Commission -->

    <owl:Class rdf:about="https://w3id.org/arco/ontology/context-description/Commission"/>
    


    <!-- https://w3id.org/arco/ontology/context-description/CulturalPropertyStage -->

    <owl:Class rdf:about="https://w3id.org/arco/ontology/context-description/CulturalPropertyStage"/>
    


    <!-- https://w3id.org/arco/ontology/context-description/Dating -->

    <owl:Class rdf:about="https://w3id.org/arco/ontology/context-description/Dating"/>
    


    <!-- https://w3id.org/arco/ontology/context-description/DetectionMethod -->

    <owl:Class rdf:about="https://w3id.org/arco/ontology/context-description/DetectionMethod"/>
    


    <!-- https://w3id.org/arco/ontology/context-description/Documentation -->

    <owl:Class rdf:about="https://w3id.org/arco/ontology/context-description/Documentation"/>
    


    <!-- https://w3id.org/arco/ontology/context-description/Estimate -->

    <owl:Class rdf:about="https://w3id.org/arco/ontology/context-description/Estimate"/>
    


    <!-- https://w3id.org/arco/ontology/context-description/ExportImportCertification -->

    <owl:Class rdf:about="https://w3id.org/arco/ontology/context-description/ExportImportCertification"/>
    


    <!-- https://w3id.org/arco/ontology/context-description/FindingContext -->

    <owl:Class rdf:about="https://w3id.org/arco/ontology/context-description/FindingContext"/>
    


    <!-- https://w3id.org/arco/ontology/context-description/Fruition -->

    <owl:Class rdf:about="https://w3id.org/arco/ontology/context-description/Fruition"/>
    


    <!-- https://w3id.org/arco/ontology/context-description/Intervention -->

    <owl:Class rdf:about="https://w3id.org/arco/ontology/context-description/Intervention"/>
    


    <!-- https://w3id.org/arco/ontology/context-description/Inventory -->

    <owl:Class rdf:about="https://w3id.org/arco/ontology/context-description/Inventory"/>
    


    <!-- https://w3id.org/arco/ontology/context-description/LegalSituation -->

    <owl:Class rdf:about="https://w3id.org/arco/ontology/context-description/LegalSituation"/>
    


    <!-- https://w3id.org/arco/ontology/context-description/NumismaticSeries -->

    <owl:Class rdf:about="https://w3id.org/arco/ontology/context-description/NumismaticSeries"/>
    


    <!-- https://w3id.org/arco/ontology/context-description/PhotographicSeriesMembership -->

    <owl:Class rdf:about="https://w3id.org/arco/ontology/context-description/PhotographicSeriesMembership"/>
    


    <!-- https://w3id.org/arco/ontology/context-description/ProtectiveMeasure -->

    <owl:Class rdf:about="https://w3id.org/arco/ontology/context-description/ProtectiveMeasure"/>
    


    <!-- https://w3id.org/arco/ontology/context-description/RelatedWorkSituation -->

    <owl:Class rdf:about="https://w3id.org/arco/ontology/context-description/RelatedWorkSituation"/>
    


    <!-- https://w3id.org/arco/ontology/context-description/Reliability -->

    <owl:Class rdf:about="https://w3id.org/arco/ontology/context-description/Reliability"/>
    


    <!-- https://w3id.org/arco/ontology/context-description/Research -->

    <owl:Class rdf:about="https://w3id.org/arco/ontology/context-description/Research"/>
    


    <!-- https://w3id.org/arco/ontology/context-description/Responsibility -->

    <owl:Class rdf:about="https://w3id.org/arco/ontology/context-description/Responsibility"/>
    


    <!-- https://w3id.org/arco/ontology/context-description/Subject -->

    <owl:Class rdf:about="https://w3id.org/arco/ontology/context-description/Subject"/>
    


    <!-- https://w3id.org/arco/ontology/context-description/Survey -->

    <owl:Class rdf:about="https://w3id.org/arco/ontology/context-description/Survey"/>
    


    <!-- https://w3id.org/arco/ontology/context-description/Title -->

    <owl:Class rdf:about="https://w3id.org/arco/ontology/context-description/Title"/>
    


    <!-- https://w3id.org/arco/ontology/context-description/UrbanPlanningInstrument -->

    <owl:Class rdf:about="https://w3id.org/arco/ontology/context-description/UrbanPlanningInstrument"/>
    


    <!-- https://w3id.org/arco/ontology/context-description/Use -->

    <owl:Class rdf:about="https://w3id.org/arco/ontology/context-description/Use"/>
    


    <!-- https://w3id.org/arco/ontology/core/Category -->

    <owl:Class rdf:about="https://w3id.org/arco/ontology/core/Category"/>
    


    <!-- https://w3id.org/arco/ontology/core/Concept -->

    <owl:Class rdf:about="https://w3id.org/arco/ontology/core/Concept"/>
    


    <!-- https://w3id.org/arco/ontology/core/CulturalEntityCharacteristic -->

    <owl:Class rdf:about="https://w3id.org/arco/ontology/core/CulturalEntityCharacteristic"/>
    


    <!-- https://w3id.org/arco/ontology/core/CulturalEntityClassification -->

    <owl:Class rdf:about="https://w3id.org/arco/ontology/core/CulturalEntityClassification"/>
    


    <!-- https://w3id.org/arco/ontology/core/Type -->

    <owl:Class rdf:about="https://w3id.org/arco/ontology/core/Type"/>
    


    <!-- https://w3id.org/arco/ontology/denotative-description/Accessory -->

    <owl:Class rdf:about="https://w3id.org/arco/ontology/denotative-description/Accessory"/>
    


    <!-- https://w3id.org/arco/ontology/denotative-description/AffixedElement -->

    <owl:Class rdf:about="https://w3id.org/arco/ontology/denotative-description/AffixedElement"/>
    


    <!-- https://w3id.org/arco/ontology/denotative-description/AgeRange -->

    <owl:Class rdf:about="https://w3id.org/arco/ontology/denotative-description/AgeRange"/>
    


    <!-- https://w3id.org/arco/ontology/denotative-description/CommunicationMedium -->

    <owl:Class rdf:about="https://w3id.org/arco/ontology/denotative-description/CommunicationMedium"/>
    


    <!-- https://w3id.org/arco/ontology/denotative-description/ConservationStatus -->

    <owl:Class rdf:about="https://w3id.org/arco/ontology/denotative-description/ConservationStatus"/>
    


    <!-- https://w3id.org/arco/ontology/denotative-description/CulturalEntityTechnicalStatus -->

    <owl:Class rdf:about="https://w3id.org/arco/ontology/denotative-description/CulturalEntityTechnicalStatus"/>
    


    <!-- https://w3id.org/arco/ontology/denotative-description/CulturalPropertyAccessibility -->

    <owl:Class rdf:about="https://w3id.org/arco/ontology/denotative-description/CulturalPropertyAccessibility"/>
    


    <!-- https://w3id.org/arco/ontology/denotative-description/CulturalPropertyAvailability -->

    <owl:Class rdf:about="https://w3id.org/arco/ontology/denotative-description/CulturalPropertyAvailability"/>
    


    <!-- https://w3id.org/arco/ontology/denotative-description/CulturalPropertyType -->

    <owl:Class rdf:about="https://w3id.org/arco/ontology/denotative-description/CulturalPropertyType"/>
    


    <!-- https://w3id.org/arco/ontology/denotative-description/DesignationInTime -->

    <owl:Class rdf:about="https://w3id.org/arco/ontology/denotative-description/DesignationInTime"/>
    


    <!-- https://w3id.org/arco/ontology/denotative-description/FontStyle -->

    <owl:Class rdf:about="https://w3id.org/arco/ontology/denotative-description/FontStyle"/>
    


    <!-- https://w3id.org/arco/ontology/denotative-description/FunctionalPurpose -->

    <owl:Class rdf:about="https://w3id.org/arco/ontology/denotative-description/FunctionalPurpose"/>
    


    <!-- https://w3id.org/arco/ontology/denotative-description/IconographicOrDecorativeApparatus -->

    <owl:Class rdf:about="https://w3id.org/arco/ontology/denotative-description/IconographicOrDecorativeApparatus"/>
    


    <!-- https://w3id.org/arco/ontology/denotative-description/Legibility -->

    <owl:Class rdf:about="https://w3id.org/arco/ontology/denotative-description/Legibility"/>
    


    <!-- https://w3id.org/arco/ontology/denotative-description/MeasurementCollection -->

    <owl:Class rdf:about="https://w3id.org/arco/ontology/denotative-description/MeasurementCollection"/>
    


    <!-- https://w3id.org/arco/ontology/denotative-description/Orientation -->

    <owl:Class rdf:about="https://w3id.org/arco/ontology/denotative-description/Orientation"/>
    


    <!-- https://w3id.org/arco/ontology/denotative-description/SampleCollected -->

    <owl:Class rdf:about="https://w3id.org/arco/ontology/denotative-description/SampleCollected"/>
    


    <!-- https://w3id.org/arco/ontology/denotative-description/TechnicalDetailOccurrence -->

    <owl:Class rdf:about="https://w3id.org/arco/ontology/denotative-description/TechnicalDetailOccurrence"/>
    


    <!-- https://w3id.org/arco/ontology/location/Altitude -->

    <owl:Class rdf:about="https://w3id.org/arco/ontology/location/Altitude"/>
    


    <!-- https://w3id.org/arco/ontology/location/CadastralIdentity -->

    <owl:Class rdf:about="https://w3id.org/arco/ontology/location/CadastralIdentity"/>
    


    <!-- https://w3id.org/arco/ontology/location/Coordinates -->

    <owl:Class rdf:about="https://w3id.org/arco/ontology/location/Coordinates"/>
    


    <!-- https://w3id.org/arco/ontology/location/TimeIndexedTypedLocation -->

    <owl:Class rdf:about="https://w3id.org/arco/ontology/location/TimeIndexedTypedLocation"/>
    


    <!-- https://w3id.org/arco/ontology/location/TypeOfContext -->

    <owl:Class rdf:about="https://w3id.org/arco/ontology/location/TypeOfContext"/>
    


    <!-- https://w3id.org/arco/ontology/movable-property/Accession -->

    <owl:Class rdf:about="https://w3id.org/arco/ontology/movable-property/Accession"/>
    


    <!-- https://w3id.org/italia/onto/CLV/Address -->

    <owl:Class rdf:about="https://w3id.org/italia/onto/CLV/Address"/>
    


    <!-- https://w3id.org/italia/onto/CLV/Feature -->

    <owl:Class rdf:about="https://w3id.org/italia/onto/CLV/Feature"/>
    


    <!-- https://w3id.org/italia/onto/CLV/Geometry -->

    <owl:Class rdf:about="https://w3id.org/italia/onto/CLV/Geometry"/>
    


    <!-- https://w3id.org/italia/onto/RO/Role -->

    <owl:Class rdf:about="https://w3id.org/italia/onto/RO/Role"/>
    


    <!-- https://w3id.org/italia/onto/TI/TimeInterval -->

    <owl:Class rdf:about="https://w3id.org/italia/onto/TI/TimeInterval"/>
    


    <!-- https://w3id.org/italia/onto/l0/Agent -->

    <owl:Class rdf:about="https://w3id.org/italia/onto/l0/Agent"/>
    


    <!-- https://w3id.org/italia/onto/l0/Characteristic -->

    <owl:Class rdf:about="https://w3id.org/italia/onto/l0/Characteristic"/>
    


    <!-- https://w3id.org/italia/onto/l0/Collection -->

    <owl:Class rdf:about="https://w3id.org/italia/onto/l0/Collection"/>
    


    <!-- https://w3id.org/italia/onto/l0/Description -->

    <owl:Class rdf:about="https://w3id.org/italia/onto/l0/Description"/>
    


    <!-- https://w3id.org/italia/onto/l0/Location -->

    <owl:Class rdf:about="https://w3id.org/italia/onto/l0/Location"/>
    


    <!-- https://w3id.org/italia/onto/l0/Topic -->

    <owl:Class rdf:about="https://w3id.org/italia/onto/l0/Topic"/>
    


    <!-- 
    ///////////////////////////////////////////////////////////////////////////////////////
    //
    // Individuals
    //
    ///////////////////////////////////////////////////////////////////////////////////////
     -->

    


    <!-- https://w3id.org/arco/ontology/arco/ArchaeologicalScope -->

    <owl:NamedIndividual rdf:about="https://w3id.org/arco/ontology/arco/ArchaeologicalScope">
        <rdf:type rdf:resource="https://w3id.org/arco/ontology/arco/MibacScopeOfProtection"/>
        <rdfs:label xml:lang="en">Archeaological</rdfs:label>
        <rdfs:label xml:lang="it">Archeologico</rdfs:label>
        <owl:versionInfo xml:lang="it">stabile</owl:versionInfo>
        <owl:versionInfo xml:lang="en">stable</owl:versionInfo>
    </owl:NamedIndividual>
    


    <!-- https://w3id.org/arco/ontology/arco/ArchitecturalLandscapeScope -->

    <owl:NamedIndividual rdf:about="https://w3id.org/arco/ontology/arco/ArchitecturalLandscapeScope">
        <rdf:type rdf:resource="https://w3id.org/arco/ontology/arco/MibacScopeOfProtection"/>
        <rdfs:label xml:lang="en">Architectural or Landscape</rdfs:label>
        <rdfs:label xml:lang="it">Architettonico o Paesaggistico</rdfs:label>
        <owl:versionInfo xml:lang="it">stabile</owl:versionInfo>
        <owl:versionInfo xml:lang="en">stable</owl:versionInfo>
    </owl:NamedIndividual>
    


    <!-- https://w3id.org/arco/ontology/arco/EthnoAnthropologicalScope -->

    <owl:NamedIndividual rdf:about="https://w3id.org/arco/ontology/arco/EthnoAnthropologicalScope">
        <rdf:type rdf:resource="https://w3id.org/arco/ontology/arco/MibacScopeOfProtection"/>
        <rdfs:label xml:lang="en">Ethno-anthropological</rdfs:label>
        <rdfs:label xml:lang="it">Etnoantropologico</rdfs:label>
        <owl:versionInfo xml:lang="it">stabile</owl:versionInfo>
        <owl:versionInfo xml:lang="en">stable</owl:versionInfo>
    </owl:NamedIndividual>
    


    <!-- https://w3id.org/arco/ontology/arco/HistoricalArtisticScope -->

    <owl:NamedIndividual rdf:about="https://w3id.org/arco/ontology/arco/HistoricalArtisticScope">
        <rdf:type rdf:resource="https://w3id.org/arco/ontology/arco/MibacScopeOfProtection"/>
        <rdfs:label xml:lang="en">Historical Artistic</rdfs:label>
        <rdfs:label xml:lang="it">Storico Artistico</rdfs:label>
        <owl:versionInfo xml:lang="it">stabile</owl:versionInfo>
        <owl:versionInfo xml:lang="en">stable</owl:versionInfo>
    </owl:NamedIndividual>
    


    <!-- 
    ///////////////////////////////////////////////////////////////////////////////////////
    //
    // General axioms
    //
    ///////////////////////////////////////////////////////////////////////////////////////
     -->

    <rdf:Description>
        <rdf:type rdf:resource="http://www.w3.org/2002/07/owl#AllDisjointClasses"/>
        <owl:members rdf:parseType="Collection">
            <rdf:Description rdf:about="https://w3id.org/arco/ontology/arco/CartographicClassification"/>
            <rdf:Description rdf:about="https://w3id.org/arco/ontology/arco/MusicalInstrumentClassification"/>
            <rdf:Description rdf:about="https://w3id.org/arco/ontology/arco/PhotographicHeritageClassification"/>
        </owl:members>
    </rdf:Description>
    <rdf:Description>
        <rdf:type rdf:resource="http://www.w3.org/2002/07/owl#AllDisjointClasses"/>
        <owl:members rdf:parseType="Collection">
            <rdf:Description rdf:about="https://w3id.org/arco/ontology/arco/CulturalPropertyCollection"/>
            <rdf:Description rdf:about="https://w3id.org/arco/ontology/context-description/ArchivalRecordSet"/>
            <rdf:Description rdf:about="https://w3id.org/arco/ontology/denotative-description/MeasurementCollection"/>
            <rdf:Description rdf:about="https://w3id.org/arco/ontology/denotative-description/SampleCollected"/>
            <rdf:Description rdf:about="https://w3id.org/arco/ontology/location/Coordinates"/>
        </owl:members>
    </rdf:Description>
    <rdf:Description>
        <rdf:type rdf:resource="http://www.w3.org/2002/07/owl#AllDisjointClasses"/>
        <owl:members rdf:parseType="Collection">
            <rdf:Description rdf:about="https://w3id.org/arco/ontology/context-description/AnomalyOrigin"/>
            <rdf:Description rdf:about="https://w3id.org/arco/ontology/denotative-description/CommunicationMedium"/>
            <rdf:Description rdf:about="https://w3id.org/arco/ontology/denotative-description/CulturalPropertyAccessibility"/>
            <rdf:Description rdf:about="https://w3id.org/arco/ontology/denotative-description/CulturalPropertyAvailability"/>
            <rdf:Description rdf:about="https://w3id.org/arco/ontology/denotative-description/FunctionalPurpose"/>
            <rdf:Description rdf:about="https://w3id.org/arco/ontology/denotative-description/Legibility"/>
        </owl:members>
    </rdf:Description>
    <rdf:Description>
        <rdf:type rdf:resource="http://www.w3.org/2002/07/owl#AllDisjointClasses"/>
        <owl:members rdf:parseType="Collection">
            <rdf:Description rdf:about="https://w3id.org/arco/ontology/context-description/CulturalPropertyStage"/>
            <rdf:Description rdf:about="https://w3id.org/arco/ontology/denotative-description/CommunicationMedium"/>
            <rdf:Description rdf:about="https://w3id.org/arco/ontology/denotative-description/CulturalPropertyAccessibility"/>
            <rdf:Description rdf:about="https://w3id.org/arco/ontology/denotative-description/CulturalPropertyAvailability"/>
            <rdf:Description rdf:about="https://w3id.org/arco/ontology/denotative-description/FunctionalPurpose"/>
            <rdf:Description rdf:about="https://w3id.org/arco/ontology/denotative-description/Legibility"/>
        </owl:members>
    </rdf:Description>
    <rdf:Description>
        <rdf:type rdf:resource="http://www.w3.org/2002/07/owl#AllDisjointClasses"/>
        <owl:members rdf:parseType="Collection">
            <rdf:Description rdf:about="https://w3id.org/arco/ontology/context-description/Reliability"/>
            <rdf:Description rdf:about="https://w3id.org/arco/ontology/core/CulturalEntityCharacteristic"/>
            <rdf:Description rdf:about="https://w3id.org/arco/ontology/denotative-description/AgeRange"/>
            <rdf:Description rdf:about="https://w3id.org/arco/ontology/denotative-description/FontStyle"/>
            <rdf:Description rdf:about="https://w3id.org/arco/ontology/denotative-description/Orientation"/>
            <rdf:Description rdf:about="https://w3id.org/arco/ontology/location/Altitude"/>
        </owl:members>
    </rdf:Description>
    <rdf:Description>
        <rdf:type rdf:resource="http://www.w3.org/2002/07/owl#AllDisjointClasses"/>
        <owl:members rdf:parseType="Collection">
            <rdf:Description rdf:about="https://w3id.org/arco/ontology/context-description/Reliability"/>
            <rdf:Description rdf:about="https://w3id.org/arco/ontology/denotative-description/AgeRange"/>
            <rdf:Description rdf:about="https://w3id.org/arco/ontology/denotative-description/FontStyle"/>
            <rdf:Description rdf:about="https://w3id.org/arco/ontology/denotative-description/Orientation"/>
            <rdf:Description rdf:about="https://w3id.org/arco/ontology/location/Altitude"/>
            <rdf:Description rdf:about="https://w3id.org/arco/ontology/location/TypeOfContext"/>
        </owl:members>
    </rdf:Description>
</rdf:RDF>



<!-- Generated by the OWL API (version 4.5.9.2019-02-01T07:24:44Z) https://github.com/owlcs/owlapi -->

